<?xml version="1.0" encoding="utf-8"?>
<rdf:RDF
  xmlns:cc="http://creativecommons.org/ns#"
  xmlns:rdf="http://www.w3.org/1999/02/22-rdf-syntax-ns#"
  xmlns:skos="http://www.w3.org/2004/02/skos/core#"
  xmlns:dcterms="http://purl.org/dc/terms/"
>
  <skos:Concept rdf:about="http://purl.org/heritagedata/schemes/eh_evd/concepts/135585">
    <skos:scopeNote xml:lang="en">A distribution of artefacts indicating the presence, or former presence, of a monument.</skos:scopeNote>
    <dcterms:identifier>http://purl.org/heritagedata/schemes/eh_evd/concepts/135585</dcterms:identifier>
    <skos:broader>
      <skos:Concept rdf:about="http://purl.org/heritagedata/schemes/eh_evd/concepts/82791">
        <cc:attributionName xml:lang="en">Historic England</cc:attributionName>
        <dcterms:publisher rdf:resource="http://www.historicengland.org.uk"/>
        <cc:license rdf:resource="http://creativecommons.org/licenses/by/3.0"/>
        <skos:prefLabel xml:lang="en">Find</skos:prefLabel>
        <skos:narrower rdf:resource="http://purl.org/heritagedata/schemes/eh_evd/concepts/111153"/>
        <cc:attributionURL rdf:resource="http://www.historicengland.org.uk"/>
        <skos:narrower rdf:resource="http://purl.org/heritagedata/schemes/eh_evd/concepts/100512"/>
        <dcterms:identifier>http://purl.org/heritagedata/schemes/eh_evd/concepts/82791</dcterms:identifier>
        <dcterms:issued rdf:datatype="http://www.w3.org/2001/XMLSchema#dateTime">2019-07-17T13:20:10</dcterms:issued>
        <skos:scopeNote xml:lang="en">Monument whose existence is indicated by the discovery of isolated artefacts or an artefact scatter. Eg a scatter of roofing tiles indicating the presence of a building. Use narrow terms where circumstances of discovery are known.</skos:scopeNote>
        <skos:narrower rdf:resource="http://purl.org/heritagedata/schemes/eh_evd/concepts/135585"/>
        <skos:inScheme rdf:resource="http://purl.org/heritagedata/schemes/eh_evd"/>
        <skos:broader rdf:resource="http://purl.org/heritagedata/schemes/eh_evd/concepts/97294"/>
      </skos:Concept>
    </skos:broader>
    <skos:inScheme>
      <skos:ConceptScheme rdf:about="http://purl.org/heritagedata/schemes/eh_evd">
        <skos:hasTopConcept rdf:resource="http://purl.org/heritagedata/schemes/eh_evd/concepts/82790"/>
        <dcterms:description xml:lang="en">Terminology covering the existing physical remains of a monument, or the means by which a monument has been identified where no physical remains exist</dcterms:description>
        <cc:license rdf:resource="http://creativecommons.org/licenses/by/3.0"/>
        <cc:attributionName xml:lang="en">Historic England</cc:attributionName>
        <dcterms:issued rdf:datatype="http://www.w3.org/2001/XMLSchema#date">2019-07-17</dcterms:issued>
        <dcterms:identifier>http://purl.org/heritagedata/schemes/eh_evd</dcterms:identifier>
        <dcterms:title xml:lang="en">FISH Evidence Thesaurus</dcterms:title>
        <dcterms:publisher rdf:resource="http://www.historicengland.org.uk"/>
        <cc:attributionURL rdf:resource="http://www.historicengland.org.uk"/>
      </skos:ConceptScheme>
    </skos:inScheme>
    <cc:license rdf:resource="http://creativecommons.org/licenses/by/3.0"/>
    <cc:attributionName xml:lang="en">Historic England</cc:attributionName>
    <skos:prefLabel xml:lang="en">Artefact Scatter</skos:prefLabel>
    <cc:attributionURL rdf:resource="http://www.historicengland.org.uk"/>
    <dcterms:publisher rdf:resource="http://www.historicengland.org.uk"/>
    <dcterms:issued rdf:datatype="http://www.w3.org/2001/XMLSchema#dateTime">2019-07-17T13:20:10</dcterms:issued>
  </skos:Concept>
  <skos:Concept rdf:about="http://purl.org/heritagedata/schemes/eh_evd/concepts/82786">
    <skos:inScheme rdf:resource="http://purl.org/heritagedata/schemes/eh_evd"/>
    <skos:scopeNote xml:lang="en">A maritime monument where the hull structure and fabric of a vessel remain wholly or mainly intact.</skos:scopeNote>
    <dcterms:issued rdf:datatype="http://www.w3.org/2001/XMLSchema#dateTime">2019-07-17T13:20:10</dcterms:issued>
    <skos:prefLabel xml:lang="en">Coherent Vessel Structure</skos:prefLabel>
    <cc:license rdf:resource="http://creativecommons.org/licenses/by/3.0"/>
    <cc:attributionName xml:lang="en">Historic England</cc:attributionName>
    <dcterms:identifier>http://purl.org/heritagedata/schemes/eh_evd/concepts/82786</dcterms:identifier>
    <dcterms:publisher rdf:resource="http://www.historicengland.org.uk"/>
    <skos:broader>
      <skos:Concept rdf:about="http://purl.org/heritagedata/schemes/eh_evd/concepts/82799">
        <dcterms:identifier>http://purl.org/heritagedata/schemes/eh_evd/concepts/82799</dcterms:identifier>
        <cc:license rdf:resource="http://creativecommons.org/licenses/by/3.0"/>
        <skos:narrower rdf:resource="http://purl.org/heritagedata/schemes/eh_evd/concepts/82793"/>
        <skos:narrower rdf:resource="http://purl.org/heritagedata/schemes/eh_evd/concepts/82787"/>
        <skos:narrower rdf:resource="http://purl.org/heritagedata/schemes/eh_evd/concepts/82786"/>
        <skos:narrower rdf:resource="http://purl.org/heritagedata/schemes/eh_evd/concepts/82795"/>
        <cc:attributionURL rdf:resource="http://www.historicengland.org.uk"/>
        <dcterms:publisher rdf:resource="http://www.historicengland.org.uk"/>
        <skos:inScheme rdf:resource="http://purl.org/heritagedata/schemes/eh_evd"/>
        <cc:attributionName xml:lang="en">Historic England</cc:attributionName>
        <dcterms:issued rdf:datatype="http://www.w3.org/2001/XMLSchema#dateTime">2019-07-17T13:20:10</dcterms:issued>
        <skos:narrower rdf:resource="http://purl.org/heritagedata/schemes/eh_evd/concepts/82785"/>
        <skos:broader rdf:resource="http://purl.org/heritagedata/schemes/eh_evd/concepts/99975"/>
        <skos:prefLabel xml:lang="en">Vessel Structure</skos:prefLabel>
        <skos:scopeNote xml:lang="en">A maritime monument where the remains of a vessel are known to exist but where no detailed information is available.</skos:scopeNote>
      </skos:Concept>
    </skos:broader>
    <cc:attributionURL rdf:resource="http://www.historicengland.org.uk"/>
  </skos:Concept>
  <skos:Concept rdf:about="http://purl.org/heritagedata/schemes/eh_evd/concepts/78252">
    <cc:attributionURL rdf:resource="http://www.historicengland.org.uk"/>
    <cc:attributionName xml:lang="en">Historic England</cc:attributionName>
    <dcterms:issued rdf:datatype="http://www.w3.org/2001/XMLSchema#dateTime">2019-07-17T13:20:10</dcterms:issued>
    <skos:inScheme rdf:resource="http://purl.org/heritagedata/schemes/eh_evd"/>
    <skos:scopeNote xml:lang="en">Monument existing as an upstanding earthwork, ditch or artificial watercourse, or as a low stone built feature not covered by the other categories.</skos:scopeNote>
    <skos:prefLabel xml:lang="en">Earthwork</skos:prefLabel>
    <cc:license rdf:resource="http://creativecommons.org/licenses/by/3.0"/>
    <skos:broader>
      <skos:Concept rdf:about="http://purl.org/heritagedata/schemes/eh_evd/concepts/97294">
        <skos:narrower rdf:resource="http://purl.org/heritagedata/schemes/eh_evd/concepts/97296"/>
        <dcterms:publisher rdf:resource="http://www.historicengland.org.uk"/>
        <skos:broader rdf:resource="http://purl.org/heritagedata/schemes/eh_evd/concepts/82790"/>
        <skos:prefLabel xml:lang="en">Physical Evidence</skos:prefLabel>
        <skos:narrower rdf:resource="http://purl.org/heritagedata/schemes/eh_evd/concepts/151454"/>
        <skos:narrower rdf:resource="http://purl.org/heritagedata/schemes/eh_evd/concepts/99975"/>
        <skos:narrower rdf:resource="http://purl.org/heritagedata/schemes/eh_evd/concepts/143015"/>
        <skos:narrower rdf:resource="http://purl.org/heritagedata/schemes/eh_evd/concepts/84568"/>
        <skos:narrower rdf:resource="http://purl.org/heritagedata/schemes/eh_evd/concepts/151455"/>
        <skos:narrower rdf:resource="http://purl.org/heritagedata/schemes/eh_evd/concepts/84570"/>
        <skos:narrower rdf:resource="http://purl.org/heritagedata/schemes/eh_evd/concepts/169985"/>
        <skos:narrower rdf:resource="http://purl.org/heritagedata/schemes/eh_evd/concepts/84569"/>
        <dcterms:issued rdf:datatype="http://www.w3.org/2001/XMLSchema#dateTime">2019-07-17T13:20:10</dcterms:issued>
        <skos:narrower rdf:resource="http://purl.org/heritagedata/schemes/eh_evd/concepts/82791"/>
        <skos:scopeNote xml:lang="en">Not to be used for indexing. Broad term used to assist retreival of all monuments where physical evidence is recorded.</skos:scopeNote>
        <skos:narrower rdf:resource="http://purl.org/heritagedata/schemes/eh_evd/concepts/167857"/>
        <skos:narrower rdf:resource="http://purl.org/heritagedata/schemes/eh_evd/concepts/99982"/>
        <cc:license rdf:resource="http://creativecommons.org/licenses/by/3.0"/>
        <skos:narrower rdf:resource="http://purl.org/heritagedata/schemes/eh_evd/concepts/84571"/>
        <skos:narrower rdf:resource="http://purl.org/heritagedata/schemes/eh_evd/concepts/99691"/>
        <skos:narrower rdf:resource="http://purl.org/heritagedata/schemes/eh_evd/concepts/84564"/>
        <skos:narrower rdf:resource="http://purl.org/heritagedata/schemes/eh_evd/concepts/84567"/>
        <skos:narrower rdf:resource="http://purl.org/heritagedata/schemes/eh_evd/concepts/78252"/>
        <skos:narrower rdf:resource="http://purl.org/heritagedata/schemes/eh_evd/concepts/170018"/>
        <skos:narrower rdf:resource="http://purl.org/heritagedata/schemes/eh_evd/concepts/139114"/>
        <skos:narrower rdf:resource="http://purl.org/heritagedata/schemes/eh_evd/concepts/78253"/>
        <cc:attributionName xml:lang="en">Historic England</cc:attributionName>
        <skos:inScheme rdf:resource="http://purl.org/heritagedata/schemes/eh_evd"/>
        <skos:narrower rdf:resource="http://purl.org/heritagedata/schemes/eh_evd/concepts/142975"/>
        <dcterms:identifier>http://purl.org/heritagedata/schemes/eh_evd/concepts/97294</dcterms:identifier>
        <skos:narrower rdf:resource="http://purl.org/heritagedata/schemes/eh_evd/concepts/100511"/>
        <cc:attributionURL rdf:resource="http://www.historicengland.org.uk"/>
      </skos:Concept>
    </skos:broader>
    <dcterms:publisher rdf:resource="http://www.historicengland.org.uk"/>
    <skos:narrower>
      <skos:Concept rdf:about="http://purl.org/heritagedata/schemes/eh_evd/concepts/99974">
        <skos:broader rdf:resource="http://purl.org/heritagedata/schemes/eh_evd/concepts/78252"/>
        <skos:inScheme rdf:resource="http://purl.org/heritagedata/schemes/eh_evd"/>
        <dcterms:issued rdf:datatype="http://www.w3.org/2001/XMLSchema#dateTime">2019-07-17T13:20:10</dcterms:issued>
        <dcterms:identifier>http://purl.org/heritagedata/schemes/eh_evd/concepts/99974</dcterms:identifier>
        <cc:attributionURL rdf:resource="http://www.historicengland.org.uk"/>
        <cc:license rdf:resource="http://creativecommons.org/licenses/by/3.0"/>
        <skos:prefLabel xml:lang="en">Levelled Earthwork</skos:prefLabel>
        <dcterms:publisher rdf:resource="http://www.historicengland.org.uk"/>
        <skos:scopeNote xml:lang="en">Monument visible as remains of former earthworks.</skos:scopeNote>
        <cc:attributionName xml:lang="en">Historic England</cc:attributionName>
        <skos:altLabel xml:lang="en">Plough Levelled Earthwork</skos:altLabel>
      </skos:Concept>
    </skos:narrower>
    <dcterms:identifier>http://purl.org/heritagedata/schemes/eh_evd/concepts/78252</dcterms:identifier>
  </skos:Concept>
  <skos:Concept rdf:about="http://purl.org/heritagedata/schemes/eh_evd/concepts/142975">
    <cc:attributionURL rdf:resource="http://www.historicengland.org.uk"/>
    <dcterms:identifier>http://purl.org/heritagedata/schemes/eh_evd/concepts/142975</dcterms:identifier>
    <cc:license rdf:resource="http://creativecommons.org/licenses/by/3.0"/>
    <skos:inScheme rdf:resource="http://purl.org/heritagedata/schemes/eh_evd"/>
    <cc:attributionName xml:lang="en">Historic England</cc:attributionName>
    <dcterms:publisher rdf:resource="http://www.historicengland.org.uk"/>
    <dcterms:issued rdf:datatype="http://www.w3.org/2001/XMLSchema#dateTime">2019-07-17T13:20:10</dcterms:issued>
    <skos:broader rdf:resource="http://purl.org/heritagedata/schemes/eh_evd/concepts/97294"/>
    <skos:prefLabel xml:lang="en">Surface Deposit</skos:prefLabel>
    <skos:scopeNote xml:lang="en">A deposit that forms the ground surface (when the evidence is collected), particularly a hard surface such as a floor or road.</skos:scopeNote>
  </skos:Concept>
  <skos:Concept rdf:about="http://purl.org/heritagedata/schemes/eh_evd/concepts/99975">
    <skos:inScheme rdf:resource="http://purl.org/heritagedata/schemes/eh_evd"/>
    <skos:prefLabel xml:lang="en">Submerged Monument</skos:prefLabel>
    <skos:altLabel xml:lang="en">Submerged</skos:altLabel>
    <cc:attributionName xml:lang="en">Historic England</cc:attributionName>
    <dcterms:issued rdf:datatype="http://www.w3.org/2001/XMLSchema#dateTime">2019-07-17T13:20:10</dcterms:issued>
    <dcterms:publisher rdf:resource="http://www.historicengland.org.uk"/>
    <cc:license rdf:resource="http://creativecommons.org/licenses/by/3.0"/>
    <cc:attributionURL rdf:resource="http://www.historicengland.org.uk"/>
    <skos:narrower rdf:resource="http://purl.org/heritagedata/schemes/eh_evd/concepts/82799"/>
    <dcterms:identifier>http://purl.org/heritagedata/schemes/eh_evd/concepts/99975</dcterms:identifier>
    <skos:broader rdf:resource="http://purl.org/heritagedata/schemes/eh_evd/concepts/97294"/>
    <skos:scopeNote xml:lang="en">Monument visible on the sea, lake or river bed, either totally submerged at all times, or exposed at low tide, low water conditions etc.</skos:scopeNote>
  </skos:Concept>
  <skos:Concept rdf:about="http://purl.org/heritagedata/schemes/eh_evd/concepts/143438">
    <dcterms:identifier>http://purl.org/heritagedata/schemes/eh_evd/concepts/143438</dcterms:identifier>
    <skos:broader>
      <skos:Concept rdf:about="http://purl.org/heritagedata/schemes/eh_evd/concepts/99976">
        <dcterms:publisher rdf:resource="http://www.historicengland.org.uk"/>
        <dcterms:issued rdf:datatype="http://www.w3.org/2001/XMLSchema#dateTime">2019-07-17T13:20:10</dcterms:issued>
        <cc:attributionName xml:lang="en">Historic England</cc:attributionName>
        <skos:prefLabel xml:lang="en">Marine Geophysical Evidence</skos:prefLabel>
        <skos:broader rdf:resource="http://purl.org/heritagedata/schemes/eh_evd/concepts/97293"/>
        <dcterms:identifier>http://purl.org/heritagedata/schemes/eh_evd/concepts/99976</dcterms:identifier>
        <skos:inScheme rdf:resource="http://purl.org/heritagedata/schemes/eh_evd"/>
        <skos:scopeNote xml:lang="en">A monument visible as a trace on marine survey equipment</skos:scopeNote>
        <skos:narrower rdf:resource="http://purl.org/heritagedata/schemes/eh_evd/concepts/143438"/>
        <skos:narrower rdf:resource="http://purl.org/heritagedata/schemes/eh_evd/concepts/111133"/>
        <skos:narrower rdf:resource="http://purl.org/heritagedata/schemes/eh_evd/concepts/82797"/>
        <cc:license rdf:resource="http://creativecommons.org/licenses/by/3.0"/>
        <cc:attributionURL rdf:resource="http://www.historicengland.org.uk"/>
        <skos:narrower rdf:resource="http://purl.org/heritagedata/schemes/eh_evd/concepts/82789"/>
      </skos:Concept>
    </skos:broader>
    <skos:prefLabel xml:lang="en">Multibeam Survey</skos:prefLabel>
    <cc:attributionURL rdf:resource="http://www.historicengland.org.uk"/>
    <dcterms:publisher rdf:resource="http://www.historicengland.org.uk"/>
    <dcterms:issued rdf:datatype="http://www.w3.org/2001/XMLSchema#dateTime">2019-07-17T13:20:10</dcterms:issued>
    <cc:license rdf:resource="http://creativecommons.org/licenses/by/3.0"/>
    <skos:scopeNote xml:lang="en">A marine survey in which a multi-element transducer provides many (30-150) individual soundings of the water depth and echo strength for each ping.</skos:scopeNote>
    <skos:inScheme rdf:resource="http://purl.org/heritagedata/schemes/eh_evd"/>
    <cc:attributionName xml:lang="en">Historic England</cc:attributionName>
  </skos:Concept>
  <skos:Concept rdf:about="http://purl.org/heritagedata/schemes/eh_evd/concepts/82798">
    <cc:attributionName xml:lang="en">Historic England</cc:attributionName>
    <skos:altLabel xml:lang="en">Uncertain</skos:altLabel>
    <dcterms:publisher rdf:resource="http://www.historicengland.org.uk"/>
    <cc:license rdf:resource="http://creativecommons.org/licenses/by/3.0"/>
    <skos:scopeNote xml:lang="en">Current recorded information does not give the evidence for a monument, or the information is regarded as unreliable.</skos:scopeNote>
    <cc:attributionURL rdf:resource="http://www.historicengland.org.uk"/>
    <dcterms:identifier>http://purl.org/heritagedata/schemes/eh_evd/concepts/82798</dcterms:identifier>
    <dcterms:issued rdf:datatype="http://www.w3.org/2001/XMLSchema#dateTime">2019-07-17T13:20:10</dcterms:issued>
    <skos:prefLabel xml:lang="en">Uncertain Evidence</skos:prefLabel>
    <skos:broader>
      <skos:Concept rdf:about="http://purl.org/heritagedata/schemes/eh_evd/concepts/82790">
        <skos:topConceptOf rdf:resource="http://purl.org/heritagedata/schemes/eh_evd"/>
        <skos:inScheme rdf:resource="http://purl.org/heritagedata/schemes/eh_evd"/>
        <skos:narrower rdf:resource="http://purl.org/heritagedata/schemes/eh_evd/concepts/84565"/>
        <skos:narrower rdf:resource="http://purl.org/heritagedata/schemes/eh_evd/concepts/97294"/>
        <dcterms:publisher rdf:resource="http://www.historicengland.org.uk"/>
        <cc:license rdf:resource="http://creativecommons.org/licenses/by/3.0"/>
        <dcterms:issued rdf:datatype="http://www.w3.org/2001/XMLSchema#dateTime">2019-07-17T13:20:10</dcterms:issued>
        <skos:scopeNote xml:lang="en">Do not use</skos:scopeNote>
        <dcterms:identifier>http://purl.org/heritagedata/schemes/eh_evd/concepts/82790</dcterms:identifier>
        <skos:narrower rdf:resource="http://purl.org/heritagedata/schemes/eh_evd/concepts/82798"/>
        <skos:narrower rdf:resource="http://purl.org/heritagedata/schemes/eh_evd/concepts/97293"/>
        <skos:prefLabel xml:lang="en">Evidence</skos:prefLabel>
        <cc:attributionName xml:lang="en">Historic England</cc:attributionName>
        <cc:attributionURL rdf:resource="http://www.historicengland.org.uk"/>
      </skos:Concept>
    </skos:broader>
    <skos:inScheme rdf:resource="http://purl.org/heritagedata/schemes/eh_evd"/>
  </skos:Concept>
  <skos:Concept rdf:about="http://purl.org/heritagedata/schemes/eh_evd/concepts/141909">
    <skos:broader>
      <skos:Concept rdf:about="http://purl.org/heritagedata/schemes/eh_evd/concepts/84570">
        <skos:altLabel xml:lang="en">Other Structure</skos:altLabel>
        <skos:narrower rdf:resource="http://purl.org/heritagedata/schemes/eh_evd/concepts/142985"/>
        <skos:altLabel xml:lang="en">Standing Structure - Unbonded</skos:altLabel>
        <cc:license rdf:resource="http://creativecommons.org/licenses/by/3.0"/>
        <skos:narrower rdf:resource="http://purl.org/heritagedata/schemes/eh_evd/concepts/142986"/>
        <skos:altLabel xml:lang="en">Standing  Monument</skos:altLabel>
        <dcterms:issued rdf:datatype="http://www.w3.org/2001/XMLSchema#dateTime">2019-07-17T13:20:10</dcterms:issued>
        <cc:attributionName xml:lang="en">Historic England</cc:attributionName>
        <skos:scopeNote xml:lang="en">Man-made building, edifice or construction of assembled material parts.</skos:scopeNote>
        <skos:altLabel xml:lang="en">Partially Destroyed Monument</skos:altLabel>
        <skos:narrower rdf:resource="http://purl.org/heritagedata/schemes/eh_evd/concepts/142987"/>
        <cc:attributionURL rdf:resource="http://www.historicengland.org.uk"/>
        <dcterms:publisher rdf:resource="http://www.historicengland.org.uk"/>
        <skos:broader rdf:resource="http://purl.org/heritagedata/schemes/eh_evd/concepts/97294"/>
        <skos:prefLabel xml:lang="en">Structure</skos:prefLabel>
        <dcterms:identifier>http://purl.org/heritagedata/schemes/eh_evd/concepts/84570</dcterms:identifier>
        <skos:inScheme rdf:resource="http://purl.org/heritagedata/schemes/eh_evd"/>
        <skos:narrower rdf:resource="http://purl.org/heritagedata/schemes/eh_evd/concepts/141909"/>
        <skos:altLabel xml:lang="en">Standing Structure - Bonded</skos:altLabel>
      </skos:Concept>
    </skos:broader>
    <skos:narrower>
      <skos:Concept rdf:about="http://purl.org/heritagedata/schemes/eh_evd/concepts/141908">
        <dcterms:issued rdf:datatype="http://www.w3.org/2001/XMLSchema#dateTime">2019-07-17T13:20:10</dcterms:issued>
        <cc:attributionName xml:lang="en">Historic England</cc:attributionName>
        <skos:inScheme rdf:resource="http://purl.org/heritagedata/schemes/eh_evd"/>
        <cc:attributionURL rdf:resource="http://www.historicengland.org.uk"/>
        <dcterms:identifier>http://purl.org/heritagedata/schemes/eh_evd/concepts/141908</dcterms:identifier>
        <skos:broader rdf:resource="http://purl.org/heritagedata/schemes/eh_evd/concepts/84564"/>
        <skos:prefLabel xml:lang="en">Moved Building</skos:prefLabel>
        <skos:scopeNote xml:lang="en">A building which has been moved from its original site either through active human intervention or natural processes such as erosion. For structures or objects such as gravestones use MOVED STRUCTURE.</skos:scopeNote>
        <skos:broader rdf:resource="http://purl.org/heritagedata/schemes/eh_evd/concepts/141909"/>
        <cc:license rdf:resource="http://creativecommons.org/licenses/by/3.0"/>
        <dcterms:publisher rdf:resource="http://www.historicengland.org.uk"/>
      </skos:Concept>
    </skos:narrower>
    <cc:attributionURL rdf:resource="http://www.historicengland.org.uk"/>
    <cc:license rdf:resource="http://creativecommons.org/licenses/by/3.0"/>
    <dcterms:publisher rdf:resource="http://www.historicengland.org.uk"/>
    <dcterms:issued rdf:datatype="http://www.w3.org/2001/XMLSchema#dateTime">2019-07-17T13:20:10</dcterms:issued>
    <cc:attributionName xml:lang="en">Historic England</cc:attributionName>
    <skos:inScheme rdf:resource="http://purl.org/heritagedata/schemes/eh_evd"/>
    <dcterms:identifier>http://purl.org/heritagedata/schemes/eh_evd/concepts/141909</dcterms:identifier>
    <skos:scopeNote xml:lang="en">A man-made construction or object (such as a gravestone) which has been moved from its original site either through active human intervention or natural processes such as erosion. For buildings which have been moved use MOVED BUILDING.</skos:scopeNote>
    <skos:prefLabel xml:lang="en">Moved Structure</skos:prefLabel>
  </skos:Concept>
  <skos:Concept rdf:about="http://purl.org/heritagedata/schemes/eh_evd/concepts/84565">
    <cc:attributionName xml:lang="en">Historic England</cc:attributionName>
    <dcterms:identifier>http://purl.org/heritagedata/schemes/eh_evd/concepts/84565</dcterms:identifier>
    <dcterms:issued rdf:datatype="http://www.w3.org/2001/XMLSchema#dateTime">2019-07-17T13:20:10</dcterms:issued>
    <skos:prefLabel xml:lang="en">Destroyed Monument</skos:prefLabel>
    <skos:broader rdf:resource="http://purl.org/heritagedata/schemes/eh_evd/concepts/82790"/>
    <skos:altLabel xml:lang="en">Partially Destroyed Monument</skos:altLabel>
    <dcterms:publisher rdf:resource="http://www.historicengland.org.uk"/>
    <cc:attributionURL rdf:resource="http://www.historicengland.org.uk"/>
    <skos:scopeNote xml:lang="en">All physical evidence for a monument has certainly been completely destroyed (allowing no future reinvestigation) by activity implying substantial ground disturbance. Eg quarrying, road cutting, or natural disaster, erosion, acts of God etc.</skos:scopeNote>
    <cc:license rdf:resource="http://creativecommons.org/licenses/by/3.0"/>
    <skos:inScheme rdf:resource="http://purl.org/heritagedata/schemes/eh_evd"/>
    <skos:altLabel xml:lang="en">Destroyed</skos:altLabel>
  </skos:Concept>
  <skos:Concept rdf:about="http://purl.org/heritagedata/schemes/eh_evd/concepts/82793">
    <dcterms:identifier>http://purl.org/heritagedata/schemes/eh_evd/concepts/82793</dcterms:identifier>
    <cc:attributionURL rdf:resource="http://www.historicengland.org.uk"/>
    <cc:license rdf:resource="http://creativecommons.org/licenses/by/3.0"/>
    <skos:broader rdf:resource="http://purl.org/heritagedata/schemes/eh_evd/concepts/82799"/>
    <dcterms:publisher rdf:resource="http://www.historicengland.org.uk"/>
    <dcterms:issued rdf:datatype="http://www.w3.org/2001/XMLSchema#dateTime">2019-07-17T13:20:10</dcterms:issued>
    <cc:attributionName xml:lang="en">Historic England</cc:attributionName>
    <skos:prefLabel xml:lang="en">Intact Vessel Structure</skos:prefLabel>
    <skos:scopeNote xml:lang="en">A maritime monument where the hull of a vessel is mostly in one piece, with large pieces of the superstructure intact.</skos:scopeNote>
    <skos:inScheme rdf:resource="http://purl.org/heritagedata/schemes/eh_evd"/>
  </skos:Concept>
  <skos:Concept rdf:about="http://purl.org/heritagedata/schemes/eh_evd/concepts/169985">
    <cc:attributionURL rdf:resource="http://www.historicengland.org.uk"/>
    <cc:license rdf:resource="http://creativecommons.org/licenses/by/3.0"/>
    <skos:inScheme rdf:resource="http://purl.org/heritagedata/schemes/eh_evd"/>
    <skos:scopeNote xml:lang="en">An element such as a window, door or wall decoration, usually associated with a larger monument but which may be found in isolation. For example a stained glass window or panelling saved from a demolished building.</skos:scopeNote>
    <cc:attributionName xml:lang="en">Historic England</cc:attributionName>
    <dcterms:publisher rdf:resource="http://www.historicengland.org.uk"/>
    <dcterms:issued rdf:datatype="http://www.w3.org/2001/XMLSchema#dateTime">2019-07-17T13:20:10</dcterms:issued>
    <dcterms:identifier>http://purl.org/heritagedata/schemes/eh_evd/concepts/169985</dcterms:identifier>
    <skos:prefLabel xml:lang="en">Architectural Element</skos:prefLabel>
    <skos:broader rdf:resource="http://purl.org/heritagedata/schemes/eh_evd/concepts/97294"/>
  </skos:Concept>
  <skos:Concept rdf:about="http://purl.org/heritagedata/schemes/eh_evd/concepts/167857">
    <skos:scopeNote xml:lang="en">Evidence of past environmental conditions, eg insect, seed, pollen remains</skos:scopeNote>
    <dcterms:issued rdf:datatype="http://www.w3.org/2001/XMLSchema#dateTime">2019-07-17T13:20:10</dcterms:issued>
    <dcterms:identifier>http://purl.org/heritagedata/schemes/eh_evd/concepts/167857</dcterms:identifier>
    <skos:inScheme rdf:resource="http://purl.org/heritagedata/schemes/eh_evd"/>
    <cc:license rdf:resource="http://creativecommons.org/licenses/by/3.0"/>
    <cc:attributionName xml:lang="en">Historic England</cc:attributionName>
    <skos:broader rdf:resource="http://purl.org/heritagedata/schemes/eh_evd/concepts/97294"/>
    <skos:prefLabel xml:lang="en">Environmental Evidence</skos:prefLabel>
    <dcterms:publisher rdf:resource="http://www.historicengland.org.uk"/>
    <cc:attributionURL rdf:resource="http://www.historicengland.org.uk"/>
  </skos:Concept>
  <skos:Concept rdf:about="http://purl.org/heritagedata/schemes/eh_evd/concepts/100510">
    <cc:attributionURL rdf:resource="http://www.historicengland.org.uk"/>
    <skos:prefLabel xml:lang="en">Demolished Building</skos:prefLabel>
    <skos:scopeNote xml:lang="en">A monument previously consisting of a built structure, but which has been demolished, such that only a ground plan and foundations or similar are thought to remain. Where all below ground traces have also been removed use DESTROYED MONUMENT.</skos:scopeNote>
    <dcterms:identifier>http://purl.org/heritagedata/schemes/eh_evd/concepts/100510</dcterms:identifier>
    <dcterms:issued rdf:datatype="http://www.w3.org/2001/XMLSchema#dateTime">2019-07-17T13:20:10</dcterms:issued>
    <dcterms:publisher rdf:resource="http://www.historicengland.org.uk"/>
    <cc:attributionName xml:lang="en">Historic England</cc:attributionName>
    <skos:inScheme rdf:resource="http://purl.org/heritagedata/schemes/eh_evd"/>
    <cc:license rdf:resource="http://creativecommons.org/licenses/by/3.0"/>
    <skos:broader>
      <skos:Concept rdf:about="http://purl.org/heritagedata/schemes/eh_evd/concepts/84564">
        <dcterms:identifier>http://purl.org/heritagedata/schemes/eh_evd/concepts/84564</dcterms:identifier>
        <dcterms:issued rdf:datatype="http://www.w3.org/2001/XMLSchema#dateTime">2019-07-17T13:20:10</dcterms:issued>
        <cc:license rdf:resource="http://creativecommons.org/licenses/by/3.0"/>
        <cc:attributionName xml:lang="en">Historic England</cc:attributionName>
        <skos:narrower rdf:resource="http://purl.org/heritagedata/schemes/eh_evd/concepts/97291"/>
        <skos:scopeNote xml:lang="en">Monument with a roof and walls or evidence of these.</skos:scopeNote>
        <dcterms:publisher rdf:resource="http://www.historicengland.org.uk"/>
        <skos:narrower rdf:resource="http://purl.org/heritagedata/schemes/eh_evd/concepts/100510"/>
        <skos:broader rdf:resource="http://purl.org/heritagedata/schemes/eh_evd/concepts/97294"/>
        <skos:inScheme rdf:resource="http://purl.org/heritagedata/schemes/eh_evd"/>
        <skos:narrower rdf:resource="http://purl.org/heritagedata/schemes/eh_evd/concepts/141908"/>
        <skos:prefLabel xml:lang="en">Building</skos:prefLabel>
        <cc:attributionURL rdf:resource="http://www.historicengland.org.uk"/>
        <skos:narrower rdf:resource="http://purl.org/heritagedata/schemes/eh_evd/concepts/87962"/>
      </skos:Concept>
    </skos:broader>
    <skos:altLabel xml:lang="en">Partially Demolished Building</skos:altLabel>
    <skos:altLabel xml:lang="en">Building Foundation</skos:altLabel>
  </skos:Concept>
  <skos:Concept rdf:about="http://purl.org/heritagedata/schemes/eh_evd/concepts/151455">
    <dcterms:issued rdf:datatype="http://www.w3.org/2001/XMLSchema#dateTime">2019-07-17T13:20:10</dcterms:issued>
    <cc:license rdf:resource="http://creativecommons.org/licenses/by/3.0"/>
    <skos:broader rdf:resource="http://purl.org/heritagedata/schemes/eh_evd/concepts/97294"/>
    <cc:attributionName xml:lang="en">Historic England</cc:attributionName>
    <skos:inScheme rdf:resource="http://purl.org/heritagedata/schemes/eh_evd"/>
    <skos:scopeNote xml:lang="en">A landscape which has been specifically designed or modified. Often indicated by proven below ground stratigraphy, revealed by deliberate investigation including geophysical survey, or other surface monuments or structures.</skos:scopeNote>
    <dcterms:identifier>http://purl.org/heritagedata/schemes/eh_evd/concepts/151455</dcterms:identifier>
    <dcterms:publisher rdf:resource="http://www.historicengland.org.uk"/>
    <cc:attributionURL rdf:resource="http://www.historicengland.org.uk"/>
    <skos:prefLabel xml:lang="en">Designed Landscape</skos:prefLabel>
  </skos:Concept>
  <skos:Concept rdf:about="http://purl.org/heritagedata/schemes/eh_evd/concepts/97293">
    <skos:narrower>
      <skos:Concept rdf:about="http://purl.org/heritagedata/schemes/eh_evd/concepts/84573">
        <cc:license rdf:resource="http://creativecommons.org/licenses/by/3.0"/>
        <cc:attributionURL rdf:resource="http://www.historicengland.org.uk"/>
        <skos:broader rdf:resource="http://purl.org/heritagedata/schemes/eh_evd/concepts/97293"/>
        <skos:inScheme rdf:resource="http://purl.org/heritagedata/schemes/eh_evd"/>
        <skos:prefLabel xml:lang="en">Conjectural Evidence</skos:prefLabel>
        <dcterms:issued rdf:datatype="http://www.w3.org/2001/XMLSchema#dateTime">2019-07-17T13:20:10</dcterms:issued>
        <dcterms:publisher rdf:resource="http://www.historicengland.org.uk"/>
        <cc:attributionName xml:lang="en">Historic England</cc:attributionName>
        <skos:scopeNote xml:lang="en">Monument type/interpretation is inferred, based on informed speculation eg by comparison with similar monuments, proximity to other monuments, topography, site character etc.</skos:scopeNote>
        <dcterms:identifier>http://purl.org/heritagedata/schemes/eh_evd/concepts/84573</dcterms:identifier>
      </skos:Concept>
    </skos:narrower>
    <cc:attributionURL rdf:resource="http://www.historicengland.org.uk"/>
    <skos:narrower>
      <skos:Concept rdf:about="http://purl.org/heritagedata/schemes/eh_evd/concepts/84574">
        <skos:broader rdf:resource="http://purl.org/heritagedata/schemes/eh_evd/concepts/97293"/>
        <skos:inScheme rdf:resource="http://purl.org/heritagedata/schemes/eh_evd"/>
        <dcterms:identifier>http://purl.org/heritagedata/schemes/eh_evd/concepts/84574</dcterms:identifier>
        <dcterms:issued rdf:datatype="http://www.w3.org/2001/XMLSchema#dateTime">2019-07-17T13:20:10</dcterms:issued>
        <skos:prefLabel xml:lang="en">Placename Evidence</skos:prefLabel>
        <cc:attributionURL rdf:resource="http://www.historicengland.org.uk"/>
        <cc:license rdf:resource="http://creativecommons.org/licenses/by/3.0"/>
        <skos:scopeNote xml:lang="en">Use where the presence or nature of a monument is inferred from placenames or placename elements.</skos:scopeNote>
        <dcterms:publisher rdf:resource="http://www.historicengland.org.uk"/>
        <cc:attributionName xml:lang="en">Historic England</cc:attributionName>
      </skos:Concept>
    </skos:narrower>
    <skos:narrower>
      <skos:Concept rdf:about="http://purl.org/heritagedata/schemes/eh_evd/concepts/146360">
        <skos:prefLabel xml:lang="en">Marine Trawling Plot</skos:prefLabel>
        <skos:inScheme rdf:resource="http://purl.org/heritagedata/schemes/eh_evd"/>
        <skos:scopeNote xml:lang="en">An object in the sea bed recorded on the Hydrographic Office plot of objects snagged by nets during trawling.</skos:scopeNote>
        <cc:license rdf:resource="http://creativecommons.org/licenses/by/3.0"/>
        <dcterms:issued rdf:datatype="http://www.w3.org/2001/XMLSchema#dateTime">2019-07-17T13:20:10</dcterms:issued>
        <dcterms:identifier>http://purl.org/heritagedata/schemes/eh_evd/concepts/146360</dcterms:identifier>
        <cc:attributionName xml:lang="en">Historic England</cc:attributionName>
        <skos:broader rdf:resource="http://purl.org/heritagedata/schemes/eh_evd/concepts/97293"/>
        <dcterms:publisher rdf:resource="http://www.historicengland.org.uk"/>
        <cc:attributionURL rdf:resource="http://www.historicengland.org.uk"/>
      </skos:Concept>
    </skos:narrower>
    <skos:narrower>
      <skos:Concept rdf:about="http://purl.org/heritagedata/schemes/eh_evd/concepts/140391">
        <cc:attributionName xml:lang="en">Historic England</cc:attributionName>
        <skos:scopeNote xml:lang="en">A monument whose presence is inferred from verbally delivered information drawn from the speaker's personal knowledge.</skos:scopeNote>
        <skos:inScheme rdf:resource="http://purl.org/heritagedata/schemes/eh_evd"/>
        <cc:license rdf:resource="http://creativecommons.org/licenses/by/3.0"/>
        <dcterms:issued rdf:datatype="http://www.w3.org/2001/XMLSchema#dateTime">2019-07-17T13:20:10</dcterms:issued>
        <dcterms:publisher rdf:resource="http://www.historicengland.org.uk"/>
        <dcterms:identifier>http://purl.org/heritagedata/schemes/eh_evd/concepts/140391</dcterms:identifier>
        <skos:prefLabel xml:lang="en">Oral Evidence</skos:prefLabel>
        <skos:broader rdf:resource="http://purl.org/heritagedata/schemes/eh_evd/concepts/97293"/>
        <cc:attributionURL rdf:resource="http://www.historicengland.org.uk"/>
      </skos:Concept>
    </skos:narrower>
    <skos:broader rdf:resource="http://purl.org/heritagedata/schemes/eh_evd/concepts/82790"/>
    <dcterms:identifier>http://purl.org/heritagedata/schemes/eh_evd/concepts/97293</dcterms:identifier>
    <skos:prefLabel xml:lang="en">Implied Evidence</skos:prefLabel>
    <skos:scopeNote xml:lang="en">Not to be used for indexing. Broad term to assist retreival of all monuments where non-physical evidence is recorded.</skos:scopeNote>
    <cc:attributionName xml:lang="en">Historic England</cc:attributionName>
    <skos:inScheme rdf:resource="http://purl.org/heritagedata/schemes/eh_evd"/>
    <dcterms:issued rdf:datatype="http://www.w3.org/2001/XMLSchema#dateTime">2019-07-17T13:20:10</dcterms:issued>
    <skos:narrower>
      <skos:Concept rdf:about="http://purl.org/heritagedata/schemes/eh_evd/concepts/82788">
        <cc:attributionURL rdf:resource="http://www.historicengland.org.uk"/>
        <cc:license rdf:resource="http://creativecommons.org/licenses/by/3.0"/>
        <skos:scopeNote xml:lang="en">Monument known only from primary documentary sources eg books, maps, legal records, where no physical evidence exists. Use also where a monument has been planned but never constructed.</skos:scopeNote>
        <dcterms:identifier>http://purl.org/heritagedata/schemes/eh_evd/concepts/82788</dcterms:identifier>
        <dcterms:publisher rdf:resource="http://www.historicengland.org.uk"/>
        <cc:attributionName xml:lang="en">Historic England</cc:attributionName>
        <skos:broader rdf:resource="http://purl.org/heritagedata/schemes/eh_evd/concepts/97293"/>
        <skos:inScheme rdf:resource="http://purl.org/heritagedata/schemes/eh_evd"/>
        <skos:prefLabel xml:lang="en">Documentary Evidence</skos:prefLabel>
        <dcterms:issued rdf:datatype="http://www.w3.org/2001/XMLSchema#dateTime">2019-07-17T13:20:10</dcterms:issued>
      </skos:Concept>
    </skos:narrower>
    <dcterms:publisher rdf:resource="http://www.historicengland.org.uk"/>
    <skos:narrower rdf:resource="http://purl.org/heritagedata/schemes/eh_evd/concepts/99976"/>
    <cc:license rdf:resource="http://creativecommons.org/licenses/by/3.0"/>
  </skos:Concept>
  <skos:Concept rdf:about="http://purl.org/heritagedata/schemes/eh_evd/concepts/84567">
    <cc:attributionURL rdf:resource="http://www.historicengland.org.uk"/>
    <cc:license rdf:resource="http://creativecommons.org/licenses/by/3.0"/>
    <skos:prefLabel xml:lang="en">Enhanced Natural Feature</skos:prefLabel>
    <dcterms:publisher rdf:resource="http://www.historicengland.org.uk"/>
    <cc:attributionName xml:lang="en">Historic England</cc:attributionName>
    <dcterms:identifier>http://purl.org/heritagedata/schemes/eh_evd/concepts/84567</dcterms:identifier>
    <skos:scopeNote xml:lang="en">Natural feature or area deliberately enhanced to construct a monument, eg rock carving, cave, rock shelter.</skos:scopeNote>
    <skos:inScheme rdf:resource="http://purl.org/heritagedata/schemes/eh_evd"/>
    <dcterms:issued rdf:datatype="http://www.w3.org/2001/XMLSchema#dateTime">2019-07-17T13:20:10</dcterms:issued>
    <skos:broader rdf:resource="http://purl.org/heritagedata/schemes/eh_evd/concepts/97294"/>
  </skos:Concept>
  <skos:Concept rdf:about="http://purl.org/heritagedata/schemes/eh_evd/concepts/111133">
    <skos:inScheme rdf:resource="http://purl.org/heritagedata/schemes/eh_evd"/>
    <skos:prefLabel xml:lang="en">Marine Magnetometer Reading</skos:prefLabel>
    <cc:license rdf:resource="http://creativecommons.org/licenses/by/3.0"/>
    <skos:broader rdf:resource="http://purl.org/heritagedata/schemes/eh_evd/concepts/99976"/>
    <dcterms:identifier>http://purl.org/heritagedata/schemes/eh_evd/concepts/111133</dcterms:identifier>
    <cc:attributionURL rdf:resource="http://www.historicengland.org.uk"/>
    <skos:scopeNote xml:lang="en">Maritime monument identified as a ferrous object lying on the sea bed detected using marine surveying equipment that detects localised anomalies in the Earth's magnetic field.</skos:scopeNote>
    <dcterms:issued rdf:datatype="http://www.w3.org/2001/XMLSchema#dateTime">2019-07-17T13:20:10</dcterms:issued>
    <dcterms:publisher rdf:resource="http://www.historicengland.org.uk"/>
    <cc:attributionName xml:lang="en">Historic England</cc:attributionName>
  </skos:Concept>
  <skos:Concept rdf:about="http://purl.org/heritagedata/schemes/eh_evd/concepts/84569">
    <cc:attributionURL rdf:resource="http://www.historicengland.org.uk"/>
    <cc:license rdf:resource="http://creativecommons.org/licenses/by/3.0"/>
    <dcterms:publisher rdf:resource="http://www.historicengland.org.uk"/>
    <skos:altLabel xml:lang="en">Geophysical Evidence</skos:altLabel>
    <cc:attributionName xml:lang="en">Historic England</cc:attributionName>
    <skos:scopeNote xml:lang="en">Monument either never or no longer visible above ground surface, but whose presence is indicated by proven below ground stratigraphy revealed by deliberate investigation, including geophysical survey, or other surface disturbance.</skos:scopeNote>
    <skos:altLabel xml:lang="en">Flat - Accumulated</skos:altLabel>
    <skos:altLabel xml:lang="en">Flat - Unaccumulated</skos:altLabel>
    <skos:prefLabel xml:lang="en">Sub Surface Deposit</skos:prefLabel>
    <skos:inScheme rdf:resource="http://purl.org/heritagedata/schemes/eh_evd"/>
    <dcterms:identifier>http://purl.org/heritagedata/schemes/eh_evd/concepts/84569</dcterms:identifier>
    <dcterms:issued rdf:datatype="http://www.w3.org/2001/XMLSchema#dateTime">2019-07-17T13:20:10</dcterms:issued>
    <skos:broader rdf:resource="http://purl.org/heritagedata/schemes/eh_evd/concepts/97294"/>
  </skos:Concept>
  <skos:Concept rdf:about="http://purl.org/heritagedata/schemes/eh_evd/concepts/84568">
    <cc:attributionURL rdf:resource="http://www.historicengland.org.uk"/>
    <skos:scopeNote xml:lang="en">Monument thought to be archaeological or historical but proved to be natural.</skos:scopeNote>
    <dcterms:publisher rdf:resource="http://www.historicengland.org.uk"/>
    <dcterms:issued rdf:datatype="http://www.w3.org/2001/XMLSchema#dateTime">2019-07-17T13:20:10</dcterms:issued>
    <cc:license rdf:resource="http://creativecommons.org/licenses/by/3.0"/>
    <dcterms:identifier>http://purl.org/heritagedata/schemes/eh_evd/concepts/84568</dcterms:identifier>
    <skos:broader rdf:resource="http://purl.org/heritagedata/schemes/eh_evd/concepts/97294"/>
    <cc:attributionName xml:lang="en">Historic England</cc:attributionName>
    <skos:inScheme rdf:resource="http://purl.org/heritagedata/schemes/eh_evd"/>
    <skos:prefLabel xml:lang="en">Natural Feature</skos:prefLabel>
  </skos:Concept>
  <skos:Concept rdf:about="http://purl.org/heritagedata/schemes/eh_evd/concepts/100511">
    <cc:attributionURL rdf:resource="http://www.historicengland.org.uk"/>
    <dcterms:identifier>http://purl.org/heritagedata/schemes/eh_evd/concepts/100511</dcterms:identifier>
    <dcterms:issued rdf:datatype="http://www.w3.org/2001/XMLSchema#dateTime">2019-07-17T13:20:10</dcterms:issued>
    <skos:prefLabel xml:lang="en">Modified Surface</skos:prefLabel>
    <cc:attributionName xml:lang="en">Historic England</cc:attributionName>
    <skos:inScheme rdf:resource="http://purl.org/heritagedata/schemes/eh_evd"/>
    <cc:license rdf:resource="http://creativecommons.org/licenses/by/3.0"/>
    <skos:scopeNote xml:lang="en">A monument where the evidence that defines the type of the monument derives from the nature of surface markings. Examples include graffitti on quarry walls.</skos:scopeNote>
    <skos:broader rdf:resource="http://purl.org/heritagedata/schemes/eh_evd/concepts/97294"/>
    <dcterms:publisher rdf:resource="http://www.historicengland.org.uk"/>
  </skos:Concept>
  <skos:Concept rdf:about="http://purl.org/heritagedata/schemes/eh_evd/concepts/99691">
    <dcterms:identifier>http://purl.org/heritagedata/schemes/eh_evd/concepts/99691</dcterms:identifier>
    <cc:attributionURL rdf:resource="http://www.historicengland.org.uk"/>
    <dcterms:publisher rdf:resource="http://www.historicengland.org.uk"/>
    <dcterms:issued rdf:datatype="http://www.w3.org/2001/XMLSchema#dateTime">2019-07-17T13:20:10</dcterms:issued>
    <cc:license rdf:resource="http://creativecommons.org/licenses/by/3.0"/>
    <skos:broader rdf:resource="http://purl.org/heritagedata/schemes/eh_evd/concepts/97294"/>
    <cc:attributionName xml:lang="en">Historic England</cc:attributionName>
    <skos:inScheme rdf:resource="http://purl.org/heritagedata/schemes/eh_evd"/>
    <skos:scopeNote xml:lang="en">A monument composed of plants or trees which are still extant. Especially relevant for park and garden features. For example tree avenue, orchard, rose garden and lawn.</skos:scopeNote>
    <skos:prefLabel xml:lang="en">Botanical Feature</skos:prefLabel>
  </skos:Concept>
  <skos:Concept rdf:about="http://purl.org/heritagedata/schemes/eh_evd/concepts/82785">
    <dcterms:identifier>http://purl.org/heritagedata/schemes/eh_evd/concepts/82785</dcterms:identifier>
    <cc:attributionURL rdf:resource="http://www.historicengland.org.uk"/>
    <dcterms:issued rdf:datatype="http://www.w3.org/2001/XMLSchema#dateTime">2019-07-17T13:20:10</dcterms:issued>
    <cc:attributionName xml:lang="en">Historic England</cc:attributionName>
    <skos:inScheme rdf:resource="http://purl.org/heritagedata/schemes/eh_evd"/>
    <cc:license rdf:resource="http://creativecommons.org/licenses/by/3.0"/>
    <skos:prefLabel xml:lang="en">Buried Vessel Structure</skos:prefLabel>
    <skos:broader rdf:resource="http://purl.org/heritagedata/schemes/eh_evd/concepts/82799"/>
    <skos:scopeNote xml:lang="en">A maritime monument where the vessel remains are buried in the sea bed.</skos:scopeNote>
    <dcterms:publisher rdf:resource="http://www.historicengland.org.uk"/>
  </skos:Concept>
  <skos:Concept rdf:about="http://purl.org/heritagedata/schemes/eh_evd/concepts/82789">
    <skos:prefLabel xml:lang="en">Echosounder Trace</skos:prefLabel>
    <cc:license rdf:resource="http://creativecommons.org/licenses/by/3.0"/>
    <dcterms:issued rdf:datatype="http://www.w3.org/2001/XMLSchema#dateTime">2019-07-17T13:20:10</dcterms:issued>
    <cc:attributionURL rdf:resource="http://www.historicengland.org.uk"/>
    <skos:scopeNote xml:lang="en">An object in the sea bed detected by marine survey equipment that shows the contours of the sea bed beneath a vessel.</skos:scopeNote>
    <dcterms:identifier>http://purl.org/heritagedata/schemes/eh_evd/concepts/82789</dcterms:identifier>
    <skos:broader rdf:resource="http://purl.org/heritagedata/schemes/eh_evd/concepts/99976"/>
    <dcterms:publisher rdf:resource="http://www.historicengland.org.uk"/>
    <cc:attributionName xml:lang="en">Historic England</cc:attributionName>
    <skos:inScheme rdf:resource="http://purl.org/heritagedata/schemes/eh_evd"/>
  </skos:Concept>
  <skos:Concept rdf:about="http://purl.org/heritagedata/schemes/eh_evd/concepts/142987">
    <skos:prefLabel xml:lang="en">Demolished Structure</skos:prefLabel>
    <cc:attributionURL rdf:resource="http://www.historicengland.org.uk"/>
    <skos:broader rdf:resource="http://purl.org/heritagedata/schemes/eh_evd/concepts/84570"/>
    <skos:scopeNote xml:lang="en">A monument consisting of a built structure, but which has been demolished so that only a ground plan and foundations, or similar, are thought to remain. Where all below ground traces have also been removed use DESTROYED MONUMENT.</skos:scopeNote>
    <dcterms:publisher rdf:resource="http://www.historicengland.org.uk"/>
    <dcterms:issued rdf:datatype="http://www.w3.org/2001/XMLSchema#dateTime">2019-07-17T13:20:10</dcterms:issued>
    <cc:license rdf:resource="http://creativecommons.org/licenses/by/3.0"/>
    <cc:attributionName xml:lang="en">Historic England</cc:attributionName>
    <skos:inScheme rdf:resource="http://purl.org/heritagedata/schemes/eh_evd"/>
    <dcterms:identifier>http://purl.org/heritagedata/schemes/eh_evd/concepts/142987</dcterms:identifier>
  </skos:Concept>
  <skos:Concept rdf:about="http://purl.org/heritagedata/schemes/eh_evd/concepts/111153">
    <cc:license rdf:resource="http://creativecommons.org/licenses/by/3.0"/>
    <cc:attributionURL rdf:resource="http://www.historicengland.org.uk"/>
    <skos:scopeNote xml:lang="en">Monument whose presence is inferred by discovery of unstratified artefacts, for instance in plough soil.</skos:scopeNote>
    <dcterms:issued rdf:datatype="http://www.w3.org/2001/XMLSchema#dateTime">2019-07-17T13:20:10</dcterms:issued>
    <dcterms:publisher rdf:resource="http://www.historicengland.org.uk"/>
    <cc:attributionName xml:lang="en">Historic England</cc:attributionName>
    <dcterms:identifier>http://purl.org/heritagedata/schemes/eh_evd/concepts/111153</dcterms:identifier>
    <skos:inScheme rdf:resource="http://purl.org/heritagedata/schemes/eh_evd"/>
    <skos:broader rdf:resource="http://purl.org/heritagedata/schemes/eh_evd/concepts/82791"/>
    <skos:prefLabel xml:lang="en">Unstratified Find</skos:prefLabel>
  </skos:Concept>
  <skos:Concept rdf:about="http://purl.org/heritagedata/schemes/eh_evd/concepts/99982">
    <skos:altLabel xml:lang="en">AP Enclosure</skos:altLabel>
    <skos:altLabel xml:lang="en">AP Macula</skos:altLabel>
    <cc:license rdf:resource="http://creativecommons.org/licenses/by/3.0"/>
    <skos:altLabel xml:lang="en">AP Site</skos:altLabel>
    <dcterms:identifier>http://purl.org/heritagedata/schemes/eh_evd/concepts/99982</dcterms:identifier>
    <cc:attributionName xml:lang="en">Historic England</cc:attributionName>
    <skos:altLabel xml:lang="en">Soil Mark</skos:altLabel>
    <skos:prefLabel xml:lang="en">Soilmark</skos:prefLabel>
    <dcterms:publisher rdf:resource="http://www.historicengland.org.uk"/>
    <cc:attributionURL rdf:resource="http://www.historicengland.org.uk"/>
    <skos:scopeNote xml:lang="en">Monument visible, usually from the air, due to the fill of features being of a different colour than the surrounding subsoil. Soilmarks show up well in ploughed fields or areas where the topsoil has been stripped.  Term derived from AN32 Glossary</skos:scopeNote>
    <skos:broader rdf:resource="http://purl.org/heritagedata/schemes/eh_evd/concepts/97294"/>
    <dcterms:issued rdf:datatype="http://www.w3.org/2001/XMLSchema#dateTime">2019-07-17T13:20:10</dcterms:issued>
    <skos:inScheme rdf:resource="http://purl.org/heritagedata/schemes/eh_evd"/>
    <skos:altLabel xml:lang="en">AP Linear Feature</skos:altLabel>
  </skos:Concept>
  <skos:Concept rdf:about="http://purl.org/heritagedata/schemes/eh_evd/concepts/82796">
    <skos:prefLabel xml:lang="en">Side Scan Sonar Contact</skos:prefLabel>
    <cc:attributionURL rdf:resource="http://www.historicengland.org.uk"/>
    <cc:license rdf:resource="http://creativecommons.org/licenses/by/3.0"/>
    <dcterms:identifier>http://purl.org/heritagedata/schemes/eh_evd/concepts/82796</dcterms:identifier>
    <dcterms:publisher rdf:resource="http://www.historicengland.org.uk"/>
    <dcterms:issued rdf:datatype="http://www.w3.org/2001/XMLSchema#dateTime">2019-07-17T13:20:10</dcterms:issued>
    <cc:attributionName xml:lang="en">Historic England</cc:attributionName>
    <skos:broader>
      <skos:Concept rdf:about="http://purl.org/heritagedata/schemes/eh_evd/concepts/82797">
        <cc:attributionURL rdf:resource="http://www.historicengland.org.uk"/>
        <cc:license rdf:resource="http://creativecommons.org/licenses/by/3.0"/>
        <skos:broader rdf:resource="http://purl.org/heritagedata/schemes/eh_evd/concepts/99976"/>
        <dcterms:identifier>http://purl.org/heritagedata/schemes/eh_evd/concepts/82797</dcterms:identifier>
        <dcterms:publisher rdf:resource="http://www.historicengland.org.uk"/>
        <skos:narrower rdf:resource="http://purl.org/heritagedata/schemes/eh_evd/concepts/82796"/>
        <cc:attributionName xml:lang="en">Historic England</cc:attributionName>
        <skos:scopeNote xml:lang="en">An object lying on the sea bed detected by marine survey equipment that emits and receives high frequency sound waves.</skos:scopeNote>
        <skos:prefLabel xml:lang="en">Sonar Contact</skos:prefLabel>
        <skos:inScheme rdf:resource="http://purl.org/heritagedata/schemes/eh_evd"/>
        <dcterms:issued rdf:datatype="http://www.w3.org/2001/XMLSchema#dateTime">2019-07-17T13:20:10</dcterms:issued>
      </skos:Concept>
    </skos:broader>
    <skos:scopeNote xml:lang="en">An object projecting out of the sea bed detected by marine survey equipment that emits and receives high frequency sound waves projected sideways from a boat or towed array.</skos:scopeNote>
    <skos:inScheme rdf:resource="http://purl.org/heritagedata/schemes/eh_evd"/>
  </skos:Concept>
  <skos:Concept rdf:about="http://purl.org/heritagedata/schemes/eh_evd/concepts/97291">
    <skos:broader rdf:resource="http://purl.org/heritagedata/schemes/eh_evd/concepts/84564"/>
    <skos:altLabel xml:lang="en">Partially Destroyed Monument</skos:altLabel>
    <skos:altLabel xml:lang="en">Uninhabited Building</skos:altLabel>
    <cc:attributionName xml:lang="en">Historic England</cc:attributionName>
    <skos:altLabel xml:lang="en">Roofed Ruin</skos:altLabel>
    <cc:license rdf:resource="http://creativecommons.org/licenses/by/3.0"/>
    <skos:prefLabel xml:lang="en">Extant Building</skos:prefLabel>
    <skos:altLabel xml:lang="en">Inhabited Building</skos:altLabel>
    <skos:scopeNote xml:lang="en">Monument with roof or walls intact or substantially intact, significant survival of original features, even if building no longer in use for original function.</skos:scopeNote>
    <skos:altLabel xml:lang="en">Building - Other</skos:altLabel>
    <skos:inScheme rdf:resource="http://purl.org/heritagedata/schemes/eh_evd"/>
    <skos:altLabel xml:lang="en">Partially Demolished Building</skos:altLabel>
    <skos:altLabel xml:lang="en">Building Complex</skos:altLabel>
    <dcterms:issued rdf:datatype="http://www.w3.org/2001/XMLSchema#dateTime">2019-07-17T13:20:10</dcterms:issued>
    <dcterms:publisher rdf:resource="http://www.historicengland.org.uk"/>
    <skos:altLabel xml:lang="en">Roofed Building</skos:altLabel>
    <cc:attributionURL rdf:resource="http://www.historicengland.org.uk"/>
    <dcterms:identifier>http://purl.org/heritagedata/schemes/eh_evd/concepts/97291</dcterms:identifier>
    <skos:altLabel xml:lang="en">Building - Bonded</skos:altLabel>
  </skos:Concept>
  <skos:Concept rdf:about="http://purl.org/heritagedata/schemes/eh_evd/concepts/84571">
    <skos:altLabel xml:lang="en">Subterranean</skos:altLabel>
    <dcterms:issued rdf:datatype="http://www.w3.org/2001/XMLSchema#dateTime">2019-07-17T13:20:10</dcterms:issued>
    <skos:inScheme rdf:resource="http://purl.org/heritagedata/schemes/eh_evd"/>
    <dcterms:identifier>http://purl.org/heritagedata/schemes/eh_evd/concepts/84571</dcterms:identifier>
    <dcterms:publisher rdf:resource="http://www.historicengland.org.uk"/>
    <cc:attributionName xml:lang="en">Historic England</cc:attributionName>
    <skos:prefLabel xml:lang="en">Subterranean Feature</skos:prefLabel>
    <cc:license rdf:resource="http://creativecommons.org/licenses/by/3.0"/>
    <skos:scopeNote xml:lang="en">Monument visible as a below ground man-made structure. Use for tunnels, mineworking, cellars, shelters.</skos:scopeNote>
    <cc:attributionURL rdf:resource="http://www.historicengland.org.uk"/>
    <skos:broader rdf:resource="http://purl.org/heritagedata/schemes/eh_evd/concepts/97294"/>
  </skos:Concept>
  <skos:Concept rdf:about="http://purl.org/heritagedata/schemes/eh_evd/concepts/87962">
    <dcterms:publisher rdf:resource="http://www.historicengland.org.uk"/>
    <cc:attributionURL rdf:resource="http://www.historicengland.org.uk"/>
    <dcterms:identifier>http://purl.org/heritagedata/schemes/eh_evd/concepts/87962</dcterms:identifier>
    <skos:prefLabel xml:lang="en">Ruined Building</skos:prefLabel>
    <skos:scopeNote xml:lang="en">Monument visible as substantial above ground remains, retaining evidence of architecture and materials, with walls partially or completely intact but with roof and interior walls substantially or completely destroyed.</skos:scopeNote>
    <skos:inScheme rdf:resource="http://purl.org/heritagedata/schemes/eh_evd"/>
    <cc:license rdf:resource="http://creativecommons.org/licenses/by/3.0"/>
    <cc:attributionName xml:lang="en">Historic England</cc:attributionName>
    <skos:altLabel xml:lang="en">Partially Demolished Building</skos:altLabel>
    <skos:broader rdf:resource="http://purl.org/heritagedata/schemes/eh_evd/concepts/84564"/>
    <dcterms:issued rdf:datatype="http://www.w3.org/2001/XMLSchema#dateTime">2019-07-17T13:20:10</dcterms:issued>
  </skos:Concept>
  <skos:Concept rdf:about="http://purl.org/heritagedata/schemes/eh_evd/concepts/78253">
    <skos:altLabel xml:lang="en">Parchmark</skos:altLabel>
    <skos:altLabel xml:lang="en">AP Linear Feature</skos:altLabel>
    <skos:altLabel xml:lang="en">AP Site</skos:altLabel>
    <skos:altLabel xml:lang="en">AP Enclosure</skos:altLabel>
    <dcterms:identifier>http://purl.org/heritagedata/schemes/eh_evd/concepts/78253</dcterms:identifier>
    <cc:license rdf:resource="http://creativecommons.org/licenses/by/3.0"/>
    <skos:prefLabel xml:lang="en">Cropmark</skos:prefLabel>
    <dcterms:publisher rdf:resource="http://www.historicengland.org.uk"/>
    <skos:broader rdf:resource="http://purl.org/heritagedata/schemes/eh_evd/concepts/97294"/>
    <cc:attributionURL rdf:resource="http://www.historicengland.org.uk"/>
    <skos:scopeNote xml:lang="en">Monument visible as a mark in standing crops or parchmarks, but where no subsurface deposits have been proven eg by excavation or other ground disturbance, in which case SUB SURFACE DEPOSIT should be used.</skos:scopeNote>
    <dcterms:issued rdf:datatype="http://www.w3.org/2001/XMLSchema#dateTime">2019-07-17T13:20:10</dcterms:issued>
    <cc:attributionName xml:lang="en">Historic England</cc:attributionName>
    <skos:inScheme rdf:resource="http://purl.org/heritagedata/schemes/eh_evd"/>
    <skos:altLabel xml:lang="en">Crop Mark</skos:altLabel>
    <skos:altLabel xml:lang="en">AP Macula</skos:altLabel>
  </skos:Concept>
  <skos:Concept rdf:about="http://purl.org/heritagedata/schemes/eh_evd/concepts/142985">
    <skos:inScheme rdf:resource="http://purl.org/heritagedata/schemes/eh_evd"/>
    <cc:license rdf:resource="http://creativecommons.org/licenses/by/3.0"/>
    <cc:attributionURL rdf:resource="http://www.historicengland.org.uk"/>
    <skos:scopeNote xml:lang="en">Man-made, roofless edifice or construction visible as substantial above-ground remains retaining evidence of architecture and materials, but which has been substantially destroyed.</skos:scopeNote>
    <skos:broader rdf:resource="http://purl.org/heritagedata/schemes/eh_evd/concepts/84570"/>
    <skos:altLabel xml:lang="en">Ruined Structure - Unbonded</skos:altLabel>
    <skos:prefLabel xml:lang="en">Ruined Structure</skos:prefLabel>
    <dcterms:identifier>http://purl.org/heritagedata/schemes/eh_evd/concepts/142985</dcterms:identifier>
    <skos:altLabel xml:lang="en">Ruined Structure - Bonded</skos:altLabel>
    <dcterms:issued rdf:datatype="http://www.w3.org/2001/XMLSchema#dateTime">2019-07-17T13:20:10</dcterms:issued>
    <skos:altLabel xml:lang="en">Partially Destroyed Monument</skos:altLabel>
    <dcterms:publisher rdf:resource="http://www.historicengland.org.uk"/>
    <cc:attributionName xml:lang="en">Historic England</cc:attributionName>
  </skos:Concept>
  <rdf:Description rdf:about="http://purl.org/heritagedata/schemes/temp/concepts/84569">
    <skos:related>
      <rdf:Description rdf:about="http://purl.org/heritagedata/schemes/temp/concepts/100510">
        <skos:related rdf:resource="http://purl.org/heritagedata/schemes/temp/concepts/84569"/>
      </rdf:Description>
    </skos:related>
    <skos:related>
      <rdf:Description rdf:about="http://purl.org/heritagedata/schemes/temp/concepts/100512">
        <skos:related rdf:resource="http://purl.org/heritagedata/schemes/temp/concepts/84569"/>
      </rdf:Description>
    </skos:related>
    <skos:related>
      <rdf:Description rdf:about="http://purl.org/heritagedata/schemes/temp/concepts/151454">
        <skos:related rdf:resource="http://purl.org/heritagedata/schemes/temp/concepts/84569"/>
      </rdf:Description>
    </skos:related>
    <skos:related>
      <rdf:Description rdf:about="http://purl.org/heritagedata/schemes/temp/concepts/99974">
        <skos:related rdf:resource="http://purl.org/heritagedata/schemes/temp/concepts/84569"/>
      </rdf:Description>
    </skos:related>
  </rdf:Description>
  <skos:Concept rdf:about="http://purl.org/heritagedata/schemes/eh_evd/concepts/142986">
    <cc:attributionName xml:lang="en">Historic England</cc:attributionName>
    <skos:inScheme rdf:resource="http://purl.org/heritagedata/schemes/eh_evd"/>
    <dcterms:issued rdf:datatype="http://www.w3.org/2001/XMLSchema#dateTime">2019-07-17T13:20:10</dcterms:issued>
    <skos:prefLabel xml:lang="en">Extant Structure</skos:prefLabel>
    <skos:broader rdf:resource="http://purl.org/heritagedata/schemes/eh_evd/concepts/84570"/>
    <dcterms:identifier>http://purl.org/heritagedata/schemes/eh_evd/concepts/142986</dcterms:identifier>
    <cc:attributionURL rdf:resource="http://www.historicengland.org.uk"/>
    <cc:license rdf:resource="http://creativecommons.org/licenses/by/3.0"/>
    <skos:scopeNote xml:lang="en">Man-made roofless edifice or construction which is intact or substantially intact, with significant survival of original features, even if no longer serving original intended function.</skos:scopeNote>
    <dcterms:publisher rdf:resource="http://www.historicengland.org.uk"/>
  </skos:Concept>
  <skos:Concept rdf:about="http://purl.org/heritagedata/schemes/eh_evd/concepts/143015">
    <cc:attributionName xml:lang="en">Historic England</cc:attributionName>
    <skos:inScheme rdf:resource="http://purl.org/heritagedata/schemes/eh_evd"/>
    <skos:scopeNote xml:lang="en">Feature visible following archaeological excavation</skos:scopeNote>
    <dcterms:issued rdf:datatype="http://www.w3.org/2001/XMLSchema#dateTime">2019-07-17T13:20:10</dcterms:issued>
    <skos:prefLabel xml:lang="en">Excavated Feature</skos:prefLabel>
    <dcterms:identifier>http://purl.org/heritagedata/schemes/eh_evd/concepts/143015</dcterms:identifier>
    <cc:attributionURL rdf:resource="http://www.historicengland.org.uk"/>
    <skos:broader rdf:resource="http://purl.org/heritagedata/schemes/eh_evd/concepts/97294"/>
    <dcterms:publisher rdf:resource="http://www.historicengland.org.uk"/>
    <cc:license rdf:resource="http://creativecommons.org/licenses/by/3.0"/>
  </skos:Concept>
  <skos:Concept rdf:about="http://purl.org/heritagedata/schemes/eh_evd/concepts/100512">
    <skos:scopeNote xml:lang="en">A Monument whose presence is inferred from artefacts found in stratified below ground deposits, as distinct from surface collection or chance find.</skos:scopeNote>
    <cc:attributionURL rdf:resource="http://www.historicengland.org.uk"/>
    <dcterms:identifier>http://purl.org/heritagedata/schemes/eh_evd/concepts/100512</dcterms:identifier>
    <dcterms:issued rdf:datatype="http://www.w3.org/2001/XMLSchema#dateTime">2019-07-17T13:20:10</dcterms:issued>
    <cc:attributionName xml:lang="en">Historic England</cc:attributionName>
    <dcterms:publisher rdf:resource="http://www.historicengland.org.uk"/>
    <skos:inScheme rdf:resource="http://purl.org/heritagedata/schemes/eh_evd"/>
    <cc:license rdf:resource="http://creativecommons.org/licenses/by/3.0"/>
    <skos:broader rdf:resource="http://purl.org/heritagedata/schemes/eh_evd/concepts/82791"/>
    <skos:prefLabel xml:lang="en">Stratified Find</skos:prefLabel>
  </skos:Concept>
  <skos:Concept rdf:about="http://purl.org/heritagedata/schemes/eh_evd/concepts/139114">
    <dcterms:issued rdf:datatype="http://www.w3.org/2001/XMLSchema#dateTime">2019-07-17T13:20:10</dcterms:issued>
    <dcterms:publisher rdf:resource="http://www.historicengland.org.uk"/>
    <cc:license rdf:resource="http://creativecommons.org/licenses/by/3.0"/>
    <skos:prefLabel xml:lang="en">Wreckage</skos:prefLabel>
    <skos:scopeNote xml:lang="en">The fragmentary or substantial remains of a vehicle or aircraft. Where recovered from excavation double index with SUB SURFACE DEPOSIT.</skos:scopeNote>
    <cc:attributionName xml:lang="en">Historic England</cc:attributionName>
    <skos:inScheme rdf:resource="http://purl.org/heritagedata/schemes/eh_evd"/>
    <skos:broader rdf:resource="http://purl.org/heritagedata/schemes/eh_evd/concepts/97294"/>
    <dcterms:identifier>http://purl.org/heritagedata/schemes/eh_evd/concepts/139114</dcterms:identifier>
    <cc:attributionURL rdf:resource="http://www.historicengland.org.uk"/>
  </skos:Concept>
  <skos:Concept rdf:about="http://purl.org/heritagedata/schemes/eh_evd/concepts/82795">
    <dcterms:identifier>http://purl.org/heritagedata/schemes/eh_evd/concepts/82795</dcterms:identifier>
    <cc:attributionURL rdf:resource="http://www.historicengland.org.uk"/>
    <dcterms:publisher rdf:resource="http://www.historicengland.org.uk"/>
    <dcterms:issued rdf:datatype="http://www.w3.org/2001/XMLSchema#dateTime">2019-07-17T13:20:10</dcterms:issued>
    <skos:broader rdf:resource="http://purl.org/heritagedata/schemes/eh_evd/concepts/82799"/>
    <cc:license rdf:resource="http://creativecommons.org/licenses/by/3.0"/>
    <skos:inScheme rdf:resource="http://purl.org/heritagedata/schemes/eh_evd"/>
    <skos:prefLabel xml:lang="en">Scattered Vessel Structure</skos:prefLabel>
    <cc:attributionName xml:lang="en">Historic England</cc:attributionName>
    <skos:scopeNote xml:lang="en">A maritime monument where the remains of a vessel are scattered over a wide area.</skos:scopeNote>
  </skos:Concept>
  <skos:Concept rdf:about="http://purl.org/heritagedata/schemes/eh_evd/concepts/170018">
    <skos:prefLabel xml:lang="en">Movable Object</skos:prefLabel>
    <cc:license rdf:resource="http://creativecommons.org/licenses/by/3.0"/>
    <dcterms:identifier>http://purl.org/heritagedata/schemes/eh_evd/concepts/170018</dcterms:identifier>
    <dcterms:publisher rdf:resource="http://www.historicengland.org.uk"/>
    <cc:attributionName xml:lang="en">Historic England</cc:attributionName>
    <skos:inScheme rdf:resource="http://purl.org/heritagedata/schemes/eh_evd"/>
    <dcterms:issued rdf:datatype="http://www.w3.org/2001/XMLSchema#dateTime">2019-07-17T13:20:10</dcterms:issued>
    <cc:attributionURL rdf:resource="http://www.historicengland.org.uk"/>
    <skos:broader rdf:resource="http://purl.org/heritagedata/schemes/eh_evd/concepts/97294"/>
    <skos:scopeNote xml:lang="en">An object such as an organ, display case or piece of furniture such as a pew, usually associated with a larger monument but which may be found in isolation. For example a war memorial roll of honour in its display case.</skos:scopeNote>
  </skos:Concept>
  <skos:Concept rdf:about="http://purl.org/heritagedata/schemes/eh_evd/concepts/97296">
    <dcterms:identifier>http://purl.org/heritagedata/schemes/eh_evd/concepts/97296</dcterms:identifier>
    <cc:license rdf:resource="http://creativecommons.org/licenses/by/3.0"/>
    <dcterms:issued rdf:datatype="http://www.w3.org/2001/XMLSchema#dateTime">2019-07-17T13:20:10</dcterms:issued>
    <cc:attributionURL rdf:resource="http://www.historicengland.org.uk"/>
    <skos:prefLabel xml:lang="en">Architectural Component</skos:prefLabel>
    <skos:scopeNote xml:lang="en">Monument whose existence is inferred from the traces of architectural features. Eg include shadow marks on building walls or beams, pillars, floors incorporated into a later structure, suggesting the existence of an earlier building.</skos:scopeNote>
    <skos:broader rdf:resource="http://purl.org/heritagedata/schemes/eh_evd/concepts/97294"/>
    <dcterms:publisher rdf:resource="http://www.historicengland.org.uk"/>
    <cc:attributionName xml:lang="en">Historic England</cc:attributionName>
    <skos:inScheme rdf:resource="http://purl.org/heritagedata/schemes/eh_evd"/>
  </skos:Concept>
  <skos:Concept rdf:about="http://purl.org/heritagedata/schemes/eh_evd/concepts/151454">
    <skos:scopeNote xml:lang="en">The deliberate deposit of a body in the ground, usually located in a special area set aside for the purpose of burial, such as a graveyard or cemetery.</skos:scopeNote>
    <dcterms:identifier>http://purl.org/heritagedata/schemes/eh_evd/concepts/151454</dcterms:identifier>
    <skos:prefLabel xml:lang="en">Burial</skos:prefLabel>
    <dcterms:publisher rdf:resource="http://www.historicengland.org.uk"/>
    <cc:attributionName xml:lang="en">Historic England</cc:attributionName>
    <skos:inScheme rdf:resource="http://purl.org/heritagedata/schemes/eh_evd"/>
    <skos:broader rdf:resource="http://purl.org/heritagedata/schemes/eh_evd/concepts/97294"/>
    <cc:license rdf:resource="http://creativecommons.org/licenses/by/3.0"/>
    <dcterms:issued rdf:datatype="http://www.w3.org/2001/XMLSchema#dateTime">2019-07-17T13:20:10</dcterms:issued>
    <cc:attributionURL rdf:resource="http://www.historicengland.org.uk"/>
  </skos:Concept>
  <skos:Concept rdf:about="http://purl.org/heritagedata/schemes/eh_evd/concepts/82787">
    <skos:prefLabel xml:lang="en">Collapsed Vessel Structure</skos:prefLabel>
    <dcterms:identifier>http://purl.org/heritagedata/schemes/eh_evd/concepts/82787</dcterms:identifier>
    <cc:attributionURL rdf:resource="http://www.historicengland.org.uk"/>
    <skos:scopeNote xml:lang="en">A maritime monument where the fabric of a vessel has collapsed, leaving the hull structure flat on the sea bed but not widely dispersed.</skos:scopeNote>
    <skos:broader rdf:resource="http://purl.org/heritagedata/schemes/eh_evd/concepts/82799"/>
    <dcterms:publisher rdf:resource="http://www.historicengland.org.uk"/>
    <dcterms:issued rdf:datatype="http://www.w3.org/2001/XMLSchema#dateTime">2019-07-17T13:20:10</dcterms:issued>
    <cc:license rdf:resource="http://creativecommons.org/licenses/by/3.0"/>
    <cc:attributionName xml:lang="en">Historic England</cc:attributionName>
    <skos:inScheme rdf:resource="http://purl.org/heritagedata/schemes/eh_evd"/>
  </skos:Concept>
  <rdf:Description rdf:about="http://purl.org/heritagedata/schemes/temp/concepts/99976">
    <skos:related>
      <rdf:Description rdf:about="http://purl.org/heritagedata/schemes/temp/concepts/99975">
        <skos:related rdf:resource="http://purl.org/heritagedata/schemes/temp/concepts/99976"/>
      </rdf:Description>
    </skos:related>
  </rdf:Description>
</rdf:RDF>