<?xml version="1.0" encoding="UTF-8"?>
<rdf:RDF
   xmlns:cc="http://creativecommons.org/ns#"
   xmlns:dcterms="http://purl.org/dc/terms/"
   xmlns:rdf="http://www.w3.org/1999/02/22-rdf-syntax-ns#"
   xmlns:skos="http://www.w3.org/2004/02/skos/core#"
>
  <rdf:Description rdf:about="http://purl.org/heritagedata/schemes/560/concepts/142981">
    <cc:attributionName xml:lang="en">Historic England</cc:attributionName>
    <cc:license rdf:resource="http://creativecommons.org/licenses/by/3.0"/>
    <dcterms:issued rdf:datatype="http://www.w3.org/2001/XMLSchema#dateTime">2019-05-23T13:12:18</dcterms:issued>
    <skos:inScheme rdf:resource="http://purl.org/heritagedata/schemes/560"/>
    <skos:prefLabel xml:lang="en">Beach Deposit</skos:prefLabel>
    <cc:attributionURL rdf:resource="http://www.historicengland.org.uk"/>
    <dcterms:identifier>http://purl.org/heritagedata/schemes/560/concepts/142981</dcterms:identifier>
    <rdf:type rdf:resource="http://www.w3.org/2004/02/skos/core#Concept"/>
    <dcterms:publisher rdf:resource="http://www.historicengland.org.uk"/>
    <skos:scopeNote xml:lang="en">A deposit formed by wave and tidal action on an estuarine or marine beach.</skos:scopeNote>
  </rdf:Description>
  <rdf:Description rdf:about="http://purl.org/heritagedata/schemes/560/concepts/170616">
    <skos:inScheme rdf:resource="http://purl.org/heritagedata/schemes/560"/>
    <cc:license rdf:resource="http://creativecommons.org/licenses/by/3.0"/>
    <rdf:type rdf:resource="http://www.w3.org/2004/02/skos/core#Concept"/>
    <dcterms:identifier>http://purl.org/heritagedata/schemes/560/concepts/170616</dcterms:identifier>
    <dcterms:publisher rdf:resource="http://www.historicengland.org.uk"/>
    <dcterms:issued rdf:datatype="http://www.w3.org/2001/XMLSchema#dateTime">2019-05-23T13:12:18</dcterms:issued>
    <cc:attributionURL rdf:resource="http://www.historicengland.org.uk"/>
    <cc:attributionName xml:lang="en">Historic England</cc:attributionName>
    <skos:prefLabel xml:lang="en">Zooarchaeology</skos:prefLabel>
    <skos:scopeNote xml:lang="en">The study of vertebrate remains, excluding human remains, preserved within archaeological deposits and palaeoenvironmental archives. Use archaeomalacology for the study of mollus remains and palaeoentomology for the study of insect remains.</skos:scopeNote>
  </rdf:Description>
  <rdf:Description rdf:about="http://purl.org/heritagedata/schemes/560/concepts/142117">
    <skos:scopeNote xml:lang="en">Wood that has been burnt and largely reduced to carbon as a result of burning in a reducing atmosphere below 500 degress C (Celsius).</skos:scopeNote>
    <skos:related rdf:resource="http://purl.org/heritagedata/schemes/560/concepts/142118"/>
    <cc:license rdf:resource="http://creativecommons.org/licenses/by/3.0"/>
    <cc:attributionName xml:lang="en">Historic England</cc:attributionName>
    <skos:inScheme rdf:resource="http://purl.org/heritagedata/schemes/560"/>
    <dcterms:issued rdf:datatype="http://www.w3.org/2001/XMLSchema#dateTime">2019-05-23T13:12:18</dcterms:issued>
    <dcterms:identifier>http://purl.org/heritagedata/schemes/560/concepts/142117</dcterms:identifier>
    <dcterms:publisher rdf:resource="http://www.historicengland.org.uk"/>
    <skos:prefLabel xml:lang="en">Charcoal</skos:prefLabel>
    <cc:attributionURL rdf:resource="http://www.historicengland.org.uk"/>
    <rdf:type rdf:resource="http://www.w3.org/2004/02/skos/core#Concept"/>
  </rdf:Description>
  <rdf:Description rdf:about="http://purl.org/heritagedata/schemes/560/concepts/144523">
    <dcterms:publisher rdf:resource="http://www.historicengland.org.uk"/>
    <skos:prefLabel xml:lang="en">Polymineral</skos:prefLabel>
    <cc:attributionURL rdf:resource="http://www.historicengland.org.uk"/>
    <cc:attributionName xml:lang="en">Historic England</cc:attributionName>
    <dcterms:identifier>http://purl.org/heritagedata/schemes/560/concepts/144523</dcterms:identifier>
    <skos:inScheme rdf:resource="http://purl.org/heritagedata/schemes/560"/>
    <cc:license rdf:resource="http://creativecommons.org/licenses/by/3.0"/>
    <rdf:type rdf:resource="http://www.w3.org/2004/02/skos/core#Concept"/>
    <dcterms:issued rdf:datatype="http://www.w3.org/2001/XMLSchema#dateTime">2019-05-23T13:12:18</dcterms:issued>
    <skos:scopeNote xml:lang="en">A general term to describe a sediment or sample that contains a variety of different minerals.</skos:scopeNote>
  </rdf:Description>
  <rdf:Description rdf:about="http://purl.org/heritagedata/schemes/560/concepts/142166">
    <skos:scopeNote xml:lang="en">Preservation of material by toxic effect of corrosion products in the immediate vicinity, or within, the material.</skos:scopeNote>
    <dcterms:publisher rdf:resource="http://www.historicengland.org.uk"/>
    <cc:attributionURL rdf:resource="http://www.historicengland.org.uk"/>
    <rdf:type rdf:resource="http://www.w3.org/2004/02/skos/core#Concept"/>
    <skos:inScheme rdf:resource="http://purl.org/heritagedata/schemes/560"/>
    <skos:prefLabel xml:lang="en">Mineral Preserved</skos:prefLabel>
    <dcterms:issued rdf:datatype="http://www.w3.org/2001/XMLSchema#dateTime">2019-05-23T13:12:18</dcterms:issued>
    <dcterms:identifier>http://purl.org/heritagedata/schemes/560/concepts/142166</dcterms:identifier>
    <cc:license rdf:resource="http://creativecommons.org/licenses/by/3.0"/>
    <cc:attributionName xml:lang="en">Historic England</cc:attributionName>
  </rdf:Description>
  <rdf:Description rdf:about="http://purl.org/heritagedata/schemes/560/concepts/142134">
    <skos:altLabel xml:lang="en">Diseased</skos:altLabel>
  </rdf:Description>
  <rdf:Description rdf:about="http://purl.org/heritagedata/schemes/560/concepts/142118">
    <skos:scopeNote xml:lang="en">Material that has been burnt and at least in part reduced to carbon as a result of burning in a reducing atmosphere below 500 degrees Celsius.</skos:scopeNote>
    <skos:inScheme rdf:resource="http://purl.org/heritagedata/schemes/560"/>
    <skos:prefLabel xml:lang="en">Charred</skos:prefLabel>
    <cc:license rdf:resource="http://creativecommons.org/licenses/by/3.0"/>
    <rdf:type rdf:resource="http://www.w3.org/2004/02/skos/core#Concept"/>
    <dcterms:identifier>http://purl.org/heritagedata/schemes/560/concepts/142118</dcterms:identifier>
    <skos:related rdf:resource="http://purl.org/heritagedata/schemes/560/concepts/142117"/>
    <dcterms:publisher rdf:resource="http://www.historicengland.org.uk"/>
    <cc:attributionURL rdf:resource="http://www.historicengland.org.uk"/>
    <cc:attributionName xml:lang="en">Historic England</cc:attributionName>
    <dcterms:issued rdf:datatype="http://www.w3.org/2001/XMLSchema#dateTime">2019-05-23T13:12:18</dcterms:issued>
  </rdf:Description>
  <rdf:Description rdf:about="http://purl.org/heritagedata/schemes/560/concepts/142152">
    <dcterms:identifier>http://purl.org/heritagedata/schemes/560/concepts/142152</dcterms:identifier>
    <cc:license rdf:resource="http://creativecommons.org/licenses/by/3.0"/>
    <skos:prefLabel xml:lang="en">Inorganic Phosphorus Analysis</skos:prefLabel>
    <cc:attributionURL rdf:resource="http://www.historicengland.org.uk"/>
    <dcterms:issued rdf:datatype="http://www.w3.org/2001/XMLSchema#dateTime">2019-05-23T13:12:18</dcterms:issued>
    <rdf:type rdf:resource="http://www.w3.org/2004/02/skos/core#Concept"/>
    <cc:attributionName xml:lang="en">Historic England</cc:attributionName>
    <skos:scopeNote xml:lang="en">The analysis of inorganic phosphorus (P).</skos:scopeNote>
    <dcterms:publisher rdf:resource="http://www.historicengland.org.uk"/>
    <skos:inScheme rdf:resource="http://purl.org/heritagedata/schemes/560"/>
  </rdf:Description>
  <rdf:Description rdf:about="http://purl.org/heritagedata/schemes/560/concepts/142212">
    <cc:license rdf:resource="http://creativecommons.org/licenses/by/3.0"/>
    <cc:attributionName xml:lang="en">Historic England</cc:attributionName>
    <skos:prefLabel xml:lang="en">Uranium Series Dating</skos:prefLabel>
    <dcterms:issued rdf:datatype="http://www.w3.org/2001/XMLSchema#dateTime">2019-05-23T13:12:18</dcterms:issued>
    <rdf:type rdf:resource="http://www.w3.org/2004/02/skos/core#Concept"/>
    <cc:attributionURL rdf:resource="http://www.historicengland.org.uk"/>
    <dcterms:identifier>http://purl.org/heritagedata/schemes/560/concepts/142212</dcterms:identifier>
    <dcterms:publisher rdf:resource="http://www.historicengland.org.uk"/>
    <skos:inScheme rdf:resource="http://purl.org/heritagedata/schemes/560"/>
    <skos:scopeNote xml:lang="en">The measurement of the decay of radioactive uranium (U) isotopes. Particularly useful for dating calcite and sometimes bone, tooth and shell up to 70,000 years old.</skos:scopeNote>
  </rdf:Description>
  <rdf:Description rdf:about="http://purl.org/heritagedata/schemes/560/concepts/142142">
    <skos:prefLabel xml:lang="en">Fluorine, Uranium And Nitrogen Tests</skos:prefLabel>
    <cc:attributionName xml:lang="en">Historic England</cc:attributionName>
    <cc:attributionURL rdf:resource="http://www.historicengland.org.uk"/>
    <skos:scopeNote xml:lang="en">A relative dating technique for assessing bones from the same deposit. Often used to check for contemporaneity of bones selected for radiocarbon dating or to check for hoaxes such as the Piltdown Man.</skos:scopeNote>
    <dcterms:publisher rdf:resource="http://www.historicengland.org.uk"/>
    <skos:inScheme rdf:resource="http://purl.org/heritagedata/schemes/560"/>
    <rdf:type rdf:resource="http://www.w3.org/2004/02/skos/core#Concept"/>
    <dcterms:issued rdf:datatype="http://www.w3.org/2001/XMLSchema#dateTime">2019-05-23T13:12:18</dcterms:issued>
    <dcterms:identifier>http://purl.org/heritagedata/schemes/560/concepts/142142</dcterms:identifier>
    <cc:license rdf:resource="http://creativecommons.org/licenses/by/3.0"/>
  </rdf:Description>
  <rdf:Description rdf:about="http://purl.org/heritagedata/schemes/560/concepts/142180">
    <skos:scopeNote xml:lang="en">Use for bone remodelling, new growth, loss or destruction caused by age, activity, disease or trauma during life.</skos:scopeNote>
    <cc:attributionURL rdf:resource="http://www.historicengland.org.uk"/>
    <dcterms:issued rdf:datatype="http://www.w3.org/2001/XMLSchema#dateTime">2019-05-23T13:12:18</dcterms:issued>
    <skos:inScheme rdf:resource="http://purl.org/heritagedata/schemes/560"/>
    <skos:prefLabel xml:lang="en">Pathology</skos:prefLabel>
    <dcterms:publisher rdf:resource="http://www.historicengland.org.uk"/>
    <rdf:type rdf:resource="http://www.w3.org/2004/02/skos/core#Concept"/>
    <dcterms:identifier>http://purl.org/heritagedata/schemes/560/concepts/142180</dcterms:identifier>
    <cc:attributionName xml:lang="en">Historic England</cc:attributionName>
    <cc:license rdf:resource="http://creativecommons.org/licenses/by/3.0"/>
  </rdf:Description>
  <rdf:Description rdf:about="http://purl.org/heritagedata/schemes/560/concepts/142980">
    <dcterms:identifier>http://purl.org/heritagedata/schemes/560/concepts/142980</dcterms:identifier>
    <skos:prefLabel xml:lang="en">Peat Deposit</skos:prefLabel>
    <dcterms:issued rdf:datatype="http://www.w3.org/2001/XMLSchema#dateTime">2019-05-23T13:12:18</dcterms:issued>
    <cc:attributionName xml:lang="en">Historic England</cc:attributionName>
    <dcterms:publisher rdf:resource="http://www.historicengland.org.uk"/>
    <cc:license rdf:resource="http://creativecommons.org/licenses/by/3.0"/>
    <rdf:type rdf:resource="http://www.w3.org/2004/02/skos/core#Concept"/>
    <skos:scopeNote xml:lang="en">A naturally occurring deposit formed by the decomposition and partial carbonisation of vegetable matter in waterlogged conditions.</skos:scopeNote>
    <skos:inScheme rdf:resource="http://purl.org/heritagedata/schemes/560"/>
    <cc:attributionURL rdf:resource="http://www.historicengland.org.uk"/>
  </rdf:Description>
  <rdf:Description rdf:about="http://purl.org/heritagedata/schemes/560/concepts/142137">
    <dcterms:issued rdf:datatype="http://www.w3.org/2001/XMLSchema#dateTime">2019-05-23T13:12:18</dcterms:issued>
    <skos:prefLabel xml:lang="en">Feather</skos:prefLabel>
    <cc:license rdf:resource="http://creativecommons.org/licenses/by/3.0"/>
    <rdf:type rdf:resource="http://www.w3.org/2004/02/skos/core#Concept"/>
    <dcterms:identifier>http://purl.org/heritagedata/schemes/560/concepts/142137</dcterms:identifier>
    <dcterms:publisher rdf:resource="http://www.historicengland.org.uk"/>
    <cc:attributionURL rdf:resource="http://www.historicengland.org.uk"/>
    <cc:attributionName xml:lang="en">Historic England</cc:attributionName>
    <skos:inScheme rdf:resource="http://purl.org/heritagedata/schemes/560"/>
    <skos:scopeNote xml:lang="en">Use for feathers, an epidermal growth found in birds consisting of a quill, shaft and two vanes of barbs.</skos:scopeNote>
  </rdf:Description>
  <rdf:Description rdf:about="http://purl.org/heritagedata/schemes/560/concepts/142119">
    <dcterms:publisher rdf:resource="http://www.historicengland.org.uk"/>
    <skos:prefLabel xml:lang="en">Chemical Techniques</skos:prefLabel>
    <cc:attributionURL rdf:resource="http://www.historicengland.org.uk"/>
    <cc:attributionName xml:lang="en">Historic England</cc:attributionName>
    <skos:scopeNote xml:lang="en">Examination of a material using chemical means.</skos:scopeNote>
    <skos:inScheme rdf:resource="http://purl.org/heritagedata/schemes/560"/>
    <dcterms:identifier>http://purl.org/heritagedata/schemes/560/concepts/142119</dcterms:identifier>
    <dcterms:issued rdf:datatype="http://www.w3.org/2001/XMLSchema#dateTime">2019-05-23T13:12:18</dcterms:issued>
    <cc:license rdf:resource="http://creativecommons.org/licenses/by/3.0"/>
    <rdf:type rdf:resource="http://www.w3.org/2004/02/skos/core#Concept"/>
  </rdf:Description>
  <rdf:Description rdf:about="http://purl.org/heritagedata/schemes/560/concepts/142147">
    <rdf:type rdf:resource="http://www.w3.org/2004/02/skos/core#Concept"/>
    <dcterms:issued rdf:datatype="http://www.w3.org/2001/XMLSchema#dateTime">2019-05-23T13:12:18</dcterms:issued>
    <skos:inScheme rdf:resource="http://purl.org/heritagedata/schemes/560"/>
    <dcterms:identifier>http://purl.org/heritagedata/schemes/560/concepts/142147</dcterms:identifier>
    <skos:scopeNote xml:lang="en">The retrieval of material from deposits by hand, normally large objects visible with the naked eye, eg. Mammal remains and marine molluscs.</skos:scopeNote>
    <cc:license rdf:resource="http://creativecommons.org/licenses/by/3.0"/>
    <cc:attributionName xml:lang="en">Historic England</cc:attributionName>
    <cc:attributionURL rdf:resource="http://www.historicengland.org.uk"/>
    <dcterms:publisher rdf:resource="http://www.historicengland.org.uk"/>
    <skos:prefLabel xml:lang="en">Hand Retrieval</skos:prefLabel>
  </rdf:Description>
  <rdf:Description rdf:about="http://purl.org/heritagedata/schemes/560/concepts/142124">
    <cc:license rdf:resource="http://creativecommons.org/licenses/by/3.0"/>
    <skos:prefLabel xml:lang="en">Coloured</skos:prefLabel>
    <cc:attributionName xml:lang="en">Historic England</cc:attributionName>
    <dcterms:issued rdf:datatype="http://www.w3.org/2001/XMLSchema#dateTime">2019-05-23T13:12:18</dcterms:issued>
    <rdf:type rdf:resource="http://www.w3.org/2004/02/skos/core#Concept"/>
    <cc:attributionURL rdf:resource="http://www.historicengland.org.uk"/>
    <skos:scopeNote xml:lang="en">Material with evidence of the application of a pigment or dye.</skos:scopeNote>
    <dcterms:identifier>http://purl.org/heritagedata/schemes/560/concepts/142124</dcterms:identifier>
    <dcterms:publisher rdf:resource="http://www.historicengland.org.uk"/>
    <skos:inScheme rdf:resource="http://purl.org/heritagedata/schemes/560"/>
  </rdf:Description>
  <rdf:Description rdf:about="http://purl.org/heritagedata/schemes/560/concepts/142182">
    <cc:attributionURL rdf:resource="http://www.historicengland.org.uk"/>
    <cc:attributionName xml:lang="en">Historic England</cc:attributionName>
    <skos:prefLabel xml:lang="en">Physical Techniques</skos:prefLabel>
    <skos:scopeNote xml:lang="en">The examination of material by physical means, including detailed observation.</skos:scopeNote>
    <dcterms:issued rdf:datatype="http://www.w3.org/2001/XMLSchema#dateTime">2019-05-23T13:12:18</dcterms:issued>
    <cc:license rdf:resource="http://creativecommons.org/licenses/by/3.0"/>
    <rdf:type rdf:resource="http://www.w3.org/2004/02/skos/core#Concept"/>
    <skos:inScheme rdf:resource="http://purl.org/heritagedata/schemes/560"/>
    <dcterms:publisher rdf:resource="http://www.historicengland.org.uk"/>
    <dcterms:identifier>http://purl.org/heritagedata/schemes/560/concepts/142182</dcterms:identifier>
  </rdf:Description>
  <rdf:Description rdf:about="http://purl.org/heritagedata/schemes/560/concepts/142173">
    <skos:prefLabel xml:lang="en">Natural Aspects</skos:prefLabel>
    <dcterms:publisher rdf:resource="http://www.historicengland.org.uk"/>
    <cc:attributionName xml:lang="en">Historic England</cc:attributionName>
    <cc:license rdf:resource="http://creativecommons.org/licenses/by/3.0"/>
    <skos:inScheme rdf:resource="http://purl.org/heritagedata/schemes/560"/>
    <skos:scopeNote xml:lang="en">Aspects associated with the genetic make up and/or factors that affected the organism from which the material is derived during its life</skos:scopeNote>
    <dcterms:identifier>http://purl.org/heritagedata/schemes/560/concepts/142173</dcterms:identifier>
    <cc:attributionURL rdf:resource="http://www.historicengland.org.uk"/>
    <dcterms:issued rdf:datatype="http://www.w3.org/2001/XMLSchema#dateTime">2019-05-23T13:12:18</dcterms:issued>
    <rdf:type rdf:resource="http://www.w3.org/2004/02/skos/core#Concept"/>
  </rdf:Description>
  <rdf:Description rdf:about="http://purl.org/heritagedata/schemes/560/concepts/142132">
    <dcterms:identifier>http://purl.org/heritagedata/schemes/560/concepts/142132</dcterms:identifier>
    <dcterms:publisher rdf:resource="http://www.historicengland.org.uk"/>
    <skos:prefLabel xml:lang="en">Desiccated</skos:prefLabel>
    <cc:license rdf:resource="http://creativecommons.org/licenses/by/3.0"/>
    <rdf:type rdf:resource="http://www.w3.org/2004/02/skos/core#Concept"/>
    <dcterms:issued rdf:datatype="http://www.w3.org/2001/XMLSchema#dateTime">2019-05-23T13:12:18</dcterms:issued>
    <cc:attributionURL rdf:resource="http://www.historicengland.org.uk"/>
    <skos:inScheme rdf:resource="http://purl.org/heritagedata/schemes/560"/>
    <skos:scopeNote xml:lang="en">Material preserved due to very low humidity which inhibits decay by micro-organisms.</skos:scopeNote>
    <cc:attributionName xml:lang="en">Historic England</cc:attributionName>
  </rdf:Description>
  <rdf:Description rdf:about="http://purl.org/heritagedata/schemes/560/concepts/144516">
    <skos:inScheme rdf:resource="http://purl.org/heritagedata/schemes/560"/>
    <dcterms:issued rdf:datatype="http://www.w3.org/2001/XMLSchema#dateTime">2019-05-23T13:12:18</dcterms:issued>
    <dcterms:identifier>http://purl.org/heritagedata/schemes/560/concepts/144516</dcterms:identifier>
    <cc:attributionURL rdf:resource="http://www.historicengland.org.uk"/>
    <dcterms:publisher rdf:resource="http://www.historicengland.org.uk"/>
    <cc:license rdf:resource="http://creativecommons.org/licenses/by/3.0"/>
    <rdf:type rdf:resource="http://www.w3.org/2004/02/skos/core#Concept"/>
    <cc:attributionName xml:lang="en">Historic England</cc:attributionName>
    <skos:scopeNote xml:lang="en">Object produced commonly by firing clay, but can include coarser material to temper it.</skos:scopeNote>
    <skos:prefLabel xml:lang="en">Pottery</skos:prefLabel>
  </rdf:Description>
  <rdf:Description rdf:about="http://purl.org/heritagedata/schemes/560/concepts/142109">
    <rdf:type rdf:resource="http://www.w3.org/2004/02/skos/core#Concept"/>
    <dcterms:issued rdf:datatype="http://www.w3.org/2001/XMLSchema#dateTime">2019-05-23T13:12:18</dcterms:issued>
    <skos:inScheme rdf:resource="http://purl.org/heritagedata/schemes/560"/>
    <dcterms:identifier>http://purl.org/heritagedata/schemes/560/concepts/142109</dcterms:identifier>
    <skos:prefLabel xml:lang="en">Bone</skos:prefLabel>
    <cc:license rdf:resource="http://creativecommons.org/licenses/by/3.0"/>
    <cc:attributionName xml:lang="en">Historic England</cc:attributionName>
    <cc:attributionURL rdf:resource="http://www.historicengland.org.uk"/>
    <skos:scopeNote xml:lang="en">Any of the pieces of hard tissue consisting largely of calcium phosphate that make up the skeleton of a vertebrate animal.</skos:scopeNote>
    <dcterms:publisher rdf:resource="http://www.historicengland.org.uk"/>
  </rdf:Description>
  <rdf:Description rdf:about="http://purl.org/heritagedata/schemes/560/concepts/142156">
    <cc:attributionName xml:lang="en">Historic England</cc:attributionName>
    <cc:attributionURL rdf:resource="http://www.historicengland.org.uk"/>
    <skos:related rdf:resource="http://purl.org/heritagedata/schemes/560/concepts/142196"/>
    <dcterms:publisher rdf:resource="http://www.historicengland.org.uk"/>
    <dcterms:identifier>http://purl.org/heritagedata/schemes/560/concepts/142156</dcterms:identifier>
    <skos:inScheme rdf:resource="http://purl.org/heritagedata/schemes/560"/>
    <rdf:type rdf:resource="http://www.w3.org/2004/02/skos/core#Concept"/>
    <dcterms:issued rdf:datatype="http://www.w3.org/2001/XMLSchema#dateTime">2019-05-23T13:12:18</dcterms:issued>
    <cc:license rdf:resource="http://creativecommons.org/licenses/by/3.0"/>
    <skos:prefLabel xml:lang="en">Leather</skos:prefLabel>
    <skos:scopeNote xml:lang="en">Animal skin that has been tanned or tawed.</skos:scopeNote>
  </rdf:Description>
  <rdf:Description rdf:about="http://purl.org/heritagedata/schemes/560/concepts/142143">
    <skos:altLabel xml:lang="en">Fossilised</skos:altLabel>
  </rdf:Description>
  <rdf:Description rdf:about="http://purl.org/heritagedata/schemes/560/concepts/142139">
    <skos:scopeNote xml:lang="en">Use for any thread-like material.</skos:scopeNote>
    <cc:attributionURL rdf:resource="http://www.historicengland.org.uk"/>
    <dcterms:identifier>http://purl.org/heritagedata/schemes/560/concepts/142139</dcterms:identifier>
    <cc:attributionName xml:lang="en">Historic England</cc:attributionName>
    <dcterms:issued rdf:datatype="http://www.w3.org/2001/XMLSchema#dateTime">2019-05-23T13:12:18</dcterms:issued>
    <skos:inScheme rdf:resource="http://purl.org/heritagedata/schemes/560"/>
    <cc:license rdf:resource="http://creativecommons.org/licenses/by/3.0"/>
    <rdf:type rdf:resource="http://www.w3.org/2004/02/skos/core#Concept"/>
    <skos:prefLabel xml:lang="en">Fibre</skos:prefLabel>
    <dcterms:publisher rdf:resource="http://www.historicengland.org.uk"/>
  </rdf:Description>
  <rdf:Description rdf:about="http://purl.org/heritagedata/schemes/560/concepts/170620">
    <skos:inScheme rdf:resource="http://purl.org/heritagedata/schemes/560"/>
    <dcterms:issued rdf:datatype="http://www.w3.org/2001/XMLSchema#dateTime">2019-05-23T13:12:18</dcterms:issued>
    <cc:attributionName xml:lang="en">Historic England</cc:attributionName>
    <dcterms:identifier>http://purl.org/heritagedata/schemes/560/concepts/170620</dcterms:identifier>
    <cc:attributionURL rdf:resource="http://www.historicengland.org.uk"/>
    <dcterms:publisher rdf:resource="http://www.historicengland.org.uk"/>
    <cc:license rdf:resource="http://creativecommons.org/licenses/by/3.0"/>
    <rdf:type rdf:resource="http://www.w3.org/2004/02/skos/core#Concept"/>
    <skos:prefLabel xml:lang="en">Palaeoentomology</skos:prefLabel>
    <skos:scopeNote xml:lang="en">The study of insect remains preserved within archaeological deposits and palaeoenvironmental archives.</skos:scopeNote>
  </rdf:Description>
  <rdf:Description rdf:about="http://purl.org/heritagedata/schemes/560/concepts/142105">
    <dcterms:identifier>http://purl.org/heritagedata/schemes/560/concepts/142105</dcterms:identifier>
    <skos:inScheme rdf:resource="http://purl.org/heritagedata/schemes/560"/>
    <dcterms:publisher rdf:resource="http://www.historicengland.org.uk"/>
    <rdf:type rdf:resource="http://www.w3.org/2004/02/skos/core#Concept"/>
    <cc:license rdf:resource="http://creativecommons.org/licenses/by/3.0"/>
    <skos:topConceptOf rdf:resource="http://purl.org/heritagedata/schemes/560"/>
    <cc:attributionName xml:lang="en">Historic England</cc:attributionName>
    <dcterms:issued rdf:datatype="http://www.w3.org/2001/XMLSchema#dateTime">2019-05-23T13:12:18</dcterms:issued>
    <skos:prefLabel xml:lang="en">Aspect</skos:prefLabel>
    <cc:attributionURL rdf:resource="http://www.historicengland.org.uk"/>
  </rdf:Description>
  <rdf:Description rdf:about="http://purl.org/heritagedata/schemes/560/concepts/142157">
    <cc:attributionURL rdf:resource="http://www.historicengland.org.uk"/>
    <skos:inScheme rdf:resource="http://purl.org/heritagedata/schemes/560"/>
    <rdf:type rdf:resource="http://www.w3.org/2004/02/skos/core#Concept"/>
    <dcterms:issued rdf:datatype="http://www.w3.org/2001/XMLSchema#dateTime">2019-05-23T13:12:18</dcterms:issued>
    <dcterms:publisher rdf:resource="http://www.historicengland.org.uk"/>
    <dcterms:identifier>http://purl.org/heritagedata/schemes/560/concepts/142157</dcterms:identifier>
    <skos:scopeNote xml:lang="en">The weight loss from low-temperature burning of material. It correlates well with organic matter (material derived from living things) content.</skos:scopeNote>
    <cc:attributionName xml:lang="en">Historic England</cc:attributionName>
    <cc:license rdf:resource="http://creativecommons.org/licenses/by/3.0"/>
    <skos:prefLabel xml:lang="en">Loss On Ignition Determination</skos:prefLabel>
  </rdf:Description>
  <rdf:Description rdf:about="http://purl.org/heritagedata/schemes/560/concepts/142185">
    <cc:license rdf:resource="http://creativecommons.org/licenses/by/3.0"/>
    <skos:inScheme rdf:resource="http://purl.org/heritagedata/schemes/560"/>
    <cc:attributionName xml:lang="en">Historic England</cc:attributionName>
    <cc:attributionURL rdf:resource="http://www.historicengland.org.uk"/>
    <skos:scopeNote xml:lang="en">Light microscopy in which vibration directions of the light are constrained into single planes.</skos:scopeNote>
    <dcterms:publisher rdf:resource="http://www.historicengland.org.uk"/>
    <rdf:type rdf:resource="http://www.w3.org/2004/02/skos/core#Concept"/>
    <dcterms:issued rdf:datatype="http://www.w3.org/2001/XMLSchema#dateTime">2019-05-23T13:12:18</dcterms:issued>
    <dcterms:identifier>http://purl.org/heritagedata/schemes/560/concepts/142185</dcterms:identifier>
    <skos:prefLabel xml:lang="en">Polarised Light Microscopy</skos:prefLabel>
  </rdf:Description>
  <rdf:Description rdf:about="http://purl.org/heritagedata/schemes/560/concepts/142202">
    <dcterms:identifier>http://purl.org/heritagedata/schemes/560/concepts/142202</dcterms:identifier>
    <skos:prefLabel xml:lang="en">Tephrochronology</skos:prefLabel>
    <skos:scopeNote xml:lang="en">The use of ash and tephra deposits characteristic of single known-date volcanic eruptions to date stratigraphic sequences.</skos:scopeNote>
    <cc:license rdf:resource="http://creativecommons.org/licenses/by/3.0"/>
    <cc:attributionName xml:lang="en">Historic England</cc:attributionName>
    <skos:inScheme rdf:resource="http://purl.org/heritagedata/schemes/560"/>
    <dcterms:issued rdf:datatype="http://www.w3.org/2001/XMLSchema#dateTime">2019-05-23T13:12:18</dcterms:issued>
    <dcterms:publisher rdf:resource="http://www.historicengland.org.uk"/>
    <cc:attributionURL rdf:resource="http://www.historicengland.org.uk"/>
    <rdf:type rdf:resource="http://www.w3.org/2004/02/skos/core#Concept"/>
  </rdf:Description>
  <rdf:Description rdf:about="http://purl.org/heritagedata/schemes/560/concepts/144520">
    <dcterms:issued rdf:datatype="http://www.w3.org/2001/XMLSchema#dateTime">2019-05-23T13:12:18</dcterms:issued>
    <cc:license rdf:resource="http://creativecommons.org/licenses/by/3.0"/>
    <dcterms:identifier>http://purl.org/heritagedata/schemes/560/concepts/144520</dcterms:identifier>
    <rdf:type rdf:resource="http://www.w3.org/2004/02/skos/core#Concept"/>
    <skos:scopeNote xml:lang="en">A mineral composed of SiO2. Commonly clear or milky in appearance. A common constituent of rocks and sediments.</skos:scopeNote>
    <dcterms:publisher rdf:resource="http://www.historicengland.org.uk"/>
    <skos:inScheme rdf:resource="http://purl.org/heritagedata/schemes/560"/>
    <cc:attributionName xml:lang="en">Historic England</cc:attributionName>
    <cc:attributionURL rdf:resource="http://www.historicengland.org.uk"/>
    <skos:prefLabel xml:lang="en">Quartz</skos:prefLabel>
  </rdf:Description>
  <rdf:Description rdf:about="http://purl.org/heritagedata/schemes/560/concepts/142208">
    <dcterms:publisher rdf:resource="http://www.historicengland.org.uk"/>
    <cc:attributionURL rdf:resource="http://www.historicengland.org.uk"/>
    <skos:prefLabel xml:lang="en">Total Phosphorus Analysis</skos:prefLabel>
    <cc:attributionName xml:lang="en">Historic England</cc:attributionName>
    <cc:license rdf:resource="http://creativecommons.org/licenses/by/3.0"/>
    <dcterms:issued rdf:datatype="http://www.w3.org/2001/XMLSchema#dateTime">2019-05-23T13:12:18</dcterms:issued>
    <dcterms:identifier>http://purl.org/heritagedata/schemes/560/concepts/142208</dcterms:identifier>
    <skos:scopeNote xml:lang="en">The analysis of organic plus inorganic phosphorus (P).</skos:scopeNote>
    <skos:inScheme rdf:resource="http://purl.org/heritagedata/schemes/560"/>
    <rdf:type rdf:resource="http://www.w3.org/2004/02/skos/core#Concept"/>
  </rdf:Description>
  <rdf:Description rdf:about="http://purl.org/heritagedata/schemes/560/concepts/142150">
    <dcterms:identifier>http://purl.org/heritagedata/schemes/560/concepts/142150</dcterms:identifier>
    <skos:inScheme rdf:resource="http://purl.org/heritagedata/schemes/560"/>
    <cc:license rdf:resource="http://creativecommons.org/licenses/by/3.0"/>
    <rdf:type rdf:resource="http://www.w3.org/2004/02/skos/core#Concept"/>
    <skos:prefLabel xml:lang="en">Impression</skos:prefLabel>
    <skos:scopeNote xml:lang="en">The negative trace left by an object type or material (eg. animal, plant or textile) on another object type or material, often on ceramics or metal corrosion products.</skos:scopeNote>
    <dcterms:issued rdf:datatype="http://www.w3.org/2001/XMLSchema#dateTime">2019-05-23T13:12:18</dcterms:issued>
    <cc:attributionName xml:lang="en">Historic England</cc:attributionName>
    <cc:attributionURL rdf:resource="http://www.historicengland.org.uk"/>
    <dcterms:publisher rdf:resource="http://www.historicengland.org.uk"/>
  </rdf:Description>
  <rdf:Description rdf:about="http://purl.org/heritagedata/schemes/560/concepts/142191">
    <skos:scopeNote xml:lang="en">A process using an electron microscope in which the surface of the specimen is scanned by a beam of electrons which are reflected to form an image. Very high magnification is possible.</skos:scopeNote>
    <dcterms:publisher rdf:resource="http://www.historicengland.org.uk"/>
    <dcterms:identifier>http://purl.org/heritagedata/schemes/560/concepts/142191</dcterms:identifier>
    <cc:attributionName xml:lang="en">Historic England</cc:attributionName>
    <cc:attributionURL rdf:resource="http://www.historicengland.org.uk"/>
    <skos:inScheme rdf:resource="http://purl.org/heritagedata/schemes/560"/>
    <dcterms:issued rdf:datatype="http://www.w3.org/2001/XMLSchema#dateTime">2019-05-23T13:12:18</dcterms:issued>
    <cc:license rdf:resource="http://creativecommons.org/licenses/by/3.0"/>
    <skos:prefLabel xml:lang="en">Scanning Electron Microscopy</skos:prefLabel>
    <rdf:type rdf:resource="http://www.w3.org/2004/02/skos/core#Concept"/>
  </rdf:Description>
  <rdf:Description rdf:about="http://purl.org/heritagedata/schemes/560/concepts/142155">
    <cc:attributionName xml:lang="en">Historic England</cc:attributionName>
    <skos:prefLabel xml:lang="en">Lead Isotope Dating</skos:prefLabel>
    <dcterms:issued rdf:datatype="http://www.w3.org/2001/XMLSchema#dateTime">2019-05-23T13:12:18</dcterms:issued>
    <skos:inScheme rdf:resource="http://purl.org/heritagedata/schemes/560"/>
    <cc:attributionURL rdf:resource="http://www.historicengland.org.uk"/>
    <rdf:type rdf:resource="http://www.w3.org/2004/02/skos/core#Concept"/>
    <skos:scopeNote xml:lang="en">A technique which uses the measurement of decay in radioactive lead (Pb) isotopes to determine a date. Useful for sediments and lead-based paints between 1 and 400 years old.</skos:scopeNote>
    <dcterms:identifier>http://purl.org/heritagedata/schemes/560/concepts/142155</dcterms:identifier>
    <dcterms:publisher rdf:resource="http://www.historicengland.org.uk"/>
    <cc:license rdf:resource="http://creativecommons.org/licenses/by/3.0"/>
  </rdf:Description>
  <rdf:Description rdf:about="http://purl.org/heritagedata/schemes/560/concepts/170642">
    <dcterms:identifier>http://purl.org/heritagedata/schemes/560/concepts/170642</dcterms:identifier>
    <dcterms:publisher rdf:resource="http://www.historicengland.org.uk"/>
    <cc:attributionURL rdf:resource="http://www.historicengland.org.uk"/>
    <rdf:type rdf:resource="http://www.w3.org/2004/02/skos/core#Concept"/>
    <skos:prefLabel xml:lang="en">Slag</skos:prefLabel>
    <skos:inScheme rdf:resource="http://purl.org/heritagedata/schemes/560"/>
    <skos:scopeNote xml:lang="en">A by-product usually from the smelting process.</skos:scopeNote>
    <dcterms:issued rdf:datatype="http://www.w3.org/2001/XMLSchema#dateTime">2019-05-23T13:12:18</dcterms:issued>
    <cc:license rdf:resource="http://creativecommons.org/licenses/by/3.0"/>
    <cc:attributionName xml:lang="en">Historic England</cc:attributionName>
  </rdf:Description>
  <rdf:Description rdf:about="http://purl.org/heritagedata/schemes/560/concepts/142149">
    <rdf:type rdf:resource="http://www.w3.org/2004/02/skos/core#Concept"/>
    <dcterms:identifier>http://purl.org/heritagedata/schemes/560/concepts/142149</dcterms:identifier>
    <skos:inScheme rdf:resource="http://purl.org/heritagedata/schemes/560"/>
    <dcterms:issued rdf:datatype="http://www.w3.org/2001/XMLSchema#dateTime">2019-05-23T13:12:18</dcterms:issued>
    <cc:license rdf:resource="http://creativecommons.org/licenses/by/3.0"/>
    <cc:attributionName xml:lang="en">Historic England</cc:attributionName>
    <cc:attributionURL rdf:resource="http://www.historicengland.org.uk"/>
    <dcterms:publisher rdf:resource="http://www.historicengland.org.uk"/>
    <skos:scopeNote xml:lang="en">The chemical breakdown of a material by water.</skos:scopeNote>
    <skos:prefLabel xml:lang="en">Hydrolysis</skos:prefLabel>
  </rdf:Description>
  <rdf:Description rdf:about="http://purl.org/heritagedata/schemes/560/concepts/142200">
    <dcterms:publisher rdf:resource="http://www.historicengland.org.uk"/>
    <cc:attributionURL rdf:resource="http://www.historicengland.org.uk"/>
    <cc:attributionName xml:lang="en">Historic England</cc:attributionName>
    <cc:license rdf:resource="http://creativecommons.org/licenses/by/3.0"/>
    <dcterms:issued rdf:datatype="http://www.w3.org/2001/XMLSchema#dateTime">2019-05-23T13:12:18</dcterms:issued>
    <skos:prefLabel xml:lang="en">Stable Isotope Analysis</skos:prefLabel>
    <dcterms:identifier>http://purl.org/heritagedata/schemes/560/concepts/142200</dcterms:identifier>
    <skos:scopeNote xml:lang="en">Comparison of different proportions of natural occurring isotopes of lead (Pb), strontium (Sr), oxygen (O), carbon (C) and nitrogen (N).</skos:scopeNote>
    <skos:inScheme rdf:resource="http://purl.org/heritagedata/schemes/560"/>
    <rdf:type rdf:resource="http://www.w3.org/2004/02/skos/core#Concept"/>
  </rdf:Description>
  <rdf:Description rdf:about="http://purl.org/heritagedata/schemes/560/concepts/142145">
    <skos:scopeNote xml:lang="en">A precious metal characterised by its yellow colour and resistance to tarnishing.</skos:scopeNote>
    <skos:prefLabel xml:lang="en">Gold</skos:prefLabel>
    <dcterms:issued rdf:datatype="http://www.w3.org/2001/XMLSchema#dateTime">2019-05-23T13:12:18</dcterms:issued>
    <dcterms:publisher rdf:resource="http://www.historicengland.org.uk"/>
    <dcterms:identifier>http://purl.org/heritagedata/schemes/560/concepts/142145</dcterms:identifier>
    <cc:license rdf:resource="http://creativecommons.org/licenses/by/3.0"/>
    <rdf:type rdf:resource="http://www.w3.org/2004/02/skos/core#Concept"/>
    <skos:inScheme rdf:resource="http://purl.org/heritagedata/schemes/560"/>
    <cc:attributionURL rdf:resource="http://www.historicengland.org.uk"/>
    <cc:attributionName xml:lang="en">Historic England</cc:attributionName>
  </rdf:Description>
  <rdf:Description rdf:about="http://purl.org/heritagedata/schemes/560/concepts/142216">
    <rdf:type rdf:resource="http://www.w3.org/2004/02/skos/core#Concept"/>
    <skos:inScheme rdf:resource="http://purl.org/heritagedata/schemes/560"/>
    <cc:license rdf:resource="http://creativecommons.org/licenses/by/3.0"/>
    <skos:scopeNote xml:lang="en">The production of an image on a photographic plate as a result of X-rays (very short wavelength electromagnetic radiation) being passed through an object.</skos:scopeNote>
    <dcterms:publisher rdf:resource="http://www.historicengland.org.uk"/>
    <dcterms:issued rdf:datatype="http://www.w3.org/2001/XMLSchema#dateTime">2019-05-23T13:12:18</dcterms:issued>
    <cc:attributionURL rdf:resource="http://www.historicengland.org.uk"/>
    <cc:attributionName xml:lang="en">Historic England</cc:attributionName>
    <skos:prefLabel xml:lang="en">X-Radiography</skos:prefLabel>
    <dcterms:identifier>http://purl.org/heritagedata/schemes/560/concepts/142216</dcterms:identifier>
  </rdf:Description>
  <rdf:Description rdf:about="http://purl.org/heritagedata/schemes/560/concepts/147276">
    <dcterms:publisher rdf:resource="http://www.historicengland.org.uk"/>
    <skos:prefLabel xml:lang="en">Micro-Charcoal</skos:prefLabel>
    <dcterms:identifier>http://purl.org/heritagedata/schemes/560/concepts/147276</dcterms:identifier>
    <cc:attributionURL rdf:resource="http://www.historicengland.org.uk"/>
    <cc:attributionName xml:lang="en">Historic England</cc:attributionName>
    <dcterms:issued rdf:datatype="http://www.w3.org/2001/XMLSchema#dateTime">2019-05-23T13:12:18</dcterms:issued>
    <skos:scopeNote xml:lang="en">Microscopic charcoal fragments that are concentrated and counted as part of standard pollen preparation techniques.</skos:scopeNote>
    <skos:inScheme rdf:resource="http://purl.org/heritagedata/schemes/560"/>
    <cc:license rdf:resource="http://creativecommons.org/licenses/by/3.0"/>
    <rdf:type rdf:resource="http://www.w3.org/2004/02/skos/core#Concept"/>
  </rdf:Description>
  <rdf:Description rdf:about="http://purl.org/heritagedata/schemes/560/concepts/142113">
    <dcterms:publisher rdf:resource="http://www.historicengland.org.uk"/>
    <skos:prefLabel xml:lang="en">Calcined</skos:prefLabel>
    <cc:attributionName xml:lang="en">Historic England</cc:attributionName>
    <cc:license rdf:resource="http://creativecommons.org/licenses/by/3.0"/>
    <skos:inScheme rdf:resource="http://purl.org/heritagedata/schemes/560"/>
    <dcterms:identifier>http://purl.org/heritagedata/schemes/560/concepts/142113</dcterms:identifier>
    <skos:scopeNote xml:lang="en">Material burnt at high temperature (above 700 degrees Celsius) leaving only the mineral component.</skos:scopeNote>
    <cc:attributionURL rdf:resource="http://www.historicengland.org.uk"/>
    <dcterms:issued rdf:datatype="http://www.w3.org/2001/XMLSchema#dateTime">2019-05-23T13:12:18</dcterms:issued>
    <rdf:type rdf:resource="http://www.w3.org/2004/02/skos/core#Concept"/>
  </rdf:Description>
  <rdf:Description rdf:about="http://purl.org/heritagedata/schemes/560/concepts/170612">
    <skos:prefLabel xml:lang="en">Palynology</skos:prefLabel>
    <dcterms:publisher rdf:resource="http://www.historicengland.org.uk"/>
    <cc:attributionName xml:lang="en">Historic England</cc:attributionName>
    <cc:attributionURL rdf:resource="http://www.historicengland.org.uk"/>
    <dcterms:identifier>http://purl.org/heritagedata/schemes/560/concepts/170612</dcterms:identifier>
    <dcterms:issued rdf:datatype="http://www.w3.org/2001/XMLSchema#dateTime">2019-05-23T13:12:18</dcterms:issued>
    <cc:license rdf:resource="http://creativecommons.org/licenses/by/3.0"/>
    <skos:inScheme rdf:resource="http://purl.org/heritagedata/schemes/560"/>
    <skos:scopeNote xml:lang="en">The study of pollen and non-pollen palyomorphs preserved within deposits, including peat.</skos:scopeNote>
    <rdf:type rdf:resource="http://www.w3.org/2004/02/skos/core#Concept"/>
  </rdf:Description>
  <rdf:Description rdf:about="http://purl.org/heritagedata/schemes/560/concepts/147278">
    <dcterms:publisher rdf:resource="http://www.historicengland.org.uk"/>
    <skos:prefLabel xml:lang="en">Peat Humification</skos:prefLabel>
    <cc:attributionURL rdf:resource="http://www.historicengland.org.uk"/>
    <cc:attributionName xml:lang="en">Historic England</cc:attributionName>
    <cc:license rdf:resource="http://creativecommons.org/licenses/by/3.0"/>
    <dcterms:identifier>http://purl.org/heritagedata/schemes/560/concepts/147278</dcterms:identifier>
    <skos:inScheme rdf:resource="http://purl.org/heritagedata/schemes/560"/>
    <skos:scopeNote xml:lang="en">A method of determining peat degradation; quantified as the percentage light transmission value of the extracted humic acids, measured at a specific wavelength.</skos:scopeNote>
    <rdf:type rdf:resource="http://www.w3.org/2004/02/skos/core#Concept"/>
    <dcterms:issued rdf:datatype="http://www.w3.org/2001/XMLSchema#dateTime">2019-05-23T13:12:18</dcterms:issued>
  </rdf:Description>
  <rdf:Description rdf:about="http://purl.org/heritagedata/schemes/560/concepts/142171">
    <dcterms:publisher rdf:resource="http://www.historicengland.org.uk"/>
    <skos:prefLabel xml:lang="en">Modification State</skos:prefLabel>
    <cc:attributionURL rdf:resource="http://www.historicengland.org.uk"/>
    <cc:attributionName xml:lang="en">Historic England</cc:attributionName>
    <dcterms:issued rdf:datatype="http://www.w3.org/2001/XMLSchema#dateTime">2019-05-23T13:12:18</dcterms:issued>
    <dcterms:identifier>http://purl.org/heritagedata/schemes/560/concepts/142171</dcterms:identifier>
    <skos:inScheme rdf:resource="http://purl.org/heritagedata/schemes/560"/>
    <cc:license rdf:resource="http://creativecommons.org/licenses/by/3.0"/>
    <rdf:type rdf:resource="http://www.w3.org/2004/02/skos/core#Concept"/>
    <skos:topConceptOf rdf:resource="http://purl.org/heritagedata/schemes/560"/>
  </rdf:Description>
  <rdf:Description rdf:about="http://purl.org/heritagedata/schemes/560/concepts/142144">
    <cc:attributionURL rdf:resource="http://www.historicengland.org.uk"/>
    <cc:attributionName xml:lang="en">Historic England</cc:attributionName>
    <skos:prefLabel xml:lang="en">Fungal Damage</skos:prefLabel>
    <dcterms:identifier>http://purl.org/heritagedata/schemes/560/concepts/142144</dcterms:identifier>
    <dcterms:issued rdf:datatype="http://www.w3.org/2001/XMLSchema#dateTime">2019-05-23T13:12:18</dcterms:issued>
    <skos:scopeNote xml:lang="en">Material that has been damaged by fungal growth or secretions.</skos:scopeNote>
    <skos:inScheme rdf:resource="http://purl.org/heritagedata/schemes/560"/>
    <cc:license rdf:resource="http://creativecommons.org/licenses/by/3.0"/>
    <rdf:type rdf:resource="http://www.w3.org/2004/02/skos/core#Concept"/>
    <dcterms:publisher rdf:resource="http://www.historicengland.org.uk"/>
  </rdf:Description>
  <rdf:Description rdf:about="http://purl.org/heritagedata/schemes/560/concepts/144522">
    <cc:attributionName xml:lang="en">Historic England</cc:attributionName>
    <dcterms:identifier>http://purl.org/heritagedata/schemes/560/concepts/144522</dcterms:identifier>
    <dcterms:issued rdf:datatype="http://www.w3.org/2001/XMLSchema#dateTime">2019-05-23T13:12:18</dcterms:issued>
    <skos:inScheme rdf:resource="http://purl.org/heritagedata/schemes/560"/>
    <cc:license rdf:resource="http://creativecommons.org/licenses/by/3.0"/>
    <cc:attributionURL rdf:resource="http://www.historicengland.org.uk"/>
    <rdf:type rdf:resource="http://www.w3.org/2004/02/skos/core#Concept"/>
    <skos:scopeNote xml:lang="en">A mineral of the composition Zr[SiO4]. Commonly brown or yellow in colour. May contain high levels of uranium and thorium. Can be used for dating using luminescence or fission track methods.</skos:scopeNote>
    <dcterms:publisher rdf:resource="http://www.historicengland.org.uk"/>
    <skos:prefLabel xml:lang="en">Zircon</skos:prefLabel>
  </rdf:Description>
  <rdf:Description rdf:about="http://purl.org/heritagedata/schemes/560/concepts/142108">
    <skos:scopeNote xml:lang="en">The removal of fragile or complex remains from an investigation as a block of earth for excavation under laboratory conditions. Typical examples are grave goods and cremation burials.</skos:scopeNote>
    <skos:inScheme rdf:resource="http://purl.org/heritagedata/schemes/560"/>
    <cc:license rdf:resource="http://creativecommons.org/licenses/by/3.0"/>
    <rdf:type rdf:resource="http://www.w3.org/2004/02/skos/core#Concept"/>
    <skos:prefLabel xml:lang="en">Block Lifting</skos:prefLabel>
    <dcterms:publisher rdf:resource="http://www.historicengland.org.uk"/>
    <dcterms:issued rdf:datatype="http://www.w3.org/2001/XMLSchema#dateTime">2019-05-23T13:12:18</dcterms:issued>
    <cc:attributionURL rdf:resource="http://www.historicengland.org.uk"/>
    <cc:attributionName xml:lang="en">Historic England</cc:attributionName>
    <dcterms:identifier>http://purl.org/heritagedata/schemes/560/concepts/142108</dcterms:identifier>
  </rdf:Description>
  <rdf:Description rdf:about="http://purl.org/heritagedata/schemes/560/concepts/142102">
    <dcterms:issued rdf:datatype="http://www.w3.org/2001/XMLSchema#dateTime">2019-05-23T13:12:18</dcterms:issued>
    <cc:license rdf:resource="http://creativecommons.org/licenses/by/3.0"/>
    <rdf:type rdf:resource="http://www.w3.org/2004/02/skos/core#Concept"/>
    <skos:inScheme rdf:resource="http://purl.org/heritagedata/schemes/560"/>
    <dcterms:identifier>http://purl.org/heritagedata/schemes/560/concepts/142102</dcterms:identifier>
    <dcterms:publisher rdf:resource="http://www.historicengland.org.uk"/>
    <skos:prefLabel xml:lang="en">Anoxic</skos:prefLabel>
    <skos:scopeNote xml:lang="en">Material preserved by the exclusion of oxygen usually due to saturation with water which inhibits decay by micro-organisms.</skos:scopeNote>
    <cc:attributionURL rdf:resource="http://www.historicengland.org.uk"/>
    <cc:attributionName xml:lang="en">Historic England</cc:attributionName>
  </rdf:Description>
  <rdf:Description rdf:about="http://purl.org/heritagedata/schemes/560/concepts/142162">
    <cc:attributionURL rdf:resource="http://www.historicengland.org.uk"/>
    <rdf:type rdf:resource="http://www.w3.org/2004/02/skos/core#Concept"/>
    <skos:prefLabel xml:lang="en">Method Of Recovery</skos:prefLabel>
    <dcterms:issued rdf:datatype="http://www.w3.org/2001/XMLSchema#dateTime">2019-05-23T13:12:18</dcterms:issued>
    <dcterms:publisher rdf:resource="http://www.historicengland.org.uk"/>
    <cc:license rdf:resource="http://creativecommons.org/licenses/by/3.0"/>
    <cc:attributionName xml:lang="en">Historic England</cc:attributionName>
    <skos:topConceptOf rdf:resource="http://purl.org/heritagedata/schemes/560"/>
    <skos:inScheme rdf:resource="http://purl.org/heritagedata/schemes/560"/>
    <dcterms:identifier>http://purl.org/heritagedata/schemes/560/concepts/142162</dcterms:identifier>
  </rdf:Description>
  <rdf:Description rdf:about="http://purl.org/heritagedata/schemes/560/concepts/142184">
    <skos:scopeNote xml:lang="en">Material that has been penetrated or disrupted by the roots or rhizomes of plants.</skos:scopeNote>
    <cc:attributionURL rdf:resource="http://www.historicengland.org.uk"/>
    <cc:attributionName xml:lang="en">Historic England</cc:attributionName>
    <skos:prefLabel xml:lang="en">Plant Damage</skos:prefLabel>
    <dcterms:identifier>http://purl.org/heritagedata/schemes/560/concepts/142184</dcterms:identifier>
    <skos:inScheme rdf:resource="http://purl.org/heritagedata/schemes/560"/>
    <cc:license rdf:resource="http://creativecommons.org/licenses/by/3.0"/>
    <rdf:type rdf:resource="http://www.w3.org/2004/02/skos/core#Concept"/>
    <dcterms:publisher rdf:resource="http://www.historicengland.org.uk"/>
    <dcterms:issued rdf:datatype="http://www.w3.org/2001/XMLSchema#dateTime">2019-05-23T13:12:18</dcterms:issued>
  </rdf:Description>
  <rdf:Description rdf:about="http://purl.org/heritagedata/schemes/560/concepts/142218">
    <dcterms:publisher rdf:resource="http://www.historicengland.org.uk"/>
    <dcterms:identifier>http://purl.org/heritagedata/schemes/560/concepts/142218</dcterms:identifier>
    <cc:attributionURL rdf:resource="http://www.historicengland.org.uk"/>
    <cc:attributionName xml:lang="en">Historic England</cc:attributionName>
    <skos:prefLabel xml:lang="en">X-Ray Fluorescence Spectrometry</skos:prefLabel>
    <skos:scopeNote xml:lang="en">A surface technique of spectroscopic analysis which relies on the interaction of primary X-rays with the sample to generate a range of secondary X-rays. These have energies characteristic of the elements present in the sample.</skos:scopeNote>
    <cc:license rdf:resource="http://creativecommons.org/licenses/by/3.0"/>
    <skos:inScheme rdf:resource="http://purl.org/heritagedata/schemes/560"/>
    <dcterms:issued rdf:datatype="http://www.w3.org/2001/XMLSchema#dateTime">2019-05-23T13:12:18</dcterms:issued>
    <rdf:type rdf:resource="http://www.w3.org/2004/02/skos/core#Concept"/>
  </rdf:Description>
  <rdf:Description rdf:about="http://purl.org/heritagedata/schemes/560/concepts/142104">
    <cc:license rdf:resource="http://creativecommons.org/licenses/by/3.0"/>
    <cc:attributionName xml:lang="en">Historic England</cc:attributionName>
    <skos:inScheme rdf:resource="http://purl.org/heritagedata/schemes/560"/>
    <rdf:type rdf:resource="http://www.w3.org/2004/02/skos/core#Concept"/>
    <dcterms:issued rdf:datatype="http://www.w3.org/2001/XMLSchema#dateTime">2019-05-23T13:12:18</dcterms:issued>
    <dcterms:identifier>http://purl.org/heritagedata/schemes/560/concepts/142104</dcterms:identifier>
    <cc:attributionURL rdf:resource="http://www.historicengland.org.uk"/>
    <skos:prefLabel xml:lang="en">Archaeomagnetism</skos:prefLabel>
    <dcterms:publisher rdf:resource="http://www.historicengland.org.uk"/>
    <skos:scopeNote xml:lang="en">Measures the remanent magnetisation direction of magnetic minerals. Useful for dating fired structures, in-situ since their last firing, and for sediments settling from non turbulent water bodies. In the UK, calibration data extends back to 1000BC.</skos:scopeNote>
  </rdf:Description>
  <rdf:Description rdf:about="http://purl.org/heritagedata/schemes/560/concepts/142214">
    <dcterms:publisher rdf:resource="http://www.historicengland.org.uk"/>
    <skos:prefLabel xml:lang="en">Wood</skos:prefLabel>
    <dcterms:identifier>http://purl.org/heritagedata/schemes/560/concepts/142214</dcterms:identifier>
    <cc:attributionName xml:lang="en">Historic England</cc:attributionName>
    <cc:license rdf:resource="http://creativecommons.org/licenses/by/3.0"/>
    <dcterms:issued rdf:datatype="http://www.w3.org/2001/XMLSchema#dateTime">2019-05-23T13:12:18</dcterms:issued>
    <skos:scopeNote xml:lang="en">Hard, compact, unprocessed, fibrous cellulose substance. The roots, trunks and branches of trees and shrubs consist of this tissue.</skos:scopeNote>
    <cc:attributionURL rdf:resource="http://www.historicengland.org.uk"/>
    <skos:inScheme rdf:resource="http://purl.org/heritagedata/schemes/560"/>
    <rdf:type rdf:resource="http://www.w3.org/2004/02/skos/core#Concept"/>
  </rdf:Description>
  <rdf:Description rdf:about="http://purl.org/heritagedata/schemes/560/concepts/142177">
    <cc:attributionURL rdf:resource="http://www.historicengland.org.uk"/>
    <cc:attributionName xml:lang="en">Historic England</cc:attributionName>
    <dcterms:identifier>http://purl.org/heritagedata/schemes/560/concepts/142177</dcterms:identifier>
    <skos:prefLabel xml:lang="en">Optically Stimulated Luminescence</skos:prefLabel>
    <skos:scopeNote xml:lang="en">The light emitted from sedimentary minerals or mineral inclusions in bricks when stimulated in the laboratory by light of a different wavelength. Used to date samples up to 250,000 years old; especially appropriate for geological sediments.</skos:scopeNote>
    <skos:inScheme rdf:resource="http://purl.org/heritagedata/schemes/560"/>
    <cc:license rdf:resource="http://creativecommons.org/licenses/by/3.0"/>
    <rdf:type rdf:resource="http://www.w3.org/2004/02/skos/core#Concept"/>
    <dcterms:publisher rdf:resource="http://www.historicengland.org.uk"/>
    <dcterms:issued rdf:datatype="http://www.w3.org/2001/XMLSchema#dateTime">2019-05-23T13:12:18</dcterms:issued>
  </rdf:Description>
  <rdf:Description rdf:about="http://purl.org/heritagedata/schemes/560/concepts/142158">
    <dcterms:issued rdf:datatype="http://www.w3.org/2001/XMLSchema#dateTime">2019-05-23T13:12:18</dcterms:issued>
    <cc:license rdf:resource="http://creativecommons.org/licenses/by/3.0"/>
    <rdf:type rdf:resource="http://www.w3.org/2004/02/skos/core#Concept"/>
    <dcterms:publisher rdf:resource="http://www.historicengland.org.uk"/>
    <skos:scopeNote xml:lang="en">The degree to which a material will become magnetised when placed in a magnetic field.</skos:scopeNote>
    <dcterms:identifier>http://purl.org/heritagedata/schemes/560/concepts/142158</dcterms:identifier>
    <skos:inScheme rdf:resource="http://purl.org/heritagedata/schemes/560"/>
    <cc:attributionURL rdf:resource="http://www.historicengland.org.uk"/>
    <cc:attributionName xml:lang="en">Historic England</cc:attributionName>
    <skos:prefLabel xml:lang="en">Magnetic Susceptibility</skos:prefLabel>
  </rdf:Description>
  <rdf:Description rdf:about="http://purl.org/heritagedata/schemes/560/concepts/170613">
    <skos:prefLabel xml:lang="en">Palaeoenvironmental Analysis</skos:prefLabel>
    <dcterms:issued rdf:datatype="http://www.w3.org/2001/XMLSchema#dateTime">2019-05-23T13:12:18</dcterms:issued>
    <cc:license rdf:resource="http://creativecommons.org/licenses/by/3.0"/>
    <dcterms:identifier>http://purl.org/heritagedata/schemes/560/concepts/170613</dcterms:identifier>
    <rdf:type rdf:resource="http://www.w3.org/2004/02/skos/core#Concept"/>
    <dcterms:publisher rdf:resource="http://www.historicengland.org.uk"/>
    <skos:scopeNote xml:lang="en">The study of biological remains preserved within  deposits, including peat.</skos:scopeNote>
    <cc:attributionURL rdf:resource="http://www.historicengland.org.uk"/>
    <cc:attributionName xml:lang="en">Historic England</cc:attributionName>
    <skos:inScheme rdf:resource="http://purl.org/heritagedata/schemes/560"/>
  </rdf:Description>
  <rdf:Description rdf:about="http://purl.org/heritagedata/schemes/560/concepts/170621">
    <skos:prefLabel xml:lang="en">Human Osteology</skos:prefLabel>
    <skos:inScheme rdf:resource="http://purl.org/heritagedata/schemes/560"/>
    <cc:license rdf:resource="http://creativecommons.org/licenses/by/3.0"/>
    <rdf:type rdf:resource="http://www.w3.org/2004/02/skos/core#Concept"/>
    <skos:scopeNote xml:lang="en">The study of human remains preserved within archaeological deposits and palaeoenvironmental archives.</skos:scopeNote>
    <dcterms:publisher rdf:resource="http://www.historicengland.org.uk"/>
    <dcterms:issued rdf:datatype="http://www.w3.org/2001/XMLSchema#dateTime">2019-05-23T13:12:18</dcterms:issued>
    <cc:attributionURL rdf:resource="http://www.historicengland.org.uk"/>
    <cc:attributionName xml:lang="en">Historic England</cc:attributionName>
    <dcterms:identifier>http://purl.org/heritagedata/schemes/560/concepts/170621</dcterms:identifier>
  </rdf:Description>
  <rdf:Description rdf:about="http://purl.org/heritagedata/schemes/560/concepts/142125">
    <dcterms:publisher rdf:resource="http://www.historicengland.org.uk"/>
    <cc:attributionName xml:lang="en">Historic England</cc:attributionName>
    <cc:license rdf:resource="http://creativecommons.org/licenses/by/3.0"/>
    <dcterms:issued rdf:datatype="http://www.w3.org/2001/XMLSchema#dateTime">2019-05-23T13:12:18</dcterms:issued>
    <skos:prefLabel xml:lang="en">Copper Alloy</skos:prefLabel>
    <dcterms:identifier>http://purl.org/heritagedata/schemes/560/concepts/142125</dcterms:identifier>
    <skos:scopeNote xml:lang="en">Use for a combination (alloy) of two or more different metals where copper (Cu) is the principal component.</skos:scopeNote>
    <cc:attributionURL rdf:resource="http://www.historicengland.org.uk"/>
    <skos:inScheme rdf:resource="http://purl.org/heritagedata/schemes/560"/>
    <rdf:type rdf:resource="http://www.w3.org/2004/02/skos/core#Concept"/>
  </rdf:Description>
  <rdf:Description rdf:about="http://purl.org/heritagedata/schemes/560/concepts/142169">
    <cc:attributionName xml:lang="en">Historic England</cc:attributionName>
    <cc:license rdf:resource="http://creativecommons.org/licenses/by/3.0"/>
    <skos:inScheme rdf:resource="http://purl.org/heritagedata/schemes/560"/>
    <skos:prefLabel xml:lang="en">Mineralogy</skos:prefLabel>
    <cc:attributionURL rdf:resource="http://www.historicengland.org.uk"/>
    <dcterms:issued rdf:datatype="http://www.w3.org/2001/XMLSchema#dateTime">2019-05-23T13:12:18</dcterms:issued>
    <rdf:type rdf:resource="http://www.w3.org/2004/02/skos/core#Concept"/>
    <dcterms:identifier>http://purl.org/heritagedata/schemes/560/concepts/142169</dcterms:identifier>
    <dcterms:publisher rdf:resource="http://www.historicengland.org.uk"/>
    <skos:scopeNote xml:lang="en">The study of minerals.</skos:scopeNote>
  </rdf:Description>
  <rdf:Description rdf:about="http://purl.org/heritagedata/schemes/560/concepts/170619">
    <skos:scopeNote xml:lang="en">The study of foraminifera preserved in deposits.</skos:scopeNote>
    <cc:attributionName xml:lang="en">Historic England</cc:attributionName>
    <skos:prefLabel xml:lang="en">Foraminifera Analysis</skos:prefLabel>
    <dcterms:publisher rdf:resource="http://www.historicengland.org.uk"/>
    <cc:license rdf:resource="http://creativecommons.org/licenses/by/3.0"/>
    <dcterms:identifier>http://purl.org/heritagedata/schemes/560/concepts/170619</dcterms:identifier>
    <rdf:type rdf:resource="http://www.w3.org/2004/02/skos/core#Concept"/>
    <dcterms:issued rdf:datatype="http://www.w3.org/2001/XMLSchema#dateTime">2019-05-23T13:12:18</dcterms:issued>
    <skos:inScheme rdf:resource="http://purl.org/heritagedata/schemes/560"/>
    <cc:attributionURL rdf:resource="http://www.historicengland.org.uk"/>
  </rdf:Description>
  <rdf:Description rdf:about="http://purl.org/heritagedata/schemes/560/concepts/142977">
    <rdf:type rdf:resource="http://www.w3.org/2004/02/skos/core#Concept"/>
    <skos:inScheme rdf:resource="http://purl.org/heritagedata/schemes/560"/>
    <dcterms:issued rdf:datatype="http://www.w3.org/2001/XMLSchema#dateTime">2019-05-23T13:12:18</dcterms:issued>
    <dcterms:identifier>http://purl.org/heritagedata/schemes/560/concepts/142977</dcterms:identifier>
    <cc:license rdf:resource="http://creativecommons.org/licenses/by/3.0"/>
    <cc:attributionName xml:lang="en">Historic England</cc:attributionName>
    <cc:attributionURL rdf:resource="http://www.historicengland.org.uk"/>
    <dcterms:publisher rdf:resource="http://www.historicengland.org.uk"/>
    <skos:scopeNote xml:lang="en">An alluvial deposit laid down in an estuary.</skos:scopeNote>
    <skos:prefLabel xml:lang="en">Estuarine Deposit</skos:prefLabel>
  </rdf:Description>
  <rdf:Description rdf:about="http://purl.org/heritagedata/schemes/560/concepts/142201">
    <cc:attributionURL rdf:resource="http://www.historicengland.org.uk"/>
    <cc:attributionName xml:lang="en">Historic England</cc:attributionName>
    <dcterms:identifier>http://purl.org/heritagedata/schemes/560/concepts/142201</dcterms:identifier>
    <skos:prefLabel xml:lang="en">Stratigraphic Description</skos:prefLabel>
    <dcterms:publisher rdf:resource="http://www.historicengland.org.uk"/>
    <cc:license rdf:resource="http://creativecommons.org/licenses/by/3.0"/>
    <rdf:type rdf:resource="http://www.w3.org/2004/02/skos/core#Concept"/>
    <skos:inScheme rdf:resource="http://purl.org/heritagedata/schemes/560"/>
    <skos:scopeNote xml:lang="en">The careful observation and written description of the physical characteristics of stratigraphy. It will normally include information on texture, colour and the nature of the different components.</skos:scopeNote>
    <dcterms:issued rdf:datatype="http://www.w3.org/2001/XMLSchema#dateTime">2019-05-23T13:12:18</dcterms:issued>
  </rdf:Description>
  <rdf:Description rdf:about="http://purl.org/heritagedata/schemes/560/concepts/142174">
    <skos:inScheme rdf:resource="http://purl.org/heritagedata/schemes/560"/>
    <dcterms:publisher rdf:resource="http://www.historicengland.org.uk"/>
    <cc:license rdf:resource="http://creativecommons.org/licenses/by/3.0"/>
    <skos:scopeNote xml:lang="en">Any metal that does not contain the chemical element Iron (Fe) as a principal component.</skos:scopeNote>
    <cc:attributionName xml:lang="en">Historic England</cc:attributionName>
    <dcterms:identifier>http://purl.org/heritagedata/schemes/560/concepts/142174</dcterms:identifier>
    <dcterms:issued rdf:datatype="http://www.w3.org/2001/XMLSchema#dateTime">2019-05-23T13:12:18</dcterms:issued>
    <skos:prefLabel xml:lang="en">Non-Ferrous Metal</skos:prefLabel>
    <rdf:type rdf:resource="http://www.w3.org/2004/02/skos/core#Concept"/>
    <cc:attributionURL rdf:resource="http://www.historicengland.org.uk"/>
  </rdf:Description>
  <rdf:Description rdf:about="http://purl.org/heritagedata/schemes/560/concepts/170615">
    <skos:prefLabel xml:lang="en">Archaeomalacology</skos:prefLabel>
    <rdf:type rdf:resource="http://www.w3.org/2004/02/skos/core#Concept"/>
    <dcterms:issued rdf:datatype="http://www.w3.org/2001/XMLSchema#dateTime">2019-05-23T13:12:18</dcterms:issued>
    <skos:inScheme rdf:resource="http://purl.org/heritagedata/schemes/560"/>
    <dcterms:identifier>http://purl.org/heritagedata/schemes/560/concepts/170615</dcterms:identifier>
    <dcterms:publisher rdf:resource="http://www.historicengland.org.uk"/>
    <cc:license rdf:resource="http://creativecommons.org/licenses/by/3.0"/>
    <cc:attributionName xml:lang="en">Historic England</cc:attributionName>
    <cc:attributionURL rdf:resource="http://www.historicengland.org.uk"/>
    <skos:scopeNote xml:lang="en">The study of mollusca remains preserved within archaeological deposits and palaeoenvironmental archives.</skos:scopeNote>
  </rdf:Description>
  <rdf:Description rdf:about="http://purl.org/heritagedata/schemes/560/concepts/142161">
    <skos:inScheme rdf:resource="http://purl.org/heritagedata/schemes/560"/>
    <dcterms:issued rdf:datatype="http://www.w3.org/2001/XMLSchema#dateTime">2019-05-23T13:12:18</dcterms:issued>
    <cc:attributionName xml:lang="en">Historic England</cc:attributionName>
    <cc:attributionURL rdf:resource="http://www.historicengland.org.uk"/>
    <skos:scopeNote xml:lang="en">Class of elements and alloys that are characteristically lustrous, ductile, fusible and malleable. These are extracted from ore minerals originally existing in nature and processed before becoming a recognisable metal.</skos:scopeNote>
    <dcterms:publisher rdf:resource="http://www.historicengland.org.uk"/>
    <cc:license rdf:resource="http://creativecommons.org/licenses/by/3.0"/>
    <dcterms:identifier>http://purl.org/heritagedata/schemes/560/concepts/142161</dcterms:identifier>
    <rdf:type rdf:resource="http://www.w3.org/2004/02/skos/core#Concept"/>
    <skos:prefLabel xml:lang="en">Metal</skos:prefLabel>
  </rdf:Description>
  <rdf:Description rdf:about="http://purl.org/heritagedata/schemes/560/concepts/142178">
    <dcterms:identifier>http://purl.org/heritagedata/schemes/560/concepts/142178</dcterms:identifier>
    <dcterms:issued rdf:datatype="http://www.w3.org/2001/XMLSchema#dateTime">2019-05-23T13:12:18</dcterms:issued>
    <cc:license rdf:resource="http://creativecommons.org/licenses/by/3.0"/>
    <rdf:type rdf:resource="http://www.w3.org/2004/02/skos/core#Concept"/>
    <skos:inScheme rdf:resource="http://purl.org/heritagedata/schemes/560"/>
    <dcterms:publisher rdf:resource="http://www.historicengland.org.uk"/>
    <cc:attributionURL rdf:resource="http://www.historicengland.org.uk"/>
    <cc:attributionName xml:lang="en">Historic England</cc:attributionName>
    <skos:scopeNote xml:lang="en">The use of oxygen (O) isotope ratios in ice or ocean sediment cores to date global environmental change.</skos:scopeNote>
    <skos:prefLabel xml:lang="en">Oxygen Isotope Analysis</skos:prefLabel>
  </rdf:Description>
  <rdf:Description rdf:about="http://purl.org/heritagedata/schemes/560/concepts/144511">
    <skos:scopeNote xml:lang="en">A range of techniques that use the build up of charge stored within a crystalline material to estimate its age</skos:scopeNote>
    <skos:inScheme rdf:resource="http://purl.org/heritagedata/schemes/560"/>
    <cc:license rdf:resource="http://creativecommons.org/licenses/by/3.0"/>
    <cc:attributionName xml:lang="en">Historic England</cc:attributionName>
    <skos:prefLabel xml:lang="en">Luminescence Dating</skos:prefLabel>
    <dcterms:issued rdf:datatype="http://www.w3.org/2001/XMLSchema#dateTime">2019-05-23T13:12:18</dcterms:issued>
    <dcterms:publisher rdf:resource="http://www.historicengland.org.uk"/>
    <dcterms:identifier>http://purl.org/heritagedata/schemes/560/concepts/144511</dcterms:identifier>
    <cc:attributionURL rdf:resource="http://www.historicengland.org.uk"/>
    <rdf:type rdf:resource="http://www.w3.org/2004/02/skos/core#Concept"/>
  </rdf:Description>
  <rdf:Description rdf:about="http://purl.org/heritagedata/schemes/560/concepts/144514">
    <dcterms:publisher rdf:resource="http://www.historicengland.org.uk"/>
    <cc:license rdf:resource="http://creativecommons.org/licenses/by/3.0"/>
    <rdf:type rdf:resource="http://www.w3.org/2004/02/skos/core#Concept"/>
    <dcterms:issued rdf:datatype="http://www.w3.org/2001/XMLSchema#dateTime">2019-05-23T13:12:18</dcterms:issued>
    <cc:attributionURL rdf:resource="http://www.historicengland.org.uk"/>
    <skos:inScheme rdf:resource="http://purl.org/heritagedata/schemes/560"/>
    <dcterms:identifier>http://purl.org/heritagedata/schemes/560/concepts/144514</dcterms:identifier>
    <skos:scopeNote xml:lang="en">A technique that uses the emission of alpha particles of specific energies to identify the presence and concentration of certain radioactive isotopes in a sample</skos:scopeNote>
    <skos:prefLabel xml:lang="en">Alpha Spectrometry</skos:prefLabel>
    <cc:attributionName xml:lang="en">Historic England</cc:attributionName>
  </rdf:Description>
  <rdf:Description rdf:about="http://purl.org/heritagedata/schemes/560/concepts/142154">
    <skos:scopeNote xml:lang="en">Use for a tusk or tooth of a mammal large enough to be carved or used to make objects such as those of mammoths, elephants, walruses and whales.</skos:scopeNote>
    <skos:inScheme rdf:resource="http://purl.org/heritagedata/schemes/560"/>
    <cc:license rdf:resource="http://creativecommons.org/licenses/by/3.0"/>
    <rdf:type rdf:resource="http://www.w3.org/2004/02/skos/core#Concept"/>
    <dcterms:publisher rdf:resource="http://www.historicengland.org.uk"/>
    <dcterms:issued rdf:datatype="http://www.w3.org/2001/XMLSchema#dateTime">2019-05-23T13:12:18</dcterms:issued>
    <cc:attributionURL rdf:resource="http://www.historicengland.org.uk"/>
    <cc:attributionName xml:lang="en">Historic England</cc:attributionName>
    <skos:prefLabel xml:lang="en">Ivory</skos:prefLabel>
    <dcterms:identifier>http://purl.org/heritagedata/schemes/560/concepts/142154</dcterms:identifier>
  </rdf:Description>
  <rdf:Description rdf:about="http://purl.org/heritagedata/schemes/560/concepts/142111">
    <dcterms:identifier>http://purl.org/heritagedata/schemes/560/concepts/142111</dcterms:identifier>
    <cc:license rdf:resource="http://creativecommons.org/licenses/by/3.0"/>
    <skos:inScheme rdf:resource="http://purl.org/heritagedata/schemes/560"/>
    <skos:scopeNote xml:lang="en">Use for material that has been burnt.</skos:scopeNote>
    <cc:attributionURL rdf:resource="http://www.historicengland.org.uk"/>
    <dcterms:issued rdf:datatype="http://www.w3.org/2001/XMLSchema#dateTime">2019-05-23T13:12:18</dcterms:issued>
    <rdf:type rdf:resource="http://www.w3.org/2004/02/skos/core#Concept"/>
    <cc:attributionName xml:lang="en">Historic England</cc:attributionName>
    <dcterms:publisher rdf:resource="http://www.historicengland.org.uk"/>
    <skos:prefLabel xml:lang="en">Burnt</skos:prefLabel>
  </rdf:Description>
  <rdf:Description rdf:about="http://purl.org/heritagedata/schemes/560/concepts/142175">
    <skos:inScheme rdf:resource="http://purl.org/heritagedata/schemes/560"/>
    <dcterms:issued rdf:datatype="http://www.w3.org/2001/XMLSchema#dateTime">2019-05-23T13:12:18</dcterms:issued>
    <cc:attributionName xml:lang="en">Historic England</cc:attributionName>
    <cc:attributionURL rdf:resource="http://www.historicengland.org.uk"/>
    <skos:prefLabel xml:lang="en">Non-Metric Traits</skos:prefLabel>
    <skos:scopeNote xml:lang="en">Use for congenital (present at birth) abnormalities (absent/extra or morphologically unusual features) present in an individual or population.</skos:scopeNote>
    <dcterms:identifier>http://purl.org/heritagedata/schemes/560/concepts/142175</dcterms:identifier>
    <dcterms:publisher rdf:resource="http://www.historicengland.org.uk"/>
    <cc:license rdf:resource="http://creativecommons.org/licenses/by/3.0"/>
    <rdf:type rdf:resource="http://www.w3.org/2004/02/skos/core#Concept"/>
  </rdf:Description>
  <rdf:Description rdf:about="http://purl.org/heritagedata/schemes/560/concepts/142099">
    <skos:prefLabel xml:lang="en">Altered By Animals</skos:prefLabel>
    <skos:inScheme rdf:resource="http://purl.org/heritagedata/schemes/560"/>
    <cc:license rdf:resource="http://creativecommons.org/licenses/by/3.0"/>
    <rdf:type rdf:resource="http://www.w3.org/2004/02/skos/core#Concept"/>
    <skos:scopeNote xml:lang="en">Modified or damaged by an animal.</skos:scopeNote>
    <dcterms:publisher rdf:resource="http://www.historicengland.org.uk"/>
    <cc:attributionURL rdf:resource="http://www.historicengland.org.uk"/>
    <cc:attributionName xml:lang="en">Historic England</cc:attributionName>
    <dcterms:issued rdf:datatype="http://www.w3.org/2001/XMLSchema#dateTime">2019-05-23T13:12:18</dcterms:issued>
    <dcterms:identifier>http://purl.org/heritagedata/schemes/560/concepts/142099</dcterms:identifier>
  </rdf:Description>
  <rdf:Description rdf:about="http://purl.org/heritagedata/schemes/560">
    <rdf:type rdf:resource="http://www.w3.org/2004/02/skos/core#ConceptScheme"/>
    <dcterms:description xml:lang="en">Terminology used for recording the techniques, recovery methods and materials associated with archaeological sciences. Maintained by Historic England on behalf of the FISH Terminology Working Group.</dcterms:description>
    <dcterms:title xml:lang="en">FISH Archaeological Sciences Thesaurus</dcterms:title>
    <skos:hasTopConcept rdf:resource="http://purl.org/heritagedata/schemes/560/concepts/142153"/>
    <skos:hasTopConcept rdf:resource="http://purl.org/heritagedata/schemes/560/concepts/142162"/>
    <cc:attributionURL rdf:resource="http://www.historicengland.org.uk"/>
    <skos:hasTopConcept rdf:resource="http://purl.org/heritagedata/schemes/560/concepts/142160"/>
    <dcterms:issued rdf:datatype="http://www.w3.org/2001/XMLSchema#date">2019-05-23</dcterms:issued>
    <dcterms:publisher rdf:resource="http://www.historicengland.org.uk"/>
    <skos:hasTopConcept rdf:resource="http://purl.org/heritagedata/schemes/560/concepts/142105"/>
    <skos:hasTopConcept rdf:resource="http://purl.org/heritagedata/schemes/560/concepts/142171"/>
    <cc:license rdf:resource="http://creativecommons.org/licenses/by/3.0"/>
    <dcterms:identifier>http://purl.org/heritagedata/schemes/560</dcterms:identifier>
    <cc:attributionName xml:lang="en">Historic England</cc:attributionName>
  </rdf:Description>
  <rdf:Description rdf:about="http://purl.org/heritagedata/schemes/560/concepts/142148">
    <dcterms:publisher rdf:resource="http://www.historicengland.org.uk"/>
    <cc:attributionName xml:lang="en">Historic England</cc:attributionName>
    <cc:attributionURL rdf:resource="http://www.historicengland.org.uk"/>
    <skos:scopeNote xml:lang="en">Aspects of a material which result from the modification or use of the material by humans.</skos:scopeNote>
    <dcterms:identifier>http://purl.org/heritagedata/schemes/560/concepts/142148</dcterms:identifier>
    <dcterms:issued rdf:datatype="http://www.w3.org/2001/XMLSchema#dateTime">2019-05-23T13:12:18</dcterms:issued>
    <cc:license rdf:resource="http://creativecommons.org/licenses/by/3.0"/>
    <skos:prefLabel xml:lang="en">Human Aspects</skos:prefLabel>
    <skos:inScheme rdf:resource="http://purl.org/heritagedata/schemes/560"/>
    <rdf:type rdf:resource="http://www.w3.org/2004/02/skos/core#Concept"/>
  </rdf:Description>
  <rdf:Description rdf:about="http://purl.org/heritagedata/schemes/560/concepts/142107">
    <skos:scopeNote xml:lang="en">A technique in which the date is deduced from the presence of fauna and/or flora considered to be characteristic of a given peirod of time or that gives and indication of a probable date.</skos:scopeNote>
    <skos:inScheme rdf:resource="http://purl.org/heritagedata/schemes/560"/>
    <cc:license rdf:resource="http://creativecommons.org/licenses/by/3.0"/>
    <rdf:type rdf:resource="http://www.w3.org/2004/02/skos/core#Concept"/>
    <dcterms:identifier>http://purl.org/heritagedata/schemes/560/concepts/142107</dcterms:identifier>
    <skos:prefLabel xml:lang="en">Biostratigraphy</skos:prefLabel>
    <dcterms:publisher rdf:resource="http://www.historicengland.org.uk"/>
    <dcterms:issued rdf:datatype="http://www.w3.org/2001/XMLSchema#dateTime">2019-05-23T13:12:18</dcterms:issued>
    <cc:attributionURL rdf:resource="http://www.historicengland.org.uk"/>
    <cc:attributionName xml:lang="en">Historic England</cc:attributionName>
  </rdf:Description>
  <rdf:Description rdf:about="http://purl.org/heritagedata/schemes/560/concepts/142167">
    <skos:prefLabel xml:lang="en">Mineral Replaced</skos:prefLabel>
    <dcterms:publisher rdf:resource="http://www.historicengland.org.uk"/>
    <cc:license rdf:resource="http://creativecommons.org/licenses/by/3.0"/>
    <rdf:type rdf:resource="http://www.w3.org/2004/02/skos/core#Concept"/>
    <dcterms:issued rdf:datatype="http://www.w3.org/2001/XMLSchema#dateTime">2019-05-23T13:12:18</dcterms:issued>
    <cc:attributionURL rdf:resource="http://www.historicengland.org.uk"/>
    <cc:attributionName xml:lang="en">Historic England</cc:attributionName>
    <skos:inScheme rdf:resource="http://purl.org/heritagedata/schemes/560"/>
    <dcterms:identifier>http://purl.org/heritagedata/schemes/560/concepts/142167</dcterms:identifier>
    <skos:scopeNote xml:lang="en">Replacement of organic material by minerals, including calcium carbonate and calcium phosphate.</skos:scopeNote>
  </rdf:Description>
  <rdf:Description rdf:about="http://purl.org/heritagedata/schemes/560/concepts/142151">
    <cc:attributionURL rdf:resource="http://www.historicengland.org.uk"/>
    <skos:inScheme rdf:resource="http://purl.org/heritagedata/schemes/560"/>
    <rdf:type rdf:resource="http://www.w3.org/2004/02/skos/core#Concept"/>
    <dcterms:issued rdf:datatype="http://www.w3.org/2001/XMLSchema#dateTime">2019-05-23T13:12:18</dcterms:issued>
    <dcterms:publisher rdf:resource="http://www.historicengland.org.uk"/>
    <cc:attributionName xml:lang="en">Historic England</cc:attributionName>
    <cc:license rdf:resource="http://creativecommons.org/licenses/by/3.0"/>
    <dcterms:identifier>http://purl.org/heritagedata/schemes/560/concepts/142151</dcterms:identifier>
    <skos:prefLabel xml:lang="en">Infra-Red Stimulated Luminescence</skos:prefLabel>
    <skos:scopeNote xml:lang="en">The light emitted from sedimentary minerals or mineral inclusions in bricks when stimulated in the laboratory by infrared light. Used to date samples up to 250,000 years old; especially appropriate for geological sediments containing feldspars</skos:scopeNote>
  </rdf:Description>
  <rdf:Description rdf:about="http://purl.org/heritagedata/schemes/560/concepts/142183">
    <skos:prefLabel xml:lang="en">Phytolith</skos:prefLabel>
    <dcterms:identifier>http://purl.org/heritagedata/schemes/560/concepts/142183</dcterms:identifier>
    <cc:attributionURL rdf:resource="http://www.historicengland.org.uk"/>
    <dcterms:issued rdf:datatype="http://www.w3.org/2001/XMLSchema#dateTime">2019-05-23T13:12:18</dcterms:issued>
    <skos:inScheme rdf:resource="http://purl.org/heritagedata/schemes/560"/>
    <skos:scopeNote xml:lang="en">Microscopic mineral body (usually silica) found in many plants.</skos:scopeNote>
    <dcterms:publisher rdf:resource="http://www.historicengland.org.uk"/>
    <rdf:type rdf:resource="http://www.w3.org/2004/02/skos/core#Concept"/>
    <cc:attributionName xml:lang="en">Historic England</cc:attributionName>
    <cc:license rdf:resource="http://creativecommons.org/licenses/by/3.0"/>
  </rdf:Description>
  <rdf:Description rdf:about="http://purl.org/heritagedata/schemes/560/concepts/142172">
    <rdf:type rdf:resource="http://www.w3.org/2004/02/skos/core#Concept"/>
    <cc:attributionURL rdf:resource="http://www.historicengland.org.uk"/>
    <dcterms:publisher rdf:resource="http://www.historicengland.org.uk"/>
    <dcterms:identifier>http://purl.org/heritagedata/schemes/560/concepts/142172</dcterms:identifier>
    <cc:license rdf:resource="http://creativecommons.org/licenses/by/3.0"/>
    <cc:attributionName xml:lang="en">Historic England</cc:attributionName>
    <skos:prefLabel xml:lang="en">Multi-Element Analysis</skos:prefLabel>
    <dcterms:issued rdf:datatype="http://www.w3.org/2001/XMLSchema#dateTime">2019-05-23T13:12:18</dcterms:issued>
    <skos:scopeNote xml:lang="en">Techniques investigating more than one element at a time.</skos:scopeNote>
    <skos:inScheme rdf:resource="http://purl.org/heritagedata/schemes/560"/>
  </rdf:Description>
  <rdf:Description rdf:about="http://purl.org/heritagedata/schemes/560/concepts/142141">
    <rdf:type rdf:resource="http://www.w3.org/2004/02/skos/core#Concept"/>
    <skos:inScheme rdf:resource="http://purl.org/heritagedata/schemes/560"/>
    <skos:prefLabel xml:lang="en">Flotation</skos:prefLabel>
    <dcterms:identifier>http://purl.org/heritagedata/schemes/560/concepts/142141</dcterms:identifier>
    <dcterms:issued rdf:datatype="http://www.w3.org/2001/XMLSchema#dateTime">2019-05-23T13:12:18</dcterms:issued>
    <cc:license rdf:resource="http://creativecommons.org/licenses/by/3.0"/>
    <cc:attributionName xml:lang="en">Historic England</cc:attributionName>
    <cc:attributionURL rdf:resource="http://www.historicengland.org.uk"/>
    <dcterms:publisher rdf:resource="http://www.historicengland.org.uk"/>
    <skos:scopeNote xml:lang="en">Method used for the recovering of material by floating large whole earth samples, usually between 40-60 litres per context (or 100% if context contains less than this).</skos:scopeNote>
  </rdf:Description>
  <rdf:Description rdf:about="http://purl.org/heritagedata/schemes/560/concepts/142136">
    <dcterms:publisher rdf:resource="http://www.historicengland.org.uk"/>
    <cc:license rdf:resource="http://creativecommons.org/licenses/by/3.0"/>
    <rdf:type rdf:resource="http://www.w3.org/2004/02/skos/core#Concept"/>
    <skos:prefLabel xml:lang="en">Electron Spin Resonance</skos:prefLabel>
    <cc:attributionURL rdf:resource="http://www.historicengland.org.uk"/>
    <dcterms:issued rdf:datatype="http://www.w3.org/2001/XMLSchema#dateTime">2019-05-23T13:12:18</dcterms:issued>
    <cc:attributionName xml:lang="en">Historic England</cc:attributionName>
    <skos:scopeNote xml:lang="en">The measurement of trapped electrons by exposure to high-frequency electromagnetic radiation. A useful technique for dating tooth enamel, shells, coral and calcite form 5,000-1,000,000 years old.</skos:scopeNote>
    <skos:inScheme rdf:resource="http://purl.org/heritagedata/schemes/560"/>
    <dcterms:identifier>http://purl.org/heritagedata/schemes/560/concepts/142136</dcterms:identifier>
  </rdf:Description>
  <rdf:Description rdf:about="http://purl.org/heritagedata/schemes/560/concepts/142120">
    <dcterms:publisher rdf:resource="http://www.historicengland.org.uk"/>
    <skos:inScheme rdf:resource="http://purl.org/heritagedata/schemes/560"/>
    <cc:attributionURL rdf:resource="http://www.historicengland.org.uk"/>
    <skos:scopeNote xml:lang="en">Material that has been altered as a result of chemical action.</skos:scopeNote>
    <dcterms:identifier>http://purl.org/heritagedata/schemes/560/concepts/142120</dcterms:identifier>
    <skos:prefLabel xml:lang="en">Chemically Altered</skos:prefLabel>
    <cc:attributionName xml:lang="en">Historic England</cc:attributionName>
    <dcterms:issued rdf:datatype="http://www.w3.org/2001/XMLSchema#dateTime">2019-05-23T13:12:18</dcterms:issued>
    <cc:license rdf:resource="http://creativecommons.org/licenses/by/3.0"/>
    <rdf:type rdf:resource="http://www.w3.org/2004/02/skos/core#Concept"/>
  </rdf:Description>
  <rdf:Description rdf:about="http://purl.org/heritagedata/schemes/560/concepts/142199">
    <rdf:type rdf:resource="http://www.w3.org/2004/02/skos/core#Concept"/>
    <cc:attributionURL rdf:resource="http://www.historicengland.org.uk"/>
    <dcterms:publisher rdf:resource="http://www.historicengland.org.uk"/>
    <skos:scopeNote xml:lang="en">The application of a chemical test to a material, usually as a rapid approximation.</skos:scopeNote>
    <dcterms:identifier>http://purl.org/heritagedata/schemes/560/concepts/142199</dcterms:identifier>
    <cc:license rdf:resource="http://creativecommons.org/licenses/by/3.0"/>
    <cc:attributionName xml:lang="en">Historic England</cc:attributionName>
    <skos:prefLabel xml:lang="en">Spot Test</skos:prefLabel>
    <dcterms:issued rdf:datatype="http://www.w3.org/2001/XMLSchema#dateTime">2019-05-23T13:12:18</dcterms:issued>
    <skos:inScheme rdf:resource="http://purl.org/heritagedata/schemes/560"/>
  </rdf:Description>
  <rdf:Description rdf:about="http://purl.org/heritagedata/schemes/560/concepts/142131">
    <cc:attributionName xml:lang="en">Historic England</cc:attributionName>
    <cc:license rdf:resource="http://creativecommons.org/licenses/by/3.0"/>
    <dcterms:identifier>http://purl.org/heritagedata/schemes/560/concepts/142131</dcterms:identifier>
    <skos:scopeNote xml:lang="en">The measuring of annual tree-ring growth shown by most tree species in temperated regions. Regional chronoliges are required to date any particular piece of wood, the longest of which, for Germany, works for the present to approximately 14,000 yrs ago.</skos:scopeNote>
    <skos:related rdf:resource="http://purl.org/heritagedata/schemes/560/concepts/142209"/>
    <rdf:type rdf:resource="http://www.w3.org/2004/02/skos/core#Concept"/>
    <cc:attributionURL rdf:resource="http://www.historicengland.org.uk"/>
    <dcterms:issued rdf:datatype="http://www.w3.org/2001/XMLSchema#dateTime">2019-05-23T13:12:18</dcterms:issued>
    <skos:inScheme rdf:resource="http://purl.org/heritagedata/schemes/560"/>
    <dcterms:publisher rdf:resource="http://www.historicengland.org.uk"/>
    <skos:prefLabel xml:lang="en">Dendrochronology</skos:prefLabel>
  </rdf:Description>
  <rdf:Description rdf:about="http://purl.org/heritagedata/schemes/560/concepts/142165">
    <cc:attributionURL rdf:resource="http://www.historicengland.org.uk"/>
    <rdf:type rdf:resource="http://www.w3.org/2004/02/skos/core#Concept"/>
    <skos:prefLabel xml:lang="en">Microscopy</skos:prefLabel>
    <dcterms:issued rdf:datatype="http://www.w3.org/2001/XMLSchema#dateTime">2019-05-23T13:12:18</dcterms:issued>
    <dcterms:publisher rdf:resource="http://www.historicengland.org.uk"/>
    <skos:scopeNote xml:lang="en">The use of magnifying equipment to examine materials not visible to the naked eye.</skos:scopeNote>
    <cc:license rdf:resource="http://creativecommons.org/licenses/by/3.0"/>
    <cc:attributionName xml:lang="en">Historic England</cc:attributionName>
    <dcterms:identifier>http://purl.org/heritagedata/schemes/560/concepts/142165</dcterms:identifier>
    <skos:inScheme rdf:resource="http://purl.org/heritagedata/schemes/560"/>
  </rdf:Description>
  <rdf:Description rdf:about="http://purl.org/heritagedata/schemes/560/concepts/144513">
    <skos:inScheme rdf:resource="http://purl.org/heritagedata/schemes/560"/>
    <dcterms:identifier>http://purl.org/heritagedata/schemes/560/concepts/144513</dcterms:identifier>
    <cc:license rdf:resource="http://creativecommons.org/licenses/by/3.0"/>
    <cc:attributionName xml:lang="en">Historic England</cc:attributionName>
    <dcterms:issued rdf:datatype="http://www.w3.org/2001/XMLSchema#dateTime">2019-05-23T13:12:18</dcterms:issued>
    <skos:scopeNote xml:lang="en">A technique that uses the emission of gamma rays of specific energies to identify the presence and concentration of certain radioactive isotopes in a sample</skos:scopeNote>
    <dcterms:publisher rdf:resource="http://www.historicengland.org.uk"/>
    <skos:prefLabel xml:lang="en">Gamma Spectrometry</skos:prefLabel>
    <cc:attributionURL rdf:resource="http://www.historicengland.org.uk"/>
    <rdf:type rdf:resource="http://www.w3.org/2004/02/skos/core#Concept"/>
  </rdf:Description>
  <rdf:Description rdf:about="http://purl.org/heritagedata/schemes/560/concepts/142160">
    <skos:prefLabel xml:lang="en">Material Type</skos:prefLabel>
    <dcterms:identifier>http://purl.org/heritagedata/schemes/560/concepts/142160</dcterms:identifier>
    <cc:attributionURL rdf:resource="http://www.historicengland.org.uk"/>
    <cc:attributionName xml:lang="en">Historic England</cc:attributionName>
    <dcterms:issued rdf:datatype="http://www.w3.org/2001/XMLSchema#dateTime">2019-05-23T13:12:18</dcterms:issued>
    <skos:inScheme rdf:resource="http://purl.org/heritagedata/schemes/560"/>
    <cc:license rdf:resource="http://creativecommons.org/licenses/by/3.0"/>
    <rdf:type rdf:resource="http://www.w3.org/2004/02/skos/core#Concept"/>
    <skos:topConceptOf rdf:resource="http://purl.org/heritagedata/schemes/560"/>
    <dcterms:publisher rdf:resource="http://www.historicengland.org.uk"/>
  </rdf:Description>
  <rdf:Description rdf:about="http://purl.org/heritagedata/schemes/560/concepts/142179">
    <cc:attributionURL rdf:resource="http://www.historicengland.org.uk"/>
    <skos:inScheme rdf:resource="http://purl.org/heritagedata/schemes/560"/>
    <rdf:type rdf:resource="http://www.w3.org/2004/02/skos/core#Concept"/>
    <dcterms:issued rdf:datatype="http://www.w3.org/2001/XMLSchema#dateTime">2019-05-23T13:12:18</dcterms:issued>
    <dcterms:publisher rdf:resource="http://www.historicengland.org.uk"/>
    <cc:attributionName xml:lang="en">Historic England</cc:attributionName>
    <cc:license rdf:resource="http://creativecommons.org/licenses/by/3.0"/>
    <dcterms:identifier>http://purl.org/heritagedata/schemes/560/concepts/142179</dcterms:identifier>
    <skos:scopeNote xml:lang="en">The analysis of the distribution and proportion of sand, silt and clay in a deposit.</skos:scopeNote>
    <skos:prefLabel xml:lang="en">Particle Size Analysis</skos:prefLabel>
  </rdf:Description>
  <rdf:Description rdf:about="http://purl.org/heritagedata/schemes/560/concepts/170618">
    <dcterms:identifier>http://purl.org/heritagedata/schemes/560/concepts/170618</dcterms:identifier>
    <dcterms:publisher rdf:resource="http://www.historicengland.org.uk"/>
    <cc:attributionName xml:lang="en">Historic England</cc:attributionName>
    <cc:license rdf:resource="http://creativecommons.org/licenses/by/3.0"/>
    <dcterms:issued rdf:datatype="http://www.w3.org/2001/XMLSchema#dateTime">2019-05-23T13:12:18</dcterms:issued>
    <skos:prefLabel xml:lang="en">Archaeobotany</skos:prefLabel>
    <skos:scopeNote xml:lang="en">The study of plant remains, typically seeds, fruits, wood, leaves etc, preserved within archaeological deposits and palaeoenvironmental archives. Use palynology when pollen and spores are being analysed as opposed to macroscopic plant remains.</skos:scopeNote>
    <cc:attributionURL rdf:resource="http://www.historicengland.org.uk"/>
    <skos:inScheme rdf:resource="http://purl.org/heritagedata/schemes/560"/>
    <rdf:type rdf:resource="http://www.w3.org/2004/02/skos/core#Concept"/>
  </rdf:Description>
  <rdf:Description rdf:about="http://purl.org/heritagedata/schemes/560/concepts/144518">
    <dcterms:issued rdf:datatype="http://www.w3.org/2001/XMLSchema#dateTime">2019-05-23T13:12:18</dcterms:issued>
    <dcterms:identifier>http://purl.org/heritagedata/schemes/560/concepts/144518</dcterms:identifier>
    <cc:attributionName xml:lang="en">Historic England</cc:attributionName>
    <skos:scopeNote xml:lang="en">A material composed of mineral grains derived from the breakdown of rocks by environmental processes.</skos:scopeNote>
    <dcterms:publisher rdf:resource="http://www.historicengland.org.uk"/>
    <cc:license rdf:resource="http://creativecommons.org/licenses/by/3.0"/>
    <rdf:type rdf:resource="http://www.w3.org/2004/02/skos/core#Concept"/>
    <skos:inScheme rdf:resource="http://purl.org/heritagedata/schemes/560"/>
    <cc:attributionURL rdf:resource="http://www.historicengland.org.uk"/>
    <skos:prefLabel xml:lang="en">Geological Sediment</skos:prefLabel>
  </rdf:Description>
  <rdf:Description rdf:about="http://purl.org/heritagedata/schemes/560/concepts/142121">
    <dcterms:identifier>http://purl.org/heritagedata/schemes/560/concepts/142121</dcterms:identifier>
    <skos:inScheme rdf:resource="http://purl.org/heritagedata/schemes/560"/>
    <skos:prefLabel xml:lang="en">Clast Lithological Analysis</skos:prefLabel>
    <dcterms:issued rdf:datatype="http://www.w3.org/2001/XMLSchema#dateTime">2019-05-23T13:12:18</dcterms:issued>
    <rdf:type rdf:resource="http://www.w3.org/2004/02/skos/core#Concept"/>
    <cc:attributionURL rdf:resource="http://www.historicengland.org.uk"/>
    <dcterms:publisher rdf:resource="http://www.historicengland.org.uk"/>
    <skos:scopeNote xml:lang="en">The identification and grouping of stone types in stratigraphy.</skos:scopeNote>
    <cc:license rdf:resource="http://creativecommons.org/licenses/by/3.0"/>
    <cc:attributionName xml:lang="en">Historic England</cc:attributionName>
  </rdf:Description>
  <rdf:Description rdf:about="http://purl.org/heritagedata/schemes/560/concepts/142153">
    <dcterms:publisher rdf:resource="http://www.historicengland.org.uk"/>
    <cc:license rdf:resource="http://creativecommons.org/licenses/by/3.0"/>
    <skos:topConceptOf rdf:resource="http://purl.org/heritagedata/schemes/560"/>
    <rdf:type rdf:resource="http://www.w3.org/2004/02/skos/core#Concept"/>
    <skos:inScheme rdf:resource="http://purl.org/heritagedata/schemes/560"/>
    <cc:attributionURL rdf:resource="http://www.historicengland.org.uk"/>
    <skos:prefLabel xml:lang="en">Investigative Techniques</skos:prefLabel>
    <dcterms:identifier>http://purl.org/heritagedata/schemes/560/concepts/142153</dcterms:identifier>
    <cc:attributionName xml:lang="en">Historic England</cc:attributionName>
    <dcterms:issued rdf:datatype="http://www.w3.org/2001/XMLSchema#dateTime">2019-05-23T13:12:18</dcterms:issued>
  </rdf:Description>
  <rdf:Description rdf:about="http://purl.org/heritagedata/schemes/560/concepts/142122">
    <rdf:type rdf:resource="http://www.w3.org/2004/02/skos/core#Concept"/>
    <dcterms:issued rdf:datatype="http://www.w3.org/2001/XMLSchema#dateTime">2019-05-23T13:12:18</dcterms:issued>
    <skos:inScheme rdf:resource="http://purl.org/heritagedata/schemes/560"/>
    <skos:prefLabel xml:lang="en">Coarse Sieving</skos:prefLabel>
    <dcterms:publisher rdf:resource="http://www.historicengland.org.uk"/>
    <cc:license rdf:resource="http://creativecommons.org/licenses/by/3.0"/>
    <cc:attributionName xml:lang="en">Historic England</cc:attributionName>
    <cc:attributionURL rdf:resource="http://www.historicengland.org.uk"/>
    <skos:scopeNote xml:lang="en">The method of retrieving animal remains, artefacts and other remains by dry or wet-sieving whole earth samples, typically over 100 litres, sieved through a 2mm or larger mesh.</skos:scopeNote>
    <dcterms:identifier>http://purl.org/heritagedata/schemes/560/concepts/142122</dcterms:identifier>
  </rdf:Description>
  <rdf:Description rdf:about="http://purl.org/heritagedata/schemes/560/concepts/144517">
    <skos:prefLabel xml:lang="en">Burnt Flint</skos:prefLabel>
    <cc:attributionName xml:lang="en">Historic England</cc:attributionName>
    <dcterms:publisher rdf:resource="http://www.historicengland.org.uk"/>
    <rdf:type rdf:resource="http://www.w3.org/2004/02/skos/core#Concept"/>
    <skos:scopeNote xml:lang="en">A form of silica, similar to quartz. Commonly black or white in colour and used for tool manufacture. Flints heated in antiquity may be dated using thermoluminescence.</skos:scopeNote>
    <dcterms:identifier>http://purl.org/heritagedata/schemes/560/concepts/144517</dcterms:identifier>
    <skos:inScheme rdf:resource="http://purl.org/heritagedata/schemes/560"/>
    <cc:attributionURL rdf:resource="http://www.historicengland.org.uk"/>
    <dcterms:issued rdf:datatype="http://www.w3.org/2001/XMLSchema#dateTime">2019-05-23T13:12:18</dcterms:issued>
    <cc:license rdf:resource="http://creativecommons.org/licenses/by/3.0"/>
  </rdf:Description>
  <rdf:Description rdf:about="http://purl.org/heritagedata/schemes/560/concepts/142186">
    <dcterms:identifier>http://purl.org/heritagedata/schemes/560/concepts/142186</dcterms:identifier>
    <dcterms:publisher rdf:resource="http://www.historicengland.org.uk"/>
    <cc:attributionURL rdf:resource="http://www.historicengland.org.uk"/>
    <cc:attributionName xml:lang="en">Historic England</cc:attributionName>
    <skos:prefLabel xml:lang="en">Pollen</skos:prefLabel>
    <skos:scopeNote xml:lang="en">Use for pollen and diaspores. Pollen consists of pollen grains which are the male gametes of flowering plants. Diaspores are the dispersive units of mosses, ferns, fern allies and some plants. To describe the actual object use PLANT REMAINS.</skos:scopeNote>
    <dcterms:issued rdf:datatype="http://www.w3.org/2001/XMLSchema#dateTime">2019-05-23T13:12:18</dcterms:issued>
    <skos:inScheme rdf:resource="http://purl.org/heritagedata/schemes/560"/>
    <rdf:type rdf:resource="http://www.w3.org/2004/02/skos/core#Concept"/>
    <cc:license rdf:resource="http://creativecommons.org/licenses/by/3.0"/>
  </rdf:Description>
  <rdf:Description rdf:about="http://purl.org/heritagedata/schemes/560/concepts/170614">
    <skos:inScheme rdf:resource="http://purl.org/heritagedata/schemes/560"/>
    <dcterms:identifier>http://purl.org/heritagedata/schemes/560/concepts/170614</dcterms:identifier>
    <rdf:type rdf:resource="http://www.w3.org/2004/02/skos/core#Concept"/>
    <skos:prefLabel xml:lang="en">Diatom Analysis</skos:prefLabel>
    <skos:scopeNote xml:lang="en">The study of diatoms preserved in deposits.</skos:scopeNote>
    <dcterms:publisher rdf:resource="http://www.historicengland.org.uk"/>
    <dcterms:issued rdf:datatype="http://www.w3.org/2001/XMLSchema#dateTime">2019-05-23T13:12:18</dcterms:issued>
    <cc:attributionURL rdf:resource="http://www.historicengland.org.uk"/>
    <cc:attributionName xml:lang="en">Historic England</cc:attributionName>
    <cc:license rdf:resource="http://creativecommons.org/licenses/by/3.0"/>
  </rdf:Description>
  <rdf:Description rdf:about="http://purl.org/heritagedata/schemes/560/concepts/142129">
    <cc:attributionURL rdf:resource="http://www.historicengland.org.uk"/>
    <cc:attributionName xml:lang="en">Historic England</cc:attributionName>
    <dcterms:identifier>http://purl.org/heritagedata/schemes/560/concepts/142129</dcterms:identifier>
    <skos:scopeNote xml:lang="en">Use where decoration is present.</skos:scopeNote>
    <skos:prefLabel xml:lang="en">Decorated</skos:prefLabel>
    <dcterms:issued rdf:datatype="http://www.w3.org/2001/XMLSchema#dateTime">2019-05-23T13:12:18</dcterms:issued>
    <cc:license rdf:resource="http://creativecommons.org/licenses/by/3.0"/>
    <rdf:type rdf:resource="http://www.w3.org/2004/02/skos/core#Concept"/>
    <dcterms:publisher rdf:resource="http://www.historicengland.org.uk"/>
    <skos:inScheme rdf:resource="http://purl.org/heritagedata/schemes/560"/>
  </rdf:Description>
  <rdf:Description rdf:about="http://purl.org/heritagedata/schemes/560/concepts/142196">
    <cc:license rdf:resource="http://creativecommons.org/licenses/by/3.0"/>
    <skos:scopeNote xml:lang="en">Use for the remains of epidermis or outermost layer. Relates to both animals and plants. If describing the actual object use PLANT REMAINS, ANIMAL REMAINS or HUMAN REMAINS.</skos:scopeNote>
    <skos:related rdf:resource="http://purl.org/heritagedata/schemes/560/concepts/142156"/>
    <skos:inScheme rdf:resource="http://purl.org/heritagedata/schemes/560"/>
    <cc:attributionName xml:lang="en">Historic England</cc:attributionName>
    <cc:attributionURL rdf:resource="http://www.historicengland.org.uk"/>
    <dcterms:publisher rdf:resource="http://www.historicengland.org.uk"/>
    <dcterms:issued rdf:datatype="http://www.w3.org/2001/XMLSchema#dateTime">2019-05-23T13:12:18</dcterms:issued>
    <rdf:type rdf:resource="http://www.w3.org/2004/02/skos/core#Concept"/>
    <dcterms:identifier>http://purl.org/heritagedata/schemes/560/concepts/142196</dcterms:identifier>
    <skos:prefLabel xml:lang="en">Skin</skos:prefLabel>
  </rdf:Description>
  <rdf:Description rdf:about="http://purl.org/heritagedata/schemes/560/concepts/142217">
    <skos:prefLabel xml:lang="en">X-Ray Diffraction</skos:prefLabel>
    <cc:attributionName xml:lang="en">Historic England</cc:attributionName>
    <dcterms:publisher rdf:resource="http://www.historicengland.org.uk"/>
    <cc:license rdf:resource="http://creativecommons.org/licenses/by/3.0"/>
    <skos:scopeNote xml:lang="en">A surface technique that uses the diffraction of X-rays to examine the mineral composition of a sample. Useful for identifying corrosion products, pigments etc. but of little use with organic compounds which consist largely of carbon, oxygen and hydrogen.</skos:scopeNote>
    <rdf:type rdf:resource="http://www.w3.org/2004/02/skos/core#Concept"/>
    <skos:inScheme rdf:resource="http://purl.org/heritagedata/schemes/560"/>
    <cc:attributionURL rdf:resource="http://www.historicengland.org.uk"/>
    <dcterms:issued rdf:datatype="http://www.w3.org/2001/XMLSchema#dateTime">2019-05-23T13:12:18</dcterms:issued>
    <dcterms:identifier>http://purl.org/heritagedata/schemes/560/concepts/142217</dcterms:identifier>
  </rdf:Description>
  <rdf:Description rdf:about="http://purl.org/heritagedata/schemes/560/concepts/148433">
    <dcterms:publisher rdf:resource="http://www.historicengland.org.uk"/>
    <skos:scopeNote xml:lang="en">The material which floats during the floatation of samples as a means of recovering charred plant remains from an archaeological context.</skos:scopeNote>
    <cc:license rdf:resource="http://creativecommons.org/licenses/by/3.0"/>
    <rdf:type rdf:resource="http://www.w3.org/2004/02/skos/core#Concept"/>
    <skos:inScheme rdf:resource="http://purl.org/heritagedata/schemes/560"/>
    <cc:attributionURL rdf:resource="http://www.historicengland.org.uk"/>
    <skos:prefLabel xml:lang="en">Flot</skos:prefLabel>
    <dcterms:issued rdf:datatype="http://www.w3.org/2001/XMLSchema#dateTime">2019-05-23T13:12:18</dcterms:issued>
    <dcterms:identifier>http://purl.org/heritagedata/schemes/560/concepts/148433</dcterms:identifier>
    <cc:attributionName xml:lang="en">Historic England</cc:attributionName>
  </rdf:Description>
  <rdf:Description rdf:about="http://purl.org/heritagedata/schemes/560/concepts/142194">
    <dcterms:publisher rdf:resource="http://www.historicengland.org.uk"/>
    <cc:license rdf:resource="http://creativecommons.org/licenses/by/3.0"/>
    <rdf:type rdf:resource="http://www.w3.org/2004/02/skos/core#Concept"/>
    <dcterms:identifier>http://purl.org/heritagedata/schemes/560/concepts/142194</dcterms:identifier>
    <dcterms:issued rdf:datatype="http://www.w3.org/2001/XMLSchema#dateTime">2019-05-23T13:12:18</dcterms:issued>
    <cc:attributionURL rdf:resource="http://www.historicengland.org.uk"/>
    <skos:inScheme rdf:resource="http://purl.org/heritagedata/schemes/560"/>
    <skos:scopeNote xml:lang="en">Use for material that has been burnt at high temperature in a good air supply such that only the silica component remains.</skos:scopeNote>
    <skos:prefLabel xml:lang="en">Silicified</skos:prefLabel>
    <cc:attributionName xml:lang="en">Historic England</cc:attributionName>
  </rdf:Description>
  <rdf:Description rdf:about="http://purl.org/heritagedata/schemes/560/concepts/142195">
    <skos:inScheme rdf:resource="http://purl.org/heritagedata/schemes/560"/>
    <dcterms:issued rdf:datatype="http://www.w3.org/2001/XMLSchema#dateTime">2019-05-23T13:12:18</dcterms:issued>
    <rdf:type rdf:resource="http://www.w3.org/2004/02/skos/core#Concept"/>
    <cc:attributionURL rdf:resource="http://www.historicengland.org.uk"/>
    <skos:scopeNote xml:lang="en">A precious metal of lustrous, white colour with great malleability and ductility.</skos:scopeNote>
    <dcterms:publisher rdf:resource="http://www.historicengland.org.uk"/>
    <dcterms:identifier>http://purl.org/heritagedata/schemes/560/concepts/142195</dcterms:identifier>
    <skos:prefLabel xml:lang="en">Silver</skos:prefLabel>
    <cc:license rdf:resource="http://creativecommons.org/licenses/by/3.0"/>
    <cc:attributionName xml:lang="en">Historic England</cc:attributionName>
  </rdf:Description>
  <rdf:Description rdf:about="http://purl.org/heritagedata/schemes/560/concepts/142176">
    <dcterms:identifier>http://purl.org/heritagedata/schemes/560/concepts/142176</dcterms:identifier>
    <skos:inScheme rdf:resource="http://purl.org/heritagedata/schemes/560"/>
    <skos:prefLabel xml:lang="en">Obsidian Hydration</skos:prefLabel>
    <rdf:type rdf:resource="http://www.w3.org/2004/02/skos/core#Concept"/>
    <dcterms:issued rdf:datatype="http://www.w3.org/2001/XMLSchema#dateTime">2019-05-23T13:12:18</dcterms:issued>
    <dcterms:publisher rdf:resource="http://www.historicengland.org.uk"/>
    <cc:attributionURL rdf:resource="http://www.historicengland.org.uk"/>
    <skos:scopeNote xml:lang="en">A technique used to date obsidian (volcanic glass) of all ages and is thus not commonly used in the UK.</skos:scopeNote>
    <cc:attributionName xml:lang="en">Historic England</cc:attributionName>
    <cc:license rdf:resource="http://creativecommons.org/licenses/by/3.0"/>
  </rdf:Description>
  <rdf:Description rdf:about="http://purl.org/heritagedata/schemes/560/concepts/142197">
    <dcterms:identifier>http://purl.org/heritagedata/schemes/560/concepts/142197</dcterms:identifier>
    <skos:prefLabel xml:lang="en">Soil Phosphorus Analysis</skos:prefLabel>
    <dcterms:publisher rdf:resource="http://www.historicengland.org.uk"/>
    <cc:attributionURL rdf:resource="http://www.historicengland.org.uk"/>
    <rdf:type rdf:resource="http://www.w3.org/2004/02/skos/core#Concept"/>
    <skos:inScheme rdf:resource="http://purl.org/heritagedata/schemes/560"/>
    <dcterms:issued rdf:datatype="http://www.w3.org/2001/XMLSchema#dateTime">2019-05-23T13:12:18</dcterms:issued>
    <cc:license rdf:resource="http://creativecommons.org/licenses/by/3.0"/>
    <cc:attributionName xml:lang="en">Historic England</cc:attributionName>
    <skos:scopeNote xml:lang="en">The analysis of the amount of phosphorus (P) present in a soil.</skos:scopeNote>
  </rdf:Description>
  <rdf:Description rdf:about="http://purl.org/heritagedata/schemes/560/concepts/144519">
    <dcterms:publisher rdf:resource="http://www.historicengland.org.uk"/>
    <cc:attributionURL rdf:resource="http://www.historicengland.org.uk"/>
    <cc:attributionName xml:lang="en">Historic England</cc:attributionName>
    <dcterms:identifier>http://purl.org/heritagedata/schemes/560/concepts/144519</dcterms:identifier>
    <skos:inScheme rdf:resource="http://purl.org/heritagedata/schemes/560"/>
    <skos:prefLabel xml:lang="en">Biogenic Carbonate</skos:prefLabel>
    <dcterms:issued rdf:datatype="http://www.w3.org/2001/XMLSchema#dateTime">2019-05-23T13:12:18</dcterms:issued>
    <cc:license rdf:resource="http://creativecommons.org/licenses/by/3.0"/>
    <rdf:type rdf:resource="http://www.w3.org/2004/02/skos/core#Concept"/>
    <skos:scopeNote xml:lang="en">Any carbonate material produced by biological activity, for instance operculae of snails.</skos:scopeNote>
  </rdf:Description>
  <rdf:Description rdf:about="http://purl.org/heritagedata/schemes/560/concepts/144521">
    <dcterms:publisher rdf:resource="http://www.historicengland.org.uk"/>
    <dcterms:identifier>http://purl.org/heritagedata/schemes/560/concepts/144521</dcterms:identifier>
    <cc:attributionURL rdf:resource="http://www.historicengland.org.uk"/>
    <rdf:type rdf:resource="http://www.w3.org/2004/02/skos/core#Concept"/>
    <skos:scopeNote xml:lang="en">A group of aluminosilicate minerals with varying compositions. The most common mineral in igneous rocks, and common in other rocks and sediments.</skos:scopeNote>
    <skos:inScheme rdf:resource="http://purl.org/heritagedata/schemes/560"/>
    <skos:prefLabel xml:lang="en">Feldspar</skos:prefLabel>
    <dcterms:issued rdf:datatype="http://www.w3.org/2001/XMLSchema#dateTime">2019-05-23T13:12:18</dcterms:issued>
    <cc:license rdf:resource="http://creativecommons.org/licenses/by/3.0"/>
    <cc:attributionName xml:lang="en">Historic England</cc:attributionName>
  </rdf:Description>
  <rdf:Description rdf:about="http://purl.org/heritagedata/schemes/560/concepts/148327">
    <dcterms:identifier>http://purl.org/heritagedata/schemes/560/concepts/148327</dcterms:identifier>
    <skos:inScheme rdf:resource="http://purl.org/heritagedata/schemes/560"/>
    <cc:license rdf:resource="http://creativecommons.org/licenses/by/3.0"/>
    <rdf:type rdf:resource="http://www.w3.org/2004/02/skos/core#Concept"/>
    <dcterms:publisher rdf:resource="http://www.historicengland.org.uk"/>
    <skos:prefLabel xml:lang="en">Carved</skos:prefLabel>
    <dcterms:issued rdf:datatype="http://www.w3.org/2001/XMLSchema#dateTime">2019-05-23T13:12:18</dcterms:issued>
    <cc:attributionURL rdf:resource="http://www.historicengland.org.uk"/>
    <cc:attributionName xml:lang="en">Historic England</cc:attributionName>
  </rdf:Description>
  <rdf:Description rdf:about="http://purl.org/heritagedata/schemes/560/concepts/142203">
    <dcterms:issued rdf:datatype="http://www.w3.org/2001/XMLSchema#dateTime">2019-05-23T13:12:18</dcterms:issued>
    <cc:attributionURL rdf:resource="http://www.historicengland.org.uk"/>
    <cc:attributionName xml:lang="en">Historic England</cc:attributionName>
    <skos:scopeNote xml:lang="en">The measurement of the light emitted from sedimentary minerals, mineral inclusions in bricks, burnt flint or unburnt calcite when they are heated. The signal relates to their prior exposure to radioactivity. Used to date samples up to 500,000 years old.</skos:scopeNote>
    <skos:inScheme rdf:resource="http://purl.org/heritagedata/schemes/560"/>
    <cc:license rdf:resource="http://creativecommons.org/licenses/by/3.0"/>
    <rdf:type rdf:resource="http://www.w3.org/2004/02/skos/core#Concept"/>
    <skos:prefLabel xml:lang="en">Thermoluminescence</skos:prefLabel>
    <dcterms:publisher rdf:resource="http://www.historicengland.org.uk"/>
    <dcterms:identifier>http://purl.org/heritagedata/schemes/560/concepts/142203</dcterms:identifier>
  </rdf:Description>
  <rdf:Description rdf:about="http://purl.org/heritagedata/schemes/560/concepts/142164">
    <skos:inScheme rdf:resource="http://purl.org/heritagedata/schemes/560"/>
    <skos:prefLabel xml:lang="en">Micromorphology</skos:prefLabel>
    <cc:license rdf:resource="http://creativecommons.org/licenses/by/3.0"/>
    <rdf:type rdf:resource="http://www.w3.org/2004/02/skos/core#Concept"/>
    <dcterms:issued rdf:datatype="http://www.w3.org/2001/XMLSchema#dateTime">2019-05-23T13:12:18</dcterms:issued>
    <cc:attributionName xml:lang="en">Historic England</cc:attributionName>
    <skos:scopeNote xml:lang="en">The microscopic analysis of thin sections of resin impregnated stratigraphy.</skos:scopeNote>
    <dcterms:publisher rdf:resource="http://www.historicengland.org.uk"/>
    <dcterms:identifier>http://purl.org/heritagedata/schemes/560/concepts/142164</dcterms:identifier>
    <cc:attributionURL rdf:resource="http://www.historicengland.org.uk"/>
  </rdf:Description>
  <rdf:Description rdf:about="http://purl.org/heritagedata/schemes/560/concepts/142187">
    <skos:inScheme rdf:resource="http://purl.org/heritagedata/schemes/560"/>
    <cc:license rdf:resource="http://creativecommons.org/licenses/by/3.0"/>
    <rdf:type rdf:resource="http://www.w3.org/2004/02/skos/core#Concept"/>
    <dcterms:identifier>http://purl.org/heritagedata/schemes/560/concepts/142187</dcterms:identifier>
    <dcterms:publisher rdf:resource="http://www.historicengland.org.uk"/>
    <dcterms:issued rdf:datatype="http://www.w3.org/2001/XMLSchema#dateTime">2019-05-23T13:12:18</dcterms:issued>
    <cc:attributionURL rdf:resource="http://www.historicengland.org.uk"/>
    <cc:attributionName xml:lang="en">Historic England</cc:attributionName>
    <skos:scopeNote xml:lang="en">The measurement of the ratio of a radioactive potassium (K) isotope and the argon (Ar) gas produced as a by-product of its decay. Useful for dating volcanic material older than 1,000 years.</skos:scopeNote>
    <skos:prefLabel xml:lang="en">Potassium Argon Dating</skos:prefLabel>
  </rdf:Description>
  <rdf:Description rdf:about="http://purl.org/heritagedata/schemes/560/concepts/142106">
    <skos:inScheme rdf:resource="http://purl.org/heritagedata/schemes/560"/>
    <cc:license rdf:resource="http://creativecommons.org/licenses/by/3.0"/>
    <cc:attributionName xml:lang="en">Historic England</cc:attributionName>
    <cc:attributionURL rdf:resource="http://www.historicengland.org.uk"/>
    <dcterms:issued rdf:datatype="http://www.w3.org/2001/XMLSchema#dateTime">2019-05-23T13:12:18</dcterms:issued>
    <dcterms:identifier>http://purl.org/heritagedata/schemes/560/concepts/142106</dcterms:identifier>
    <skos:prefLabel xml:lang="en">Available Phosphorus Analysis</skos:prefLabel>
    <dcterms:publisher rdf:resource="http://www.historicengland.org.uk"/>
    <skos:scopeNote xml:lang="en">The analysis of the amount of phosphorus (P) (liable fraction) available to plants.</skos:scopeNote>
    <rdf:type rdf:resource="http://www.w3.org/2004/02/skos/core#Concept"/>
  </rdf:Description>
  <rdf:Description rdf:about="http://purl.org/heritagedata/schemes/560/concepts/142979">
    <dcterms:publisher rdf:resource="http://www.historicengland.org.uk"/>
    <skos:scopeNote xml:lang="en">A naturally occuring deposit of calcareous tufa ('shell marl') sometimes found in alluvial deposits.</skos:scopeNote>
    <cc:attributionName xml:lang="en">Historic England</cc:attributionName>
    <cc:attributionURL rdf:resource="http://www.historicengland.org.uk"/>
    <dcterms:identifier>http://purl.org/heritagedata/schemes/560/concepts/142979</dcterms:identifier>
    <dcterms:issued rdf:datatype="http://www.w3.org/2001/XMLSchema#dateTime">2019-05-23T13:12:18</dcterms:issued>
    <skos:prefLabel xml:lang="en">Tufaceous Deposit</skos:prefLabel>
    <cc:license rdf:resource="http://creativecommons.org/licenses/by/3.0"/>
    <skos:inScheme rdf:resource="http://purl.org/heritagedata/schemes/560"/>
    <rdf:type rdf:resource="http://www.w3.org/2004/02/skos/core#Concept"/>
  </rdf:Description>
  <rdf:Description rdf:about="http://purl.org/heritagedata/schemes/560/concepts/144515">
    <dcterms:issued rdf:datatype="http://www.w3.org/2001/XMLSchema#dateTime">2019-05-23T13:12:18</dcterms:issued>
    <dcterms:identifier>http://purl.org/heritagedata/schemes/560/concepts/144515</dcterms:identifier>
    <cc:attributionName xml:lang="en">Historic England</cc:attributionName>
    <dcterms:publisher rdf:resource="http://www.historicengland.org.uk"/>
    <cc:license rdf:resource="http://creativecommons.org/licenses/by/3.0"/>
    <skos:scopeNote xml:lang="en">Material used for construction, commonly fired in its manufacture.</skos:scopeNote>
    <rdf:type rdf:resource="http://www.w3.org/2004/02/skos/core#Concept"/>
    <skos:inScheme rdf:resource="http://purl.org/heritagedata/schemes/560"/>
    <cc:attributionURL rdf:resource="http://www.historicengland.org.uk"/>
    <skos:prefLabel xml:lang="en">Brick</skos:prefLabel>
  </rdf:Description>
  <rdf:Description rdf:about="http://purl.org/heritagedata/schemes/560/concepts/142181">
    <dcterms:identifier>http://purl.org/heritagedata/schemes/560/concepts/142181</dcterms:identifier>
    <dcterms:publisher rdf:resource="http://www.historicengland.org.uk"/>
    <cc:attributionURL rdf:resource="http://www.historicengland.org.uk"/>
    <cc:attributionName xml:lang="en">Historic England</cc:attributionName>
    <skos:prefLabel xml:lang="en">Ph Determination</skos:prefLabel>
    <skos:inScheme rdf:resource="http://purl.org/heritagedata/schemes/560"/>
    <dcterms:issued rdf:datatype="http://www.w3.org/2001/XMLSchema#dateTime">2019-05-23T13:12:18</dcterms:issued>
    <cc:license rdf:resource="http://creativecommons.org/licenses/by/3.0"/>
    <rdf:type rdf:resource="http://www.w3.org/2004/02/skos/core#Concept"/>
    <skos:scopeNote xml:lang="en">The degree of acidity or alkalinity of a material.</skos:scopeNote>
  </rdf:Description>
  <rdf:Description rdf:about="http://purl.org/heritagedata/schemes/560/concepts/142209">
    <dcterms:issued rdf:datatype="http://www.w3.org/2001/XMLSchema#dateTime">2019-05-23T13:12:18</dcterms:issued>
    <cc:license rdf:resource="http://creativecommons.org/licenses/by/3.0"/>
    <dcterms:identifier>http://purl.org/heritagedata/schemes/560/concepts/142209</dcterms:identifier>
    <rdf:type rdf:resource="http://www.w3.org/2004/02/skos/core#Concept"/>
    <dcterms:publisher rdf:resource="http://www.historicengland.org.uk"/>
    <skos:related rdf:resource="http://purl.org/heritagedata/schemes/560/concepts/142131"/>
    <skos:inScheme rdf:resource="http://purl.org/heritagedata/schemes/560"/>
    <cc:attributionURL rdf:resource="http://www.historicengland.org.uk"/>
    <cc:attributionName xml:lang="en">Historic England</cc:attributionName>
    <skos:scopeNote xml:lang="en">The use of annual incremental growth in temperate trees to investigate environmental, especially local, parameters and the history of individual trees.</skos:scopeNote>
    <skos:prefLabel xml:lang="en">Tree-Ring Analysis</skos:prefLabel>
  </rdf:Description>
  <rdf:Description rdf:about="http://purl.org/heritagedata/schemes/560/concepts/142103">
    <skos:scopeNote xml:lang="en">Outgrowths of bone borne by most members of the deer family (Cervidae). They are shed and re-grow each year.</skos:scopeNote>
    <dcterms:issued rdf:datatype="http://www.w3.org/2001/XMLSchema#dateTime">2019-05-23T13:12:18</dcterms:issued>
    <cc:license rdf:resource="http://creativecommons.org/licenses/by/3.0"/>
    <rdf:type rdf:resource="http://www.w3.org/2004/02/skos/core#Concept"/>
    <skos:prefLabel xml:lang="en">Antler</skos:prefLabel>
    <dcterms:publisher rdf:resource="http://www.historicengland.org.uk"/>
    <cc:attributionURL rdf:resource="http://www.historicengland.org.uk"/>
    <cc:attributionName xml:lang="en">Historic England</cc:attributionName>
    <dcterms:identifier>http://purl.org/heritagedata/schemes/560/concepts/142103</dcterms:identifier>
    <skos:inScheme rdf:resource="http://purl.org/heritagedata/schemes/560"/>
  </rdf:Description>
  <rdf:Description rdf:about="http://purl.org/heritagedata/schemes/560/concepts/142207">
    <cc:attributionURL rdf:resource="http://www.historicengland.org.uk"/>
    <cc:attributionName xml:lang="en">Historic England</cc:attributionName>
    <skos:prefLabel xml:lang="en">Tooth</skos:prefLabel>
    <dcterms:identifier>http://purl.org/heritagedata/schemes/560/concepts/142207</dcterms:identifier>
    <dcterms:issued rdf:datatype="http://www.w3.org/2001/XMLSchema#dateTime">2019-05-23T13:12:18</dcterms:issued>
    <cc:license rdf:resource="http://creativecommons.org/licenses/by/3.0"/>
    <rdf:type rdf:resource="http://www.w3.org/2004/02/skos/core#Concept"/>
    <skos:inScheme rdf:resource="http://purl.org/heritagedata/schemes/560"/>
    <dcterms:publisher rdf:resource="http://www.historicengland.org.uk"/>
    <skos:scopeNote xml:lang="en">Use for teeth, hard structures found in the jaws of vertebrates used principally for chewing and eating.</skos:scopeNote>
  </rdf:Description>
  <rdf:Description rdf:about="http://purl.org/heritagedata/schemes/560/concepts/142127">
    <skos:altLabel xml:lang="en">Cremated</skos:altLabel>
  </rdf:Description>
  <rdf:Description rdf:about="http://purl.org/heritagedata/schemes/560/concepts/142170">
    <dcterms:publisher rdf:resource="http://www.historicengland.org.uk"/>
    <cc:attributionURL rdf:resource="http://www.historicengland.org.uk"/>
    <cc:attributionName xml:lang="en">Historic England</cc:attributionName>
    <dcterms:identifier>http://purl.org/heritagedata/schemes/560/concepts/142170</dcterms:identifier>
    <skos:scopeNote xml:lang="en">A dating technique for the founding of individual populations based on the assumption of steady rates of mutation in mitochondrial DNA. Sometimes used to produce dates for stratigraphic layers containing fossil specimens of populations.</skos:scopeNote>
    <skos:prefLabel xml:lang="en">Mitochondrial Dna</skos:prefLabel>
    <skos:inScheme rdf:resource="http://purl.org/heritagedata/schemes/560"/>
    <dcterms:issued rdf:datatype="http://www.w3.org/2001/XMLSchema#dateTime">2019-05-23T13:12:18</dcterms:issued>
    <cc:license rdf:resource="http://creativecommons.org/licenses/by/3.0"/>
    <rdf:type rdf:resource="http://www.w3.org/2004/02/skos/core#Concept"/>
  </rdf:Description>
  <rdf:Description rdf:about="http://purl.org/heritagedata/schemes/560/concepts/144524">
    <skos:altLabel xml:lang="en">OSL</skos:altLabel>
  </rdf:Description>
  <rdf:Description rdf:about="http://purl.org/heritagedata/schemes/560/concepts/142189">
    <dcterms:identifier>http://purl.org/heritagedata/schemes/560/concepts/142189</dcterms:identifier>
    <skos:inScheme rdf:resource="http://purl.org/heritagedata/schemes/560"/>
    <cc:attributionURL rdf:resource="http://www.historicengland.org.uk"/>
    <cc:attributionName xml:lang="en">Historic England</cc:attributionName>
    <skos:scopeNote xml:lang="en">Material comprising entrie or partial transverse sections of stems. Bark may be present or not. Can include complete sections of tree trunk but generally comprises smaller (&lt;20cm diameter) material.</skos:scopeNote>
    <dcterms:issued rdf:datatype="http://www.w3.org/2001/XMLSchema#dateTime">2019-05-23T13:12:18</dcterms:issued>
    <cc:license rdf:resource="http://creativecommons.org/licenses/by/3.0"/>
    <rdf:type rdf:resource="http://www.w3.org/2004/02/skos/core#Concept"/>
    <dcterms:publisher rdf:resource="http://www.historicengland.org.uk"/>
    <skos:prefLabel xml:lang="en">Roundwood</skos:prefLabel>
  </rdf:Description>
  <rdf:Description rdf:about="http://purl.org/heritagedata/schemes/560/concepts/142215">
    <cc:license rdf:resource="http://creativecommons.org/licenses/by/3.0"/>
    <cc:attributionName xml:lang="en">Historic England</cc:attributionName>
    <skos:scopeNote xml:lang="en">Use for any material that shows evidence of modification by humans.</skos:scopeNote>
    <skos:prefLabel xml:lang="en">Worked</skos:prefLabel>
    <dcterms:issued rdf:datatype="http://www.w3.org/2001/XMLSchema#dateTime">2019-05-23T13:12:18</dcterms:issued>
    <rdf:type rdf:resource="http://www.w3.org/2004/02/skos/core#Concept"/>
    <cc:attributionURL rdf:resource="http://www.historicengland.org.uk"/>
    <dcterms:publisher rdf:resource="http://www.historicengland.org.uk"/>
    <skos:inScheme rdf:resource="http://purl.org/heritagedata/schemes/560"/>
    <dcterms:identifier>http://purl.org/heritagedata/schemes/560/concepts/142215</dcterms:identifier>
  </rdf:Description>
  <rdf:Description rdf:about="http://purl.org/heritagedata/schemes/560/concepts/142135">
    <skos:prefLabel xml:lang="en">Egg Shell</skos:prefLabel>
    <cc:attributionURL rdf:resource="http://www.historicengland.org.uk"/>
    <skos:inScheme rdf:resource="http://purl.org/heritagedata/schemes/560"/>
    <dcterms:issued rdf:datatype="http://www.w3.org/2001/XMLSchema#dateTime">2019-05-23T13:12:18</dcterms:issued>
    <dcterms:identifier>http://purl.org/heritagedata/schemes/560/concepts/142135</dcterms:identifier>
    <dcterms:publisher rdf:resource="http://www.historicengland.org.uk"/>
    <rdf:type rdf:resource="http://www.w3.org/2004/02/skos/core#Concept"/>
    <skos:scopeNote xml:lang="en">Use for the remains of an egg whether from a bird, reptile or amphibian.</skos:scopeNote>
    <cc:attributionName xml:lang="en">Historic England</cc:attributionName>
    <cc:license rdf:resource="http://creativecommons.org/licenses/by/3.0"/>
  </rdf:Description>
  <rdf:Description rdf:about="http://purl.org/heritagedata/schemes/560/concepts/142146">
    <cc:attributionName xml:lang="en">Historic England</cc:attributionName>
    <cc:attributionURL rdf:resource="http://www.historicengland.org.uk"/>
    <skos:scopeNote xml:lang="en">Use for hair, fur etc: filaments growing out of the outermost layer of mammalian skin.</skos:scopeNote>
    <skos:prefLabel xml:lang="en">Hair</skos:prefLabel>
    <dcterms:publisher rdf:resource="http://www.historicengland.org.uk"/>
    <dcterms:identifier>http://purl.org/heritagedata/schemes/560/concepts/142146</dcterms:identifier>
    <skos:inScheme rdf:resource="http://purl.org/heritagedata/schemes/560"/>
    <rdf:type rdf:resource="http://www.w3.org/2004/02/skos/core#Concept"/>
    <dcterms:issued rdf:datatype="http://www.w3.org/2001/XMLSchema#dateTime">2019-05-23T13:12:18</dcterms:issued>
    <cc:license rdf:resource="http://creativecommons.org/licenses/by/3.0"/>
  </rdf:Description>
  <rdf:Description rdf:about="http://purl.org/heritagedata/schemes/560/concepts/142101">
    <cc:attributionName xml:lang="en">Historic England</cc:attributionName>
    <skos:prefLabel xml:lang="en">Ancient Biomolecular Analysis</skos:prefLabel>
    <dcterms:identifier>http://purl.org/heritagedata/schemes/560/concepts/142101</dcterms:identifier>
    <dcterms:issued rdf:datatype="http://www.w3.org/2001/XMLSchema#dateTime">2019-05-23T13:12:18</dcterms:issued>
    <skos:inScheme rdf:resource="http://purl.org/heritagedata/schemes/560"/>
    <cc:attributionURL rdf:resource="http://www.historicengland.org.uk"/>
    <rdf:type rdf:resource="http://www.w3.org/2004/02/skos/core#Concept"/>
    <skos:scopeNote xml:lang="en">Characterisation of organic molecules extracted from fossil or sub-fossil materials, including lipids, DNA etc.</skos:scopeNote>
    <dcterms:publisher rdf:resource="http://www.historicengland.org.uk"/>
    <cc:license rdf:resource="http://creativecommons.org/licenses/by/3.0"/>
  </rdf:Description>
  <rdf:Description rdf:about="http://purl.org/heritagedata/schemes/560/concepts/142115">
    <skos:altLabel xml:lang="en">Carbon Dating</skos:altLabel>
  </rdf:Description>
  <rdf:Description rdf:about="http://purl.org/heritagedata/schemes/560/concepts/142138">
    <skos:scopeNote xml:lang="en">Any metal prinicipally composed of the chemical element Iron (Fe).</skos:scopeNote>
    <dcterms:identifier>http://purl.org/heritagedata/schemes/560/concepts/142138</dcterms:identifier>
    <dcterms:publisher rdf:resource="http://www.historicengland.org.uk"/>
    <cc:attributionURL rdf:resource="http://www.historicengland.org.uk"/>
    <rdf:type rdf:resource="http://www.w3.org/2004/02/skos/core#Concept"/>
    <skos:inScheme rdf:resource="http://purl.org/heritagedata/schemes/560"/>
    <skos:prefLabel xml:lang="en">Ferrous Metal</skos:prefLabel>
    <dcterms:issued rdf:datatype="http://www.w3.org/2001/XMLSchema#dateTime">2019-05-23T13:12:18</dcterms:issued>
    <cc:license rdf:resource="http://creativecommons.org/licenses/by/3.0"/>
    <cc:attributionName xml:lang="en">Historic England</cc:attributionName>
  </rdf:Description>
  <rdf:Description rdf:about="http://purl.org/heritagedata/schemes/560/concepts/142219">
    <skos:altLabel xml:lang="en">XRD</skos:altLabel>
  </rdf:Description>
  <rdf:Description rdf:about="http://purl.org/heritagedata/schemes/560/concepts/142100">
    <dcterms:publisher rdf:resource="http://www.historicengland.org.uk"/>
    <cc:license rdf:resource="http://creativecommons.org/licenses/by/3.0"/>
    <rdf:type rdf:resource="http://www.w3.org/2004/02/skos/core#Concept"/>
    <dcterms:issued rdf:datatype="http://www.w3.org/2001/XMLSchema#dateTime">2019-05-23T13:12:18</dcterms:issued>
    <cc:attributionURL rdf:resource="http://www.historicengland.org.uk"/>
    <dcterms:identifier>http://purl.org/heritagedata/schemes/560/concepts/142100</dcterms:identifier>
    <skos:inScheme rdf:resource="http://purl.org/heritagedata/schemes/560"/>
    <skos:scopeNote xml:lang="en">The measurement of chemical alterations in the amino acids in protein molecules from bones, shells and teeth. Date range can be between 1,000 and several million years.</skos:scopeNote>
    <skos:prefLabel xml:lang="en">Amino Acid Racemisation</skos:prefLabel>
    <cc:attributionName xml:lang="en">Historic England</cc:attributionName>
  </rdf:Description>
  <rdf:Description rdf:about="http://purl.org/heritagedata/schemes/560/concepts/142128">
    <dcterms:identifier>http://purl.org/heritagedata/schemes/560/concepts/142128</dcterms:identifier>
    <cc:attributionURL rdf:resource="http://www.historicengland.org.uk"/>
    <cc:attributionName xml:lang="en">Historic England</cc:attributionName>
    <skos:prefLabel xml:lang="en">Dating Techniques</skos:prefLabel>
    <dcterms:issued rdf:datatype="http://www.w3.org/2001/XMLSchema#dateTime">2019-05-23T13:12:18</dcterms:issued>
    <cc:license rdf:resource="http://creativecommons.org/licenses/by/3.0"/>
    <rdf:type rdf:resource="http://www.w3.org/2004/02/skos/core#Concept"/>
    <skos:inScheme rdf:resource="http://purl.org/heritagedata/schemes/560"/>
    <dcterms:publisher rdf:resource="http://www.historicengland.org.uk"/>
    <skos:scopeNote xml:lang="en">Techniques applied to a material in order to date it or material associated with it. Use more specific terms.</skos:scopeNote>
  </rdf:Description>
  <rdf:Description rdf:about="http://purl.org/heritagedata/schemes/560/concepts/148434">
    <dcterms:publisher rdf:resource="http://www.historicengland.org.uk"/>
    <cc:license rdf:resource="http://creativecommons.org/licenses/by/3.0"/>
    <rdf:type rdf:resource="http://www.w3.org/2004/02/skos/core#Concept"/>
    <dcterms:identifier>http://purl.org/heritagedata/schemes/560/concepts/148434</dcterms:identifier>
    <skos:inScheme rdf:resource="http://purl.org/heritagedata/schemes/560"/>
    <cc:attributionURL rdf:resource="http://www.historicengland.org.uk"/>
    <dcterms:issued rdf:datatype="http://www.w3.org/2001/XMLSchema#dateTime">2019-05-23T13:12:18</dcterms:issued>
    <skos:scopeNote xml:lang="en">The material that does not float during the floatation of samples as a means of recovering charred plant remains from an archaeological context. Also, the material remaining following wet or dry sieving of course sieved samples.</skos:scopeNote>
    <cc:attributionName xml:lang="en">Historic England</cc:attributionName>
    <skos:prefLabel xml:lang="en">Residue</skos:prefLabel>
  </rdf:Description>
  <rdf:Description rdf:about="http://purl.org/heritagedata/schemes/560/concepts/148328">
    <skos:prefLabel xml:lang="en">Waterworn</skos:prefLabel>
    <dcterms:identifier>http://purl.org/heritagedata/schemes/560/concepts/148328</dcterms:identifier>
    <dcterms:publisher rdf:resource="http://www.historicengland.org.uk"/>
    <cc:attributionURL rdf:resource="http://www.historicengland.org.uk"/>
    <rdf:type rdf:resource="http://www.w3.org/2004/02/skos/core#Concept"/>
    <skos:inScheme rdf:resource="http://purl.org/heritagedata/schemes/560"/>
    <skos:scopeNote xml:lang="en">Material, especially rock, worn smooth by the passage of water.</skos:scopeNote>
    <dcterms:issued rdf:datatype="http://www.w3.org/2001/XMLSchema#dateTime">2019-05-23T13:12:18</dcterms:issued>
    <cc:license rdf:resource="http://creativecommons.org/licenses/by/3.0"/>
    <cc:attributionName xml:lang="en">Historic England</cc:attributionName>
  </rdf:Description>
  <rdf:Description rdf:about="http://purl.org/heritagedata/schemes/560/concepts/142159">
    <dcterms:identifier>http://purl.org/heritagedata/schemes/560/concepts/142159</dcterms:identifier>
    <skos:scopeNote xml:lang="en">Use where the material presents debris or waste from manufacturing.</skos:scopeNote>
    <dcterms:issued rdf:datatype="http://www.w3.org/2001/XMLSchema#dateTime">2019-05-23T13:12:18</dcterms:issued>
    <cc:license rdf:resource="http://creativecommons.org/licenses/by/3.0"/>
    <rdf:type rdf:resource="http://www.w3.org/2004/02/skos/core#Concept"/>
    <skos:inScheme rdf:resource="http://purl.org/heritagedata/schemes/560"/>
    <dcterms:publisher rdf:resource="http://www.historicengland.org.uk"/>
    <skos:prefLabel xml:lang="en">Manufacturing Debris</skos:prefLabel>
    <cc:attributionURL rdf:resource="http://www.historicengland.org.uk"/>
    <cc:attributionName xml:lang="en">Historic England</cc:attributionName>
  </rdf:Description>
  <rdf:Description rdf:about="http://purl.org/heritagedata/schemes/560/concepts/142211">
    <skos:prefLabel xml:lang="en">Twig</skos:prefLabel>
    <dcterms:publisher rdf:resource="http://www.historicengland.org.uk"/>
    <cc:attributionName xml:lang="en">Historic England</cc:attributionName>
    <cc:license rdf:resource="http://creativecommons.org/licenses/by/3.0"/>
    <skos:scopeNote xml:lang="en">Small (&lt;2cm diameter) roundwood often complete with buds or leaf scars.</skos:scopeNote>
    <dcterms:issued rdf:datatype="http://www.w3.org/2001/XMLSchema#dateTime">2019-05-23T13:12:18</dcterms:issued>
    <dcterms:identifier>http://purl.org/heritagedata/schemes/560/concepts/142211</dcterms:identifier>
    <cc:attributionURL rdf:resource="http://www.historicengland.org.uk"/>
    <skos:inScheme rdf:resource="http://purl.org/heritagedata/schemes/560"/>
    <rdf:type rdf:resource="http://www.w3.org/2004/02/skos/core#Concept"/>
  </rdf:Description>
  <rdf:Description rdf:about="http://purl.org/heritagedata/schemes/560/concepts/142220">
    <skos:altLabel xml:lang="en">XRF</skos:altLabel>
  </rdf:Description>
  <rdf:Description rdf:about="http://purl.org/heritagedata/schemes/560/concepts/142198">
    <cc:attributionURL rdf:resource="http://www.historicengland.org.uk"/>
    <rdf:type rdf:resource="http://www.w3.org/2004/02/skos/core#Concept"/>
    <dcterms:identifier>http://purl.org/heritagedata/schemes/560/concepts/142198</dcterms:identifier>
    <skos:inScheme rdf:resource="http://purl.org/heritagedata/schemes/560"/>
    <dcterms:publisher rdf:resource="http://www.historicengland.org.uk"/>
    <cc:license rdf:resource="http://creativecommons.org/licenses/by/3.0"/>
    <cc:attributionName xml:lang="en">Historic England</cc:attributionName>
    <skos:prefLabel xml:lang="en">Specialist Sampling</skos:prefLabel>
    <skos:scopeNote xml:lang="en">The recovery of material from samples collected during field investigations, usually taken by specialists with a particular area of expertise. Normally processed in the laboratory. Also use for the processing of samples subsequent to investigation.</skos:scopeNote>
    <dcterms:issued rdf:datatype="http://www.w3.org/2001/XMLSchema#dateTime">2019-05-23T13:12:18</dcterms:issued>
  </rdf:Description>
  <rdf:Description rdf:about="http://purl.org/heritagedata/schemes/560/concepts/142190">
    <skos:altLabel xml:lang="en">S.E.M.</skos:altLabel>
  </rdf:Description>
  <rdf:Description rdf:about="http://purl.org/heritagedata/schemes/560/concepts/147277">
    <dcterms:identifier>http://purl.org/heritagedata/schemes/560/concepts/147277</dcterms:identifier>
    <dcterms:issued rdf:datatype="http://www.w3.org/2001/XMLSchema#dateTime">2019-05-23T13:12:18</dcterms:issued>
    <cc:attributionName xml:lang="en">Historic England</cc:attributionName>
    <dcterms:publisher rdf:resource="http://www.historicengland.org.uk"/>
    <cc:license rdf:resource="http://creativecommons.org/licenses/by/3.0"/>
    <skos:scopeNote xml:lang="en">A measure of the proportion of water within a sample.</skos:scopeNote>
    <rdf:type rdf:resource="http://www.w3.org/2004/02/skos/core#Concept"/>
    <cc:attributionURL rdf:resource="http://www.historicengland.org.uk"/>
    <skos:inScheme rdf:resource="http://purl.org/heritagedata/schemes/560"/>
    <skos:prefLabel xml:lang="en">Moisture Content</skos:prefLabel>
  </rdf:Description>
  <rdf:Description rdf:about="http://purl.org/heritagedata/schemes/560/concepts/142116">
    <skos:altLabel xml:lang="en">Carbonised</skos:altLabel>
  </rdf:Description>
  <rdf:Description rdf:about="http://purl.org/heritagedata/schemes/560/concepts/142205">
    <cc:attributionURL rdf:resource="http://www.historicengland.org.uk"/>
    <skos:inScheme rdf:resource="http://purl.org/heritagedata/schemes/560"/>
    <rdf:type rdf:resource="http://www.w3.org/2004/02/skos/core#Concept"/>
    <skos:scopeNote xml:lang="en">Use where evidence of tool marks is present</skos:scopeNote>
    <dcterms:issued rdf:datatype="http://www.w3.org/2001/XMLSchema#dateTime">2019-05-23T13:12:18</dcterms:issued>
    <dcterms:identifier>http://purl.org/heritagedata/schemes/560/concepts/142205</dcterms:identifier>
    <dcterms:publisher rdf:resource="http://www.historicengland.org.uk"/>
    <skos:prefLabel xml:lang="en">Tool Marked</skos:prefLabel>
    <cc:attributionName xml:lang="en">Historic England</cc:attributionName>
    <cc:license rdf:resource="http://creativecommons.org/licenses/by/3.0"/>
  </rdf:Description>
  <rdf:Description rdf:about="http://purl.org/heritagedata/schemes/560/concepts/142188">
    <dcterms:identifier>http://purl.org/heritagedata/schemes/560/concepts/142188</dcterms:identifier>
    <skos:inScheme rdf:resource="http://purl.org/heritagedata/schemes/560"/>
    <cc:license rdf:resource="http://creativecommons.org/licenses/by/3.0"/>
    <cc:attributionName xml:lang="en">Historic England</cc:attributionName>
    <dcterms:issued rdf:datatype="http://www.w3.org/2001/XMLSchema#dateTime">2019-05-23T13:12:18</dcterms:issued>
    <skos:prefLabel xml:lang="en">Radiocarbon Dating</skos:prefLabel>
    <skos:scopeNote xml:lang="en">The measurement of the ratio of the radioactive Carbon 14 (C-14) isotope and non-radioactive carbon isotopes. Useful for dating organic materials such as wood and bone between 500 and 45,000 years old.</skos:scopeNote>
    <dcterms:publisher rdf:resource="http://www.historicengland.org.uk"/>
    <cc:attributionURL rdf:resource="http://www.historicengland.org.uk"/>
    <rdf:type rdf:resource="http://www.w3.org/2004/02/skos/core#Concept"/>
  </rdf:Description>
  <rdf:Description rdf:about="http://purl.org/heritagedata/schemes/560/concepts/142193">
    <dcterms:identifier>http://purl.org/heritagedata/schemes/560/concepts/142193</dcterms:identifier>
    <cc:attributionURL rdf:resource="http://www.historicengland.org.uk"/>
    <dcterms:issued rdf:datatype="http://www.w3.org/2001/XMLSchema#dateTime">2019-05-23T13:12:18</dcterms:issued>
    <skos:scopeNote xml:lang="en">Use for any shell of an animal, principally, molluscs, crabs etc.</skos:scopeNote>
    <skos:inScheme rdf:resource="http://purl.org/heritagedata/schemes/560"/>
    <dcterms:publisher rdf:resource="http://www.historicengland.org.uk"/>
    <skos:prefLabel xml:lang="en">Shell</skos:prefLabel>
    <rdf:type rdf:resource="http://www.w3.org/2004/02/skos/core#Concept"/>
    <cc:attributionName xml:lang="en">Historic England</cc:attributionName>
    <cc:license rdf:resource="http://creativecommons.org/licenses/by/3.0"/>
  </rdf:Description>
  <rdf:Description rdf:about="http://purl.org/heritagedata/schemes/560/concepts/142126">
    <skos:scopeNote xml:lang="en">Waste material from the digestive tract of animals. The term coprolite comes from the Greek 'kopros' meaning dung and 'lithos' meaning stone, and is used for faecal matter that has been preserved by mineral replacement or dessication.</skos:scopeNote>
    <cc:attributionURL rdf:resource="http://www.historicengland.org.uk"/>
    <cc:attributionName xml:lang="en">Historic England</cc:attributionName>
    <dcterms:publisher rdf:resource="http://www.historicengland.org.uk"/>
    <skos:inScheme rdf:resource="http://purl.org/heritagedata/schemes/560"/>
    <cc:license rdf:resource="http://creativecommons.org/licenses/by/3.0"/>
    <rdf:type rdf:resource="http://www.w3.org/2004/02/skos/core#Concept"/>
    <dcterms:issued rdf:datatype="http://www.w3.org/2001/XMLSchema#dateTime">2019-05-23T13:12:18</dcterms:issued>
    <dcterms:identifier>http://purl.org/heritagedata/schemes/560/concepts/142126</dcterms:identifier>
    <skos:prefLabel xml:lang="en">Coprolite</skos:prefLabel>
  </rdf:Description>
  <rdf:Description rdf:about="http://purl.org/heritagedata/schemes/560/concepts/142140">
    <skos:inScheme rdf:resource="http://purl.org/heritagedata/schemes/560"/>
    <cc:attributionURL rdf:resource="http://www.historicengland.org.uk"/>
    <cc:attributionName xml:lang="en">Historic England</cc:attributionName>
    <dcterms:identifier>http://purl.org/heritagedata/schemes/560/concepts/142140</dcterms:identifier>
    <skos:scopeNote xml:lang="en">A technique for the dating of damage tracks in volcanic materials caused by the fissioning of decaying radioactive uranium (U) isotopes. Useful in samples more than 50,000 years old.</skos:scopeNote>
    <dcterms:issued rdf:datatype="http://www.w3.org/2001/XMLSchema#dateTime">2019-05-23T13:12:18</dcterms:issued>
    <cc:license rdf:resource="http://creativecommons.org/licenses/by/3.0"/>
    <rdf:type rdf:resource="http://www.w3.org/2004/02/skos/core#Concept"/>
    <skos:prefLabel xml:lang="en">Fission Track Analysis</skos:prefLabel>
    <dcterms:publisher rdf:resource="http://www.historicengland.org.uk"/>
  </rdf:Description>
  <rdf:Description rdf:about="http://purl.org/heritagedata/schemes/560/concepts/142112">
    <skos:altLabel xml:lang="en">C14 Dating</skos:altLabel>
  </rdf:Description>
  <rdf:Description rdf:about="http://purl.org/heritagedata/schemes/560/concepts/170623">
    <skos:altLabel xml:lang="en">Osteoarchaeology</skos:altLabel>
  </rdf:Description>
  <rdf:Description rdf:about="http://purl.org/heritagedata/schemes/560/concepts/142204">
    <skos:altLabel xml:lang="en">TL Dating</skos:altLabel>
  </rdf:Description>
  <rdf:Description rdf:about="http://purl.org/heritagedata/schemes/560/concepts/142206">
    <skos:altLabel xml:lang="en">Tool Marks</skos:altLabel>
  </rdf:Description>
  <rdf:Description rdf:about="http://purl.org/heritagedata/schemes/560/concepts/170622">
    <skos:altLabel xml:lang="en">Bioarchaeology</skos:altLabel>
  </rdf:Description>
  <rdf:Description rdf:about="http://purl.org/heritagedata/schemes/560/concepts/142192">
    <skos:altLabel xml:lang="en">Sem</skos:altLabel>
  </rdf:Description>
  <rdf:Description rdf:about="http://purl.org/heritagedata/schemes/560/concepts/144512">
    <skos:altLabel xml:lang="en">TL</skos:altLabel>
  </rdf:Description>
  <rdf:Description rdf:about="http://purl.org/heritagedata/schemes/560/concepts/148435">
    <skos:altLabel xml:lang="en">Heavy Residue</skos:altLabel>
  </rdf:Description>
  <rdf:Description rdf:about="http://purl.org/heritagedata/schemes/560/concepts/142133">
    <skos:altLabel xml:lang="en">Disease</skos:altLabel>
  </rdf:Description>
  <rdf:Description rdf:about="http://purl.org/heritagedata/schemes/560/concepts/142163">
    <skos:altLabel xml:lang="en">Microfossils</skos:altLabel>
  </rdf:Description>
  <rdf:Description rdf:about="http://purl.org/heritagedata/schemes/560/concepts/142114">
    <skos:altLabel xml:lang="en">Carbon 14 Dating</skos:altLabel>
  </rdf:Description>
  <rdf:Description rdf:about="http://purl.org/heritagedata/schemes/560/concepts/144527">
    <skos:altLabel xml:lang="en">IRSL Dating</skos:altLabel>
  </rdf:Description>
  <rdf:Description rdf:about="http://purl.org/heritagedata/schemes/560/concepts/142123">
    <skos:altLabel xml:lang="en">Colored</skos:altLabel>
  </rdf:Description>
  <rdf:Description rdf:about="http://purl.org/heritagedata/schemes/560/concepts/144525">
    <skos:altLabel xml:lang="en">OSL Dating</skos:altLabel>
  </rdf:Description>
  <rdf:Description rdf:about="http://purl.org/heritagedata/schemes/560/concepts/142978">
    <skos:altLabel xml:lang="en">Burnt Deposit</skos:altLabel>
  </rdf:Description>
  <rdf:Description rdf:about="http://purl.org/heritagedata/schemes/560/concepts/142168">
    <skos:altLabel xml:lang="en">Mineralised</skos:altLabel>
  </rdf:Description>
  <rdf:Description rdf:about="http://purl.org/heritagedata/schemes/560/concepts/142213">
    <skos:altLabel xml:lang="en">Waterlogged</skos:altLabel>
  </rdf:Description>
  <rdf:Description rdf:about="http://purl.org/heritagedata/schemes/560/concepts/170617">
    <skos:altLabel xml:lang="en">Archaeozoology</skos:altLabel>
  </rdf:Description>
  <rdf:Description rdf:about="http://purl.org/heritagedata/schemes/560/concepts/142130">
    <skos:altLabel xml:lang="en">Decoration</skos:altLabel>
  </rdf:Description>
  <rdf:Description rdf:about="http://purl.org/heritagedata/schemes/560/concepts/144526">
    <skos:altLabel xml:lang="en">IRSL</skos:altLabel>
  </rdf:Description>
  <rdf:Description rdf:about="http://purl.org/heritagedata/schemes/560/concepts/142110">
    <skos:altLabel xml:lang="en">Bulk Sampling</skos:altLabel>
  </rdf:Description>
  <rdf:Description rdf:about="http://purl.org/heritagedata/schemes/560/concepts/142210">
    <skos:altLabel xml:lang="en">Tree-Ring Studies</skos:altLabel>
  </rdf:Description>
</rdf:RDF>