<?xml version="1.0" encoding="UTF-8"?>
<rdf:RDF
   xmlns:cc="http://creativecommons.org/ns#"
   xmlns:dcterms="http://purl.org/dc/terms/"
   xmlns:ns1="http://www.w3.org/2004/02/skos/core#skos:"
   xmlns:rdf="http://www.w3.org/1999/02/22-rdf-syntax-ns#"
   xmlns:skos="http://www.w3.org/2004/02/skos/core#"
>
  <rdf:Description rdf:about="http://purl.org/heritagedata/schemes/225/concepts/136231">
    <dcterms:identifier>http://purl.org/heritagedata/schemes/225/concepts/136231</dcterms:identifier>
    <dcterms:publisher rdf:resource="http://www.historicengland.org.uk"/>
    <rdf:type rdf:resource="http://www.w3.org/2004/02/skos/core#Concept"/>
    <ns1:related rdf:resource="http://purl.org/heritagedata/schemes/225/concepts/167000"/>
    <skos:scopeNote xml:lang="en">Single-engine, single-seat biplane seaplane built for the 1924 Schneider Cup Race.</skos:scopeNote>
    <dcterms:issued rdf:datatype="http://www.w3.org/2001/XMLSchema#dateTime">2019-03-26T16:45:43</dcterms:issued>
    <skos:inScheme rdf:resource="http://purl.org/heritagedata/schemes/225"/>
    <cc:attributionURL rdf:resource="http://www.historicengland.org.uk"/>
    <skos:broader rdf:resource="http://purl.org/heritagedata/schemes/225/concepts/111413"/>
    <skos:broader rdf:resource="http://purl.org/heritagedata/schemes/225/concepts/134997"/>
    <cc:attributionName xml:lang="en">Historic England</cc:attributionName>
    <cc:license rdf:resource="http://creativecommons.org/licenses/by/3.0"/>
    <skos:prefLabel xml:lang="en">Gloster II</skos:prefLabel>
    <skos:broader rdf:resource="http://purl.org/heritagedata/schemes/225/concepts/111403"/>
  </rdf:Description>
  <rdf:Description rdf:about="http://purl.org/heritagedata/schemes/225/concepts/137215">
    <cc:license rdf:resource="http://creativecommons.org/licenses/by/3.0"/>
    <rdf:type rdf:resource="http://www.w3.org/2004/02/skos/core#Concept"/>
    <cc:attributionURL rdf:resource="http://www.historicengland.org.uk"/>
    <skos:inScheme rdf:resource="http://purl.org/heritagedata/schemes/225"/>
    <skos:broader rdf:resource="http://purl.org/heritagedata/schemes/225/concepts/137213"/>
    <dcterms:issued rdf:datatype="http://www.w3.org/2001/XMLSchema#dateTime">2019-03-26T16:45:43</dcterms:issued>
    <skos:prefLabel xml:lang="en">Buffalo</skos:prefLabel>
    <skos:broader rdf:resource="http://purl.org/heritagedata/schemes/225/concepts/111402"/>
    <skos:scopeNote xml:lang="en">American, all-metal-construction, fighter. Entered service in 1941. 209 were delivered to RAF/FAA, most of which were used in the Far East.</skos:scopeNote>
    <dcterms:publisher rdf:resource="http://www.historicengland.org.uk"/>
    <cc:attributionName xml:lang="en">Historic England</cc:attributionName>
    <dcterms:identifier>http://purl.org/heritagedata/schemes/225/concepts/137215</dcterms:identifier>
    <skos:broader rdf:resource="http://purl.org/heritagedata/schemes/225/concepts/111397"/>
  </rdf:Description>
  <rdf:Description rdf:about="http://purl.org/heritagedata/schemes/225/concepts/137236">
    <rdf:type rdf:resource="http://www.w3.org/2004/02/skos/core#Concept"/>
    <skos:broader rdf:resource="http://purl.org/heritagedata/schemes/225/concepts/111424"/>
    <cc:license rdf:resource="http://creativecommons.org/licenses/by/3.0"/>
    <cc:attributionName xml:lang="en">Historic England</cc:attributionName>
    <cc:attributionURL rdf:resource="http://www.historicengland.org.uk"/>
    <skos:inScheme rdf:resource="http://purl.org/heritagedata/schemes/225"/>
    <skos:broader rdf:resource="http://purl.org/heritagedata/schemes/225/concepts/111398"/>
    <skos:broader rdf:resource="http://purl.org/heritagedata/schemes/225/concepts/111402"/>
    <dcterms:issued rdf:datatype="http://www.w3.org/2001/XMLSchema#dateTime">2019-03-26T16:45:43</dcterms:issued>
    <skos:broader rdf:resource="http://purl.org/heritagedata/schemes/225/concepts/133214"/>
    <dcterms:publisher rdf:resource="http://www.historicengland.org.uk"/>
    <skos:prefLabel xml:lang="en">Fw200</skos:prefLabel>
    <skos:scopeNote xml:lang="en">Long-range, four-engine reconnaissance-bomber. Initially produced as a transport, converted and used against Allied convoys in the Channel and the Atlantic. Also served as a VIP transport, one of which was the Immelmann III: Hitler's personal aircraft.</skos:scopeNote>
    <skos:broader rdf:resource="http://purl.org/heritagedata/schemes/225/concepts/135730"/>
    <dcterms:identifier>http://purl.org/heritagedata/schemes/225/concepts/137236</dcterms:identifier>
  </rdf:Description>
  <rdf:Description rdf:about="http://purl.org/heritagedata/schemes/225/concepts/125516">
    <rdf:type rdf:resource="http://www.w3.org/2004/02/skos/core#Concept"/>
    <cc:license rdf:resource="http://creativecommons.org/licenses/by/3.0"/>
    <cc:attributionName xml:lang="en">Historic England</cc:attributionName>
    <cc:attributionURL rdf:resource="http://www.historicengland.org.uk"/>
    <skos:inScheme rdf:resource="http://purl.org/heritagedata/schemes/225"/>
    <skos:narrower rdf:resource="http://purl.org/heritagedata/schemes/225/concepts/125517"/>
    <dcterms:identifier>http://purl.org/heritagedata/schemes/225/concepts/125516</dcterms:identifier>
    <skos:broader rdf:resource="http://purl.org/heritagedata/schemes/225/concepts/111358"/>
    <dcterms:issued rdf:datatype="http://www.w3.org/2001/XMLSchema#dateTime">2019-03-26T16:45:43</dcterms:issued>
    <skos:scopeNote xml:lang="en">The Lockheed Aircraft Corporation. Founded in 1916 by Allen and Malcolm Loughead. In 1926 the company moved to Burbank and changed its name to The Lockheed Aircraft Company, and was then incorporated in 1932.</skos:scopeNote>
    <skos:narrower rdf:resource="http://purl.org/heritagedata/schemes/225/concepts/133203"/>
    <dcterms:publisher rdf:resource="http://www.historicengland.org.uk"/>
    <skos:narrower rdf:resource="http://purl.org/heritagedata/schemes/225/concepts/135769"/>
    <skos:prefLabel xml:lang="en">Lockheed</skos:prefLabel>
  </rdf:Description>
  <rdf:Description rdf:about="http://purl.org/heritagedata/schemes/225/concepts/111403">
    <cc:attributionName xml:lang="en">Historic England</cc:attributionName>
    <skos:narrower rdf:resource="http://purl.org/heritagedata/schemes/225/concepts/138536"/>
    <dcterms:issued rdf:datatype="http://www.w3.org/2001/XMLSchema#dateTime">2019-03-26T16:45:43</dcterms:issued>
    <skos:broader rdf:resource="http://purl.org/heritagedata/schemes/225/concepts/111393"/>
    <skos:narrower rdf:resource="http://purl.org/heritagedata/schemes/225/concepts/167011"/>
    <dcterms:publisher rdf:resource="http://www.historicengland.org.uk"/>
    <skos:narrower rdf:resource="http://purl.org/heritagedata/schemes/225/concepts/167009"/>
    <skos:narrower rdf:resource="http://purl.org/heritagedata/schemes/225/concepts/140425"/>
    <skos:narrower rdf:resource="http://purl.org/heritagedata/schemes/225/concepts/133195"/>
    <skos:narrower rdf:resource="http://purl.org/heritagedata/schemes/225/concepts/167015"/>
    <skos:narrower rdf:resource="http://purl.org/heritagedata/schemes/225/concepts/140140"/>
    <cc:attributionURL rdf:resource="http://www.historicengland.org.uk"/>
    <skos:inScheme rdf:resource="http://purl.org/heritagedata/schemes/225"/>
    <skos:narrower rdf:resource="http://purl.org/heritagedata/schemes/225/concepts/136525"/>
    <skos:narrower rdf:resource="http://purl.org/heritagedata/schemes/225/concepts/138542"/>
    <skos:narrower rdf:resource="http://purl.org/heritagedata/schemes/225/concepts/167000"/>
    <skos:narrower rdf:resource="http://purl.org/heritagedata/schemes/225/concepts/136233"/>
    <skos:narrower rdf:resource="http://purl.org/heritagedata/schemes/225/concepts/169972"/>
    <skos:narrower rdf:resource="http://purl.org/heritagedata/schemes/225/concepts/136521"/>
    <skos:narrower rdf:resource="http://purl.org/heritagedata/schemes/225/concepts/136510"/>
    <skos:narrower rdf:resource="http://purl.org/heritagedata/schemes/225/concepts/111442"/>
    <skos:narrower rdf:resource="http://purl.org/heritagedata/schemes/225/concepts/138535"/>
    <skos:narrower rdf:resource="http://purl.org/heritagedata/schemes/225/concepts/138546"/>
    <skos:narrower rdf:resource="http://purl.org/heritagedata/schemes/225/concepts/138533"/>
    <skos:narrower rdf:resource="http://purl.org/heritagedata/schemes/225/concepts/140065"/>
    <skos:narrower rdf:resource="http://purl.org/heritagedata/schemes/225/concepts/139374"/>
    <skos:narrower rdf:resource="http://purl.org/heritagedata/schemes/225/concepts/141207"/>
    <skos:narrower rdf:resource="http://purl.org/heritagedata/schemes/225/concepts/138537"/>
    <skos:narrower rdf:resource="http://purl.org/heritagedata/schemes/225/concepts/138540"/>
    <skos:narrower rdf:resource="http://purl.org/heritagedata/schemes/225/concepts/136250"/>
    <skos:narrower rdf:resource="http://purl.org/heritagedata/schemes/225/concepts/140416"/>
    <skos:narrower rdf:resource="http://purl.org/heritagedata/schemes/225/concepts/135586"/>
    <skos:narrower rdf:resource="http://purl.org/heritagedata/schemes/225/concepts/137208"/>
    <skos:narrower rdf:resource="http://purl.org/heritagedata/schemes/225/concepts/136610"/>
    <skos:narrower rdf:resource="http://purl.org/heritagedata/schemes/225/concepts/135850"/>
    <cc:license rdf:resource="http://creativecommons.org/licenses/by/3.0"/>
    <skos:narrower rdf:resource="http://purl.org/heritagedata/schemes/225/concepts/138541"/>
    <skos:narrower rdf:resource="http://purl.org/heritagedata/schemes/225/concepts/136231"/>
    <skos:narrower rdf:resource="http://purl.org/heritagedata/schemes/225/concepts/140424"/>
    <skos:narrower rdf:resource="http://purl.org/heritagedata/schemes/225/concepts/167008"/>
    <skos:narrower rdf:resource="http://purl.org/heritagedata/schemes/225/concepts/136593"/>
    <dcterms:identifier>http://purl.org/heritagedata/schemes/225/concepts/111403</dcterms:identifier>
    <skos:narrower rdf:resource="http://purl.org/heritagedata/schemes/225/concepts/138532"/>
    <rdf:type rdf:resource="http://www.w3.org/2004/02/skos/core#Concept"/>
    <skos:narrower rdf:resource="http://purl.org/heritagedata/schemes/225/concepts/138538"/>
    <skos:narrower rdf:resource="http://purl.org/heritagedata/schemes/225/concepts/137197"/>
    <skos:prefLabel xml:lang="en">Biplane</skos:prefLabel>
    <skos:narrower rdf:resource="http://purl.org/heritagedata/schemes/225/concepts/136522"/>
    <skos:narrower rdf:resource="http://purl.org/heritagedata/schemes/225/concepts/138539"/>
    <skos:narrower rdf:resource="http://purl.org/heritagedata/schemes/225/concepts/136526"/>
    <skos:narrower rdf:resource="http://purl.org/heritagedata/schemes/225/concepts/136524"/>
    <skos:narrower rdf:resource="http://purl.org/heritagedata/schemes/225/concepts/136251"/>
    <skos:scopeNote xml:lang="en">An aeroplane with two wings, or planes, placed one above the other either side of the fuselage.</skos:scopeNote>
    <skos:narrower rdf:resource="http://purl.org/heritagedata/schemes/225/concepts/140095"/>
    <skos:narrower rdf:resource="http://purl.org/heritagedata/schemes/225/concepts/138534"/>
    <skos:narrower rdf:resource="http://purl.org/heritagedata/schemes/225/concepts/167014"/>
    <skos:narrower rdf:resource="http://purl.org/heritagedata/schemes/225/concepts/136234"/>
  </rdf:Description>
  <rdf:Description rdf:about="http://purl.org/heritagedata/schemes/225/concepts/111400">
    <cc:attributionURL rdf:resource="http://www.historicengland.org.uk"/>
    <skos:broader rdf:resource="http://purl.org/heritagedata/schemes/225/concepts/135730"/>
    <dcterms:publisher rdf:resource="http://www.historicengland.org.uk"/>
    <skos:narrower rdf:resource="http://purl.org/heritagedata/schemes/225/concepts/141268"/>
    <skos:narrower rdf:resource="http://purl.org/heritagedata/schemes/225/concepts/137192"/>
    <skos:scopeNote xml:lang="en">A camera-equipped aircraft intended to fly over enemy territory and gather photographic evidence of strategic features and/or the position and strength of any military presence.</skos:scopeNote>
    <dcterms:issued rdf:datatype="http://www.w3.org/2001/XMLSchema#dateTime">2019-03-26T16:45:43</dcterms:issued>
    <skos:inScheme rdf:resource="http://purl.org/heritagedata/schemes/225"/>
    <skos:prefLabel xml:lang="en">Photo Reconnaissance</skos:prefLabel>
    <rdf:type rdf:resource="http://www.w3.org/2004/02/skos/core#Concept"/>
    <dcterms:identifier>http://purl.org/heritagedata/schemes/225/concepts/111400</dcterms:identifier>
    <cc:attributionName xml:lang="en">Historic England</cc:attributionName>
    <cc:license rdf:resource="http://creativecommons.org/licenses/by/3.0"/>
  </rdf:Description>
  <rdf:Description rdf:about="http://purl.org/heritagedata/schemes/225/concepts/136234">
    <dcterms:issued rdf:datatype="http://www.w3.org/2001/XMLSchema#dateTime">2019-03-26T16:45:43</dcterms:issued>
    <dcterms:publisher rdf:resource="http://www.historicengland.org.uk"/>
    <cc:attributionName xml:lang="en">Historic England</cc:attributionName>
    <skos:scopeNote xml:lang="en">Twin-engined, four-crew bomber. Wooden framed, with linen covering, entered service in 1924, equipping several RAF squadrons.</skos:scopeNote>
    <dcterms:identifier>http://purl.org/heritagedata/schemes/225/concepts/136234</dcterms:identifier>
    <cc:license rdf:resource="http://creativecommons.org/licenses/by/3.0"/>
    <skos:prefLabel xml:lang="en">Virginia</skos:prefLabel>
    <cc:attributionURL rdf:resource="http://www.historicengland.org.uk"/>
    <skos:inScheme rdf:resource="http://purl.org/heritagedata/schemes/225"/>
    <skos:broader rdf:resource="http://purl.org/heritagedata/schemes/225/concepts/111398"/>
    <skos:broader rdf:resource="http://purl.org/heritagedata/schemes/225/concepts/111403"/>
    <skos:broader rdf:resource="http://purl.org/heritagedata/schemes/225/concepts/111420"/>
    <rdf:type rdf:resource="http://www.w3.org/2004/02/skos/core#Concept"/>
  </rdf:Description>
  <rdf:Description rdf:about="http://purl.org/heritagedata/schemes/225/concepts/140074">
    <rdf:type rdf:resource="http://www.w3.org/2004/02/skos/core#Concept"/>
    <dcterms:identifier>http://purl.org/heritagedata/schemes/225/concepts/140074</dcterms:identifier>
    <skos:broader rdf:resource="http://purl.org/heritagedata/schemes/225/concepts/111394"/>
    <dcterms:publisher rdf:resource="http://www.historicengland.org.uk"/>
    <skos:scopeNote xml:lang="en">An aircraft equipped to deploy explosive mines.</skos:scopeNote>
    <cc:license rdf:resource="http://creativecommons.org/licenses/by/3.0"/>
    <cc:attributionName xml:lang="en">Historic England</cc:attributionName>
    <skos:narrower rdf:resource="http://purl.org/heritagedata/schemes/225/concepts/134996"/>
    <skos:inScheme rdf:resource="http://purl.org/heritagedata/schemes/225"/>
    <skos:prefLabel xml:lang="en">Minelayer</skos:prefLabel>
    <dcterms:issued rdf:datatype="http://www.w3.org/2001/XMLSchema#dateTime">2019-03-26T16:45:43</dcterms:issued>
    <cc:attributionURL rdf:resource="http://www.historicengland.org.uk"/>
  </rdf:Description>
  <rdf:Description rdf:about="http://purl.org/heritagedata/schemes/225/concepts/135586">
    <skos:scopeNote xml:lang="en">Single-engine, two-seat, light, biplane, elementary-flying trainer. Adapted from a civilian design, and constructed from tubular steel and spruce with plywood and fabric covering, entered service in 1931 and was available in land-plane or seaplane forms.</skos:scopeNote>
    <cc:license rdf:resource="http://creativecommons.org/licenses/by/3.0"/>
    <cc:attributionName xml:lang="en">Historic England</cc:attributionName>
    <cc:attributionURL rdf:resource="http://www.historicengland.org.uk"/>
    <skos:inScheme rdf:resource="http://purl.org/heritagedata/schemes/225"/>
    <skos:broader rdf:resource="http://purl.org/heritagedata/schemes/225/concepts/111401"/>
    <dcterms:issued rdf:datatype="http://www.w3.org/2001/XMLSchema#dateTime">2019-03-26T16:45:43</dcterms:issued>
    <skos:broader rdf:resource="http://purl.org/heritagedata/schemes/225/concepts/111368"/>
    <ns1:related rdf:resource="http://purl.org/heritagedata/schemes/225/concepts/135850"/>
    <skos:prefLabel xml:lang="en">Tiger Moth</skos:prefLabel>
    <skos:broader rdf:resource="http://purl.org/heritagedata/schemes/225/concepts/111403"/>
    <dcterms:identifier>http://purl.org/heritagedata/schemes/225/concepts/135586</dcterms:identifier>
    <dcterms:publisher rdf:resource="http://www.historicengland.org.uk"/>
    <rdf:type rdf:resource="http://www.w3.org/2004/02/skos/core#Concept"/>
  </rdf:Description>
  <rdf:Description rdf:about="http://purl.org/heritagedata/schemes/225/concepts/111414">
    <cc:license rdf:resource="http://creativecommons.org/licenses/by/3.0"/>
    <cc:attributionName xml:lang="en">Historic England</cc:attributionName>
    <cc:attributionURL rdf:resource="http://www.historicengland.org.uk"/>
    <skos:inScheme rdf:resource="http://purl.org/heritagedata/schemes/225"/>
    <dcterms:identifier>http://purl.org/heritagedata/schemes/225/concepts/111414</dcterms:identifier>
    <skos:scopeNote xml:lang="en">The RAF's first jet fighter, flown operationally during 1944-5, with later versions serving for a further ten years after the war. The Meteor's first active operations were in the interception and destruction of V.1. flying bombs.</skos:scopeNote>
    <rdf:type rdf:resource="http://www.w3.org/2004/02/skos/core#Concept"/>
    <dcterms:issued rdf:datatype="http://www.w3.org/2001/XMLSchema#dateTime">2019-03-26T16:45:43</dcterms:issued>
    <skos:broader rdf:resource="http://purl.org/heritagedata/schemes/225/concepts/111402"/>
    <skos:broader rdf:resource="http://purl.org/heritagedata/schemes/225/concepts/111413"/>
    <skos:broader rdf:resource="http://purl.org/heritagedata/schemes/225/concepts/111397"/>
    <dcterms:publisher rdf:resource="http://www.historicengland.org.uk"/>
    <skos:prefLabel xml:lang="en">Meteor</skos:prefLabel>
  </rdf:Description>
  <rdf:Description rdf:about="http://purl.org/heritagedata/schemes/225/concepts/141399">
    <skos:inScheme rdf:resource="http://purl.org/heritagedata/schemes/225"/>
    <dcterms:issued rdf:datatype="http://www.w3.org/2001/XMLSchema#dateTime">2019-03-26T16:45:43</dcterms:issued>
    <dcterms:identifier>http://purl.org/heritagedata/schemes/225/concepts/141399</dcterms:identifier>
    <skos:broader rdf:resource="http://purl.org/heritagedata/schemes/225/concepts/111368"/>
    <skos:broader rdf:resource="http://purl.org/heritagedata/schemes/225/concepts/111402"/>
    <cc:license rdf:resource="http://creativecommons.org/licenses/by/3.0"/>
    <cc:attributionURL rdf:resource="http://www.historicengland.org.uk"/>
    <rdf:type rdf:resource="http://www.w3.org/2004/02/skos/core#Concept"/>
    <dcterms:publisher rdf:resource="http://www.historicengland.org.uk"/>
    <skos:scopeNote xml:lang="en">Three-seat, single engine, high wing braced monoplane designed for civil use and first flown in 1929. Saw military service in World War 2 in an Army co-operation and communications role.</skos:scopeNote>
    <skos:broader rdf:resource="http://purl.org/heritagedata/schemes/225/concepts/136031"/>
    <skos:broader rdf:resource="http://purl.org/heritagedata/schemes/225/concepts/141359"/>
    <skos:prefLabel xml:lang="en">Puss Moth</skos:prefLabel>
    <cc:attributionName xml:lang="en">Historic England</cc:attributionName>
  </rdf:Description>
  <rdf:Description rdf:about="http://purl.org/heritagedata/schemes/225/concepts/141208">
    <rdf:type rdf:resource="http://www.w3.org/2004/02/skos/core#Concept"/>
    <cc:license rdf:resource="http://creativecommons.org/licenses/by/3.0"/>
    <cc:attributionName xml:lang="en">Historic England</cc:attributionName>
    <cc:attributionURL rdf:resource="http://www.historicengland.org.uk"/>
    <skos:inScheme rdf:resource="http://purl.org/heritagedata/schemes/225"/>
    <skos:prefLabel xml:lang="en">MkV</skos:prefLabel>
    <dcterms:issued rdf:datatype="http://www.w3.org/2001/XMLSchema#dateTime">2019-03-26T16:45:43</dcterms:issued>
    <dcterms:identifier>http://purl.org/heritagedata/schemes/225/concepts/141208</dcterms:identifier>
    <dcterms:publisher rdf:resource="http://www.historicengland.org.uk"/>
    <skos:scopeNote xml:lang="en">Mark 5 or the fifth variant of an aircraft with its associated modifications.</skos:scopeNote>
    <skos:broader rdf:resource="http://purl.org/heritagedata/schemes/225/concepts/141131"/>
  </rdf:Description>
  <rdf:Description rdf:about="http://purl.org/heritagedata/schemes/225/concepts/111368">
    <dcterms:publisher rdf:resource="http://www.historicengland.org.uk"/>
    <skos:scopeNote xml:lang="en">The de Havilland Aircraft Co., Ltd., founded in 1920 by Sir Geoffrey de Havilland, C.B.E., A.F.C., F.R.Ae.S. Originally developers of commercial aircraft, were responsible for such notable wartime aircraft as the Mosquito and the Tiger Moth.</skos:scopeNote>
    <skos:narrower rdf:resource="http://purl.org/heritagedata/schemes/225/concepts/135850"/>
    <cc:license rdf:resource="http://creativecommons.org/licenses/by/3.0"/>
    <dcterms:identifier>http://purl.org/heritagedata/schemes/225/concepts/111368</dcterms:identifier>
    <skos:narrower rdf:resource="http://purl.org/heritagedata/schemes/225/concepts/169972"/>
    <skos:narrower rdf:resource="http://purl.org/heritagedata/schemes/225/concepts/141353"/>
    <skos:narrower rdf:resource="http://purl.org/heritagedata/schemes/225/concepts/138542"/>
    <dcterms:issued rdf:datatype="http://www.w3.org/2001/XMLSchema#dateTime">2019-03-26T16:45:43</dcterms:issued>
    <skos:narrower rdf:resource="http://purl.org/heritagedata/schemes/225/concepts/135586"/>
    <cc:attributionName xml:lang="en">Historic England</cc:attributionName>
    <skos:inScheme rdf:resource="http://purl.org/heritagedata/schemes/225"/>
    <skos:narrower rdf:resource="http://purl.org/heritagedata/schemes/225/concepts/136030"/>
    <skos:narrower rdf:resource="http://purl.org/heritagedata/schemes/225/concepts/151472"/>
    <rdf:type rdf:resource="http://www.w3.org/2004/02/skos/core#Concept"/>
    <cc:attributionURL rdf:resource="http://www.historicengland.org.uk"/>
    <skos:narrower rdf:resource="http://purl.org/heritagedata/schemes/225/concepts/141399"/>
    <skos:narrower rdf:resource="http://purl.org/heritagedata/schemes/225/concepts/135606"/>
    <skos:broader rdf:resource="http://purl.org/heritagedata/schemes/225/concepts/111358"/>
    <skos:narrower rdf:resource="http://purl.org/heritagedata/schemes/225/concepts/111369"/>
    <skos:prefLabel xml:lang="en">De Havilland</skos:prefLabel>
  </rdf:Description>
  <rdf:Description rdf:about="http://purl.org/heritagedata/schemes/225/concepts/134998">
    <dcterms:publisher rdf:resource="http://www.historicengland.org.uk"/>
    <skos:prefLabel xml:lang="en">Typhoon</skos:prefLabel>
    <rdf:type rdf:resource="http://www.w3.org/2004/02/skos/core#Concept"/>
    <cc:license rdf:resource="http://creativecommons.org/licenses/by/3.0"/>
    <ns1:related rdf:resource="http://purl.org/heritagedata/schemes/225/concepts/137204"/>
    <skos:broader rdf:resource="http://purl.org/heritagedata/schemes/225/concepts/111359"/>
    <cc:attributionURL rdf:resource="http://www.historicengland.org.uk"/>
    <dcterms:issued rdf:datatype="http://www.w3.org/2001/XMLSchema#dateTime">2019-03-26T16:45:43</dcterms:issued>
    <skos:broader rdf:resource="http://purl.org/heritagedata/schemes/225/concepts/111399"/>
    <dcterms:identifier>http://purl.org/heritagedata/schemes/225/concepts/134998</dcterms:identifier>
    <skos:inScheme rdf:resource="http://purl.org/heritagedata/schemes/225"/>
    <cc:attributionName xml:lang="en">Historic England</cc:attributionName>
    <skos:broader rdf:resource="http://purl.org/heritagedata/schemes/225/concepts/111402"/>
    <skos:scopeNote xml:lang="en">Single-engine, single-seat fighter-bomber. Designed to replace the Hurricane as an interceptor, excelled as a rocket-projectile-firing ground-attack fighter. Entered RAF service in 1941.</skos:scopeNote>
  </rdf:Description>
  <rdf:Description rdf:about="http://purl.org/heritagedata/schemes/225/concepts/135769">
    <skos:inScheme rdf:resource="http://purl.org/heritagedata/schemes/225"/>
    <skos:narrower rdf:resource="http://purl.org/heritagedata/schemes/225/concepts/134999"/>
    <dcterms:identifier>http://purl.org/heritagedata/schemes/225/concepts/135769</dcterms:identifier>
    <skos:broader rdf:resource="http://purl.org/heritagedata/schemes/225/concepts/125516"/>
    <cc:license rdf:resource="http://creativecommons.org/licenses/by/3.0"/>
    <cc:attributionURL rdf:resource="http://www.historicengland.org.uk"/>
    <cc:attributionName xml:lang="en">Historic England</cc:attributionName>
    <skos:prefLabel xml:lang="en">Lockheed Vega</skos:prefLabel>
    <rdf:type rdf:resource="http://www.w3.org/2004/02/skos/core#Concept"/>
    <dcterms:issued rdf:datatype="http://www.w3.org/2001/XMLSchema#dateTime">2019-03-26T16:45:43</dcterms:issued>
    <dcterms:publisher rdf:resource="http://www.historicengland.org.uk"/>
    <skos:scopeNote xml:lang="en">A subsidiary of Lockheed.</skos:scopeNote>
  </rdf:Description>
  <rdf:Description rdf:about="http://purl.org/heritagedata/schemes/225/concepts/111402">
    <skos:narrower rdf:resource="http://purl.org/heritagedata/schemes/225/concepts/133193"/>
    <skos:narrower rdf:resource="http://purl.org/heritagedata/schemes/225/concepts/151472"/>
    <skos:narrower rdf:resource="http://purl.org/heritagedata/schemes/225/concepts/152401"/>
    <skos:narrower rdf:resource="http://purl.org/heritagedata/schemes/225/concepts/137219"/>
    <skos:narrower rdf:resource="http://purl.org/heritagedata/schemes/225/concepts/133194"/>
    <skos:narrower rdf:resource="http://purl.org/heritagedata/schemes/225/concepts/137199"/>
    <skos:narrower rdf:resource="http://purl.org/heritagedata/schemes/225/concepts/137215"/>
    <skos:narrower rdf:resource="http://purl.org/heritagedata/schemes/225/concepts/134952"/>
    <skos:narrower rdf:resource="http://purl.org/heritagedata/schemes/225/concepts/125573"/>
    <skos:narrower rdf:resource="http://purl.org/heritagedata/schemes/225/concepts/111333"/>
    <skos:narrower rdf:resource="http://purl.org/heritagedata/schemes/225/concepts/111373"/>
    <skos:narrower rdf:resource="http://purl.org/heritagedata/schemes/225/concepts/140447"/>
    <skos:narrower rdf:resource="http://purl.org/heritagedata/schemes/225/concepts/137198"/>
    <skos:narrower rdf:resource="http://purl.org/heritagedata/schemes/225/concepts/136591"/>
    <skos:scopeNote xml:lang="en">An aircraft with a single wing, or plane, either side of its fuselage.</skos:scopeNote>
    <skos:narrower rdf:resource="http://purl.org/heritagedata/schemes/225/concepts/137203"/>
    <skos:narrower rdf:resource="http://purl.org/heritagedata/schemes/225/concepts/111427"/>
    <skos:narrower rdf:resource="http://purl.org/heritagedata/schemes/225/concepts/137238"/>
    <skos:narrower rdf:resource="http://purl.org/heritagedata/schemes/225/concepts/137236"/>
    <skos:narrower rdf:resource="http://purl.org/heritagedata/schemes/225/concepts/111416"/>
    <skos:narrower rdf:resource="http://purl.org/heritagedata/schemes/225/concepts/137220"/>
    <skos:narrower rdf:resource="http://purl.org/heritagedata/schemes/225/concepts/111414"/>
    <dcterms:issued rdf:datatype="http://www.w3.org/2001/XMLSchema#dateTime">2019-03-26T16:45:43</dcterms:issued>
    <skos:narrower rdf:resource="http://purl.org/heritagedata/schemes/225/concepts/136532"/>
    <skos:narrower rdf:resource="http://purl.org/heritagedata/schemes/225/concepts/137202"/>
    <skos:narrower rdf:resource="http://purl.org/heritagedata/schemes/225/concepts/111363"/>
    <skos:narrower rdf:resource="http://purl.org/heritagedata/schemes/225/concepts/111419"/>
    <skos:narrower rdf:resource="http://purl.org/heritagedata/schemes/225/concepts/137192"/>
    <skos:narrower rdf:resource="http://purl.org/heritagedata/schemes/225/concepts/136592"/>
    <skos:narrower rdf:resource="http://purl.org/heritagedata/schemes/225/concepts/141211"/>
    <skos:narrower rdf:resource="http://purl.org/heritagedata/schemes/225/concepts/137130"/>
    <skos:narrower rdf:resource="http://purl.org/heritagedata/schemes/225/concepts/111422"/>
    <skos:narrower rdf:resource="http://purl.org/heritagedata/schemes/225/concepts/137209"/>
    <skos:narrower rdf:resource="http://purl.org/heritagedata/schemes/225/concepts/134998"/>
    <skos:inScheme rdf:resource="http://purl.org/heritagedata/schemes/225"/>
    <skos:narrower rdf:resource="http://purl.org/heritagedata/schemes/225/concepts/135729"/>
    <skos:narrower rdf:resource="http://purl.org/heritagedata/schemes/225/concepts/141268"/>
    <skos:narrower rdf:resource="http://purl.org/heritagedata/schemes/225/concepts/137235"/>
    <skos:narrower rdf:resource="http://purl.org/heritagedata/schemes/225/concepts/135606"/>
    <skos:narrower rdf:resource="http://purl.org/heritagedata/schemes/225/concepts/125518"/>
    <skos:narrower rdf:resource="http://purl.org/heritagedata/schemes/225/concepts/137228"/>
    <skos:narrower rdf:resource="http://purl.org/heritagedata/schemes/225/concepts/111370"/>
    <skos:narrower rdf:resource="http://purl.org/heritagedata/schemes/225/concepts/135932"/>
    <skos:narrower rdf:resource="http://purl.org/heritagedata/schemes/225/concepts/137237"/>
    <skos:narrower rdf:resource="http://purl.org/heritagedata/schemes/225/concepts/137212"/>
    <skos:narrower rdf:resource="http://purl.org/heritagedata/schemes/225/concepts/134999"/>
    <skos:narrower rdf:resource="http://purl.org/heritagedata/schemes/225/concepts/111435"/>
    <dcterms:identifier>http://purl.org/heritagedata/schemes/225/concepts/111402</dcterms:identifier>
    <skos:broader rdf:resource="http://purl.org/heritagedata/schemes/225/concepts/111393"/>
    <skos:narrower rdf:resource="http://purl.org/heritagedata/schemes/225/concepts/167002"/>
    <skos:narrower rdf:resource="http://purl.org/heritagedata/schemes/225/concepts/137221"/>
    <skos:narrower rdf:resource="http://purl.org/heritagedata/schemes/225/concepts/137214"/>
    <skos:narrower rdf:resource="http://purl.org/heritagedata/schemes/225/concepts/137174"/>
    <skos:narrower rdf:resource="http://purl.org/heritagedata/schemes/225/concepts/137111"/>
    <skos:narrower rdf:resource="http://purl.org/heritagedata/schemes/225/concepts/137232"/>
    <skos:narrower rdf:resource="http://purl.org/heritagedata/schemes/225/concepts/125514"/>
    <skos:narrower rdf:resource="http://purl.org/heritagedata/schemes/225/concepts/111377"/>
    <skos:narrower rdf:resource="http://purl.org/heritagedata/schemes/225/concepts/133202"/>
    <cc:license rdf:resource="http://creativecommons.org/licenses/by/3.0"/>
    <rdf:type rdf:resource="http://www.w3.org/2004/02/skos/core#Concept"/>
    <skos:narrower rdf:resource="http://purl.org/heritagedata/schemes/225/concepts/141353"/>
    <skos:narrower rdf:resource="http://purl.org/heritagedata/schemes/225/concepts/135931"/>
    <skos:narrower rdf:resource="http://purl.org/heritagedata/schemes/225/concepts/133206"/>
    <skos:narrower rdf:resource="http://purl.org/heritagedata/schemes/225/concepts/136531"/>
    <skos:narrower rdf:resource="http://purl.org/heritagedata/schemes/225/concepts/137204"/>
    <skos:narrower rdf:resource="http://purl.org/heritagedata/schemes/225/concepts/133203"/>
    <skos:narrower rdf:resource="http://purl.org/heritagedata/schemes/225/concepts/137224"/>
    <skos:narrower rdf:resource="http://purl.org/heritagedata/schemes/225/concepts/125533"/>
    <skos:narrower rdf:resource="http://purl.org/heritagedata/schemes/225/concepts/137234"/>
    <skos:narrower rdf:resource="http://purl.org/heritagedata/schemes/225/concepts/111364"/>
    <skos:narrower rdf:resource="http://purl.org/heritagedata/schemes/225/concepts/111443"/>
    <skos:narrower rdf:resource="http://purl.org/heritagedata/schemes/225/concepts/135750"/>
    <skos:narrower rdf:resource="http://purl.org/heritagedata/schemes/225/concepts/137239"/>
    <skos:narrower rdf:resource="http://purl.org/heritagedata/schemes/225/concepts/137153"/>
    <skos:narrower rdf:resource="http://purl.org/heritagedata/schemes/225/concepts/141296"/>
    <skos:narrower rdf:resource="http://purl.org/heritagedata/schemes/225/concepts/133209"/>
    <skos:narrower rdf:resource="http://purl.org/heritagedata/schemes/225/concepts/141213"/>
    <skos:narrower rdf:resource="http://purl.org/heritagedata/schemes/225/concepts/125593"/>
    <skos:narrower rdf:resource="http://purl.org/heritagedata/schemes/225/concepts/133201"/>
    <skos:narrower rdf:resource="http://purl.org/heritagedata/schemes/225/concepts/125517"/>
    <skos:narrower rdf:resource="http://purl.org/heritagedata/schemes/225/concepts/111360"/>
    <skos:narrower rdf:resource="http://purl.org/heritagedata/schemes/225/concepts/133204"/>
    <cc:attributionURL rdf:resource="http://www.historicengland.org.uk"/>
    <dcterms:publisher rdf:resource="http://www.historicengland.org.uk"/>
    <skos:prefLabel xml:lang="en">Monoplane</skos:prefLabel>
    <skos:narrower rdf:resource="http://purl.org/heritagedata/schemes/225/concepts/111366"/>
    <skos:narrower rdf:resource="http://purl.org/heritagedata/schemes/225/concepts/137206"/>
    <skos:narrower rdf:resource="http://purl.org/heritagedata/schemes/225/concepts/137151"/>
    <skos:narrower rdf:resource="http://purl.org/heritagedata/schemes/225/concepts/136530"/>
    <skos:narrower rdf:resource="http://purl.org/heritagedata/schemes/225/concepts/111429"/>
    <skos:narrower rdf:resource="http://purl.org/heritagedata/schemes/225/concepts/111428"/>
    <skos:narrower rdf:resource="http://purl.org/heritagedata/schemes/225/concepts/137150"/>
    <skos:narrower rdf:resource="http://purl.org/heritagedata/schemes/225/concepts/125554"/>
    <skos:narrower rdf:resource="http://purl.org/heritagedata/schemes/225/concepts/133173"/>
    <skos:narrower rdf:resource="http://purl.org/heritagedata/schemes/225/concepts/111367"/>
    <skos:narrower rdf:resource="http://purl.org/heritagedata/schemes/225/concepts/138485"/>
    <skos:narrower rdf:resource="http://purl.org/heritagedata/schemes/225/concepts/141399"/>
    <skos:narrower rdf:resource="http://purl.org/heritagedata/schemes/225/concepts/137229"/>
    <skos:narrower rdf:resource="http://purl.org/heritagedata/schemes/225/concepts/138543"/>
    <skos:narrower rdf:resource="http://purl.org/heritagedata/schemes/225/concepts/136030"/>
    <skos:narrower rdf:resource="http://purl.org/heritagedata/schemes/225/concepts/167858"/>
    <skos:narrower rdf:resource="http://purl.org/heritagedata/schemes/225/concepts/137193"/>
    <skos:narrower rdf:resource="http://purl.org/heritagedata/schemes/225/concepts/125553"/>
    <skos:narrower rdf:resource="http://purl.org/heritagedata/schemes/225/concepts/134996"/>
    <cc:attributionName xml:lang="en">Historic England</cc:attributionName>
    <skos:narrower rdf:resource="http://purl.org/heritagedata/schemes/225/concepts/111375"/>
    <skos:narrower rdf:resource="http://purl.org/heritagedata/schemes/225/concepts/111426"/>
    <skos:narrower rdf:resource="http://purl.org/heritagedata/schemes/225/concepts/167004"/>
    <skos:narrower rdf:resource="http://purl.org/heritagedata/schemes/225/concepts/136220"/>
    <skos:narrower rdf:resource="http://purl.org/heritagedata/schemes/225/concepts/137216"/>
    <skos:narrower rdf:resource="http://purl.org/heritagedata/schemes/225/concepts/167001"/>
    <skos:narrower rdf:resource="http://purl.org/heritagedata/schemes/225/concepts/111334"/>
    <skos:narrower rdf:resource="http://purl.org/heritagedata/schemes/225/concepts/111369"/>
    <skos:narrower rdf:resource="http://purl.org/heritagedata/schemes/225/concepts/137201"/>
    <skos:narrower rdf:resource="http://purl.org/heritagedata/schemes/225/concepts/137195"/>
    <skos:narrower rdf:resource="http://purl.org/heritagedata/schemes/225/concepts/133199"/>
    <skos:narrower rdf:resource="http://purl.org/heritagedata/schemes/225/concepts/125493"/>
    <skos:narrower rdf:resource="http://purl.org/heritagedata/schemes/225/concepts/137226"/>
    <skos:narrower rdf:resource="http://purl.org/heritagedata/schemes/225/concepts/137196"/>
    <skos:narrower rdf:resource="http://purl.org/heritagedata/schemes/225/concepts/167003"/>
  </rdf:Description>
  <rdf:Description rdf:about="http://purl.org/heritagedata/schemes/225/concepts/137153">
    <skos:scopeNote xml:lang="en">Single-engine, advanced-pilot trainer. Spruce and plywood in construction, entered service in 1939, continuing to serve as a trainer, and also a target tug, until 1950.</skos:scopeNote>
    <skos:inScheme rdf:resource="http://purl.org/heritagedata/schemes/225"/>
    <rdf:type rdf:resource="http://www.w3.org/2004/02/skos/core#Concept"/>
    <dcterms:identifier>http://purl.org/heritagedata/schemes/225/concepts/137153</dcterms:identifier>
    <skos:broader rdf:resource="http://purl.org/heritagedata/schemes/225/concepts/133205"/>
    <skos:broader rdf:resource="http://purl.org/heritagedata/schemes/225/concepts/111402"/>
    <skos:prefLabel xml:lang="en">Martinet</skos:prefLabel>
    <cc:license rdf:resource="http://creativecommons.org/licenses/by/3.0"/>
    <cc:attributionURL rdf:resource="http://www.historicengland.org.uk"/>
    <dcterms:issued rdf:datatype="http://www.w3.org/2001/XMLSchema#dateTime">2019-03-26T16:45:43</dcterms:issued>
    <cc:attributionName xml:lang="en">Historic England</cc:attributionName>
    <dcterms:publisher rdf:resource="http://www.historicengland.org.uk"/>
    <skos:broader rdf:resource="http://purl.org/heritagedata/schemes/225/concepts/111401"/>
  </rdf:Description>
  <rdf:Description rdf:about="http://purl.org/heritagedata/schemes/225/concepts/141297">
    <cc:license rdf:resource="http://creativecommons.org/licenses/by/3.0"/>
    <cc:attributionName xml:lang="en">Historic England</cc:attributionName>
    <cc:attributionURL rdf:resource="http://www.historicengland.org.uk"/>
    <skos:inScheme rdf:resource="http://purl.org/heritagedata/schemes/225"/>
    <skos:scopeNote xml:lang="en">A Mark 2 aircraft which has undergone slight modifications to enhance performance or armament.</skos:scopeNote>
    <dcterms:issued rdf:datatype="http://www.w3.org/2001/XMLSchema#dateTime">2019-03-26T16:45:43</dcterms:issued>
    <skos:prefLabel xml:lang="en">MkIIA</skos:prefLabel>
    <rdf:type rdf:resource="http://www.w3.org/2004/02/skos/core#Concept"/>
    <dcterms:publisher rdf:resource="http://www.historicengland.org.uk"/>
    <dcterms:identifier>http://purl.org/heritagedata/schemes/225/concepts/141297</dcterms:identifier>
    <skos:broader rdf:resource="http://purl.org/heritagedata/schemes/225/concepts/141131"/>
  </rdf:Description>
  <rdf:Description rdf:about="http://purl.org/heritagedata/schemes/225/concepts/136522">
    <skos:prefLabel xml:lang="en">Siskin</skos:prefLabel>
    <cc:attributionName xml:lang="en">Historic England</cc:attributionName>
    <skos:inScheme rdf:resource="http://purl.org/heritagedata/schemes/225"/>
    <skos:broader rdf:resource="http://purl.org/heritagedata/schemes/225/concepts/111403"/>
    <dcterms:publisher rdf:resource="http://www.historicengland.org.uk"/>
    <skos:broader rdf:resource="http://purl.org/heritagedata/schemes/225/concepts/111376"/>
    <dcterms:identifier>http://purl.org/heritagedata/schemes/225/concepts/136522</dcterms:identifier>
    <rdf:type rdf:resource="http://www.w3.org/2004/02/skos/core#Concept"/>
    <skos:broader rdf:resource="http://purl.org/heritagedata/schemes/225/concepts/111397"/>
    <cc:license rdf:resource="http://creativecommons.org/licenses/by/3.0"/>
    <skos:scopeNote xml:lang="en">Single-engine, single-seat biplane day fighter developed by Siddeley. Variations included an all-metal, fabric-covered Mk.III, which became the RAF's main fighter in the 1920s.</skos:scopeNote>
    <cc:attributionURL rdf:resource="http://www.historicengland.org.uk"/>
    <dcterms:issued rdf:datatype="http://www.w3.org/2001/XMLSchema#dateTime">2019-03-26T16:45:43</dcterms:issued>
  </rdf:Description>
  <rdf:Description rdf:about="http://purl.org/heritagedata/schemes/225/concepts/137202">
    <skos:broader rdf:resource="http://purl.org/heritagedata/schemes/225/concepts/137200"/>
    <skos:broader rdf:resource="http://purl.org/heritagedata/schemes/225/concepts/111402"/>
    <dcterms:publisher rdf:resource="http://www.historicengland.org.uk"/>
    <skos:broader rdf:resource="http://purl.org/heritagedata/schemes/225/concepts/137110"/>
    <dcterms:identifier>http://purl.org/heritagedata/schemes/225/concepts/137202</dcterms:identifier>
    <rdf:type rdf:resource="http://www.w3.org/2004/02/skos/core#Concept"/>
    <skos:prefLabel xml:lang="en">Hotspur</skos:prefLabel>
    <cc:attributionName xml:lang="en">Historic England</cc:attributionName>
    <cc:license rdf:resource="http://creativecommons.org/licenses/by/3.0"/>
    <skos:inScheme rdf:resource="http://purl.org/heritagedata/schemes/225"/>
    <cc:attributionURL rdf:resource="http://www.historicengland.org.uk"/>
    <dcterms:issued rdf:datatype="http://www.w3.org/2001/XMLSchema#dateTime">2019-03-26T16:45:43</dcterms:issued>
    <skos:broader rdf:resource="http://purl.org/heritagedata/schemes/225/concepts/111401"/>
    <skos:scopeNote xml:lang="en">Principal glider-pilot training glider fitted with tandem seats. Spruce and plywood in construction, the Hotspur served with the Glider Pilot Regiment between 1941 and 1945.</skos:scopeNote>
  </rdf:Description>
  <rdf:Description rdf:about="http://purl.org/heritagedata/schemes/225/concepts/137237">
    <dcterms:issued rdf:datatype="http://www.w3.org/2001/XMLSchema#dateTime">2019-03-26T16:45:43</dcterms:issued>
    <dcterms:publisher rdf:resource="http://www.historicengland.org.uk"/>
    <skos:prefLabel xml:lang="en">He177</skos:prefLabel>
    <skos:broader rdf:resource="http://purl.org/heritagedata/schemes/225/concepts/111356"/>
    <skos:broader rdf:resource="http://purl.org/heritagedata/schemes/225/concepts/137190"/>
    <skos:scopeNote xml:lang="en">Twin-engined, six-crew, heavy bomber. Conceived as a rival to the Lancaster and Flying Fortress, the HE177 was dogged by mechanical and structural problems. Of a thousand produced, only about two hundred saw action.</skos:scopeNote>
    <cc:license rdf:resource="http://creativecommons.org/licenses/by/3.0"/>
    <cc:attributionName xml:lang="en">Historic England</cc:attributionName>
    <cc:attributionURL rdf:resource="http://www.historicengland.org.uk"/>
    <skos:inScheme rdf:resource="http://purl.org/heritagedata/schemes/225"/>
    <dcterms:identifier>http://purl.org/heritagedata/schemes/225/concepts/137237</dcterms:identifier>
    <skos:broader rdf:resource="http://purl.org/heritagedata/schemes/225/concepts/111402"/>
    <rdf:type rdf:resource="http://www.w3.org/2004/02/skos/core#Concept"/>
  </rdf:Description>
  <rdf:Description rdf:about="http://purl.org/heritagedata/schemes/225/concepts/167008">
    <skos:broader rdf:resource="http://purl.org/heritagedata/schemes/225/concepts/167007"/>
    <cc:attributionName xml:lang="en">Historic England</cc:attributionName>
    <skos:broader rdf:resource="http://purl.org/heritagedata/schemes/225/concepts/111403"/>
    <rdf:type rdf:resource="http://www.w3.org/2004/02/skos/core#Concept"/>
    <dcterms:issued rdf:datatype="http://www.w3.org/2001/XMLSchema#dateTime">2019-03-26T16:45:43</dcterms:issued>
    <cc:attributionURL rdf:resource="http://www.historicengland.org.uk"/>
    <skos:prefLabel xml:lang="en">Nieuport Delage Nid 30</skos:prefLabel>
    <cc:license rdf:resource="http://creativecommons.org/licenses/by/3.0"/>
    <skos:broader rdf:resource="http://purl.org/heritagedata/schemes/225/concepts/111424"/>
    <dcterms:publisher rdf:resource="http://www.historicengland.org.uk"/>
    <skos:inScheme rdf:resource="http://purl.org/heritagedata/schemes/225"/>
    <skos:scopeNote xml:lang="en">A French airliner which entered service in 1920. A conventional biplane design with enclosed cabin for four passengers and open cockpit for the pilot. Fitted with an early audible guidance system. Withdrawn from service in 1921.</skos:scopeNote>
    <dcterms:identifier>http://purl.org/heritagedata/schemes/225/concepts/167008</dcterms:identifier>
  </rdf:Description>
  <rdf:Description rdf:about="http://purl.org/heritagedata/schemes/225/concepts/135750">
    <dcterms:issued rdf:datatype="http://www.w3.org/2001/XMLSchema#dateTime">2019-03-26T16:45:43</dcterms:issued>
    <skos:broader rdf:resource="http://purl.org/heritagedata/schemes/225/concepts/111402"/>
    <cc:attributionURL rdf:resource="http://www.historicengland.org.uk"/>
    <rdf:type rdf:resource="http://www.w3.org/2004/02/skos/core#Concept"/>
    <skos:broader rdf:resource="http://purl.org/heritagedata/schemes/225/concepts/111423"/>
    <skos:broader rdf:resource="http://purl.org/heritagedata/schemes/225/concepts/135749"/>
    <dcterms:publisher rdf:resource="http://www.historicengland.org.uk"/>
    <skos:scopeNote xml:lang="en">British single-engine, two-seat night fighter. Originally intended as a day fighter, but withdrawn and converted in August 1940, this was the first fighter to incorporate a power-driven gun turret.</skos:scopeNote>
    <cc:license rdf:resource="http://creativecommons.org/licenses/by/3.0"/>
    <skos:inScheme rdf:resource="http://purl.org/heritagedata/schemes/225"/>
    <dcterms:identifier>http://purl.org/heritagedata/schemes/225/concepts/135750</dcterms:identifier>
    <cc:attributionName xml:lang="en">Historic England</cc:attributionName>
    <skos:prefLabel xml:lang="en">Defiant</skos:prefLabel>
  </rdf:Description>
  <rdf:Description rdf:about="http://purl.org/heritagedata/schemes/225/concepts/137197">
    <skos:broader rdf:resource="http://purl.org/heritagedata/schemes/225/concepts/111441"/>
    <skos:broader rdf:resource="http://purl.org/heritagedata/schemes/225/concepts/111403"/>
    <dcterms:publisher rdf:resource="http://www.historicengland.org.uk"/>
    <dcterms:identifier>http://purl.org/heritagedata/schemes/225/concepts/137197</dcterms:identifier>
    <cc:license rdf:resource="http://creativecommons.org/licenses/by/3.0"/>
    <cc:attributionName xml:lang="en">Historic England</cc:attributionName>
    <cc:attributionURL rdf:resource="http://www.historicengland.org.uk"/>
    <skos:inScheme rdf:resource="http://purl.org/heritagedata/schemes/225"/>
    <skos:broader rdf:resource="http://purl.org/heritagedata/schemes/225/concepts/136511"/>
    <skos:scopeNote xml:lang="en">A biplane torpedo-bomber designed to be flown from aircraft carriers. Equipped with foldable wings for ease of storage. Joined Fleet Air Arm service in 1940, intended as a replacement for the Swordfish.</skos:scopeNote>
    <rdf:type rdf:resource="http://www.w3.org/2004/02/skos/core#Concept"/>
    <dcterms:issued rdf:datatype="http://www.w3.org/2001/XMLSchema#dateTime">2019-03-26T16:45:43</dcterms:issued>
    <skos:prefLabel xml:lang="en">Albacore</skos:prefLabel>
  </rdf:Description>
  <rdf:Description rdf:about="http://purl.org/heritagedata/schemes/225/concepts/137231">
    <skos:scopeNote xml:lang="en">Noorduyn Aviation Limited. Formed in 1934 by Mr R.B.C. Noorduyn as a successor to Noorduyn Aircraft Limited, which was formed in 1933. The company's most notable production aircraft was the Norseman transport.</skos:scopeNote>
    <cc:attributionName xml:lang="en">Historic England</cc:attributionName>
    <cc:license rdf:resource="http://creativecommons.org/licenses/by/3.0"/>
    <skos:inScheme rdf:resource="http://purl.org/heritagedata/schemes/225"/>
    <cc:attributionURL rdf:resource="http://www.historicengland.org.uk"/>
    <dcterms:issued rdf:datatype="http://www.w3.org/2001/XMLSchema#dateTime">2019-03-26T16:45:43</dcterms:issued>
    <dcterms:identifier>http://purl.org/heritagedata/schemes/225/concepts/137231</dcterms:identifier>
    <skos:narrower rdf:resource="http://purl.org/heritagedata/schemes/225/concepts/137232"/>
    <skos:broader rdf:resource="http://purl.org/heritagedata/schemes/225/concepts/111358"/>
    <dcterms:publisher rdf:resource="http://www.historicengland.org.uk"/>
    <skos:prefLabel xml:lang="en">Noorduyn</skos:prefLabel>
    <rdf:type rdf:resource="http://www.w3.org/2004/02/skos/core#Concept"/>
  </rdf:Description>
  <rdf:Description rdf:about="http://purl.org/heritagedata/schemes/225/concepts/135749">
    <cc:attributionURL rdf:resource="http://www.historicengland.org.uk"/>
    <rdf:type rdf:resource="http://www.w3.org/2004/02/skos/core#Concept"/>
    <skos:scopeNote xml:lang="en">Boulton Paul Aircraft, Ltd., formed in 1934 to take over the  Aircraft Department of Boulton &amp; Paul, Ltd.</skos:scopeNote>
    <cc:attributionName xml:lang="en">Historic England</cc:attributionName>
    <cc:license rdf:resource="http://creativecommons.org/licenses/by/3.0"/>
    <dcterms:identifier>http://purl.org/heritagedata/schemes/225/concepts/135749</dcterms:identifier>
    <skos:narrower rdf:resource="http://purl.org/heritagedata/schemes/225/concepts/135750"/>
    <skos:broader rdf:resource="http://purl.org/heritagedata/schemes/225/concepts/111358"/>
    <dcterms:publisher rdf:resource="http://www.historicengland.org.uk"/>
    <skos:prefLabel xml:lang="en">Boulton Paul</skos:prefLabel>
    <dcterms:issued rdf:datatype="http://www.w3.org/2001/XMLSchema#dateTime">2019-03-26T16:45:43</dcterms:issued>
    <skos:inScheme rdf:resource="http://purl.org/heritagedata/schemes/225"/>
  </rdf:Description>
  <rdf:Description rdf:about="http://purl.org/heritagedata/schemes/225/concepts/111426">
    <skos:scopeNote xml:lang="en">A streamlined, twin-engined bomber, the DO17 entered service in 1937 with the Condor Legion, having started life as a high-speed mail and passenger transport aircraft, a role for which it was ill-suited due to the narrowness of the fuselage.</skos:scopeNote>
    <cc:attributionURL rdf:resource="http://www.historicengland.org.uk"/>
    <skos:broader rdf:resource="http://purl.org/heritagedata/schemes/225/concepts/111402"/>
    <rdf:type rdf:resource="http://www.w3.org/2004/02/skos/core#Concept"/>
    <dcterms:identifier>http://purl.org/heritagedata/schemes/225/concepts/111426</dcterms:identifier>
    <dcterms:publisher rdf:resource="http://www.historicengland.org.uk"/>
    <cc:attributionName xml:lang="en">Historic England</cc:attributionName>
    <dcterms:issued rdf:datatype="http://www.w3.org/2001/XMLSchema#dateTime">2019-03-26T16:45:43</dcterms:issued>
    <skos:inScheme rdf:resource="http://purl.org/heritagedata/schemes/225"/>
    <skos:prefLabel xml:lang="en">Do17</skos:prefLabel>
    <cc:license rdf:resource="http://creativecommons.org/licenses/by/3.0"/>
    <skos:broader rdf:resource="http://purl.org/heritagedata/schemes/225/concepts/111361"/>
    <skos:broader rdf:resource="http://purl.org/heritagedata/schemes/225/concepts/111398"/>
  </rdf:Description>
  <rdf:Description rdf:about="http://purl.org/heritagedata/schemes/225/concepts/136515">
    <skos:altLabel xml:lang="en">Dh4</skos:altLabel>
  </rdf:Description>
  <rdf:Description rdf:about="http://purl.org/heritagedata/schemes/225/concepts/125613">
    <cc:license rdf:resource="http://creativecommons.org/licenses/by/3.0"/>
    <dcterms:issued rdf:datatype="http://www.w3.org/2001/XMLSchema#dateTime">2019-03-26T16:45:43</dcterms:issued>
    <dcterms:publisher rdf:resource="http://www.historicengland.org.uk"/>
    <skos:broader rdf:resource="http://purl.org/heritagedata/schemes/225/concepts/111358"/>
    <cc:attributionName xml:lang="en">Historic England</cc:attributionName>
    <skos:inScheme rdf:resource="http://purl.org/heritagedata/schemes/225"/>
    <dcterms:identifier>http://purl.org/heritagedata/schemes/225/concepts/125613</dcterms:identifier>
    <skos:scopeNote xml:lang="en">The Glenn L. Martin Company, established in 1909 by Glenn L Martin. Produced the first successful American-designed twin-engined aeroplane, the Martin Twin, which was then converted for use as a passenger aircraft.</skos:scopeNote>
    <skos:prefLabel xml:lang="en">Martin</skos:prefLabel>
    <skos:narrower rdf:resource="http://purl.org/heritagedata/schemes/225/concepts/125593"/>
    <rdf:type rdf:resource="http://www.w3.org/2004/02/skos/core#Concept"/>
    <cc:attributionURL rdf:resource="http://www.historicengland.org.uk"/>
  </rdf:Description>
  <rdf:Description rdf:about="http://purl.org/heritagedata/schemes/225/concepts/137232">
    <dcterms:issued rdf:datatype="http://www.w3.org/2001/XMLSchema#dateTime">2019-03-26T16:45:43</dcterms:issued>
    <skos:broader rdf:resource="http://purl.org/heritagedata/schemes/225/concepts/137231"/>
    <dcterms:publisher rdf:resource="http://www.historicengland.org.uk"/>
    <skos:broader rdf:resource="http://purl.org/heritagedata/schemes/225/concepts/111402"/>
    <cc:attributionName xml:lang="en">Historic England</cc:attributionName>
    <skos:inScheme rdf:resource="http://purl.org/heritagedata/schemes/225"/>
    <skos:scopeNote xml:lang="en">Canadian-built, single-engine, high-wing transport and communications aircraft converted from a civilian model. Metal-framed with fabric covering, saw service in 1944-5. Was capable of being equipped with wheels, floats or skis.</skos:scopeNote>
    <skos:broader rdf:resource="http://purl.org/heritagedata/schemes/225/concepts/111424"/>
    <dcterms:identifier>http://purl.org/heritagedata/schemes/225/concepts/137232</dcterms:identifier>
    <skos:prefLabel xml:lang="en">UC64 Norseman</skos:prefLabel>
    <cc:license rdf:resource="http://creativecommons.org/licenses/by/3.0"/>
    <rdf:type rdf:resource="http://www.w3.org/2004/02/skos/core#Concept"/>
    <cc:attributionURL rdf:resource="http://www.historicengland.org.uk"/>
  </rdf:Description>
  <rdf:Description rdf:about="http://purl.org/heritagedata/schemes/225/concepts/144618">
    <skos:inScheme rdf:resource="http://purl.org/heritagedata/schemes/225"/>
    <rdf:type rdf:resource="http://www.w3.org/2004/02/skos/core#Concept"/>
    <skos:prefLabel xml:lang="en">Zeppelin</skos:prefLabel>
    <skos:scopeNote xml:lang="en">A rigid frame type of airship pioneered by Count Zeppelin and used by the Germans in WWI for military purposes: do not use asa generic name for airships</skos:scopeNote>
    <dcterms:identifier>http://purl.org/heritagedata/schemes/225/concepts/144618</dcterms:identifier>
    <cc:license rdf:resource="http://creativecommons.org/licenses/by/3.0"/>
    <cc:attributionURL rdf:resource="http://www.historicengland.org.uk"/>
    <dcterms:issued rdf:datatype="http://www.w3.org/2001/XMLSchema#dateTime">2019-03-26T16:45:43</dcterms:issued>
    <skos:broader rdf:resource="http://purl.org/heritagedata/schemes/225/concepts/137194"/>
    <dcterms:publisher rdf:resource="http://www.historicengland.org.uk"/>
    <cc:attributionName xml:lang="en">Historic England</cc:attributionName>
  </rdf:Description>
  <rdf:Description rdf:about="http://purl.org/heritagedata/schemes/225/concepts/134999">
    <skos:inScheme rdf:resource="http://purl.org/heritagedata/schemes/225"/>
    <dcterms:identifier>http://purl.org/heritagedata/schemes/225/concepts/134999</dcterms:identifier>
    <skos:prefLabel xml:lang="en">Ventura</skos:prefLabel>
    <cc:license rdf:resource="http://creativecommons.org/licenses/by/3.0"/>
    <cc:attributionURL rdf:resource="http://www.historicengland.org.uk"/>
    <skos:broader rdf:resource="http://purl.org/heritagedata/schemes/225/concepts/111398"/>
    <skos:broader rdf:resource="http://purl.org/heritagedata/schemes/225/concepts/111402"/>
    <cc:attributionName xml:lang="en">Historic England</cc:attributionName>
    <rdf:type rdf:resource="http://www.w3.org/2004/02/skos/core#Concept"/>
    <skos:scopeNote xml:lang="en">Second World War allied patrol-bomber built by Lockheed Vega, a Lockheed subsidiary. This aircraft was a military development of the Lodestar, USAF designation B-34.</skos:scopeNote>
    <dcterms:issued rdf:datatype="http://www.w3.org/2001/XMLSchema#dateTime">2019-03-26T16:45:43</dcterms:issued>
    <dcterms:publisher rdf:resource="http://www.historicengland.org.uk"/>
    <skos:broader rdf:resource="http://purl.org/heritagedata/schemes/225/concepts/135769"/>
  </rdf:Description>
  <rdf:Description rdf:about="http://purl.org/heritagedata/schemes/225/concepts/141134">
    <cc:attributionName xml:lang="en">Historic England</cc:attributionName>
    <skos:inScheme rdf:resource="http://purl.org/heritagedata/schemes/225"/>
    <dcterms:identifier>http://purl.org/heritagedata/schemes/225/concepts/141134</dcterms:identifier>
    <rdf:type rdf:resource="http://www.w3.org/2004/02/skos/core#Concept"/>
    <cc:license rdf:resource="http://creativecommons.org/licenses/by/3.0"/>
    <cc:attributionURL rdf:resource="http://www.historicengland.org.uk"/>
    <skos:prefLabel xml:lang="en">MkVI</skos:prefLabel>
    <skos:broader rdf:resource="http://purl.org/heritagedata/schemes/225/concepts/141131"/>
    <dcterms:issued rdf:datatype="http://www.w3.org/2001/XMLSchema#dateTime">2019-03-26T16:45:43</dcterms:issued>
    <dcterms:publisher rdf:resource="http://www.historicengland.org.uk"/>
    <skos:scopeNote xml:lang="en">Mark 6 or the sixth variant of an aircraft with its associated modifications.</skos:scopeNote>
  </rdf:Description>
  <rdf:Description rdf:about="http://purl.org/heritagedata/schemes/225/concepts/138535">
    <dcterms:issued rdf:datatype="http://www.w3.org/2001/XMLSchema#dateTime">2019-03-26T16:45:43</dcterms:issued>
    <dcterms:publisher rdf:resource="http://www.historicengland.org.uk"/>
    <cc:attributionURL rdf:resource="http://www.historicengland.org.uk"/>
    <skos:inScheme rdf:resource="http://purl.org/heritagedata/schemes/225"/>
    <dcterms:identifier>http://purl.org/heritagedata/schemes/225/concepts/138535</dcterms:identifier>
    <cc:license rdf:resource="http://creativecommons.org/licenses/by/3.0"/>
    <cc:attributionName xml:lang="en">Historic England</cc:attributionName>
    <skos:broader rdf:resource="http://purl.org/heritagedata/schemes/225/concepts/111397"/>
    <skos:broader rdf:resource="http://purl.org/heritagedata/schemes/225/concepts/136512"/>
    <skos:prefLabel xml:lang="en">Airco DH5</skos:prefLabel>
    <skos:broader rdf:resource="http://purl.org/heritagedata/schemes/225/concepts/111403"/>
    <rdf:type rdf:resource="http://www.w3.org/2004/02/skos/core#Concept"/>
    <skos:scopeNote xml:lang="en">The DH5 was an attempt to give a tractor-type fighter a good forward view. However it suffered from unpleasant flying characteristics and, as a result, had a short service career.</skos:scopeNote>
  </rdf:Description>
  <rdf:Description rdf:about="http://purl.org/heritagedata/schemes/225/concepts/111364">
    <dcterms:identifier>http://purl.org/heritagedata/schemes/225/concepts/111364</dcterms:identifier>
    <skos:broader rdf:resource="http://purl.org/heritagedata/schemes/225/concepts/111402"/>
    <dcterms:publisher rdf:resource="http://www.historicengland.org.uk"/>
    <cc:license rdf:resource="http://creativecommons.org/licenses/by/3.0"/>
    <rdf:type rdf:resource="http://www.w3.org/2004/02/skos/core#Concept"/>
    <cc:attributionURL rdf:resource="http://www.historicengland.org.uk"/>
    <skos:inScheme rdf:resource="http://purl.org/heritagedata/schemes/225"/>
    <cc:attributionName xml:lang="en">Historic England</cc:attributionName>
    <skos:broader rdf:resource="http://purl.org/heritagedata/schemes/225/concepts/111362"/>
    <dcterms:issued rdf:datatype="http://www.w3.org/2001/XMLSchema#dateTime">2019-03-26T16:45:43</dcterms:issued>
    <skos:prefLabel xml:lang="en">Ju88</skos:prefLabel>
    <ns1:related rdf:resource="http://purl.org/heritagedata/schemes/225/concepts/134952"/>
    <skos:scopeNote xml:lang="en">A twin-engined, multi-role aircraft built by Junkers. Originally designed as a medium bomber with the speed of a fighter, but its adaptability allowed it to fulfil the roles of night fighter, torpedo-bomber, anti-tank aircraft and photo-reconnaissance.</skos:scopeNote>
  </rdf:Description>
  <rdf:Description rdf:about="http://purl.org/heritagedata/schemes/225/concepts/137192">
    <skos:broader rdf:resource="http://purl.org/heritagedata/schemes/225/concepts/111397"/>
    <cc:license rdf:resource="http://creativecommons.org/licenses/by/3.0"/>
    <skos:broader rdf:resource="http://purl.org/heritagedata/schemes/225/concepts/111441"/>
    <skos:prefLabel xml:lang="en">Firefly</skos:prefLabel>
    <dcterms:publisher rdf:resource="http://www.historicengland.org.uk"/>
    <skos:inScheme rdf:resource="http://purl.org/heritagedata/schemes/225"/>
    <dcterms:identifier>http://purl.org/heritagedata/schemes/225/concepts/137192</dcterms:identifier>
    <cc:attributionName xml:lang="en">Historic England</cc:attributionName>
    <skos:broader rdf:resource="http://purl.org/heritagedata/schemes/225/concepts/111400"/>
    <skos:broader rdf:resource="http://purl.org/heritagedata/schemes/225/concepts/111402"/>
    <rdf:type rdf:resource="http://www.w3.org/2004/02/skos/core#Concept"/>
    <skos:scopeNote xml:lang="en">A single-engine, photo-reconnaissance fighter designed for operation from aircraft carriers. Later adapted as a night fighter, it entered service in 1943 and remained in production until 1956.</skos:scopeNote>
    <dcterms:issued rdf:datatype="http://www.w3.org/2001/XMLSchema#dateTime">2019-03-26T16:45:43</dcterms:issued>
    <cc:attributionURL rdf:resource="http://www.historicengland.org.uk"/>
  </rdf:Description>
  <rdf:Description rdf:about="http://purl.org/heritagedata/schemes/225/concepts/167858">
    <skos:broader rdf:resource="http://purl.org/heritagedata/schemes/225/concepts/111413"/>
    <skos:broader rdf:resource="http://purl.org/heritagedata/schemes/225/concepts/111402"/>
    <skos:scopeNote xml:lang="en">All-weather fighter/interceptor first flow in 1951, introduced into service in 1956 and retired from the RAF in 1968.</skos:scopeNote>
    <dcterms:publisher rdf:resource="http://www.historicengland.org.uk"/>
    <dcterms:identifier>http://purl.org/heritagedata/schemes/225/concepts/167858</dcterms:identifier>
    <cc:license rdf:resource="http://creativecommons.org/licenses/by/3.0"/>
    <rdf:type rdf:resource="http://www.w3.org/2004/02/skos/core#Concept"/>
    <skos:prefLabel xml:lang="en">Javelin</skos:prefLabel>
    <skos:inScheme rdf:resource="http://purl.org/heritagedata/schemes/225"/>
    <cc:attributionName xml:lang="en">Historic England</cc:attributionName>
    <skos:broader rdf:resource="http://purl.org/heritagedata/schemes/225/concepts/111397"/>
    <dcterms:issued rdf:datatype="http://www.w3.org/2001/XMLSchema#dateTime">2019-03-26T16:45:43</dcterms:issued>
    <cc:attributionURL rdf:resource="http://www.historicengland.org.uk"/>
  </rdf:Description>
  <rdf:Description rdf:about="http://purl.org/heritagedata/schemes/225/concepts/137216">
    <skos:broader rdf:resource="http://purl.org/heritagedata/schemes/225/concepts/111402"/>
    <skos:scopeNote xml:lang="en">Single-seat, single-engine fighter-bomber: Curtiss P40 Warhawk, known to the RAF as the Tomahawk, later renamed Kittyhawk. Serving from 1941 to 1942, control difficulties in dive attacks impeded bombing accuracy, resulting in use for larger targets only.</skos:scopeNote>
    <dcterms:issued rdf:datatype="http://www.w3.org/2001/XMLSchema#dateTime">2019-03-26T16:45:43</dcterms:issued>
    <skos:prefLabel xml:lang="en">Kittyhawk</skos:prefLabel>
    <cc:attributionName xml:lang="en">Historic England</cc:attributionName>
    <cc:license rdf:resource="http://creativecommons.org/licenses/by/3.0"/>
    <skos:inScheme rdf:resource="http://purl.org/heritagedata/schemes/225"/>
    <cc:attributionURL rdf:resource="http://www.historicengland.org.uk"/>
    <dcterms:identifier>http://purl.org/heritagedata/schemes/225/concepts/137216</dcterms:identifier>
    <skos:broader rdf:resource="http://purl.org/heritagedata/schemes/225/concepts/137217"/>
    <dcterms:publisher rdf:resource="http://www.historicengland.org.uk"/>
    <rdf:type rdf:resource="http://www.w3.org/2004/02/skos/core#Concept"/>
    <skos:broader rdf:resource="http://purl.org/heritagedata/schemes/225/concepts/111399"/>
  </rdf:Description>
  <rdf:Description rdf:about="http://purl.org/heritagedata/schemes/225/concepts/125533">
    <skos:broader rdf:resource="http://purl.org/heritagedata/schemes/225/concepts/111402"/>
    <rdf:type rdf:resource="http://www.w3.org/2004/02/skos/core#Concept"/>
    <skos:prefLabel xml:lang="en">B24 Liberator</skos:prefLabel>
    <ns1:related rdf:resource="http://purl.org/heritagedata/schemes/225/concepts/141296"/>
    <dcterms:publisher rdf:resource="http://www.historicengland.org.uk"/>
    <dcterms:identifier>http://purl.org/heritagedata/schemes/225/concepts/125533</dcterms:identifier>
    <skos:broader rdf:resource="http://purl.org/heritagedata/schemes/225/concepts/138507"/>
    <skos:broader rdf:resource="http://purl.org/heritagedata/schemes/225/concepts/137190"/>
    <cc:attributionName xml:lang="en">Historic England</cc:attributionName>
    <cc:attributionURL rdf:resource="http://www.historicengland.org.uk"/>
    <skos:inScheme rdf:resource="http://purl.org/heritagedata/schemes/225"/>
    <cc:license rdf:resource="http://creativecommons.org/licenses/by/3.0"/>
    <skos:scopeNote xml:lang="en">American, four-engined, long range, medium/heavy day bomber. Produced in greater numbers than any other American aircraft during the war.</skos:scopeNote>
    <dcterms:issued rdf:datatype="http://www.w3.org/2001/XMLSchema#dateTime">2019-03-26T16:45:43</dcterms:issued>
  </rdf:Description>
  <rdf:Description rdf:about="http://purl.org/heritagedata/schemes/225/concepts/111435">
    <skos:scopeNote xml:lang="en">American twin-engined medium bomber and ground-attack aircraft that entered service in 1941. A small number were delivered to the RAF under the British designation Mitchell I.</skos:scopeNote>
    <dcterms:identifier>http://purl.org/heritagedata/schemes/225/concepts/111435</dcterms:identifier>
    <skos:broader rdf:resource="http://purl.org/heritagedata/schemes/225/concepts/125513"/>
    <skos:prefLabel xml:lang="en">B25 Mitchell</skos:prefLabel>
    <cc:attributionName xml:lang="en">Historic England</cc:attributionName>
    <skos:inScheme rdf:resource="http://purl.org/heritagedata/schemes/225"/>
    <skos:broader rdf:resource="http://purl.org/heritagedata/schemes/225/concepts/139626"/>
    <skos:broader rdf:resource="http://purl.org/heritagedata/schemes/225/concepts/111402"/>
    <dcterms:publisher rdf:resource="http://www.historicengland.org.uk"/>
    <rdf:type rdf:resource="http://www.w3.org/2004/02/skos/core#Concept"/>
    <cc:license rdf:resource="http://creativecommons.org/licenses/by/3.0"/>
    <cc:attributionURL rdf:resource="http://www.historicengland.org.uk"/>
    <dcterms:issued rdf:datatype="http://www.w3.org/2001/XMLSchema#dateTime">2019-03-26T16:45:43</dcterms:issued>
  </rdf:Description>
  <rdf:Description rdf:about="http://purl.org/heritagedata/schemes/225/concepts/125573">
    <cc:attributionName xml:lang="en">Historic England</cc:attributionName>
    <cc:license rdf:resource="http://creativecommons.org/licenses/by/3.0"/>
    <skos:inScheme rdf:resource="http://purl.org/heritagedata/schemes/225"/>
    <cc:attributionURL rdf:resource="http://www.historicengland.org.uk"/>
    <dcterms:issued rdf:datatype="http://www.w3.org/2001/XMLSchema#dateTime">2019-03-26T16:45:43</dcterms:issued>
    <skos:scopeNote xml:lang="en">Four-engine, long range heavy bomber. Developed from the Lancaster, and originally designated the Lancaster Mk. IV, it was larger in size, bombload and fuel capacity. Never used operationally in World War Two.</skos:scopeNote>
    <skos:broader rdf:resource="http://purl.org/heritagedata/schemes/225/concepts/111355"/>
    <skos:broader rdf:resource="http://purl.org/heritagedata/schemes/225/concepts/137190"/>
    <skos:broader rdf:resource="http://purl.org/heritagedata/schemes/225/concepts/111402"/>
    <dcterms:publisher rdf:resource="http://www.historicengland.org.uk"/>
    <ns1:related rdf:resource="http://purl.org/heritagedata/schemes/225/concepts/111367"/>
    <dcterms:identifier>http://purl.org/heritagedata/schemes/225/concepts/125573</dcterms:identifier>
    <skos:prefLabel xml:lang="en">Lincoln</skos:prefLabel>
    <rdf:type rdf:resource="http://www.w3.org/2004/02/skos/core#Concept"/>
  </rdf:Description>
  <rdf:Description rdf:about="http://purl.org/heritagedata/schemes/225/concepts/140140">
    <dcterms:identifier>http://purl.org/heritagedata/schemes/225/concepts/140140</dcterms:identifier>
    <cc:attributionName xml:lang="en">Historic England</cc:attributionName>
    <cc:license rdf:resource="http://creativecommons.org/licenses/by/3.0"/>
    <skos:broader rdf:resource="http://purl.org/heritagedata/schemes/225/concepts/135730"/>
    <cc:attributionURL rdf:resource="http://www.historicengland.org.uk"/>
    <skos:scopeNote xml:lang="en">Twin-engined, four-crew German seaplane. Entered service in 1932 as a torpedo bomber and naval reconnaisance aircraft, though by World War 2 those still serving were used mainly for air sea rescue.</skos:scopeNote>
    <dcterms:publisher rdf:resource="http://www.historicengland.org.uk"/>
    <dcterms:issued rdf:datatype="http://www.w3.org/2001/XMLSchema#dateTime">2019-03-26T16:45:43</dcterms:issued>
    <skos:broader rdf:resource="http://purl.org/heritagedata/schemes/225/concepts/111403"/>
    <rdf:type rdf:resource="http://www.w3.org/2004/02/skos/core#Concept"/>
    <skos:broader rdf:resource="http://purl.org/heritagedata/schemes/225/concepts/134997"/>
    <skos:inScheme rdf:resource="http://purl.org/heritagedata/schemes/225"/>
    <skos:prefLabel xml:lang="en">He59</skos:prefLabel>
    <skos:broader rdf:resource="http://purl.org/heritagedata/schemes/225/concepts/111356"/>
    <skos:broader rdf:resource="http://purl.org/heritagedata/schemes/225/concepts/136511"/>
  </rdf:Description>
  <rdf:Description rdf:about="http://purl.org/heritagedata/schemes/225/concepts/141283">
    <skos:broader rdf:resource="http://purl.org/heritagedata/schemes/225/concepts/141131"/>
    <skos:scopeNote xml:lang="en">A Mark 3 aircraft which has undergone slight modifications to enhance performance or armament.</skos:scopeNote>
    <dcterms:identifier>http://purl.org/heritagedata/schemes/225/concepts/141283</dcterms:identifier>
    <skos:prefLabel xml:lang="en">MkIIIA</skos:prefLabel>
    <cc:attributionName xml:lang="en">Historic England</cc:attributionName>
    <skos:inScheme rdf:resource="http://purl.org/heritagedata/schemes/225"/>
    <dcterms:publisher rdf:resource="http://www.historicengland.org.uk"/>
    <rdf:type rdf:resource="http://www.w3.org/2004/02/skos/core#Concept"/>
    <cc:license rdf:resource="http://creativecommons.org/licenses/by/3.0"/>
    <cc:attributionURL rdf:resource="http://www.historicengland.org.uk"/>
    <dcterms:issued rdf:datatype="http://www.w3.org/2001/XMLSchema#dateTime">2019-03-26T16:45:43</dcterms:issued>
  </rdf:Description>
  <rdf:Description rdf:about="http://purl.org/heritagedata/schemes/225/concepts/137217">
    <skos:scopeNote xml:lang="en">The Curtiss-Wright Corporation, Airplane Division, established in 1910. Notable aircraft produced include the Kittyhawk.</skos:scopeNote>
    <dcterms:publisher rdf:resource="http://www.historicengland.org.uk"/>
    <cc:license rdf:resource="http://creativecommons.org/licenses/by/3.0"/>
    <dcterms:identifier>http://purl.org/heritagedata/schemes/225/concepts/137217</dcterms:identifier>
    <skos:broader rdf:resource="http://purl.org/heritagedata/schemes/225/concepts/111358"/>
    <skos:narrower rdf:resource="http://purl.org/heritagedata/schemes/225/concepts/137216"/>
    <rdf:type rdf:resource="http://www.w3.org/2004/02/skos/core#Concept"/>
    <cc:attributionURL rdf:resource="http://www.historicengland.org.uk"/>
    <skos:inScheme rdf:resource="http://purl.org/heritagedata/schemes/225"/>
    <cc:attributionName xml:lang="en">Historic England</cc:attributionName>
    <dcterms:issued rdf:datatype="http://www.w3.org/2001/XMLSchema#dateTime">2019-03-26T16:45:43</dcterms:issued>
    <skos:prefLabel xml:lang="en">Curtiss</skos:prefLabel>
  </rdf:Description>
  <rdf:Description rdf:about="http://purl.org/heritagedata/schemes/225/concepts/141207">
    <cc:attributionURL rdf:resource="http://www.historicengland.org.uk"/>
    <cc:attributionName xml:lang="en">Historic England</cc:attributionName>
    <skos:broader rdf:resource="http://purl.org/heritagedata/schemes/225/concepts/111403"/>
    <dcterms:identifier>http://purl.org/heritagedata/schemes/225/concepts/141207</dcterms:identifier>
    <dcterms:publisher rdf:resource="http://www.historicengland.org.uk"/>
    <skos:inScheme rdf:resource="http://purl.org/heritagedata/schemes/225"/>
    <skos:scopeNote xml:lang="en">A WWII British biplane produced by Hawker Aircraft, used for army cooperation duties.</skos:scopeNote>
    <rdf:type rdf:resource="http://www.w3.org/2004/02/skos/core#Concept"/>
    <skos:broader rdf:resource="http://purl.org/heritagedata/schemes/225/concepts/136031"/>
    <cc:license rdf:resource="http://creativecommons.org/licenses/by/3.0"/>
    <skos:broader rdf:resource="http://purl.org/heritagedata/schemes/225/concepts/111359"/>
    <skos:prefLabel xml:lang="en">Hector</skos:prefLabel>
    <dcterms:issued rdf:datatype="http://www.w3.org/2001/XMLSchema#dateTime">2019-03-26T16:45:43</dcterms:issued>
  </rdf:Description>
  <rdf:Description rdf:about="http://purl.org/heritagedata/schemes/225/concepts/136512">
    <skos:narrower rdf:resource="http://purl.org/heritagedata/schemes/225/concepts/138533"/>
    <dcterms:issued rdf:datatype="http://www.w3.org/2001/XMLSchema#dateTime">2019-03-26T16:45:43</dcterms:issued>
    <skos:narrower rdf:resource="http://purl.org/heritagedata/schemes/225/concepts/138537"/>
    <dcterms:publisher rdf:resource="http://www.historicengland.org.uk"/>
    <skos:narrower rdf:resource="http://purl.org/heritagedata/schemes/225/concepts/138536"/>
    <skos:narrower rdf:resource="http://purl.org/heritagedata/schemes/225/concepts/138534"/>
    <dcterms:identifier>http://purl.org/heritagedata/schemes/225/concepts/136512</dcterms:identifier>
    <skos:prefLabel xml:lang="en">Airco</skos:prefLabel>
    <skos:scopeNote xml:lang="en">Aircraft Manufacturing Co., Ltd. Established in 1912 by Mr G. Holt Thomas. In 1914 secured the services of Capt. Geoffrey de Havilland as designer-in-chief, who went on to lend his initials to a number of highly successful machines.</skos:scopeNote>
    <skos:narrower rdf:resource="http://purl.org/heritagedata/schemes/225/concepts/138532"/>
    <cc:attributionURL rdf:resource="http://www.historicengland.org.uk"/>
    <cc:attributionName xml:lang="en">Historic England</cc:attributionName>
    <skos:broader rdf:resource="http://purl.org/heritagedata/schemes/225/concepts/111358"/>
    <rdf:type rdf:resource="http://www.w3.org/2004/02/skos/core#Concept"/>
    <skos:inScheme rdf:resource="http://purl.org/heritagedata/schemes/225"/>
    <skos:narrower rdf:resource="http://purl.org/heritagedata/schemes/225/concepts/138535"/>
    <cc:license rdf:resource="http://creativecommons.org/licenses/by/3.0"/>
  </rdf:Description>
  <rdf:Description rdf:about="http://purl.org/heritagedata/schemes/225/concepts/136252">
    <skos:broader rdf:resource="http://purl.org/heritagedata/schemes/225/concepts/111358"/>
    <skos:prefLabel xml:lang="en">Felixstowe</skos:prefLabel>
    <dcterms:publisher rdf:resource="http://www.historicengland.org.uk"/>
    <skos:narrower rdf:resource="http://purl.org/heritagedata/schemes/225/concepts/138546"/>
    <skos:scopeNote xml:lang="en">Marine Aircraft Experimental Establishment, RAF Felixstowe. Developed seaplanes and flying boats until World War Two, when the establishment moved to Helensburg, Scotland.</skos:scopeNote>
    <dcterms:issued rdf:datatype="http://www.w3.org/2001/XMLSchema#dateTime">2019-03-26T16:45:43</dcterms:issued>
    <skos:inScheme rdf:resource="http://purl.org/heritagedata/schemes/225"/>
    <cc:attributionURL rdf:resource="http://www.historicengland.org.uk"/>
    <rdf:type rdf:resource="http://www.w3.org/2004/02/skos/core#Concept"/>
    <cc:attributionName xml:lang="en">Historic England</cc:attributionName>
    <cc:license rdf:resource="http://creativecommons.org/licenses/by/3.0"/>
    <dcterms:identifier>http://purl.org/heritagedata/schemes/225/concepts/136252</dcterms:identifier>
  </rdf:Description>
  <rdf:Description rdf:about="http://purl.org/heritagedata/schemes/225/concepts/111353">
    <skos:narrower rdf:resource="http://purl.org/heritagedata/schemes/225/concepts/111334"/>
    <dcterms:publisher rdf:resource="http://www.historicengland.org.uk"/>
    <skos:narrower rdf:resource="http://purl.org/heritagedata/schemes/225/concepts/137209"/>
    <cc:license rdf:resource="http://creativecommons.org/licenses/by/3.0"/>
    <cc:attributionName xml:lang="en">Historic England</cc:attributionName>
    <skos:inScheme rdf:resource="http://purl.org/heritagedata/schemes/225"/>
    <dcterms:identifier>http://purl.org/heritagedata/schemes/225/concepts/111353</dcterms:identifier>
    <skos:broader rdf:resource="http://purl.org/heritagedata/schemes/225/concepts/138508"/>
    <skos:prefLabel xml:lang="en">Supermarine</skos:prefLabel>
    <skos:narrower rdf:resource="http://purl.org/heritagedata/schemes/225/concepts/137208"/>
    <dcterms:issued rdf:datatype="http://www.w3.org/2001/XMLSchema#dateTime">2019-03-26T16:45:43</dcterms:issued>
    <skos:scopeNote xml:lang="en">The Supermarine Company was formed in 1912 and specialised in producing sea-going aircraft, including several Schneider Trophy winners. Taken over by Vickers-Armstrongs Ltd., in 1938.</skos:scopeNote>
    <rdf:type rdf:resource="http://www.w3.org/2004/02/skos/core#Concept"/>
    <cc:attributionURL rdf:resource="http://www.historicengland.org.uk"/>
    <skos:narrower rdf:resource="http://purl.org/heritagedata/schemes/225/concepts/133209"/>
    <skos:narrower rdf:resource="http://purl.org/heritagedata/schemes/225/concepts/136250"/>
  </rdf:Description>
  <rdf:Description rdf:about="http://purl.org/heritagedata/schemes/225/concepts/141210">
    <dcterms:identifier>http://purl.org/heritagedata/schemes/225/concepts/141210</dcterms:identifier>
    <skos:prefLabel xml:lang="en">Cessna</skos:prefLabel>
    <cc:attributionName xml:lang="en">Historic England</cc:attributionName>
    <skos:inScheme rdf:resource="http://purl.org/heritagedata/schemes/225"/>
    <skos:narrower rdf:resource="http://purl.org/heritagedata/schemes/225/concepts/141211"/>
    <dcterms:publisher rdf:resource="http://www.historicengland.org.uk"/>
    <cc:attributionURL rdf:resource="http://www.historicengland.org.uk"/>
    <skos:scopeNote xml:lang="en">A US aircraft manufacturer. The Cessna Aircraft Co Inc was established in 1927</skos:scopeNote>
    <dcterms:issued rdf:datatype="http://www.w3.org/2001/XMLSchema#dateTime">2019-03-26T16:45:43</dcterms:issued>
    <cc:license rdf:resource="http://creativecommons.org/licenses/by/3.0"/>
    <skos:broader rdf:resource="http://purl.org/heritagedata/schemes/225/concepts/111358"/>
    <rdf:type rdf:resource="http://www.w3.org/2004/02/skos/core#Concept"/>
  </rdf:Description>
  <rdf:Description rdf:about="http://purl.org/heritagedata/schemes/225/concepts/136251">
    <cc:license rdf:resource="http://creativecommons.org/licenses/by/3.0"/>
    <skos:inScheme rdf:resource="http://purl.org/heritagedata/schemes/225"/>
    <skos:broader rdf:resource="http://purl.org/heritagedata/schemes/225/concepts/135730"/>
    <dcterms:publisher rdf:resource="http://www.historicengland.org.uk"/>
    <skos:broader rdf:resource="http://purl.org/heritagedata/schemes/225/concepts/111374"/>
    <skos:scopeNote xml:lang="en">Large, three-engined, long range reconnaissance flying boat. Wooden hull and frame construction, with linen covering. Entered service in 1930.</skos:scopeNote>
    <skos:prefLabel xml:lang="en">Iris</skos:prefLabel>
    <cc:attributionName xml:lang="en">Historic England</cc:attributionName>
    <skos:broader rdf:resource="http://purl.org/heritagedata/schemes/225/concepts/111403"/>
    <rdf:type rdf:resource="http://www.w3.org/2004/02/skos/core#Concept"/>
    <dcterms:issued rdf:datatype="http://www.w3.org/2001/XMLSchema#dateTime">2019-03-26T16:45:43</dcterms:issued>
    <skos:broader rdf:resource="http://purl.org/heritagedata/schemes/225/concepts/111395"/>
    <cc:attributionURL rdf:resource="http://www.historicengland.org.uk"/>
    <dcterms:identifier>http://purl.org/heritagedata/schemes/225/concepts/136251</dcterms:identifier>
  </rdf:Description>
  <rdf:Description rdf:about="http://purl.org/heritagedata/schemes/225/concepts/111415">
    <dcterms:publisher rdf:resource="http://www.historicengland.org.uk"/>
    <cc:license rdf:resource="http://creativecommons.org/licenses/by/3.0"/>
    <skos:prefLabel xml:lang="en">Handley Page</skos:prefLabel>
    <skos:narrower rdf:resource="http://purl.org/heritagedata/schemes/225/concepts/137203"/>
    <dcterms:identifier>http://purl.org/heritagedata/schemes/225/concepts/111415</dcterms:identifier>
    <dcterms:issued rdf:datatype="http://www.w3.org/2001/XMLSchema#dateTime">2019-03-26T16:45:43</dcterms:issued>
    <cc:attributionName xml:lang="en">Historic England</cc:attributionName>
    <skos:inScheme rdf:resource="http://purl.org/heritagedata/schemes/225"/>
    <skos:narrower rdf:resource="http://purl.org/heritagedata/schemes/225/concepts/167015"/>
    <skos:narrower rdf:resource="http://purl.org/heritagedata/schemes/225/concepts/111416"/>
    <rdf:type rdf:resource="http://www.w3.org/2004/02/skos/core#Concept"/>
    <cc:attributionURL rdf:resource="http://www.historicengland.org.uk"/>
    <skos:scopeNote xml:lang="en">Handley Page, Ltd.. Founded by Sir Frederick Handley Page, this was the first limited company to be incorporated in Great Britain for the purpose of aircraft manufacture.</skos:scopeNote>
    <skos:narrower rdf:resource="http://purl.org/heritagedata/schemes/225/concepts/133173"/>
    <skos:broader rdf:resource="http://purl.org/heritagedata/schemes/225/concepts/111358"/>
    <skos:narrower rdf:resource="http://purl.org/heritagedata/schemes/225/concepts/140425"/>
  </rdf:Description>
  <rdf:Description rdf:about="http://purl.org/heritagedata/schemes/225/concepts/167000">
    <cc:attributionURL rdf:resource="http://www.historicengland.org.uk"/>
    <skos:broader rdf:resource="http://purl.org/heritagedata/schemes/225/concepts/111413"/>
    <skos:broader rdf:resource="http://purl.org/heritagedata/schemes/225/concepts/111403"/>
    <skos:broader rdf:resource="http://purl.org/heritagedata/schemes/225/concepts/111397"/>
    <ns1:related rdf:resource="http://purl.org/heritagedata/schemes/225/concepts/136231"/>
    <dcterms:publisher rdf:resource="http://www.historicengland.org.uk"/>
    <skos:scopeNote xml:lang="en">The Gloster Grebe was the Royal Air Force's first post WWI fighter aircraft, entering service in 1923. Designed by Henry Folland, a single-seat, single-engined biplane of fabric-covered wood construction with two Vickers machine guns (133 planes built).</skos:scopeNote>
    <cc:attributionName xml:lang="en">Historic England</cc:attributionName>
    <rdf:type rdf:resource="http://www.w3.org/2004/02/skos/core#Concept"/>
    <skos:inScheme rdf:resource="http://purl.org/heritagedata/schemes/225"/>
    <dcterms:identifier>http://purl.org/heritagedata/schemes/225/concepts/167000</dcterms:identifier>
    <skos:prefLabel xml:lang="en">Grebe</skos:prefLabel>
    <dcterms:issued rdf:datatype="http://www.w3.org/2001/XMLSchema#dateTime">2019-03-26T16:45:43</dcterms:issued>
    <cc:license rdf:resource="http://creativecommons.org/licenses/by/3.0"/>
  </rdf:Description>
  <rdf:Description rdf:about="http://purl.org/heritagedata/schemes/225/concepts/138543">
    <cc:attributionName xml:lang="en">Historic England</cc:attributionName>
    <skos:broader rdf:resource="http://purl.org/heritagedata/schemes/225/concepts/133207"/>
    <skos:inScheme rdf:resource="http://purl.org/heritagedata/schemes/225"/>
    <skos:prefLabel xml:lang="en">Folland Fo108</skos:prefLabel>
    <skos:scopeNote xml:lang="en">Single-engine, testbed monoplane built to Air Ministry Specification 43/37. Only twelve were produced, the first of which tested the Sabre I engine in 1940, and were used throughout the war. The cockpit could seat two observers behind the pilot.</skos:scopeNote>
    <dcterms:identifier>http://purl.org/heritagedata/schemes/225/concepts/138543</dcterms:identifier>
    <cc:license rdf:resource="http://creativecommons.org/licenses/by/3.0"/>
    <cc:attributionURL rdf:resource="http://www.historicengland.org.uk"/>
    <skos:broader rdf:resource="http://purl.org/heritagedata/schemes/225/concepts/111402"/>
    <dcterms:issued rdf:datatype="http://www.w3.org/2001/XMLSchema#dateTime">2019-03-26T16:45:43</dcterms:issued>
    <dcterms:publisher rdf:resource="http://www.historicengland.org.uk"/>
    <rdf:type rdf:resource="http://www.w3.org/2004/02/skos/core#Concept"/>
  </rdf:Description>
  <rdf:Description rdf:about="http://purl.org/heritagedata/schemes/225/concepts/133214">
    <skos:narrower rdf:resource="http://purl.org/heritagedata/schemes/225/concepts/137236"/>
    <cc:license rdf:resource="http://creativecommons.org/licenses/by/3.0"/>
    <skos:inScheme rdf:resource="http://purl.org/heritagedata/schemes/225"/>
    <dcterms:publisher rdf:resource="http://www.historicengland.org.uk"/>
    <cc:attributionURL rdf:resource="http://www.historicengland.org.uk"/>
    <skos:prefLabel xml:lang="en">Focke Wulf</skos:prefLabel>
    <cc:attributionName xml:lang="en">Historic England</cc:attributionName>
    <skos:broader rdf:resource="http://purl.org/heritagedata/schemes/225/concepts/111358"/>
    <rdf:type rdf:resource="http://www.w3.org/2004/02/skos/core#Concept"/>
    <dcterms:identifier>http://purl.org/heritagedata/schemes/225/concepts/133214</dcterms:identifier>
    <dcterms:issued rdf:datatype="http://www.w3.org/2001/XMLSchema#dateTime">2019-03-26T16:45:43</dcterms:issued>
    <skos:narrower rdf:resource="http://purl.org/heritagedata/schemes/225/concepts/111366"/>
    <skos:scopeNote xml:lang="en">Focke-Wulf Flugzeugbau G.m.b.H.. Founded in 1924 and amalgamated in 1931 with the Albatross-Flugzeugwerke G.m.b.H.. Converted to a G.m.b.H. in 1937.</skos:scopeNote>
  </rdf:Description>
  <rdf:Description rdf:about="http://purl.org/heritagedata/schemes/225/concepts/136232">
    <skos:broader rdf:resource="http://purl.org/heritagedata/schemes/225/concepts/111358"/>
    <cc:license rdf:resource="http://creativecommons.org/licenses/by/3.0"/>
    <rdf:type rdf:resource="http://www.w3.org/2004/02/skos/core#Concept"/>
    <cc:attributionURL rdf:resource="http://www.historicengland.org.uk"/>
    <skos:inScheme rdf:resource="http://purl.org/heritagedata/schemes/225"/>
    <cc:attributionName xml:lang="en">Historic England</cc:attributionName>
    <skos:scopeNote xml:lang="en">The Sopwith Aviation Co., Ltd.. Established in 1911 by the noted aviator Mr T. O. M. Sopwith. Produced many notable aircraft, including the Camel and a Schneider Cup-winning seaplane.</skos:scopeNote>
    <dcterms:issued rdf:datatype="http://www.w3.org/2001/XMLSchema#dateTime">2019-03-26T16:45:43</dcterms:issued>
    <skos:narrower rdf:resource="http://purl.org/heritagedata/schemes/225/concepts/136233"/>
    <dcterms:identifier>http://purl.org/heritagedata/schemes/225/concepts/136232</dcterms:identifier>
    <skos:narrower rdf:resource="http://purl.org/heritagedata/schemes/225/concepts/140416"/>
    <dcterms:publisher rdf:resource="http://www.historicengland.org.uk"/>
    <skos:prefLabel xml:lang="en">Sopwith</skos:prefLabel>
  </rdf:Description>
  <rdf:Description rdf:about="http://purl.org/heritagedata/schemes/225/concepts/134952">
    <skos:broader rdf:resource="http://purl.org/heritagedata/schemes/225/concepts/135730"/>
    <skos:prefLabel xml:lang="en">Ju188</skos:prefLabel>
    <skos:broader rdf:resource="http://purl.org/heritagedata/schemes/225/concepts/111402"/>
    <dcterms:publisher rdf:resource="http://www.historicengland.org.uk"/>
    <dcterms:identifier>http://purl.org/heritagedata/schemes/225/concepts/134952</dcterms:identifier>
    <rdf:type rdf:resource="http://www.w3.org/2004/02/skos/core#Concept"/>
    <cc:attributionName xml:lang="en">Historic England</cc:attributionName>
    <cc:license rdf:resource="http://creativecommons.org/licenses/by/3.0"/>
    <skos:inScheme rdf:resource="http://purl.org/heritagedata/schemes/225"/>
    <cc:attributionURL rdf:resource="http://www.historicengland.org.uk"/>
    <dcterms:issued rdf:datatype="http://www.w3.org/2001/XMLSchema#dateTime">2019-03-26T16:45:43</dcterms:issued>
    <skos:broader rdf:resource="http://purl.org/heritagedata/schemes/225/concepts/111362"/>
    <ns1:related rdf:resource="http://purl.org/heritagedata/schemes/225/concepts/111364"/>
    <skos:scopeNote xml:lang="en">A twin-engined development of the JU88, the JU188 had a higher service ceiling and greater maximum speed. JU188s operated over the UK from 1944 onwards as night intruders and reconnaissance aircraft.</skos:scopeNote>
  </rdf:Description>
  <rdf:Description rdf:about="http://purl.org/heritagedata/schemes/225/concepts/141353">
    <cc:attributionName xml:lang="en">Historic England</cc:attributionName>
    <skos:broader rdf:resource="http://purl.org/heritagedata/schemes/225/concepts/111402"/>
    <rdf:type rdf:resource="http://www.w3.org/2004/02/skos/core#Concept"/>
    <dcterms:issued rdf:datatype="http://www.w3.org/2001/XMLSchema#dateTime">2019-03-26T16:45:43</dcterms:issued>
    <cc:attributionURL rdf:resource="http://www.historicengland.org.uk"/>
    <skos:prefLabel xml:lang="en">Leopard Moth</skos:prefLabel>
    <cc:license rdf:resource="http://creativecommons.org/licenses/by/3.0"/>
    <dcterms:identifier>http://purl.org/heritagedata/schemes/225/concepts/141353</dcterms:identifier>
    <skos:scopeNote xml:lang="en">A single engine two seat cabin monoplane tourer, first flown in 1933 as a successor to the Puss Moth. Impressed into military sevice in WWII by the RAF and the Fleet Air Arm as a liaison and communications aircraft, also used by training units.</skos:scopeNote>
    <dcterms:publisher rdf:resource="http://www.historicengland.org.uk"/>
    <skos:broader rdf:resource="http://purl.org/heritagedata/schemes/225/concepts/111368"/>
    <skos:inScheme rdf:resource="http://purl.org/heritagedata/schemes/225"/>
    <skos:broader rdf:resource="http://purl.org/heritagedata/schemes/225/concepts/141359"/>
  </rdf:Description>
  <rdf:Description rdf:about="http://purl.org/heritagedata/schemes/225/concepts/137239">
    <dcterms:identifier>http://purl.org/heritagedata/schemes/225/concepts/137239</dcterms:identifier>
    <cc:license rdf:resource="http://creativecommons.org/licenses/by/3.0"/>
    <skos:broader rdf:resource="http://purl.org/heritagedata/schemes/225/concepts/111362"/>
    <skos:broader rdf:resource="http://purl.org/heritagedata/schemes/225/concepts/135730"/>
    <cc:attributionURL rdf:resource="http://www.historicengland.org.uk"/>
    <skos:scopeNote xml:lang="en">Two-crew, twin-engined bomber. Entered production in 1934 and designed for dual use as a high-speed commercial transport. Technical problems hindered its use as a bomber and led to conversion to high-altitude reconnaissance.</skos:scopeNote>
    <dcterms:issued rdf:datatype="http://www.w3.org/2001/XMLSchema#dateTime">2019-03-26T16:45:43</dcterms:issued>
    <skos:prefLabel xml:lang="en">Ju86</skos:prefLabel>
    <skos:broader rdf:resource="http://purl.org/heritagedata/schemes/225/concepts/111402"/>
    <rdf:type rdf:resource="http://www.w3.org/2004/02/skos/core#Concept"/>
    <skos:inScheme rdf:resource="http://purl.org/heritagedata/schemes/225"/>
    <cc:attributionName xml:lang="en">Historic England</cc:attributionName>
    <dcterms:publisher rdf:resource="http://www.historicengland.org.uk"/>
  </rdf:Description>
  <rdf:Description rdf:about="http://purl.org/heritagedata/schemes/225/concepts/137219">
    <cc:attributionURL rdf:resource="http://www.historicengland.org.uk"/>
    <rdf:type rdf:resource="http://www.w3.org/2004/02/skos/core#Concept"/>
    <cc:attributionName xml:lang="en">Historic England</cc:attributionName>
    <cc:license rdf:resource="http://creativecommons.org/licenses/by/3.0"/>
    <skos:prefLabel xml:lang="en">TBF Avenger</skos:prefLabel>
    <dcterms:identifier>http://purl.org/heritagedata/schemes/225/concepts/137219</dcterms:identifier>
    <skos:broader rdf:resource="http://purl.org/heritagedata/schemes/225/concepts/137218"/>
    <skos:scopeNote xml:lang="en">Three-crew, single-engine carrierborne torpedo-bomber. Entered service in 1942, first seeing action during the Battle of Midway. Served with the US Navy until 1956.</skos:scopeNote>
    <dcterms:publisher rdf:resource="http://www.historicengland.org.uk"/>
    <skos:broader rdf:resource="http://purl.org/heritagedata/schemes/225/concepts/136511"/>
    <skos:inScheme rdf:resource="http://purl.org/heritagedata/schemes/225"/>
    <dcterms:issued rdf:datatype="http://www.w3.org/2001/XMLSchema#dateTime">2019-03-26T16:45:43</dcterms:issued>
    <skos:broader rdf:resource="http://purl.org/heritagedata/schemes/225/concepts/111402"/>
  </rdf:Description>
  <rdf:Description rdf:about="http://purl.org/heritagedata/schemes/225/concepts/135931">
    <dcterms:issued rdf:datatype="http://www.w3.org/2001/XMLSchema#dateTime">2019-03-26T16:45:43</dcterms:issued>
    <skos:inScheme rdf:resource="http://purl.org/heritagedata/schemes/225"/>
    <cc:attributionURL rdf:resource="http://www.historicengland.org.uk"/>
    <skos:prefLabel xml:lang="en">Whirlwind</skos:prefLabel>
    <skos:broader rdf:resource="http://purl.org/heritagedata/schemes/225/concepts/135930"/>
    <cc:attributionName xml:lang="en">Historic England</cc:attributionName>
    <cc:license rdf:resource="http://creativecommons.org/licenses/by/3.0"/>
    <dcterms:publisher rdf:resource="http://www.historicengland.org.uk"/>
    <skos:broader rdf:resource="http://purl.org/heritagedata/schemes/225/concepts/111399"/>
    <skos:scopeNote xml:lang="en">Twin-engined fighter-bomber. All metal in construction, entered service in 1940. Supported bombing operations and participated in attacks on France, but not widely used due to engine faults.</skos:scopeNote>
    <skos:broader rdf:resource="http://purl.org/heritagedata/schemes/225/concepts/111402"/>
    <rdf:type rdf:resource="http://www.w3.org/2004/02/skos/core#Concept"/>
    <dcterms:identifier>http://purl.org/heritagedata/schemes/225/concepts/135931</dcterms:identifier>
  </rdf:Description>
  <rdf:Description rdf:about="http://purl.org/heritagedata/schemes/225/concepts/136510">
    <skos:broader rdf:resource="http://purl.org/heritagedata/schemes/225/concepts/111403"/>
    <skos:scopeNote xml:lang="en">A torpedo-bomber and reconnaissance biplane in service with the Fleet Air Arm 1935-1938. Rendered obsolete after 1938 by the Swordfish and withdrawn from service.</skos:scopeNote>
    <rdf:type rdf:resource="http://www.w3.org/2004/02/skos/core#Concept"/>
    <dcterms:publisher rdf:resource="http://www.historicengland.org.uk"/>
    <skos:broader rdf:resource="http://purl.org/heritagedata/schemes/225/concepts/136511"/>
    <cc:attributionName xml:lang="en">Historic England</cc:attributionName>
    <dcterms:identifier>http://purl.org/heritagedata/schemes/225/concepts/136510</dcterms:identifier>
    <cc:license rdf:resource="http://creativecommons.org/licenses/by/3.0"/>
    <skos:broader rdf:resource="http://purl.org/heritagedata/schemes/225/concepts/135730"/>
    <cc:attributionURL rdf:resource="http://www.historicengland.org.uk"/>
    <skos:inScheme rdf:resource="http://purl.org/heritagedata/schemes/225"/>
    <skos:broader rdf:resource="http://purl.org/heritagedata/schemes/225/concepts/111374"/>
    <skos:prefLabel xml:lang="en">Shark</skos:prefLabel>
    <dcterms:issued rdf:datatype="http://www.w3.org/2001/XMLSchema#dateTime">2019-03-26T16:45:43</dcterms:issued>
  </rdf:Description>
  <rdf:Description rdf:about="http://purl.org/heritagedata/schemes/225/concepts/141249">
    <dcterms:identifier>http://purl.org/heritagedata/schemes/225/concepts/141249</dcterms:identifier>
    <dcterms:issued rdf:datatype="http://www.w3.org/2001/XMLSchema#dateTime">2019-03-26T16:45:43</dcterms:issued>
    <dcterms:publisher rdf:resource="http://www.historicengland.org.uk"/>
    <skos:scopeNote xml:lang="en">A Mark 6B aircraft which has undergone further modifications to enhance performance or armament.</skos:scopeNote>
    <skos:broader rdf:resource="http://purl.org/heritagedata/schemes/225/concepts/141131"/>
    <cc:license rdf:resource="http://creativecommons.org/licenses/by/3.0"/>
    <cc:attributionName xml:lang="en">Historic England</cc:attributionName>
    <cc:attributionURL rdf:resource="http://www.historicengland.org.uk"/>
    <skos:inScheme rdf:resource="http://purl.org/heritagedata/schemes/225"/>
    <skos:prefLabel xml:lang="en">MkVIC</skos:prefLabel>
    <rdf:type rdf:resource="http://www.w3.org/2004/02/skos/core#Concept"/>
  </rdf:Description>
  <rdf:Description rdf:about="http://purl.org/heritagedata/schemes/225/concepts/169971">
    <rdf:type rdf:resource="http://www.w3.org/2004/02/skos/core#Concept"/>
    <dcterms:issued rdf:datatype="http://www.w3.org/2001/XMLSchema#dateTime">2019-03-26T16:45:43</dcterms:issued>
    <skos:broader rdf:resource="http://purl.org/heritagedata/schemes/225/concepts/111355"/>
    <dcterms:publisher rdf:resource="http://www.historicengland.org.uk"/>
    <cc:license rdf:resource="http://creativecommons.org/licenses/by/3.0"/>
    <dcterms:identifier>http://purl.org/heritagedata/schemes/225/concepts/169971</dcterms:identifier>
    <skos:scopeNote xml:lang="en">A jet-powered tailless delta wing high-altitude strategic bomber plane, operated by the RAF from 1956 until 1984. Typically armed with nuclear weapons but capable of conventional bombing missions. Used as a nuclear deterrent in the Cold War.</skos:scopeNote>
    <skos:prefLabel xml:lang="en">Vulcan</skos:prefLabel>
    <skos:broader rdf:resource="http://purl.org/heritagedata/schemes/225/concepts/111398"/>
    <cc:attributionName xml:lang="en">Historic England</cc:attributionName>
    <cc:attributionURL rdf:resource="http://www.historicengland.org.uk"/>
    <skos:inScheme rdf:resource="http://purl.org/heritagedata/schemes/225"/>
  </rdf:Description>
  <rdf:Description rdf:about="http://purl.org/heritagedata/schemes/225/concepts/167012">
    <dcterms:identifier>http://purl.org/heritagedata/schemes/225/concepts/167012</dcterms:identifier>
    <skos:inScheme rdf:resource="http://purl.org/heritagedata/schemes/225"/>
    <skos:scopeNote xml:lang="en">A French aircraft manufacturer founded by Louis Bleriot and Gabriel Voisin, both aviators and inventors, in 1903, dissolved in 1906. After World War I Bleriot founded Bleriot Aeronautique developing commercial aircraft.</skos:scopeNote>
    <dcterms:publisher rdf:resource="http://www.historicengland.org.uk"/>
    <cc:attributionName xml:lang="en">Historic England</cc:attributionName>
    <skos:broader rdf:resource="http://purl.org/heritagedata/schemes/225/concepts/111358"/>
    <dcterms:issued rdf:datatype="http://www.w3.org/2001/XMLSchema#dateTime">2019-03-26T16:45:43</dcterms:issued>
    <skos:narrower rdf:resource="http://purl.org/heritagedata/schemes/225/concepts/167014"/>
    <rdf:type rdf:resource="http://www.w3.org/2004/02/skos/core#Concept"/>
    <skos:prefLabel xml:lang="en">Bleriot</skos:prefLabel>
    <cc:license rdf:resource="http://creativecommons.org/licenses/by/3.0"/>
    <cc:attributionURL rdf:resource="http://www.historicengland.org.uk"/>
  </rdf:Description>
  <rdf:Description rdf:about="http://purl.org/heritagedata/schemes/225/concepts/111419">
    <dcterms:identifier>http://purl.org/heritagedata/schemes/225/concepts/111419</dcterms:identifier>
    <dcterms:issued rdf:datatype="http://www.w3.org/2001/XMLSchema#dateTime">2019-03-26T16:45:43</dcterms:issued>
    <dcterms:publisher rdf:resource="http://www.historicengland.org.uk"/>
    <skos:prefLabel xml:lang="en">Wellington</skos:prefLabel>
    <rdf:type rdf:resource="http://www.w3.org/2004/02/skos/core#Concept"/>
    <skos:broader rdf:resource="http://purl.org/heritagedata/schemes/225/concepts/111420"/>
    <skos:broader rdf:resource="http://purl.org/heritagedata/schemes/225/concepts/111402"/>
    <skos:broader rdf:resource="http://purl.org/heritagedata/schemes/225/concepts/139626"/>
    <ns1:related rdf:resource="http://purl.org/heritagedata/schemes/225/concepts/137130"/>
    <cc:attributionName xml:lang="en">Historic England</cc:attributionName>
    <cc:license rdf:resource="http://creativecommons.org/licenses/by/3.0"/>
    <skos:inScheme rdf:resource="http://purl.org/heritagedata/schemes/225"/>
    <cc:attributionURL rdf:resource="http://www.historicengland.org.uk"/>
    <skos:scopeNote xml:lang="en">Six-crew, twin-engined medium night-bomber. Entered service in 1938 and was the RAF's principal bomber until 1943, participating in the first bombing raid of the war. Later versions served as torpedo and reconnaissance-bombers, transports and trainers.</skos:scopeNote>
  </rdf:Description>
  <rdf:Description rdf:about="http://purl.org/heritagedata/schemes/225/concepts/125494">
    <cc:license rdf:resource="http://creativecommons.org/licenses/by/3.0"/>
    <cc:attributionName xml:lang="en">Historic England</cc:attributionName>
    <cc:attributionURL rdf:resource="http://www.historicengland.org.uk"/>
    <skos:inScheme rdf:resource="http://purl.org/heritagedata/schemes/225"/>
    <skos:narrower rdf:resource="http://purl.org/heritagedata/schemes/225/concepts/167001"/>
    <dcterms:issued rdf:datatype="http://www.w3.org/2001/XMLSchema#dateTime">2019-03-26T16:45:43</dcterms:issued>
    <dcterms:identifier>http://purl.org/heritagedata/schemes/225/concepts/125494</dcterms:identifier>
    <rdf:type rdf:resource="http://www.w3.org/2004/02/skos/core#Concept"/>
    <skos:narrower rdf:resource="http://purl.org/heritagedata/schemes/225/concepts/125493"/>
    <dcterms:publisher rdf:resource="http://www.historicengland.org.uk"/>
    <skos:prefLabel xml:lang="en">Republic</skos:prefLabel>
    <skos:scopeNote xml:lang="en">The Republic Aviation Corporation. Developed from the Seversky Aircraft Corporation, founded by Alexander P. de Seversky in 1931 after the collapse of his previous company, the Seversky Aero Corporation, in the 1929 stock market crash.</skos:scopeNote>
    <skos:broader rdf:resource="http://purl.org/heritagedata/schemes/225/concepts/111358"/>
  </rdf:Description>
  <rdf:Description rdf:about="http://purl.org/heritagedata/schemes/225/concepts/111358">
    <skos:narrower rdf:resource="http://purl.org/heritagedata/schemes/225/concepts/137217"/>
    <skos:narrower rdf:resource="http://purl.org/heritagedata/schemes/225/concepts/151396"/>
    <skos:narrower rdf:resource="http://purl.org/heritagedata/schemes/225/concepts/133214"/>
    <skos:narrower rdf:resource="http://purl.org/heritagedata/schemes/225/concepts/133205"/>
    <skos:narrower rdf:resource="http://purl.org/heritagedata/schemes/225/concepts/135930"/>
    <skos:narrower rdf:resource="http://purl.org/heritagedata/schemes/225/concepts/111361"/>
    <skos:narrower rdf:resource="http://purl.org/heritagedata/schemes/225/concepts/133198"/>
    <skos:narrower rdf:resource="http://purl.org/heritagedata/schemes/225/concepts/140455"/>
    <skos:narrower rdf:resource="http://purl.org/heritagedata/schemes/225/concepts/111359"/>
    <skos:narrower rdf:resource="http://purl.org/heritagedata/schemes/225/concepts/111441"/>
    <skos:prefLabel xml:lang="en">Aircraft &lt;By Manufacturer&gt;</skos:prefLabel>
    <skos:narrower rdf:resource="http://purl.org/heritagedata/schemes/225/concepts/133200"/>
    <skos:narrower rdf:resource="http://purl.org/heritagedata/schemes/225/concepts/138484"/>
    <skos:narrower rdf:resource="http://purl.org/heritagedata/schemes/225/concepts/111415"/>
    <skos:inScheme rdf:resource="http://purl.org/heritagedata/schemes/225"/>
    <skos:narrower rdf:resource="http://purl.org/heritagedata/schemes/225/concepts/118653"/>
    <skos:narrower rdf:resource="http://purl.org/heritagedata/schemes/225/concepts/137218"/>
    <skos:narrower rdf:resource="http://purl.org/heritagedata/schemes/225/concepts/125614"/>
    <skos:narrower rdf:resource="http://purl.org/heritagedata/schemes/225/concepts/140097"/>
    <skos:narrower rdf:resource="http://purl.org/heritagedata/schemes/225/concepts/167007"/>
    <skos:narrower rdf:resource="http://purl.org/heritagedata/schemes/225/concepts/137213"/>
    <skos:narrower rdf:resource="http://purl.org/heritagedata/schemes/225/concepts/152400"/>
    <skos:narrower rdf:resource="http://purl.org/heritagedata/schemes/225/concepts/141212"/>
    <skos:narrower rdf:resource="http://purl.org/heritagedata/schemes/225/concepts/167002"/>
    <skos:narrower rdf:resource="http://purl.org/heritagedata/schemes/225/concepts/111376"/>
    <skos:narrower rdf:resource="http://purl.org/heritagedata/schemes/225/concepts/135749"/>
    <skos:narrower rdf:resource="http://purl.org/heritagedata/schemes/225/concepts/125613"/>
    <cc:license rdf:resource="http://creativecommons.org/licenses/by/3.0"/>
    <skos:narrower rdf:resource="http://purl.org/heritagedata/schemes/225/concepts/137211"/>
    <cc:attributionName xml:lang="en">Historic England</cc:attributionName>
    <skos:narrower rdf:resource="http://purl.org/heritagedata/schemes/225/concepts/137223"/>
    <skos:narrower rdf:resource="http://purl.org/heritagedata/schemes/225/concepts/111355"/>
    <skos:narrower rdf:resource="http://purl.org/heritagedata/schemes/225/concepts/137231"/>
    <skos:narrower rdf:resource="http://purl.org/heritagedata/schemes/225/concepts/138507"/>
    <skos:narrower rdf:resource="http://purl.org/heritagedata/schemes/225/concepts/111421"/>
    <skos:narrower rdf:resource="http://purl.org/heritagedata/schemes/225/concepts/111413"/>
    <cc:attributionURL rdf:resource="http://www.historicengland.org.uk"/>
    <skos:narrower rdf:resource="http://purl.org/heritagedata/schemes/225/concepts/133207"/>
    <skos:narrower rdf:resource="http://purl.org/heritagedata/schemes/225/concepts/136252"/>
    <skos:scopeNote xml:lang="en">Aircraft grouped according to their manufacturer.</skos:scopeNote>
    <skos:narrower rdf:resource="http://purl.org/heritagedata/schemes/225/concepts/138508"/>
    <skos:narrower rdf:resource="http://purl.org/heritagedata/schemes/225/concepts/167010"/>
    <skos:narrower rdf:resource="http://purl.org/heritagedata/schemes/225/concepts/125516"/>
    <skos:narrower rdf:resource="http://purl.org/heritagedata/schemes/225/concepts/137227"/>
    <skos:narrower rdf:resource="http://purl.org/heritagedata/schemes/225/concepts/111356"/>
    <skos:narrower rdf:resource="http://purl.org/heritagedata/schemes/225/concepts/125494"/>
    <skos:narrower rdf:resource="http://purl.org/heritagedata/schemes/225/concepts/111368"/>
    <skos:narrower rdf:resource="http://purl.org/heritagedata/schemes/225/concepts/137205"/>
    <rdf:type rdf:resource="http://www.w3.org/2004/02/skos/core#Concept"/>
    <skos:narrower rdf:resource="http://purl.org/heritagedata/schemes/225/concepts/111357"/>
    <skos:narrower rdf:resource="http://purl.org/heritagedata/schemes/225/concepts/137207"/>
    <skos:narrower rdf:resource="http://purl.org/heritagedata/schemes/225/concepts/141210"/>
    <skos:broader rdf:resource="http://purl.org/heritagedata/schemes/225/concepts/123733"/>
    <skos:narrower rdf:resource="http://purl.org/heritagedata/schemes/225/concepts/136512"/>
    <dcterms:publisher rdf:resource="http://www.historicengland.org.uk"/>
    <skos:narrower rdf:resource="http://purl.org/heritagedata/schemes/225/concepts/137200"/>
    <dcterms:issued rdf:datatype="http://www.w3.org/2001/XMLSchema#dateTime">2019-03-26T16:45:43</dcterms:issued>
    <skos:narrower rdf:resource="http://purl.org/heritagedata/schemes/225/concepts/136232"/>
    <skos:narrower rdf:resource="http://purl.org/heritagedata/schemes/225/concepts/125513"/>
    <skos:narrower rdf:resource="http://purl.org/heritagedata/schemes/225/concepts/167012"/>
    <dcterms:identifier>http://purl.org/heritagedata/schemes/225/concepts/111358</dcterms:identifier>
    <skos:narrower rdf:resource="http://purl.org/heritagedata/schemes/225/concepts/111362"/>
    <skos:narrower rdf:resource="http://purl.org/heritagedata/schemes/225/concepts/111433"/>
    <skos:narrower rdf:resource="http://purl.org/heritagedata/schemes/225/concepts/111374"/>
  </rdf:Description>
  <rdf:Description rdf:about="http://purl.org/heritagedata/schemes/225/concepts/111398">
    <cc:attributionURL rdf:resource="http://www.historicengland.org.uk"/>
    <rdf:type rdf:resource="http://www.w3.org/2004/02/skos/core#Concept"/>
    <dcterms:identifier>http://purl.org/heritagedata/schemes/225/concepts/111398</dcterms:identifier>
    <skos:narrower rdf:resource="http://purl.org/heritagedata/schemes/225/concepts/111427"/>
    <cc:attributionName xml:lang="en">Historic England</cc:attributionName>
    <cc:license rdf:resource="http://creativecommons.org/licenses/by/3.0"/>
    <skos:narrower rdf:resource="http://purl.org/heritagedata/schemes/225/concepts/134999"/>
    <skos:narrower rdf:resource="http://purl.org/heritagedata/schemes/225/concepts/138537"/>
    <skos:narrower rdf:resource="http://purl.org/heritagedata/schemes/225/concepts/111399"/>
    <skos:narrower rdf:resource="http://purl.org/heritagedata/schemes/225/concepts/137236"/>
    <skos:narrower rdf:resource="http://purl.org/heritagedata/schemes/225/concepts/139626"/>
    <skos:broader rdf:resource="http://purl.org/heritagedata/schemes/225/concepts/111394"/>
    <skos:narrower rdf:resource="http://purl.org/heritagedata/schemes/225/concepts/136524"/>
    <skos:narrower rdf:resource="http://purl.org/heritagedata/schemes/225/concepts/136511"/>
    <skos:inScheme rdf:resource="http://purl.org/heritagedata/schemes/225"/>
    <skos:scopeNote xml:lang="en">A large, powerful aircraft, usually with two or more engines, designed to carry a payload of bombs.</skos:scopeNote>
    <skos:narrower rdf:resource="http://purl.org/heritagedata/schemes/225/concepts/111426"/>
    <skos:narrower rdf:resource="http://purl.org/heritagedata/schemes/225/concepts/138534"/>
    <skos:narrower rdf:resource="http://purl.org/heritagedata/schemes/225/concepts/140411"/>
    <skos:narrower rdf:resource="http://purl.org/heritagedata/schemes/225/concepts/136234"/>
    <skos:narrower rdf:resource="http://purl.org/heritagedata/schemes/225/concepts/137190"/>
    <dcterms:publisher rdf:resource="http://www.historicengland.org.uk"/>
    <skos:narrower rdf:resource="http://purl.org/heritagedata/schemes/225/concepts/133203"/>
    <skos:narrower rdf:resource="http://purl.org/heritagedata/schemes/225/concepts/137189"/>
    <skos:narrower rdf:resource="http://purl.org/heritagedata/schemes/225/concepts/133199"/>
    <skos:narrower rdf:resource="http://purl.org/heritagedata/schemes/225/concepts/137195"/>
    <skos:narrower rdf:resource="http://purl.org/heritagedata/schemes/225/concepts/169971"/>
    <skos:narrower rdf:resource="http://purl.org/heritagedata/schemes/225/concepts/111363"/>
    <dcterms:issued rdf:datatype="http://www.w3.org/2001/XMLSchema#dateTime">2019-03-26T16:45:43</dcterms:issued>
    <skos:narrower rdf:resource="http://purl.org/heritagedata/schemes/225/concepts/138539"/>
    <skos:prefLabel xml:lang="en">Bomber</skos:prefLabel>
  </rdf:Description>
  <rdf:Description rdf:about="http://purl.org/heritagedata/schemes/225/concepts/141256">
    <dcterms:identifier>http://purl.org/heritagedata/schemes/225/concepts/141256</dcterms:identifier>
    <rdf:type rdf:resource="http://www.w3.org/2004/02/skos/core#Concept"/>
    <skos:prefLabel xml:lang="en">MkXIV</skos:prefLabel>
    <skos:broader rdf:resource="http://purl.org/heritagedata/schemes/225/concepts/141131"/>
    <dcterms:issued rdf:datatype="http://www.w3.org/2001/XMLSchema#dateTime">2019-03-26T16:45:43</dcterms:issued>
    <dcterms:publisher rdf:resource="http://www.historicengland.org.uk"/>
    <cc:attributionName xml:lang="en">Historic England</cc:attributionName>
    <skos:inScheme rdf:resource="http://purl.org/heritagedata/schemes/225"/>
    <skos:scopeNote xml:lang="en">Mark 14 or the fourteenth variant of an aircraft with its associated modifications.</skos:scopeNote>
    <cc:license rdf:resource="http://creativecommons.org/licenses/by/3.0"/>
    <cc:attributionURL rdf:resource="http://www.historicengland.org.uk"/>
  </rdf:Description>
  <rdf:Description rdf:about="http://purl.org/heritagedata/schemes/225/concepts/137200">
    <dcterms:publisher rdf:resource="http://www.historicengland.org.uk"/>
    <skos:narrower rdf:resource="http://purl.org/heritagedata/schemes/225/concepts/137202"/>
    <skos:scopeNote xml:lang="en">General Aircraft Limited.</skos:scopeNote>
    <cc:license rdf:resource="http://creativecommons.org/licenses/by/3.0"/>
    <rdf:type rdf:resource="http://www.w3.org/2004/02/skos/core#Concept"/>
    <cc:attributionURL rdf:resource="http://www.historicengland.org.uk"/>
    <dcterms:identifier>http://purl.org/heritagedata/schemes/225/concepts/137200</dcterms:identifier>
    <dcterms:issued rdf:datatype="http://www.w3.org/2001/XMLSchema#dateTime">2019-03-26T16:45:43</dcterms:issued>
    <skos:prefLabel xml:lang="en">General Aircraft</skos:prefLabel>
    <skos:broader rdf:resource="http://purl.org/heritagedata/schemes/225/concepts/111358"/>
    <skos:narrower rdf:resource="http://purl.org/heritagedata/schemes/225/concepts/137201"/>
    <cc:attributionName xml:lang="en">Historic England</cc:attributionName>
    <skos:inScheme rdf:resource="http://purl.org/heritagedata/schemes/225"/>
  </rdf:Description>
  <rdf:Description rdf:about="http://purl.org/heritagedata/schemes/225/concepts/133202">
    <skos:prefLabel xml:lang="en">Me410</skos:prefLabel>
    <dcterms:issued rdf:datatype="http://www.w3.org/2001/XMLSchema#dateTime">2019-03-26T16:45:43</dcterms:issued>
    <skos:broader rdf:resource="http://purl.org/heritagedata/schemes/225/concepts/111402"/>
    <cc:attributionURL rdf:resource="http://www.historicengland.org.uk"/>
    <rdf:type rdf:resource="http://www.w3.org/2004/02/skos/core#Concept"/>
    <skos:broader rdf:resource="http://purl.org/heritagedata/schemes/225/concepts/111423"/>
    <skos:inScheme rdf:resource="http://purl.org/heritagedata/schemes/225"/>
    <skos:broader rdf:resource="http://purl.org/heritagedata/schemes/225/concepts/118653"/>
    <cc:license rdf:resource="http://creativecommons.org/licenses/by/3.0"/>
    <ns1:related rdf:resource="http://purl.org/heritagedata/schemes/225/concepts/137238"/>
    <dcterms:identifier>http://purl.org/heritagedata/schemes/225/concepts/133202</dcterms:identifier>
    <skos:scopeNote xml:lang="en">Developed from the ill-fated ME210, the ME410 Hornisse entered service in May 1943. Although underpowered as a day fighter the ME410 saw service over the UK as a night fighter from 1943-45.</skos:scopeNote>
    <dcterms:publisher rdf:resource="http://www.historicengland.org.uk"/>
    <cc:attributionName xml:lang="en">Historic England</cc:attributionName>
  </rdf:Description>
  <rdf:Description rdf:about="http://purl.org/heritagedata/schemes/225/concepts/125553">
    <dcterms:issued rdf:datatype="http://www.w3.org/2001/XMLSchema#dateTime">2019-03-26T16:45:43</dcterms:issued>
    <dcterms:publisher rdf:resource="http://www.historicengland.org.uk"/>
    <dcterms:identifier>http://purl.org/heritagedata/schemes/225/concepts/125553</dcterms:identifier>
    <skos:broader rdf:resource="http://purl.org/heritagedata/schemes/225/concepts/137190"/>
    <rdf:type rdf:resource="http://www.w3.org/2004/02/skos/core#Concept"/>
    <cc:license rdf:resource="http://creativecommons.org/licenses/by/3.0"/>
    <cc:attributionName xml:lang="en">Historic England</cc:attributionName>
    <cc:attributionURL rdf:resource="http://www.historicengland.org.uk"/>
    <skos:inScheme rdf:resource="http://purl.org/heritagedata/schemes/225"/>
    <skos:broader rdf:resource="http://purl.org/heritagedata/schemes/225/concepts/111433"/>
    <skos:broader rdf:resource="http://purl.org/heritagedata/schemes/225/concepts/111402"/>
    <skos:prefLabel xml:lang="en">B17 Flying Fortress</skos:prefLabel>
    <skos:scopeNote xml:lang="en">American, four-engined, medium/heavy day bomber. Entered service in 1937. The prototype was nicknamed the Flying Fortress, which later became a registered trademark.</skos:scopeNote>
  </rdf:Description>
  <rdf:Description rdf:about="http://purl.org/heritagedata/schemes/225/concepts/136591">
    <skos:prefLabel xml:lang="en">Lerwick</skos:prefLabel>
    <skos:broader rdf:resource="http://purl.org/heritagedata/schemes/225/concepts/111402"/>
    <rdf:type rdf:resource="http://www.w3.org/2004/02/skos/core#Concept"/>
    <dcterms:publisher rdf:resource="http://www.historicengland.org.uk"/>
    <skos:scopeNote xml:lang="en">Six-crew, medium-range, twin-engined reconnaissance flying-boat. Entered service with 209 Squadron in 1939 but, due to design and operation problems, saw little action and was not produced in large numbers.</skos:scopeNote>
    <dcterms:identifier>http://purl.org/heritagedata/schemes/225/concepts/136591</dcterms:identifier>
    <cc:attributionName xml:lang="en">Historic England</cc:attributionName>
    <cc:license rdf:resource="http://creativecommons.org/licenses/by/3.0"/>
    <skos:broader rdf:resource="http://purl.org/heritagedata/schemes/225/concepts/135730"/>
    <skos:broader rdf:resource="http://purl.org/heritagedata/schemes/225/concepts/137207"/>
    <skos:inScheme rdf:resource="http://purl.org/heritagedata/schemes/225"/>
    <dcterms:issued rdf:datatype="http://www.w3.org/2001/XMLSchema#dateTime">2019-03-26T16:45:43</dcterms:issued>
    <cc:attributionURL rdf:resource="http://www.historicengland.org.uk"/>
    <skos:broader rdf:resource="http://purl.org/heritagedata/schemes/225/concepts/111395"/>
  </rdf:Description>
  <rdf:Description rdf:about="http://purl.org/heritagedata/schemes/225/concepts/141131">
    <skos:narrower rdf:resource="http://purl.org/heritagedata/schemes/225/concepts/141253"/>
    <skos:narrower rdf:resource="http://purl.org/heritagedata/schemes/225/concepts/142898"/>
    <skos:narrower rdf:resource="http://purl.org/heritagedata/schemes/225/concepts/141303"/>
    <skos:narrower rdf:resource="http://purl.org/heritagedata/schemes/225/concepts/141209"/>
    <skos:narrower rdf:resource="http://purl.org/heritagedata/schemes/225/concepts/141196"/>
    <skos:narrower rdf:resource="http://purl.org/heritagedata/schemes/225/concepts/141214"/>
    <skos:narrower rdf:resource="http://purl.org/heritagedata/schemes/225/concepts/141257"/>
    <skos:prefLabel xml:lang="en">Aircraft Mark</skos:prefLabel>
    <rdf:type rdf:resource="http://www.w3.org/2004/02/skos/core#Concept"/>
    <skos:narrower rdf:resource="http://purl.org/heritagedata/schemes/225/concepts/141254"/>
    <skos:narrower rdf:resource="http://purl.org/heritagedata/schemes/225/concepts/141134"/>
    <skos:narrower rdf:resource="http://purl.org/heritagedata/schemes/225/concepts/141283"/>
    <skos:scopeNote xml:lang="en">Used to identify the variations of an aircraft. Index with Manufacturer, Form and Function.</skos:scopeNote>
    <skos:broader rdf:resource="http://purl.org/heritagedata/schemes/225/concepts/123733"/>
    <skos:narrower rdf:resource="http://purl.org/heritagedata/schemes/225/concepts/141208"/>
    <skos:narrower rdf:resource="http://purl.org/heritagedata/schemes/225/concepts/141204"/>
    <skos:narrower rdf:resource="http://purl.org/heritagedata/schemes/225/concepts/141215"/>
    <skos:narrower rdf:resource="http://purl.org/heritagedata/schemes/225/concepts/141297"/>
    <skos:narrower rdf:resource="http://purl.org/heritagedata/schemes/225/concepts/141258"/>
    <skos:narrower rdf:resource="http://purl.org/heritagedata/schemes/225/concepts/141132"/>
    <skos:narrower rdf:resource="http://purl.org/heritagedata/schemes/225/concepts/141274"/>
    <skos:narrower rdf:resource="http://purl.org/heritagedata/schemes/225/concepts/141249"/>
    <dcterms:publisher rdf:resource="http://www.historicengland.org.uk"/>
    <cc:attributionName xml:lang="en">Historic England</cc:attributionName>
    <dcterms:issued rdf:datatype="http://www.w3.org/2001/XMLSchema#dateTime">2019-03-26T16:45:43</dcterms:issued>
    <cc:attributionURL rdf:resource="http://www.historicengland.org.uk"/>
    <cc:license rdf:resource="http://creativecommons.org/licenses/by/3.0"/>
    <skos:narrower rdf:resource="http://purl.org/heritagedata/schemes/225/concepts/141256"/>
    <skos:narrower rdf:resource="http://purl.org/heritagedata/schemes/225/concepts/141226"/>
    <skos:inScheme rdf:resource="http://purl.org/heritagedata/schemes/225"/>
    <dcterms:identifier>http://purl.org/heritagedata/schemes/225/concepts/141131</dcterms:identifier>
    <skos:narrower rdf:resource="http://purl.org/heritagedata/schemes/225/concepts/141225"/>
  </rdf:Description>
  <rdf:Description rdf:about="http://purl.org/heritagedata/schemes/225/concepts/137235">
    <skos:broader rdf:resource="http://purl.org/heritagedata/schemes/225/concepts/111424"/>
    <cc:license rdf:resource="http://creativecommons.org/licenses/by/3.0"/>
    <cc:attributionName xml:lang="en">Historic England</cc:attributionName>
    <cc:attributionURL rdf:resource="http://www.historicengland.org.uk"/>
    <skos:inScheme rdf:resource="http://purl.org/heritagedata/schemes/225"/>
    <skos:broader rdf:resource="http://purl.org/heritagedata/schemes/225/concepts/111402"/>
    <dcterms:issued rdf:datatype="http://www.w3.org/2001/XMLSchema#dateTime">2019-03-26T16:45:43</dcterms:issued>
    <rdf:type rdf:resource="http://www.w3.org/2004/02/skos/core#Concept"/>
    <skos:scopeNote xml:lang="en">German three-engined air/sea rescue and transport flying boat. Entered service in 1940 as a replacement for the DO18.</skos:scopeNote>
    <skos:broader rdf:resource="http://purl.org/heritagedata/schemes/225/concepts/111395"/>
    <dcterms:publisher rdf:resource="http://www.historicengland.org.uk"/>
    <skos:broader rdf:resource="http://purl.org/heritagedata/schemes/225/concepts/111361"/>
    <skos:prefLabel xml:lang="en">Do24</skos:prefLabel>
    <dcterms:identifier>http://purl.org/heritagedata/schemes/225/concepts/137235</dcterms:identifier>
  </rdf:Description>
  <rdf:Description rdf:about="http://purl.org/heritagedata/schemes/225/concepts/111417">
    <dcterms:issued rdf:datatype="http://www.w3.org/2001/XMLSchema#dateTime">2019-03-26T16:45:43</dcterms:issued>
    <dcterms:publisher rdf:resource="http://www.historicengland.org.uk"/>
    <dcterms:identifier>http://purl.org/heritagedata/schemes/225/concepts/111417</dcterms:identifier>
    <cc:attributionURL rdf:resource="http://www.historicengland.org.uk"/>
    <skos:inScheme rdf:resource="http://purl.org/heritagedata/schemes/225"/>
    <skos:broader rdf:resource="http://purl.org/heritagedata/schemes/225/concepts/138507"/>
    <cc:license rdf:resource="http://creativecommons.org/licenses/by/3.0"/>
    <cc:attributionName xml:lang="en">Historic England</cc:attributionName>
    <skos:narrower rdf:resource="http://purl.org/heritagedata/schemes/225/concepts/141296"/>
    <skos:narrower rdf:resource="http://purl.org/heritagedata/schemes/225/concepts/137150"/>
    <skos:scopeNote xml:lang="en">The Consolidated Aircraft Corporation. In 1943 merged with Vultee Aircraft, Inc. to form the Consolidated Vultee Aircraft Corporation.</skos:scopeNote>
    <skos:prefLabel xml:lang="en">Consolidated</skos:prefLabel>
    <rdf:type rdf:resource="http://www.w3.org/2004/02/skos/core#Concept"/>
  </rdf:Description>
  <rdf:Description rdf:about="http://purl.org/heritagedata/schemes/225/concepts/111433">
    <cc:license rdf:resource="http://creativecommons.org/licenses/by/3.0"/>
    <cc:attributionName xml:lang="en">Historic England</cc:attributionName>
    <cc:attributionURL rdf:resource="http://www.historicengland.org.uk"/>
    <skos:inScheme rdf:resource="http://purl.org/heritagedata/schemes/225"/>
    <skos:prefLabel xml:lang="en">Boeing</skos:prefLabel>
    <dcterms:identifier>http://purl.org/heritagedata/schemes/225/concepts/111433</dcterms:identifier>
    <dcterms:issued rdf:datatype="http://www.w3.org/2001/XMLSchema#dateTime">2019-03-26T16:45:43</dcterms:issued>
    <skos:narrower rdf:resource="http://purl.org/heritagedata/schemes/225/concepts/125554"/>
    <rdf:type rdf:resource="http://www.w3.org/2004/02/skos/core#Concept"/>
    <dcterms:publisher rdf:resource="http://www.historicengland.org.uk"/>
    <skos:narrower rdf:resource="http://purl.org/heritagedata/schemes/225/concepts/141268"/>
    <skos:narrower rdf:resource="http://purl.org/heritagedata/schemes/225/concepts/125553"/>
    <skos:scopeNote xml:lang="en">The Boeing Aircraft Company, established 1916. A subsidiary of The Boeing Airplane Company. Notable aircraft produced include the B17 Flying Fortress and the B29 Superfortress.</skos:scopeNote>
    <skos:broader rdf:resource="http://purl.org/heritagedata/schemes/225/concepts/111358"/>
  </rdf:Description>
  <rdf:Description rdf:about="http://purl.org/heritagedata/schemes/225/concepts/139049">
    <skos:scopeNote xml:lang="en">An aircraft used for towing gliders aloft.</skos:scopeNote>
    <dcterms:issued rdf:datatype="http://www.w3.org/2001/XMLSchema#dateTime">2019-03-26T16:45:43</dcterms:issued>
    <skos:broader rdf:resource="http://purl.org/heritagedata/schemes/225/concepts/139053"/>
    <rdf:type rdf:resource="http://www.w3.org/2004/02/skos/core#Concept"/>
    <skos:inScheme rdf:resource="http://purl.org/heritagedata/schemes/225"/>
    <dcterms:publisher rdf:resource="http://www.historicengland.org.uk"/>
    <cc:license rdf:resource="http://creativecommons.org/licenses/by/3.0"/>
    <dcterms:identifier>http://purl.org/heritagedata/schemes/225/concepts/139049</dcterms:identifier>
    <cc:attributionURL rdf:resource="http://www.historicengland.org.uk"/>
    <skos:prefLabel xml:lang="en">Glider Tug</skos:prefLabel>
    <cc:attributionName xml:lang="en">Historic England</cc:attributionName>
  </rdf:Description>
  <rdf:Description rdf:about="http://purl.org/heritagedata/schemes/225/concepts/138541">
    <cc:license rdf:resource="http://creativecommons.org/licenses/by/3.0"/>
    <cc:attributionName xml:lang="en">Historic England</cc:attributionName>
    <cc:attributionURL rdf:resource="http://www.historicengland.org.uk"/>
    <skos:inScheme rdf:resource="http://purl.org/heritagedata/schemes/225"/>
    <skos:broader rdf:resource="http://purl.org/heritagedata/schemes/225/concepts/111357"/>
    <skos:broader rdf:resource="http://purl.org/heritagedata/schemes/225/concepts/111397"/>
    <skos:broader rdf:resource="http://purl.org/heritagedata/schemes/225/concepts/111403"/>
    <rdf:type rdf:resource="http://www.w3.org/2004/02/skos/core#Concept"/>
    <dcterms:issued rdf:datatype="http://www.w3.org/2001/XMLSchema#dateTime">2019-03-26T16:45:43</dcterms:issued>
    <dcterms:publisher rdf:resource="http://www.historicengland.org.uk"/>
    <skos:prefLabel xml:lang="en">Bristol F2B</skos:prefLabel>
    <dcterms:identifier>http://purl.org/heritagedata/schemes/225/concepts/138541</dcterms:identifier>
    <skos:broader rdf:resource="http://purl.org/heritagedata/schemes/225/concepts/135730"/>
    <skos:scopeNote xml:lang="en">Highly successful, two-seat, biplane fighter and reconnaissance aircraft with both forward and rear facing guns. Designed to replace the BE2, it entered service with the RFC in mid-1917 and remained in service until 1932.</skos:scopeNote>
  </rdf:Description>
  <rdf:Description rdf:about="http://purl.org/heritagedata/schemes/225/concepts/135730">
    <skos:narrower rdf:resource="http://purl.org/heritagedata/schemes/225/concepts/138541"/>
    <skos:narrower rdf:resource="http://purl.org/heritagedata/schemes/225/concepts/140447"/>
    <skos:narrower rdf:resource="http://purl.org/heritagedata/schemes/225/concepts/133203"/>
    <skos:narrower rdf:resource="http://purl.org/heritagedata/schemes/225/concepts/133193"/>
    <skos:narrower rdf:resource="http://purl.org/heritagedata/schemes/225/concepts/135729"/>
    <skos:narrower rdf:resource="http://purl.org/heritagedata/schemes/225/concepts/137150"/>
    <skos:narrower rdf:resource="http://purl.org/heritagedata/schemes/225/concepts/111375"/>
    <cc:attributionURL rdf:resource="http://www.historicengland.org.uk"/>
    <skos:inScheme rdf:resource="http://purl.org/heritagedata/schemes/225"/>
    <rdf:type rdf:resource="http://www.w3.org/2004/02/skos/core#Concept"/>
    <skos:narrower rdf:resource="http://purl.org/heritagedata/schemes/225/concepts/111400"/>
    <dcterms:identifier>http://purl.org/heritagedata/schemes/225/concepts/135730</dcterms:identifier>
    <skos:narrower rdf:resource="http://purl.org/heritagedata/schemes/225/concepts/138546"/>
    <skos:narrower rdf:resource="http://purl.org/heritagedata/schemes/225/concepts/138536"/>
    <skos:scopeNote xml:lang="en">An aircraft, often fitted with cameras, intended to fly over enemy territory to ascertain its strategic features and/or the position and strength of any military presence.</skos:scopeNote>
    <skos:narrower rdf:resource="http://purl.org/heritagedata/schemes/225/concepts/111442"/>
    <dcterms:publisher rdf:resource="http://www.historicengland.org.uk"/>
    <skos:broader rdf:resource="http://purl.org/heritagedata/schemes/225/concepts/111394"/>
    <skos:narrower rdf:resource="http://purl.org/heritagedata/schemes/225/concepts/141296"/>
    <skos:narrower rdf:resource="http://purl.org/heritagedata/schemes/225/concepts/140140"/>
    <dcterms:issued rdf:datatype="http://www.w3.org/2001/XMLSchema#dateTime">2019-03-26T16:45:43</dcterms:issued>
    <skos:narrower rdf:resource="http://purl.org/heritagedata/schemes/225/concepts/137236"/>
    <skos:narrower rdf:resource="http://purl.org/heritagedata/schemes/225/concepts/137234"/>
    <skos:narrower rdf:resource="http://purl.org/heritagedata/schemes/225/concepts/136525"/>
    <cc:license rdf:resource="http://creativecommons.org/licenses/by/3.0"/>
    <skos:narrower rdf:resource="http://purl.org/heritagedata/schemes/225/concepts/136510"/>
    <skos:narrower rdf:resource="http://purl.org/heritagedata/schemes/225/concepts/137208"/>
    <skos:narrower rdf:resource="http://purl.org/heritagedata/schemes/225/concepts/136610"/>
    <skos:prefLabel xml:lang="en">Reconnaissance</skos:prefLabel>
    <skos:narrower rdf:resource="http://purl.org/heritagedata/schemes/225/concepts/136591"/>
    <skos:narrower rdf:resource="http://purl.org/heritagedata/schemes/225/concepts/137130"/>
    <skos:narrower rdf:resource="http://purl.org/heritagedata/schemes/225/concepts/136251"/>
    <skos:narrower rdf:resource="http://purl.org/heritagedata/schemes/225/concepts/137195"/>
    <skos:narrower rdf:resource="http://purl.org/heritagedata/schemes/225/concepts/137239"/>
    <skos:narrower rdf:resource="http://purl.org/heritagedata/schemes/225/concepts/134952"/>
    <skos:narrower rdf:resource="http://purl.org/heritagedata/schemes/225/concepts/136250"/>
    <skos:narrower rdf:resource="http://purl.org/heritagedata/schemes/225/concepts/138538"/>
    <cc:attributionName xml:lang="en">Historic England</cc:attributionName>
    <skos:narrower rdf:resource="http://purl.org/heritagedata/schemes/225/concepts/134996"/>
    <skos:narrower rdf:resource="http://purl.org/heritagedata/schemes/225/concepts/138539"/>
  </rdf:Description>
  <rdf:Description rdf:about="http://purl.org/heritagedata/schemes/225/concepts/125518">
    <cc:attributionName xml:lang="en">Historic England</cc:attributionName>
    <skos:inScheme rdf:resource="http://purl.org/heritagedata/schemes/225"/>
    <dcterms:identifier>http://purl.org/heritagedata/schemes/225/concepts/125518</dcterms:identifier>
    <skos:broader rdf:resource="http://purl.org/heritagedata/schemes/225/concepts/125614"/>
    <skos:broader rdf:resource="http://purl.org/heritagedata/schemes/225/concepts/111397"/>
    <cc:license rdf:resource="http://creativecommons.org/licenses/by/3.0"/>
    <cc:attributionURL rdf:resource="http://www.historicengland.org.uk"/>
    <skos:prefLabel xml:lang="en">Lightning</skos:prefLabel>
    <skos:scopeNote xml:lang="en">Twin-engined jet-fighter. The first British aircraft to exceed Mach 1 in level flight, later to exceed Mach 2. Entered service in 1960. After 13 years was superseded in its primary defence role by the Phantom, though remained in RAF service until 1988.</skos:scopeNote>
    <rdf:type rdf:resource="http://www.w3.org/2004/02/skos/core#Concept"/>
    <skos:broader rdf:resource="http://purl.org/heritagedata/schemes/225/concepts/111402"/>
    <dcterms:issued rdf:datatype="http://www.w3.org/2001/XMLSchema#dateTime">2019-03-26T16:45:43</dcterms:issued>
    <dcterms:publisher rdf:resource="http://www.historicengland.org.uk"/>
  </rdf:Description>
  <rdf:Description rdf:about="http://purl.org/heritagedata/schemes/225/concepts/111394">
    <skos:narrower rdf:resource="http://purl.org/heritagedata/schemes/225/concepts/111424"/>
    <cc:license rdf:resource="http://creativecommons.org/licenses/by/3.0"/>
    <skos:narrower rdf:resource="http://purl.org/heritagedata/schemes/225/concepts/135851"/>
    <skos:narrower rdf:resource="http://purl.org/heritagedata/schemes/225/concepts/133208"/>
    <skos:inScheme rdf:resource="http://purl.org/heritagedata/schemes/225"/>
    <skos:narrower rdf:resource="http://purl.org/heritagedata/schemes/225/concepts/139053"/>
    <skos:narrower rdf:resource="http://purl.org/heritagedata/schemes/225/concepts/140074"/>
    <rdf:type rdf:resource="http://www.w3.org/2004/02/skos/core#Concept"/>
    <skos:narrower rdf:resource="http://purl.org/heritagedata/schemes/225/concepts/141359"/>
    <dcterms:issued rdf:datatype="http://www.w3.org/2001/XMLSchema#dateTime">2019-03-26T16:45:43</dcterms:issued>
    <cc:attributionURL rdf:resource="http://www.historicengland.org.uk"/>
    <skos:narrower rdf:resource="http://purl.org/heritagedata/schemes/225/concepts/141497"/>
    <skos:narrower rdf:resource="http://purl.org/heritagedata/schemes/225/concepts/135730"/>
    <cc:attributionName xml:lang="en">Historic England</cc:attributionName>
    <dcterms:publisher rdf:resource="http://www.historicengland.org.uk"/>
    <skos:broader rdf:resource="http://purl.org/heritagedata/schemes/225/concepts/123733"/>
    <dcterms:identifier>http://purl.org/heritagedata/schemes/225/concepts/111394</dcterms:identifier>
    <skos:narrower rdf:resource="http://purl.org/heritagedata/schemes/225/concepts/111401"/>
    <skos:prefLabel xml:lang="en">Aircraft &lt;By Function&gt;</skos:prefLabel>
    <skos:narrower rdf:resource="http://purl.org/heritagedata/schemes/225/concepts/111398"/>
    <skos:narrower rdf:resource="http://purl.org/heritagedata/schemes/225/concepts/111397"/>
    <skos:narrower rdf:resource="http://purl.org/heritagedata/schemes/225/concepts/136031"/>
    <skos:scopeNote xml:lang="en">Aircraft grouped according to their function.</skos:scopeNote>
  </rdf:Description>
  <rdf:Description rdf:about="http://purl.org/heritagedata/schemes/225/concepts/118653">
    <skos:prefLabel xml:lang="en">Messerschmitt</skos:prefLabel>
    <cc:attributionName xml:lang="en">Historic England</cc:attributionName>
    <skos:narrower rdf:resource="http://purl.org/heritagedata/schemes/225/concepts/111333"/>
    <skos:inScheme rdf:resource="http://purl.org/heritagedata/schemes/225"/>
    <skos:scopeNote xml:lang="en">Founded by Professor Willy Messerschmitt as the Bayerische Flugzeugwerke. Reconstituted in 1938 as the Messerschmitt A.G..</skos:scopeNote>
    <dcterms:publisher rdf:resource="http://www.historicengland.org.uk"/>
    <cc:attributionURL rdf:resource="http://www.historicengland.org.uk"/>
    <rdf:type rdf:resource="http://www.w3.org/2004/02/skos/core#Concept"/>
    <skos:narrower rdf:resource="http://purl.org/heritagedata/schemes/225/concepts/137238"/>
    <skos:narrower rdf:resource="http://purl.org/heritagedata/schemes/225/concepts/133202"/>
    <skos:narrower rdf:resource="http://purl.org/heritagedata/schemes/225/concepts/111373"/>
    <cc:license rdf:resource="http://creativecommons.org/licenses/by/3.0"/>
    <dcterms:identifier>http://purl.org/heritagedata/schemes/225/concepts/118653</dcterms:identifier>
    <skos:broader rdf:resource="http://purl.org/heritagedata/schemes/225/concepts/111358"/>
    <dcterms:issued rdf:datatype="http://www.w3.org/2001/XMLSchema#dateTime">2019-03-26T16:45:43</dcterms:issued>
  </rdf:Description>
  <rdf:Description rdf:about="http://purl.org/heritagedata/schemes/225/concepts/133200">
    <dcterms:publisher rdf:resource="http://www.historicengland.org.uk"/>
    <rdf:type rdf:resource="http://www.w3.org/2004/02/skos/core#Concept"/>
    <skos:narrower rdf:resource="http://purl.org/heritagedata/schemes/225/concepts/167003"/>
    <skos:narrower rdf:resource="http://purl.org/heritagedata/schemes/225/concepts/133201"/>
    <cc:license rdf:resource="http://creativecommons.org/licenses/by/3.0"/>
    <cc:attributionURL rdf:resource="http://www.historicengland.org.uk"/>
    <dcterms:issued rdf:datatype="http://www.w3.org/2001/XMLSchema#dateTime">2019-03-26T16:45:43</dcterms:issued>
    <skos:prefLabel xml:lang="en">Airspeed</skos:prefLabel>
    <dcterms:identifier>http://purl.org/heritagedata/schemes/225/concepts/133200</dcterms:identifier>
    <skos:broader rdf:resource="http://purl.org/heritagedata/schemes/225/concepts/111358"/>
    <skos:narrower rdf:resource="http://purl.org/heritagedata/schemes/225/concepts/137111"/>
    <cc:attributionName xml:lang="en">Historic England</cc:attributionName>
    <skos:inScheme rdf:resource="http://purl.org/heritagedata/schemes/225"/>
    <skos:scopeNote xml:lang="en">Airspeed (1934) Ltd. registered in 1934 when associated with shipbuilders Swan, Hunter and Wigham Richardson Ltd.. Acquired by de Havilland in 1940, maintaining own identity and changing name to Airspeed Ltd. in 1944.</skos:scopeNote>
  </rdf:Description>
  <rdf:Description rdf:about="http://purl.org/heritagedata/schemes/225/concepts/111441">
    <cc:license rdf:resource="http://creativecommons.org/licenses/by/3.0"/>
    <cc:attributionURL rdf:resource="http://www.historicengland.org.uk"/>
    <skos:prefLabel xml:lang="en">Fairey</skos:prefLabel>
    <skos:scopeNote xml:lang="en">The Fairey Aviation Co. Ltd., established 1916 by Sir Richard Fairey. During WW2 formed a group production scheme with Blackburn Aircraft, Ltd. and Boulton Paul Aircraft, Ltd..</skos:scopeNote>
    <skos:narrower rdf:resource="http://purl.org/heritagedata/schemes/225/concepts/137199"/>
    <skos:narrower rdf:resource="http://purl.org/heritagedata/schemes/225/concepts/111443"/>
    <skos:inScheme rdf:resource="http://purl.org/heritagedata/schemes/225"/>
    <dcterms:identifier>http://purl.org/heritagedata/schemes/225/concepts/111441</dcterms:identifier>
    <skos:broader rdf:resource="http://purl.org/heritagedata/schemes/225/concepts/111358"/>
    <skos:narrower rdf:resource="http://purl.org/heritagedata/schemes/225/concepts/140065"/>
    <skos:narrower rdf:resource="http://purl.org/heritagedata/schemes/225/concepts/137198"/>
    <skos:narrower rdf:resource="http://purl.org/heritagedata/schemes/225/concepts/139374"/>
    <skos:narrower rdf:resource="http://purl.org/heritagedata/schemes/225/concepts/137197"/>
    <skos:narrower rdf:resource="http://purl.org/heritagedata/schemes/225/concepts/111442"/>
    <dcterms:publisher rdf:resource="http://www.historicengland.org.uk"/>
    <cc:attributionName xml:lang="en">Historic England</cc:attributionName>
    <skos:narrower rdf:resource="http://purl.org/heritagedata/schemes/225/concepts/140411"/>
    <skos:narrower rdf:resource="http://purl.org/heritagedata/schemes/225/concepts/137192"/>
    <dcterms:issued rdf:datatype="http://www.w3.org/2001/XMLSchema#dateTime">2019-03-26T16:45:43</dcterms:issued>
    <rdf:type rdf:resource="http://www.w3.org/2004/02/skos/core#Concept"/>
  </rdf:Description>
  <rdf:Description rdf:about="http://purl.org/heritagedata/schemes/225/concepts/111420">
    <dcterms:issued rdf:datatype="http://www.w3.org/2001/XMLSchema#dateTime">2019-03-26T16:45:43</dcterms:issued>
    <skos:inScheme rdf:resource="http://purl.org/heritagedata/schemes/225"/>
    <cc:attributionURL rdf:resource="http://www.historicengland.org.uk"/>
    <skos:broader rdf:resource="http://purl.org/heritagedata/schemes/225/concepts/138508"/>
    <dcterms:identifier>http://purl.org/heritagedata/schemes/225/concepts/111420</dcterms:identifier>
    <cc:attributionName xml:lang="en">Historic England</cc:attributionName>
    <cc:license rdf:resource="http://creativecommons.org/licenses/by/3.0"/>
    <skos:prefLabel xml:lang="en">Vickers</skos:prefLabel>
    <dcterms:publisher rdf:resource="http://www.historicengland.org.uk"/>
    <skos:narrower rdf:resource="http://purl.org/heritagedata/schemes/225/concepts/137130"/>
    <skos:narrower rdf:resource="http://purl.org/heritagedata/schemes/225/concepts/136234"/>
    <skos:narrower rdf:resource="http://purl.org/heritagedata/schemes/225/concepts/111419"/>
    <skos:narrower rdf:resource="http://purl.org/heritagedata/schemes/225/concepts/140424"/>
    <rdf:type rdf:resource="http://www.w3.org/2004/02/skos/core#Concept"/>
    <skos:scopeNote xml:lang="en">Vickers (Aviation) Ltd. formed in 1911, as the aviation division of Vickers Ltd., and took control of Supermarine Aviation Works Ltd. the same year. Taken over by Vickers-Armstrongs Ltd. in 1938.</skos:scopeNote>
  </rdf:Description>
  <rdf:Description rdf:about="http://purl.org/heritagedata/schemes/225/concepts/111362">
    <skos:scopeNote xml:lang="en">Junkers Flugzeug und Motorenwerke, A.G.. Formed in 1910 with Professor Junkers being granted a patent for an all-wing aeroplane. Produced first successful all-metal aeroplane, the Junkers J1, in 1915.</skos:scopeNote>
    <dcterms:issued rdf:datatype="http://www.w3.org/2001/XMLSchema#dateTime">2019-03-26T16:45:43</dcterms:issued>
    <skos:prefLabel xml:lang="en">Junkers</skos:prefLabel>
    <skos:inScheme rdf:resource="http://purl.org/heritagedata/schemes/225"/>
    <cc:attributionURL rdf:resource="http://www.historicengland.org.uk"/>
    <skos:narrower rdf:resource="http://purl.org/heritagedata/schemes/225/concepts/111364"/>
    <skos:narrower rdf:resource="http://purl.org/heritagedata/schemes/225/concepts/137239"/>
    <cc:attributionName xml:lang="en">Historic England</cc:attributionName>
    <skos:narrower rdf:resource="http://purl.org/heritagedata/schemes/225/concepts/134952"/>
    <skos:broader rdf:resource="http://purl.org/heritagedata/schemes/225/concepts/111358"/>
    <rdf:type rdf:resource="http://www.w3.org/2004/02/skos/core#Concept"/>
    <dcterms:publisher rdf:resource="http://www.historicengland.org.uk"/>
    <dcterms:identifier>http://purl.org/heritagedata/schemes/225/concepts/111362</dcterms:identifier>
    <skos:narrower rdf:resource="http://purl.org/heritagedata/schemes/225/concepts/111363"/>
    <cc:license rdf:resource="http://creativecommons.org/licenses/by/3.0"/>
  </rdf:Description>
  <rdf:Description rdf:about="http://purl.org/heritagedata/schemes/225/concepts/141133">
    <skos:altLabel xml:lang="en">Mk1</skos:altLabel>
  </rdf:Description>
  <rdf:Description rdf:about="http://purl.org/heritagedata/schemes/225/concepts/137225">
    <skos:prefLabel xml:lang="en">Vultee</skos:prefLabel>
    <skos:scopeNote xml:lang="en">Vultee Aircraft, Inc.. In 1943 merged with The Consolidated Aircraft Corporation to form The Consolidated Vultee Aircraft Corporation.</skos:scopeNote>
    <dcterms:issued rdf:datatype="http://www.w3.org/2001/XMLSchema#dateTime">2019-03-26T16:45:43</dcterms:issued>
    <skos:broader rdf:resource="http://purl.org/heritagedata/schemes/225/concepts/138507"/>
    <cc:attributionURL rdf:resource="http://www.historicengland.org.uk"/>
    <rdf:type rdf:resource="http://www.w3.org/2004/02/skos/core#Concept"/>
    <dcterms:identifier>http://purl.org/heritagedata/schemes/225/concepts/137225</dcterms:identifier>
    <cc:license rdf:resource="http://creativecommons.org/licenses/by/3.0"/>
    <skos:inScheme rdf:resource="http://purl.org/heritagedata/schemes/225"/>
    <skos:narrower rdf:resource="http://purl.org/heritagedata/schemes/225/concepts/137226"/>
    <dcterms:publisher rdf:resource="http://www.historicengland.org.uk"/>
    <cc:attributionName xml:lang="en">Historic England</cc:attributionName>
  </rdf:Description>
  <rdf:Description rdf:about="http://purl.org/heritagedata/schemes/225/concepts/135606">
    <rdf:type rdf:resource="http://www.w3.org/2004/02/skos/core#Concept"/>
    <dcterms:issued rdf:datatype="http://www.w3.org/2001/XMLSchema#dateTime">2019-03-26T16:45:43</dcterms:issued>
    <dcterms:publisher rdf:resource="http://www.historicengland.org.uk"/>
    <dcterms:identifier>http://purl.org/heritagedata/schemes/225/concepts/135606</dcterms:identifier>
    <skos:scopeNote xml:lang="en">Post-World War Two, single-engine, high-wing utility transport. Manufactured by De Havilland Canada, was also produced in a seaplane version. Known as the U6A from 1962.</skos:scopeNote>
    <skos:broader rdf:resource="http://purl.org/heritagedata/schemes/225/concepts/111424"/>
    <skos:prefLabel xml:lang="en">L20A Beaver</skos:prefLabel>
    <skos:broader rdf:resource="http://purl.org/heritagedata/schemes/225/concepts/111368"/>
    <cc:license rdf:resource="http://creativecommons.org/licenses/by/3.0"/>
    <cc:attributionName xml:lang="en">Historic England</cc:attributionName>
    <cc:attributionURL rdf:resource="http://www.historicengland.org.uk"/>
    <skos:inScheme rdf:resource="http://purl.org/heritagedata/schemes/225"/>
    <skos:broader rdf:resource="http://purl.org/heritagedata/schemes/225/concepts/111402"/>
  </rdf:Description>
  <rdf:Description rdf:about="http://purl.org/heritagedata/schemes/225/concepts/141254">
    <cc:attributionURL rdf:resource="http://www.historicengland.org.uk"/>
    <rdf:type rdf:resource="http://www.w3.org/2004/02/skos/core#Concept"/>
    <cc:attributionName xml:lang="en">Historic England</cc:attributionName>
    <cc:license rdf:resource="http://creativecommons.org/licenses/by/3.0"/>
    <skos:prefLabel xml:lang="en">MkXII</skos:prefLabel>
    <skos:broader rdf:resource="http://purl.org/heritagedata/schemes/225/concepts/141131"/>
    <skos:scopeNote xml:lang="en">Mark 12 or the twelfth variant of an aircraft with its associated modifications.</skos:scopeNote>
    <dcterms:identifier>http://purl.org/heritagedata/schemes/225/concepts/141254</dcterms:identifier>
    <dcterms:publisher rdf:resource="http://www.historicengland.org.uk"/>
    <dcterms:issued rdf:datatype="http://www.w3.org/2001/XMLSchema#dateTime">2019-03-26T16:45:43</dcterms:issued>
    <skos:inScheme rdf:resource="http://purl.org/heritagedata/schemes/225"/>
  </rdf:Description>
  <rdf:Description rdf:about="http://purl.org/heritagedata/schemes/225/concepts/167004">
    <cc:attributionURL rdf:resource="http://www.historicengland.org.uk"/>
    <rdf:type rdf:resource="http://www.w3.org/2004/02/skos/core#Concept"/>
    <skos:broader rdf:resource="http://purl.org/heritagedata/schemes/225/concepts/111397"/>
    <cc:license rdf:resource="http://creativecommons.org/licenses/by/3.0"/>
    <dcterms:identifier>http://purl.org/heritagedata/schemes/225/concepts/167004</dcterms:identifier>
    <skos:broader rdf:resource="http://purl.org/heritagedata/schemes/225/concepts/125513"/>
    <skos:scopeNote xml:lang="en">A transonic jet fighter, first introduced by North American Aviation in 1947. Best known as the United States's first swept wing fighter. Total production at 9,860 units. Important fighter aircraft in the Korean War. Retired in 1994 (Bolivia).</skos:scopeNote>
    <dcterms:publisher rdf:resource="http://www.historicengland.org.uk"/>
    <cc:attributionName xml:lang="en">Historic England</cc:attributionName>
    <skos:prefLabel xml:lang="en">F86 Sabre</skos:prefLabel>
    <skos:inScheme rdf:resource="http://purl.org/heritagedata/schemes/225"/>
    <dcterms:issued rdf:datatype="http://www.w3.org/2001/XMLSchema#dateTime">2019-03-26T16:45:43</dcterms:issued>
    <skos:broader rdf:resource="http://purl.org/heritagedata/schemes/225/concepts/111402"/>
  </rdf:Description>
  <rdf:Description rdf:about="http://purl.org/heritagedata/schemes/225/concepts/111421">
    <skos:inScheme rdf:resource="http://purl.org/heritagedata/schemes/225"/>
    <dcterms:issued rdf:datatype="http://www.w3.org/2001/XMLSchema#dateTime">2019-03-26T16:45:43</dcterms:issued>
    <skos:narrower rdf:resource="http://purl.org/heritagedata/schemes/225/concepts/135729"/>
    <skos:narrower rdf:resource="http://purl.org/heritagedata/schemes/225/concepts/111422"/>
    <skos:broader rdf:resource="http://purl.org/heritagedata/schemes/225/concepts/111358"/>
    <cc:license rdf:resource="http://creativecommons.org/licenses/by/3.0"/>
    <cc:attributionURL rdf:resource="http://www.historicengland.org.uk"/>
    <rdf:type rdf:resource="http://www.w3.org/2004/02/skos/core#Concept"/>
    <dcterms:identifier>http://purl.org/heritagedata/schemes/225/concepts/111421</dcterms:identifier>
    <skos:prefLabel xml:lang="en">Short</skos:prefLabel>
    <skos:scopeNote xml:lang="en">Short Bros. (Rochester &amp; Bedford), Ltd. founded by Eustace and Oswald Short in 1898, originally manufacturing spherical balloons. In 1936 became Short &amp; Harland Ltd. in collaboration with Belfast shipbuilders Harland and Wolff.</skos:scopeNote>
    <dcterms:publisher rdf:resource="http://www.historicengland.org.uk"/>
    <cc:attributionName xml:lang="en">Historic England</cc:attributionName>
  </rdf:Description>
  <rdf:Description rdf:about="http://purl.org/heritagedata/schemes/225/concepts/136233">
    <skos:broader rdf:resource="http://purl.org/heritagedata/schemes/225/concepts/111397"/>
    <cc:license rdf:resource="http://creativecommons.org/licenses/by/3.0"/>
    <ns1:related rdf:resource="http://purl.org/heritagedata/schemes/225/concepts/140416"/>
    <skos:scopeNote xml:lang="en">Single-engined fighter, developed from the Camel. Entered service in 1918 and became the RAF's first mainstay peacetime fighter.</skos:scopeNote>
    <dcterms:identifier>http://purl.org/heritagedata/schemes/225/concepts/136233</dcterms:identifier>
    <dcterms:publisher rdf:resource="http://www.historicengland.org.uk"/>
    <cc:attributionURL rdf:resource="http://www.historicengland.org.uk"/>
    <skos:inScheme rdf:resource="http://purl.org/heritagedata/schemes/225"/>
    <cc:attributionName xml:lang="en">Historic England</cc:attributionName>
    <skos:prefLabel xml:lang="en">Snipe</skos:prefLabel>
    <skos:broader rdf:resource="http://purl.org/heritagedata/schemes/225/concepts/136232"/>
    <rdf:type rdf:resource="http://www.w3.org/2004/02/skos/core#Concept"/>
    <dcterms:issued rdf:datatype="http://www.w3.org/2001/XMLSchema#dateTime">2019-03-26T16:45:43</dcterms:issued>
    <skos:broader rdf:resource="http://purl.org/heritagedata/schemes/225/concepts/111403"/>
  </rdf:Description>
  <rdf:Description rdf:about="http://purl.org/heritagedata/schemes/225/concepts/111355">
    <cc:license rdf:resource="http://creativecommons.org/licenses/by/3.0"/>
    <skos:inScheme rdf:resource="http://purl.org/heritagedata/schemes/225"/>
    <skos:narrower rdf:resource="http://purl.org/heritagedata/schemes/225/concepts/111367"/>
    <skos:narrower rdf:resource="http://purl.org/heritagedata/schemes/225/concepts/125573"/>
    <skos:narrower rdf:resource="http://purl.org/heritagedata/schemes/225/concepts/136524"/>
    <skos:narrower rdf:resource="http://purl.org/heritagedata/schemes/225/concepts/169971"/>
    <skos:scopeNote xml:lang="en">A. V. Roe &amp; Co., Ltd. formed in 1909. A subsidiary  of the Hawker Siddeley Aircraft Co., Ltd. from 1935, having formerly been a member of the Siddeley group. Produced such notable aircraft as the Lancaster, the York and the Anson.</skos:scopeNote>
    <skos:narrower rdf:resource="http://purl.org/heritagedata/schemes/225/concepts/136525"/>
    <dcterms:issued rdf:datatype="http://www.w3.org/2001/XMLSchema#dateTime">2019-03-26T16:45:43</dcterms:issued>
    <cc:attributionURL rdf:resource="http://www.historicengland.org.uk"/>
    <dcterms:identifier>http://purl.org/heritagedata/schemes/225/concepts/111355</dcterms:identifier>
    <skos:narrower rdf:resource="http://purl.org/heritagedata/schemes/225/concepts/133193"/>
    <cc:attributionName xml:lang="en">Historic England</cc:attributionName>
    <dcterms:publisher rdf:resource="http://www.historicengland.org.uk"/>
    <skos:narrower rdf:resource="http://purl.org/heritagedata/schemes/225/concepts/138540"/>
    <skos:narrower rdf:resource="http://purl.org/heritagedata/schemes/225/concepts/136526"/>
    <skos:prefLabel xml:lang="en">Avro</skos:prefLabel>
    <skos:broader rdf:resource="http://purl.org/heritagedata/schemes/225/concepts/111358"/>
    <skos:narrower rdf:resource="http://purl.org/heritagedata/schemes/225/concepts/136220"/>
    <skos:narrower rdf:resource="http://purl.org/heritagedata/schemes/225/concepts/137193"/>
    <rdf:type rdf:resource="http://www.w3.org/2004/02/skos/core#Concept"/>
  </rdf:Description>
  <rdf:Description rdf:about="http://purl.org/heritagedata/schemes/225">
    <dcterms:identifier>http://purl.org/heritagedata/schemes/225</dcterms:identifier>
    <skos:hasTopConcept rdf:resource="http://purl.org/heritagedata/schemes/225/concepts/123733"/>
    <cc:attributionName xml:lang="en">Historic England</cc:attributionName>
    <dcterms:publisher rdf:resource="http://www.historicengland.org.uk"/>
    <dcterms:description xml:lang="en">Indexing terminology for the recording of aircraft remains and crash sites, listing aircraft types by form (eg. Monoplane, Biplane), function (eg. Fighter, Bomber) and manufacturer (e.g. Atlas, Target, Westland).</dcterms:description>
    <rdf:type rdf:resource="http://www.w3.org/2004/02/skos/core#ConceptScheme"/>
    <cc:license rdf:resource="http://creativecommons.org/licenses/by/3.0"/>
    <cc:attributionURL rdf:resource="http://www.historicengland.org.uk"/>
    <dcterms:issued rdf:datatype="http://www.w3.org/2001/XMLSchema#date">2019-03-26</dcterms:issued>
    <dcterms:title xml:lang="en">FISH Historic Aircraft Type</dcterms:title>
  </rdf:Description>
  <rdf:Description rdf:about="http://purl.org/heritagedata/schemes/225/concepts/125513">
    <rdf:type rdf:resource="http://www.w3.org/2004/02/skos/core#Concept"/>
    <skos:narrower rdf:resource="http://purl.org/heritagedata/schemes/225/concepts/111435"/>
    <skos:narrower rdf:resource="http://purl.org/heritagedata/schemes/225/concepts/167004"/>
    <skos:narrower rdf:resource="http://purl.org/heritagedata/schemes/225/concepts/125514"/>
    <cc:license rdf:resource="http://creativecommons.org/licenses/by/3.0"/>
    <cc:attributionName xml:lang="en">Historic England</cc:attributionName>
    <cc:attributionURL rdf:resource="http://www.historicengland.org.uk"/>
    <skos:inScheme rdf:resource="http://purl.org/heritagedata/schemes/225"/>
    <skos:prefLabel xml:lang="en">North American</skos:prefLabel>
    <dcterms:issued rdf:datatype="http://www.w3.org/2001/XMLSchema#dateTime">2019-03-26T16:45:43</dcterms:issued>
    <skos:scopeNote xml:lang="en">North American Aviation, Inc., incorporated in Delaware in 1928.</skos:scopeNote>
    <dcterms:publisher rdf:resource="http://www.historicengland.org.uk"/>
    <dcterms:identifier>http://purl.org/heritagedata/schemes/225/concepts/125513</dcterms:identifier>
    <skos:broader rdf:resource="http://purl.org/heritagedata/schemes/225/concepts/111358"/>
    <skos:narrower rdf:resource="http://purl.org/heritagedata/schemes/225/concepts/133204"/>
  </rdf:Description>
  <rdf:Description rdf:about="http://purl.org/heritagedata/schemes/225/concepts/135932">
    <dcterms:publisher rdf:resource="http://www.historicengland.org.uk"/>
    <skos:broader rdf:resource="http://purl.org/heritagedata/schemes/225/concepts/111402"/>
    <rdf:type rdf:resource="http://www.w3.org/2004/02/skos/core#Concept"/>
    <skos:prefLabel xml:lang="en">Lysander</skos:prefLabel>
    <dcterms:issued rdf:datatype="http://www.w3.org/2001/XMLSchema#dateTime">2019-03-26T16:45:43</dcterms:issued>
    <skos:inScheme rdf:resource="http://purl.org/heritagedata/schemes/225"/>
    <cc:attributionURL rdf:resource="http://www.historicengland.org.uk"/>
    <skos:scopeNote xml:lang="en">Single-engine, two-crew multi-role aircraft designed for RAF Army co-operation. Entered RAF service in 1938. Noted for its role dropping agents into Europe, also served as a night-fighter, day ground-attack aircraft and target tug.</skos:scopeNote>
    <skos:broader rdf:resource="http://purl.org/heritagedata/schemes/225/concepts/135930"/>
    <cc:attributionName xml:lang="en">Historic England</cc:attributionName>
    <cc:license rdf:resource="http://creativecommons.org/licenses/by/3.0"/>
    <dcterms:identifier>http://purl.org/heritagedata/schemes/225/concepts/135932</dcterms:identifier>
  </rdf:Description>
  <rdf:Description rdf:about="http://purl.org/heritagedata/schemes/225/concepts/139374">
    <dcterms:identifier>http://purl.org/heritagedata/schemes/225/concepts/139374</dcterms:identifier>
    <skos:broader rdf:resource="http://purl.org/heritagedata/schemes/225/concepts/111403"/>
    <rdf:type rdf:resource="http://www.w3.org/2004/02/skos/core#Concept"/>
    <dcterms:issued rdf:datatype="http://www.w3.org/2001/XMLSchema#dateTime">2019-03-26T16:45:43</dcterms:issued>
    <dcterms:publisher rdf:resource="http://www.historicengland.org.uk"/>
    <skos:broader rdf:resource="http://purl.org/heritagedata/schemes/225/concepts/137189"/>
    <cc:attributionName xml:lang="en">Historic England</cc:attributionName>
    <cc:license rdf:resource="http://creativecommons.org/licenses/by/3.0"/>
    <skos:inScheme rdf:resource="http://purl.org/heritagedata/schemes/225"/>
    <skos:prefLabel xml:lang="en">Fawn</skos:prefLabel>
    <skos:broader rdf:resource="http://purl.org/heritagedata/schemes/225/concepts/111441"/>
    <skos:scopeNote xml:lang="en">British, single-engined, light day bomber biplane. Built in 1923, this was the RAF's first interbellum designed day bomber.</skos:scopeNote>
    <cc:attributionURL rdf:resource="http://www.historicengland.org.uk"/>
  </rdf:Description>
  <rdf:Description rdf:about="http://purl.org/heritagedata/schemes/225/concepts/140097">
    <cc:attributionURL rdf:resource="http://www.historicengland.org.uk"/>
    <skos:broader rdf:resource="http://purl.org/heritagedata/schemes/225/concepts/111358"/>
    <rdf:type rdf:resource="http://www.w3.org/2004/02/skos/core#Concept"/>
    <dcterms:publisher rdf:resource="http://www.historicengland.org.uk"/>
    <cc:attributionName xml:lang="en">Historic England</cc:attributionName>
    <dcterms:issued rdf:datatype="http://www.w3.org/2001/XMLSchema#dateTime">2019-03-26T16:45:43</dcterms:issued>
    <skos:inScheme rdf:resource="http://purl.org/heritagedata/schemes/225"/>
    <dcterms:identifier>http://purl.org/heritagedata/schemes/225/concepts/140097</dcterms:identifier>
    <skos:prefLabel xml:lang="en">Gotha</skos:prefLabel>
    <skos:scopeNote xml:lang="en">Gothauer Waggonfabrik A.G., based in Gotha, Thuringia (Germany). During World War 2 produced mostly training and light commercial aircraft and troop and freight-carrying gliders.</skos:scopeNote>
    <skos:narrower rdf:resource="http://purl.org/heritagedata/schemes/225/concepts/140095"/>
    <cc:license rdf:resource="http://creativecommons.org/licenses/by/3.0"/>
  </rdf:Description>
  <rdf:Description rdf:about="http://purl.org/heritagedata/schemes/225/concepts/137227">
    <skos:scopeNote xml:lang="en">The Waco Aircraft Company, established in 1921. One of the largest pre-war producers of civil aircraft in America, Waco specialised in the production of troop and cargo carrying gliders during World War Two.</skos:scopeNote>
    <skos:narrower rdf:resource="http://purl.org/heritagedata/schemes/225/concepts/137228"/>
    <skos:broader rdf:resource="http://purl.org/heritagedata/schemes/225/concepts/111358"/>
    <dcterms:publisher rdf:resource="http://www.historicengland.org.uk"/>
    <dcterms:identifier>http://purl.org/heritagedata/schemes/225/concepts/137227</dcterms:identifier>
    <rdf:type rdf:resource="http://www.w3.org/2004/02/skos/core#Concept"/>
    <cc:attributionName xml:lang="en">Historic England</cc:attributionName>
    <cc:license rdf:resource="http://creativecommons.org/licenses/by/3.0"/>
    <skos:inScheme rdf:resource="http://purl.org/heritagedata/schemes/225"/>
    <cc:attributionURL rdf:resource="http://www.historicengland.org.uk"/>
    <dcterms:issued rdf:datatype="http://www.w3.org/2001/XMLSchema#dateTime">2019-03-26T16:45:43</dcterms:issued>
    <skos:prefLabel xml:lang="en">Waco</skos:prefLabel>
  </rdf:Description>
  <rdf:Description rdf:about="http://purl.org/heritagedata/schemes/225/concepts/137198">
    <skos:inScheme rdf:resource="http://purl.org/heritagedata/schemes/225"/>
    <skos:prefLabel xml:lang="en">Barracuda</skos:prefLabel>
    <skos:broader rdf:resource="http://purl.org/heritagedata/schemes/225/concepts/111441"/>
    <dcterms:identifier>http://purl.org/heritagedata/schemes/225/concepts/137198</dcterms:identifier>
    <skos:scopeNote xml:lang="en">British multi-purpose, single-engined monoplane that served as a torpedo-bomber, dive-bomber, reconnaissance aircraft and in other roles. Equipped with folding wings for use aboard aircraft carriers.</skos:scopeNote>
    <cc:license rdf:resource="http://creativecommons.org/licenses/by/3.0"/>
    <cc:attributionURL rdf:resource="http://www.historicengland.org.uk"/>
    <skos:broader rdf:resource="http://purl.org/heritagedata/schemes/225/concepts/111402"/>
    <rdf:type rdf:resource="http://www.w3.org/2004/02/skos/core#Concept"/>
    <dcterms:issued rdf:datatype="http://www.w3.org/2001/XMLSchema#dateTime">2019-03-26T16:45:43</dcterms:issued>
    <dcterms:publisher rdf:resource="http://www.historicengland.org.uk"/>
    <cc:attributionName xml:lang="en">Historic England</cc:attributionName>
  </rdf:Description>
  <rdf:Description rdf:about="http://purl.org/heritagedata/schemes/225/concepts/111356">
    <skos:broader rdf:resource="http://purl.org/heritagedata/schemes/225/concepts/111358"/>
    <dcterms:publisher rdf:resource="http://www.historicengland.org.uk"/>
    <dcterms:identifier>http://purl.org/heritagedata/schemes/225/concepts/111356</dcterms:identifier>
    <skos:prefLabel xml:lang="en">Heinkel</skos:prefLabel>
    <rdf:type rdf:resource="http://www.w3.org/2004/02/skos/core#Concept"/>
    <cc:license rdf:resource="http://creativecommons.org/licenses/by/3.0"/>
    <skos:narrower rdf:resource="http://purl.org/heritagedata/schemes/225/concepts/134996"/>
    <dcterms:issued rdf:datatype="http://www.w3.org/2001/XMLSchema#dateTime">2019-03-26T16:45:43</dcterms:issued>
    <cc:attributionURL rdf:resource="http://www.historicengland.org.uk"/>
    <skos:scopeNote xml:lang="en">Ernst Heinkel A.G.. Formed in 1922 by Dr. Ernst Heinkel, previously Chief Designer with Hansa-Brandenburgische Flugzeugwerke, where he produced many notable seaplanes during World War One.</skos:scopeNote>
    <skos:narrower rdf:resource="http://purl.org/heritagedata/schemes/225/concepts/140140"/>
    <cc:attributionName xml:lang="en">Historic England</cc:attributionName>
    <skos:inScheme rdf:resource="http://purl.org/heritagedata/schemes/225"/>
    <skos:narrower rdf:resource="http://purl.org/heritagedata/schemes/225/concepts/111370"/>
    <skos:narrower rdf:resource="http://purl.org/heritagedata/schemes/225/concepts/137237"/>
  </rdf:Description>
  <rdf:Description rdf:about="http://purl.org/heritagedata/schemes/225/concepts/137193">
    <dcterms:publisher rdf:resource="http://www.historicengland.org.uk"/>
    <skos:broader rdf:resource="http://purl.org/heritagedata/schemes/225/concepts/111402"/>
    <skos:broader rdf:resource="http://purl.org/heritagedata/schemes/225/concepts/111355"/>
    <dcterms:issued rdf:datatype="http://www.w3.org/2001/XMLSchema#dateTime">2019-03-26T16:45:43</dcterms:issued>
    <skos:prefLabel xml:lang="en">York</skos:prefLabel>
    <skos:scopeNote xml:lang="en">Transport version of the four-engined Lancaster bomber. Serving from 1943 to 1951, and all metal in construction, this aircraft was used extensively during the Berlin airlift.</skos:scopeNote>
    <rdf:type rdf:resource="http://www.w3.org/2004/02/skos/core#Concept"/>
    <ns1:related rdf:resource="http://purl.org/heritagedata/schemes/225/concepts/111367"/>
    <skos:inScheme rdf:resource="http://purl.org/heritagedata/schemes/225"/>
    <cc:attributionURL rdf:resource="http://www.historicengland.org.uk"/>
    <cc:attributionName xml:lang="en">Historic England</cc:attributionName>
    <cc:license rdf:resource="http://creativecommons.org/licenses/by/3.0"/>
    <dcterms:identifier>http://purl.org/heritagedata/schemes/225/concepts/137193</dcterms:identifier>
    <skos:broader rdf:resource="http://purl.org/heritagedata/schemes/225/concepts/111424"/>
  </rdf:Description>
  <rdf:Description rdf:about="http://purl.org/heritagedata/schemes/225/concepts/139626">
    <skos:narrower rdf:resource="http://purl.org/heritagedata/schemes/225/concepts/111369"/>
    <dcterms:publisher rdf:resource="http://www.historicengland.org.uk"/>
    <dcterms:identifier>http://purl.org/heritagedata/schemes/225/concepts/139626</dcterms:identifier>
    <skos:prefLabel xml:lang="en">Medium Bomber</skos:prefLabel>
    <skos:scopeNote xml:lang="en">A bomber designed to operate with medium bombloads over medium distances.The medium bomber was generally considered to be any design that delivered about 4,000 lb (1.8 t) over ranges of about 1,500 to 2,000 miles (2,400 to 3,200 km).</skos:scopeNote>
    <cc:license rdf:resource="http://creativecommons.org/licenses/by/3.0"/>
    <cc:attributionName xml:lang="en">Historic England</cc:attributionName>
    <skos:narrower rdf:resource="http://purl.org/heritagedata/schemes/225/concepts/111428"/>
    <skos:inScheme rdf:resource="http://purl.org/heritagedata/schemes/225"/>
    <dcterms:issued rdf:datatype="http://www.w3.org/2001/XMLSchema#dateTime">2019-03-26T16:45:43</dcterms:issued>
    <skos:narrower rdf:resource="http://purl.org/heritagedata/schemes/225/concepts/111435"/>
    <skos:narrower rdf:resource="http://purl.org/heritagedata/schemes/225/concepts/137229"/>
    <skos:narrower rdf:resource="http://purl.org/heritagedata/schemes/225/concepts/125593"/>
    <rdf:type rdf:resource="http://www.w3.org/2004/02/skos/core#Concept"/>
    <skos:narrower rdf:resource="http://purl.org/heritagedata/schemes/225/concepts/111370"/>
    <skos:narrower rdf:resource="http://purl.org/heritagedata/schemes/225/concepts/111419"/>
    <cc:attributionURL rdf:resource="http://www.historicengland.org.uk"/>
    <skos:narrower rdf:resource="http://purl.org/heritagedata/schemes/225/concepts/137203"/>
    <skos:narrower rdf:resource="http://purl.org/heritagedata/schemes/225/concepts/136220"/>
    <skos:narrower rdf:resource="http://purl.org/heritagedata/schemes/225/concepts/133173"/>
    <skos:broader rdf:resource="http://purl.org/heritagedata/schemes/225/concepts/111398"/>
  </rdf:Description>
  <rdf:Description rdf:about="http://purl.org/heritagedata/schemes/225/concepts/137174">
    <skos:broader rdf:resource="http://purl.org/heritagedata/schemes/225/concepts/111402"/>
    <skos:broader rdf:resource="http://purl.org/heritagedata/schemes/225/concepts/111423"/>
    <rdf:type rdf:resource="http://www.w3.org/2004/02/skos/core#Concept"/>
    <dcterms:issued rdf:datatype="http://www.w3.org/2001/XMLSchema#dateTime">2019-03-26T16:45:43</dcterms:issued>
    <dcterms:publisher rdf:resource="http://www.historicengland.org.uk"/>
    <skos:broader rdf:resource="http://purl.org/heritagedata/schemes/225/concepts/137189"/>
    <skos:scopeNote xml:lang="en">Originally a light day-bomber, the Boston II, re-christened the Havoc, was adapted for night-flying in the fighter-intruder role. Was capable of a top speed in excess of 300 mph.</skos:scopeNote>
    <cc:attributionName xml:lang="en">Historic England</cc:attributionName>
    <skos:inScheme rdf:resource="http://purl.org/heritagedata/schemes/225"/>
    <skos:prefLabel xml:lang="en">Havoc</skos:prefLabel>
    <ns1:related rdf:resource="http://purl.org/heritagedata/schemes/225/concepts/133199"/>
    <dcterms:identifier>http://purl.org/heritagedata/schemes/225/concepts/137174</dcterms:identifier>
    <skos:broader rdf:resource="http://purl.org/heritagedata/schemes/225/concepts/133198"/>
    <cc:license rdf:resource="http://creativecommons.org/licenses/by/3.0"/>
    <cc:attributionURL rdf:resource="http://www.historicengland.org.uk"/>
  </rdf:Description>
  <rdf:Description rdf:about="http://purl.org/heritagedata/schemes/225/concepts/111416">
    <skos:broader rdf:resource="http://purl.org/heritagedata/schemes/225/concepts/111402"/>
    <rdf:type rdf:resource="http://www.w3.org/2004/02/skos/core#Concept"/>
    <dcterms:identifier>http://purl.org/heritagedata/schemes/225/concepts/111416</dcterms:identifier>
    <cc:license rdf:resource="http://creativecommons.org/licenses/by/3.0"/>
    <skos:inScheme rdf:resource="http://purl.org/heritagedata/schemes/225"/>
    <cc:attributionURL rdf:resource="http://www.historicengland.org.uk"/>
    <cc:attributionName xml:lang="en">Historic England</cc:attributionName>
    <skos:scopeNote xml:lang="en">Four-engine, seven-crew heavy bomber. Entered service with RAF Bomber Command in 1940, becoming one of the twin sources of bomber strength along with the Lancaster. Also used for transport and glider tug duties.</skos:scopeNote>
    <skos:broader rdf:resource="http://purl.org/heritagedata/schemes/225/concepts/137190"/>
    <dcterms:publisher rdf:resource="http://www.historicengland.org.uk"/>
    <skos:broader rdf:resource="http://purl.org/heritagedata/schemes/225/concepts/111415"/>
    <dcterms:issued rdf:datatype="http://www.w3.org/2001/XMLSchema#dateTime">2019-03-26T16:45:43</dcterms:issued>
    <skos:prefLabel xml:lang="en">Halifax</skos:prefLabel>
  </rdf:Description>
  <rdf:Description rdf:about="http://purl.org/heritagedata/schemes/225/concepts/111442">
    <cc:license rdf:resource="http://creativecommons.org/licenses/by/3.0"/>
    <dcterms:identifier>http://purl.org/heritagedata/schemes/225/concepts/111442</dcterms:identifier>
    <cc:attributionURL rdf:resource="http://www.historicengland.org.uk"/>
    <skos:inScheme rdf:resource="http://purl.org/heritagedata/schemes/225"/>
    <dcterms:publisher rdf:resource="http://www.historicengland.org.uk"/>
    <cc:attributionName xml:lang="en">Historic England</cc:attributionName>
    <dcterms:issued rdf:datatype="http://www.w3.org/2001/XMLSchema#dateTime">2019-03-26T16:45:43</dcterms:issued>
    <skos:broader rdf:resource="http://purl.org/heritagedata/schemes/225/concepts/111441"/>
    <skos:broader rdf:resource="http://purl.org/heritagedata/schemes/225/concepts/111403"/>
    <skos:scopeNote xml:lang="en">Single-engine, three-crew torpedo-spotter, reconnaissance and anti-submarine biplane. Entered Naval service in 1936, designed for operation from aircraft carriers and equipped with folding wings.</skos:scopeNote>
    <rdf:type rdf:resource="http://www.w3.org/2004/02/skos/core#Concept"/>
    <skos:prefLabel xml:lang="en">Swordfish</skos:prefLabel>
    <skos:broader rdf:resource="http://purl.org/heritagedata/schemes/225/concepts/135730"/>
  </rdf:Description>
  <rdf:Description rdf:about="http://purl.org/heritagedata/schemes/225/concepts/111399">
    <skos:prefLabel xml:lang="en">Fighter Bomber</skos:prefLabel>
    <skos:scopeNote xml:lang="en">A light, high speed aircraft designed to engage in aerial combat and also equipped to carry bombs.</skos:scopeNote>
    <skos:narrower rdf:resource="http://purl.org/heritagedata/schemes/225/concepts/137212"/>
    <cc:attributionURL rdf:resource="http://www.historicengland.org.uk"/>
    <rdf:type rdf:resource="http://www.w3.org/2004/02/skos/core#Concept"/>
    <skos:narrower rdf:resource="http://purl.org/heritagedata/schemes/225/concepts/135931"/>
    <cc:license rdf:resource="http://creativecommons.org/licenses/by/3.0"/>
    <skos:narrower rdf:resource="http://purl.org/heritagedata/schemes/225/concepts/125493"/>
    <skos:broader rdf:resource="http://purl.org/heritagedata/schemes/225/concepts/111398"/>
    <skos:narrower rdf:resource="http://purl.org/heritagedata/schemes/225/concepts/125517"/>
    <skos:inScheme rdf:resource="http://purl.org/heritagedata/schemes/225"/>
    <skos:narrower rdf:resource="http://purl.org/heritagedata/schemes/225/concepts/133194"/>
    <skos:narrower rdf:resource="http://purl.org/heritagedata/schemes/225/concepts/134998"/>
    <dcterms:issued rdf:datatype="http://www.w3.org/2001/XMLSchema#dateTime">2019-03-26T16:45:43</dcterms:issued>
    <skos:narrower rdf:resource="http://purl.org/heritagedata/schemes/225/concepts/137238"/>
    <skos:broader rdf:resource="http://purl.org/heritagedata/schemes/225/concepts/111397"/>
    <skos:narrower rdf:resource="http://purl.org/heritagedata/schemes/225/concepts/137204"/>
    <dcterms:identifier>http://purl.org/heritagedata/schemes/225/concepts/111399</dcterms:identifier>
    <skos:narrower rdf:resource="http://purl.org/heritagedata/schemes/225/concepts/111366"/>
    <skos:narrower rdf:resource="http://purl.org/heritagedata/schemes/225/concepts/137216"/>
    <skos:narrower rdf:resource="http://purl.org/heritagedata/schemes/225/concepts/167001"/>
    <skos:narrower rdf:resource="http://purl.org/heritagedata/schemes/225/concepts/141453"/>
    <dcterms:publisher rdf:resource="http://www.historicengland.org.uk"/>
    <cc:attributionName xml:lang="en">Historic England</cc:attributionName>
  </rdf:Description>
  <rdf:Description rdf:about="http://purl.org/heritagedata/schemes/225/concepts/111423">
    <dcterms:identifier>http://purl.org/heritagedata/schemes/225/concepts/111423</dcterms:identifier>
    <skos:narrower rdf:resource="http://purl.org/heritagedata/schemes/225/concepts/135750"/>
    <rdf:type rdf:resource="http://www.w3.org/2004/02/skos/core#Concept"/>
    <skos:narrower rdf:resource="http://purl.org/heritagedata/schemes/225/concepts/111429"/>
    <dcterms:issued rdf:datatype="http://www.w3.org/2001/XMLSchema#dateTime">2019-03-26T16:45:43</dcterms:issued>
    <skos:inScheme rdf:resource="http://purl.org/heritagedata/schemes/225"/>
    <cc:attributionURL rdf:resource="http://www.historicengland.org.uk"/>
    <cc:attributionName xml:lang="en">Historic England</cc:attributionName>
    <skos:prefLabel xml:lang="en">Nightfighter</skos:prefLabel>
    <dcterms:publisher rdf:resource="http://www.historicengland.org.uk"/>
    <skos:narrower rdf:resource="http://purl.org/heritagedata/schemes/225/concepts/133202"/>
    <skos:scopeNote xml:lang="en">A light, high speed aircraft equipped specifically to engage in night combat.</skos:scopeNote>
    <skos:narrower rdf:resource="http://purl.org/heritagedata/schemes/225/concepts/137174"/>
    <skos:narrower rdf:resource="http://purl.org/heritagedata/schemes/225/concepts/111373"/>
    <skos:broader rdf:resource="http://purl.org/heritagedata/schemes/225/concepts/111397"/>
    <cc:license rdf:resource="http://creativecommons.org/licenses/by/3.0"/>
  </rdf:Description>
  <rdf:Description rdf:about="http://purl.org/heritagedata/schemes/225/concepts/167003">
    <cc:attributionName xml:lang="en">Historic England</cc:attributionName>
    <cc:license rdf:resource="http://creativecommons.org/licenses/by/3.0"/>
    <skos:inScheme rdf:resource="http://purl.org/heritagedata/schemes/225"/>
    <cc:attributionURL rdf:resource="http://www.historicengland.org.uk"/>
    <dcterms:issued rdf:datatype="http://www.w3.org/2001/XMLSchema#dateTime">2019-03-26T16:45:43</dcterms:issued>
    <skos:scopeNote xml:lang="en">A British six-seat single-engined light aircraft, built by Airspeed Limited. First flew in 1933, saw some use as an airliner. The first British type with a retractable undercarriage. Designed by Hessell Tiltman (co-founder). 16 Couriers built.</skos:scopeNote>
    <skos:prefLabel xml:lang="en">Courier</skos:prefLabel>
    <skos:broader rdf:resource="http://purl.org/heritagedata/schemes/225/concepts/133200"/>
    <skos:broader rdf:resource="http://purl.org/heritagedata/schemes/225/concepts/111430"/>
    <skos:broader rdf:resource="http://purl.org/heritagedata/schemes/225/concepts/111402"/>
    <dcterms:identifier>http://purl.org/heritagedata/schemes/225/concepts/167003</dcterms:identifier>
    <skos:broader rdf:resource="http://purl.org/heritagedata/schemes/225/concepts/111424"/>
    <dcterms:publisher rdf:resource="http://www.historicengland.org.uk"/>
    <rdf:type rdf:resource="http://www.w3.org/2004/02/skos/core#Concept"/>
  </rdf:Description>
  <rdf:Description rdf:about="http://purl.org/heritagedata/schemes/225/concepts/138533">
    <dcterms:issued rdf:datatype="http://www.w3.org/2001/XMLSchema#dateTime">2019-03-26T16:45:43</dcterms:issued>
    <skos:broader rdf:resource="http://purl.org/heritagedata/schemes/225/concepts/111403"/>
    <cc:attributionURL rdf:resource="http://www.historicengland.org.uk"/>
    <rdf:type rdf:resource="http://www.w3.org/2004/02/skos/core#Concept"/>
    <skos:broader rdf:resource="http://purl.org/heritagedata/schemes/225/concepts/111397"/>
    <cc:license rdf:resource="http://creativecommons.org/licenses/by/3.0"/>
    <skos:scopeNote xml:lang="en">A single-seat fighter which began service with the RFC's fighter squadron in 1916. Some short-term success in dealing with new Fokkers but was withdrawn from service in mid-1917.</skos:scopeNote>
    <skos:prefLabel xml:lang="en">Airco DH2</skos:prefLabel>
    <skos:inScheme rdf:resource="http://purl.org/heritagedata/schemes/225"/>
    <dcterms:identifier>http://purl.org/heritagedata/schemes/225/concepts/138533</dcterms:identifier>
    <skos:broader rdf:resource="http://purl.org/heritagedata/schemes/225/concepts/136512"/>
    <dcterms:publisher rdf:resource="http://www.historicengland.org.uk"/>
    <cc:attributionName xml:lang="en">Historic England</cc:attributionName>
  </rdf:Description>
  <rdf:Description rdf:about="http://purl.org/heritagedata/schemes/225/concepts/136531">
    <cc:license rdf:resource="http://creativecommons.org/licenses/by/3.0"/>
    <dcterms:issued rdf:datatype="http://www.w3.org/2001/XMLSchema#dateTime">2019-03-26T16:45:43</dcterms:issued>
    <skos:scopeNote xml:lang="en">A fighter version of the SKUA fitted with a four-gun turret. The majority were converted to target tugs for use by the RAF and Fleet Air Arm.</skos:scopeNote>
    <rdf:type rdf:resource="http://www.w3.org/2004/02/skos/core#Concept"/>
    <skos:broader rdf:resource="http://purl.org/heritagedata/schemes/225/concepts/111402"/>
    <ns1:related rdf:resource="http://purl.org/heritagedata/schemes/225/concepts/133194"/>
    <cc:attributionName xml:lang="en">Historic England</cc:attributionName>
    <skos:inScheme rdf:resource="http://purl.org/heritagedata/schemes/225"/>
    <cc:attributionURL rdf:resource="http://www.historicengland.org.uk"/>
    <dcterms:publisher rdf:resource="http://www.historicengland.org.uk"/>
    <skos:broader rdf:resource="http://purl.org/heritagedata/schemes/225/concepts/111374"/>
    <dcterms:identifier>http://purl.org/heritagedata/schemes/225/concepts/136531</dcterms:identifier>
    <skos:prefLabel xml:lang="en">Roc</skos:prefLabel>
    <skos:broader rdf:resource="http://purl.org/heritagedata/schemes/225/concepts/135751"/>
    <skos:broader rdf:resource="http://purl.org/heritagedata/schemes/225/concepts/111397"/>
  </rdf:Description>
  <rdf:Description rdf:about="http://purl.org/heritagedata/schemes/225/concepts/137238">
    <skos:broader rdf:resource="http://purl.org/heritagedata/schemes/225/concepts/118653"/>
    <cc:attributionName xml:lang="en">Historic England</cc:attributionName>
    <cc:license rdf:resource="http://creativecommons.org/licenses/by/3.0"/>
    <skos:inScheme rdf:resource="http://purl.org/heritagedata/schemes/225"/>
    <cc:attributionURL rdf:resource="http://www.historicengland.org.uk"/>
    <dcterms:issued rdf:datatype="http://www.w3.org/2001/XMLSchema#dateTime">2019-03-26T16:45:43</dcterms:issued>
    <skos:prefLabel xml:lang="en">Me210</skos:prefLabel>
    <rdf:type rdf:resource="http://www.w3.org/2004/02/skos/core#Concept"/>
    <dcterms:identifier>http://purl.org/heritagedata/schemes/225/concepts/137238</dcterms:identifier>
    <skos:broader rdf:resource="http://purl.org/heritagedata/schemes/225/concepts/111402"/>
    <skos:broader rdf:resource="http://purl.org/heritagedata/schemes/225/concepts/111399"/>
    <dcterms:publisher rdf:resource="http://www.historicengland.org.uk"/>
    <ns1:related rdf:resource="http://purl.org/heritagedata/schemes/225/concepts/133202"/>
    <skos:scopeNote xml:lang="en">Two-seat, twin-engined fighter/fighter-bomber designed as a replacement for the Bf110. Of the 600 or so produced, only 258 reached the Luftwaffe due to serious design faults. The ME210 was superseded by the ME410 Hornisse.</skos:scopeNote>
  </rdf:Description>
  <rdf:Description rdf:about="http://purl.org/heritagedata/schemes/225/concepts/111397">
    <skos:narrower rdf:resource="http://purl.org/heritagedata/schemes/225/concepts/133195"/>
    <skos:narrower rdf:resource="http://purl.org/heritagedata/schemes/225/concepts/137209"/>
    <skos:narrower rdf:resource="http://purl.org/heritagedata/schemes/225/concepts/169973"/>
    <skos:prefLabel xml:lang="en">Fighter</skos:prefLabel>
    <skos:inScheme rdf:resource="http://purl.org/heritagedata/schemes/225"/>
    <skos:narrower rdf:resource="http://purl.org/heritagedata/schemes/225/concepts/136233"/>
    <skos:narrower rdf:resource="http://purl.org/heritagedata/schemes/225/concepts/111423"/>
    <skos:narrower rdf:resource="http://purl.org/heritagedata/schemes/225/concepts/138533"/>
    <skos:narrower rdf:resource="http://purl.org/heritagedata/schemes/225/concepts/167004"/>
    <skos:narrower rdf:resource="http://purl.org/heritagedata/schemes/225/concepts/167858"/>
    <skos:narrower rdf:resource="http://purl.org/heritagedata/schemes/225/concepts/152401"/>
    <skos:narrower rdf:resource="http://purl.org/heritagedata/schemes/225/concepts/137221"/>
    <skos:narrower rdf:resource="http://purl.org/heritagedata/schemes/225/concepts/111334"/>
    <cc:attributionName xml:lang="en">Historic England</cc:attributionName>
    <skos:narrower rdf:resource="http://purl.org/heritagedata/schemes/225/concepts/125514"/>
    <skos:narrower rdf:resource="http://purl.org/heritagedata/schemes/225/concepts/138541"/>
    <skos:narrower rdf:resource="http://purl.org/heritagedata/schemes/225/concepts/137196"/>
    <skos:narrower rdf:resource="http://purl.org/heritagedata/schemes/225/concepts/111399"/>
    <cc:license rdf:resource="http://creativecommons.org/licenses/by/3.0"/>
    <dcterms:issued rdf:datatype="http://www.w3.org/2001/XMLSchema#dateTime">2019-03-26T16:45:43</dcterms:issued>
    <skos:narrower rdf:resource="http://purl.org/heritagedata/schemes/225/concepts/136522"/>
    <skos:narrower rdf:resource="http://purl.org/heritagedata/schemes/225/concepts/137199"/>
    <skos:narrower rdf:resource="http://purl.org/heritagedata/schemes/225/concepts/151472"/>
    <skos:narrower rdf:resource="http://purl.org/heritagedata/schemes/225/concepts/136593"/>
    <skos:narrower rdf:resource="http://purl.org/heritagedata/schemes/225/concepts/111333"/>
    <skos:narrower rdf:resource="http://purl.org/heritagedata/schemes/225/concepts/138485"/>
    <skos:narrower rdf:resource="http://purl.org/heritagedata/schemes/225/concepts/140416"/>
    <skos:narrower rdf:resource="http://purl.org/heritagedata/schemes/225/concepts/137220"/>
    <skos:scopeNote xml:lang="en">A light, high-speed aircraft designed to engage in aerial combat.</skos:scopeNote>
    <skos:narrower rdf:resource="http://purl.org/heritagedata/schemes/225/concepts/136531"/>
    <skos:narrower rdf:resource="http://purl.org/heritagedata/schemes/225/concepts/140065"/>
    <skos:narrower rdf:resource="http://purl.org/heritagedata/schemes/225/concepts/138535"/>
    <dcterms:identifier>http://purl.org/heritagedata/schemes/225/concepts/111397</dcterms:identifier>
    <skos:broader rdf:resource="http://purl.org/heritagedata/schemes/225/concepts/111394"/>
    <skos:narrower rdf:resource="http://purl.org/heritagedata/schemes/225/concepts/111360"/>
    <skos:narrower rdf:resource="http://purl.org/heritagedata/schemes/225/concepts/133209"/>
    <skos:narrower rdf:resource="http://purl.org/heritagedata/schemes/225/concepts/137192"/>
    <skos:narrower rdf:resource="http://purl.org/heritagedata/schemes/225/concepts/167000"/>
    <skos:narrower rdf:resource="http://purl.org/heritagedata/schemes/225/concepts/111414"/>
    <dcterms:publisher rdf:resource="http://www.historicengland.org.uk"/>
    <skos:narrower rdf:resource="http://purl.org/heritagedata/schemes/225/concepts/137215"/>
    <rdf:type rdf:resource="http://www.w3.org/2004/02/skos/core#Concept"/>
    <skos:narrower rdf:resource="http://purl.org/heritagedata/schemes/225/concepts/138532"/>
    <cc:attributionURL rdf:resource="http://www.historicengland.org.uk"/>
    <skos:narrower rdf:resource="http://purl.org/heritagedata/schemes/225/concepts/125518"/>
  </rdf:Description>
  <rdf:Description rdf:about="http://purl.org/heritagedata/schemes/225/concepts/133203">
    <skos:scopeNote xml:lang="en">Twin-engined maritime-reconnaissance bomber adapted from pre-war American airliners, the A-28 and A-29, evident from the row of portholes along its fuselage. Entered service with RAF Coastal Command just before the outbreak of World War Two.</skos:scopeNote>
    <dcterms:publisher rdf:resource="http://www.historicengland.org.uk"/>
    <skos:prefLabel xml:lang="en">Hudson</skos:prefLabel>
    <rdf:type rdf:resource="http://www.w3.org/2004/02/skos/core#Concept"/>
    <skos:broader rdf:resource="http://purl.org/heritagedata/schemes/225/concepts/111398"/>
    <dcterms:identifier>http://purl.org/heritagedata/schemes/225/concepts/133203</dcterms:identifier>
    <skos:broader rdf:resource="http://purl.org/heritagedata/schemes/225/concepts/135730"/>
    <cc:license rdf:resource="http://creativecommons.org/licenses/by/3.0"/>
    <cc:attributionURL rdf:resource="http://www.historicengland.org.uk"/>
    <dcterms:issued rdf:datatype="http://www.w3.org/2001/XMLSchema#dateTime">2019-03-26T16:45:43</dcterms:issued>
    <skos:broader rdf:resource="http://purl.org/heritagedata/schemes/225/concepts/125516"/>
    <cc:attributionName xml:lang="en">Historic England</cc:attributionName>
    <skos:broader rdf:resource="http://purl.org/heritagedata/schemes/225/concepts/111402"/>
    <skos:inScheme rdf:resource="http://purl.org/heritagedata/schemes/225"/>
  </rdf:Description>
  <rdf:Description rdf:about="http://purl.org/heritagedata/schemes/225/concepts/133194">
    <cc:license rdf:resource="http://creativecommons.org/licenses/by/3.0"/>
    <cc:attributionName xml:lang="en">Historic England</cc:attributionName>
    <cc:attributionURL rdf:resource="http://www.historicengland.org.uk"/>
    <skos:inScheme rdf:resource="http://purl.org/heritagedata/schemes/225"/>
    <skos:broader rdf:resource="http://purl.org/heritagedata/schemes/225/concepts/111374"/>
    <dcterms:publisher rdf:resource="http://www.historicengland.org.uk"/>
    <dcterms:issued rdf:datatype="http://www.w3.org/2001/XMLSchema#dateTime">2019-03-26T16:45:43</dcterms:issued>
    <dcterms:identifier>http://purl.org/heritagedata/schemes/225/concepts/133194</dcterms:identifier>
    <rdf:type rdf:resource="http://www.w3.org/2004/02/skos/core#Concept"/>
    <skos:broader rdf:resource="http://purl.org/heritagedata/schemes/225/concepts/111402"/>
    <skos:scopeNote xml:lang="en">Single-engine fighter/dive-bomber. The Fleet Air Arm's first operational monoplane, and its first aircraft to shoot down an enemy during the war.</skos:scopeNote>
    <skos:prefLabel xml:lang="en">Skua</skos:prefLabel>
    <ns1:related rdf:resource="http://purl.org/heritagedata/schemes/225/concepts/136531"/>
    <skos:broader rdf:resource="http://purl.org/heritagedata/schemes/225/concepts/111399"/>
  </rdf:Description>
  <rdf:Description rdf:about="http://purl.org/heritagedata/schemes/225/concepts/136031">
    <dcterms:issued rdf:datatype="http://www.w3.org/2001/XMLSchema#dateTime">2019-03-26T16:45:43</dcterms:issued>
    <dcterms:publisher rdf:resource="http://www.historicengland.org.uk"/>
    <skos:broader rdf:resource="http://purl.org/heritagedata/schemes/225/concepts/111394"/>
    <skos:narrower rdf:resource="http://purl.org/heritagedata/schemes/225/concepts/167009"/>
    <cc:attributionURL rdf:resource="http://www.historicengland.org.uk"/>
    <skos:prefLabel xml:lang="en">Army Cooperation</skos:prefLabel>
    <skos:narrower rdf:resource="http://purl.org/heritagedata/schemes/225/concepts/141399"/>
    <cc:license rdf:resource="http://creativecommons.org/licenses/by/3.0"/>
    <cc:attributionName xml:lang="en">Historic England</cc:attributionName>
    <dcterms:identifier>http://purl.org/heritagedata/schemes/225/concepts/136031</dcterms:identifier>
    <skos:inScheme rdf:resource="http://purl.org/heritagedata/schemes/225"/>
    <skos:scopeNote xml:lang="en">An aircraft used in the assistance of ground-based military operations.</skos:scopeNote>
    <rdf:type rdf:resource="http://www.w3.org/2004/02/skos/core#Concept"/>
    <skos:narrower rdf:resource="http://purl.org/heritagedata/schemes/225/concepts/141207"/>
  </rdf:Description>
  <rdf:Description rdf:about="http://purl.org/heritagedata/schemes/225/concepts/167014">
    <dcterms:publisher rdf:resource="http://www.historicengland.org.uk"/>
    <skos:prefLabel xml:lang="en">Bleriot 155</skos:prefLabel>
    <skos:broader rdf:resource="http://purl.org/heritagedata/schemes/225/concepts/111403"/>
    <rdf:type rdf:resource="http://www.w3.org/2004/02/skos/core#Concept"/>
    <dcterms:issued rdf:datatype="http://www.w3.org/2001/XMLSchema#dateTime">2019-03-26T16:45:43</dcterms:issued>
    <skos:broader rdf:resource="http://purl.org/heritagedata/schemes/225/concepts/167012"/>
    <skos:inScheme rdf:resource="http://purl.org/heritagedata/schemes/225"/>
    <cc:attributionURL rdf:resource="http://www.historicengland.org.uk"/>
    <skos:scopeNote xml:lang="en">A French airliner produced in 1925. A four-engined biplane developed from the Bleriot 115 and 135 but larger than these. Two were built for Air Union (the Paris-London route). Both crashed with fatalaties in 1926 (Kent).</skos:scopeNote>
    <cc:attributionName xml:lang="en">Historic England</cc:attributionName>
    <cc:license rdf:resource="http://creativecommons.org/licenses/by/3.0"/>
    <dcterms:identifier>http://purl.org/heritagedata/schemes/225/concepts/167014</dcterms:identifier>
    <skos:broader rdf:resource="http://purl.org/heritagedata/schemes/225/concepts/111424"/>
  </rdf:Description>
  <rdf:Description rdf:about="http://purl.org/heritagedata/schemes/225/concepts/142898">
    <cc:attributionURL rdf:resource="http://www.historicengland.org.uk"/>
    <rdf:type rdf:resource="http://www.w3.org/2004/02/skos/core#Concept"/>
    <dcterms:identifier>http://purl.org/heritagedata/schemes/225/concepts/142898</dcterms:identifier>
    <dcterms:issued rdf:datatype="http://www.w3.org/2001/XMLSchema#dateTime">2019-03-26T16:45:43</dcterms:issued>
    <cc:attributionName xml:lang="en">Historic England</cc:attributionName>
    <cc:license rdf:resource="http://creativecommons.org/licenses/by/3.0"/>
    <skos:broader rdf:resource="http://purl.org/heritagedata/schemes/225/concepts/141131"/>
    <skos:scopeNote xml:lang="en">Mark 8 or the eighth variant of an aircraft with its associated modifications.</skos:scopeNote>
    <dcterms:publisher rdf:resource="http://www.historicengland.org.uk"/>
    <skos:prefLabel xml:lang="en">MkVIII</skos:prefLabel>
    <skos:inScheme rdf:resource="http://purl.org/heritagedata/schemes/225"/>
  </rdf:Description>
  <rdf:Description rdf:about="http://purl.org/heritagedata/schemes/225/concepts/125514">
    <cc:license rdf:resource="http://creativecommons.org/licenses/by/3.0"/>
    <cc:attributionName xml:lang="en">Historic England</cc:attributionName>
    <cc:attributionURL rdf:resource="http://www.historicengland.org.uk"/>
    <skos:inScheme rdf:resource="http://purl.org/heritagedata/schemes/225"/>
    <dcterms:issued rdf:datatype="http://www.w3.org/2001/XMLSchema#dateTime">2019-03-26T16:45:43</dcterms:issued>
    <skos:broader rdf:resource="http://purl.org/heritagedata/schemes/225/concepts/111402"/>
    <rdf:type rdf:resource="http://www.w3.org/2004/02/skos/core#Concept"/>
    <skos:broader rdf:resource="http://purl.org/heritagedata/schemes/225/concepts/111397"/>
    <skos:prefLabel xml:lang="en">P51 Mustang</skos:prefLabel>
    <dcterms:publisher rdf:resource="http://www.historicengland.org.uk"/>
    <skos:scopeNote xml:lang="en">Single-engine, single-seat, long range fighter originally designed in 1940 to a British requirement. Outstanding low-level speed and range resulted in its assignment to the ground support (Army co-operation) role.</skos:scopeNote>
    <skos:broader rdf:resource="http://purl.org/heritagedata/schemes/225/concepts/125513"/>
    <dcterms:identifier>http://purl.org/heritagedata/schemes/225/concepts/125514</dcterms:identifier>
  </rdf:Description>
  <rdf:Description rdf:about="http://purl.org/heritagedata/schemes/225/concepts/137151">
    <dcterms:issued rdf:datatype="http://www.w3.org/2001/XMLSchema#dateTime">2019-03-26T16:45:43</dcterms:issued>
    <skos:broader rdf:resource="http://purl.org/heritagedata/schemes/225/concepts/111402"/>
    <cc:attributionURL rdf:resource="http://www.historicengland.org.uk"/>
    <rdf:type rdf:resource="http://www.w3.org/2004/02/skos/core#Concept"/>
    <cc:license rdf:resource="http://creativecommons.org/licenses/by/3.0"/>
    <skos:broader rdf:resource="http://purl.org/heritagedata/schemes/225/concepts/133198"/>
    <skos:scopeNote xml:lang="en">Also known as the C-47 Skytrain, this twin-engined, military transport was developed from the DC-3 twenty-eight-seat commercial airliner and was the most extensively employed transport of the Second World War.</skos:scopeNote>
    <dcterms:identifier>http://purl.org/heritagedata/schemes/225/concepts/137151</dcterms:identifier>
    <skos:inScheme rdf:resource="http://purl.org/heritagedata/schemes/225"/>
    <skos:broader rdf:resource="http://purl.org/heritagedata/schemes/225/concepts/111424"/>
    <dcterms:publisher rdf:resource="http://www.historicengland.org.uk"/>
    <cc:attributionName xml:lang="en">Historic England</cc:attributionName>
    <skos:prefLabel xml:lang="en">Dakota</skos:prefLabel>
  </rdf:Description>
  <rdf:Description rdf:about="http://purl.org/heritagedata/schemes/225/concepts/141274">
    <skos:scopeNote xml:lang="en">Mark 16 or the sixteenth variant of an aircraft with its associated modifications.</skos:scopeNote>
    <skos:inScheme rdf:resource="http://purl.org/heritagedata/schemes/225"/>
    <dcterms:publisher rdf:resource="http://www.historicengland.org.uk"/>
    <cc:attributionName xml:lang="en">Historic England</cc:attributionName>
    <skos:prefLabel xml:lang="en">MkXVI</skos:prefLabel>
    <dcterms:issued rdf:datatype="http://www.w3.org/2001/XMLSchema#dateTime">2019-03-26T16:45:43</dcterms:issued>
    <skos:broader rdf:resource="http://purl.org/heritagedata/schemes/225/concepts/141131"/>
    <cc:attributionURL rdf:resource="http://www.historicengland.org.uk"/>
    <rdf:type rdf:resource="http://www.w3.org/2004/02/skos/core#Concept"/>
    <dcterms:identifier>http://purl.org/heritagedata/schemes/225/concepts/141274</dcterms:identifier>
    <cc:license rdf:resource="http://creativecommons.org/licenses/by/3.0"/>
  </rdf:Description>
  <rdf:Description rdf:about="http://purl.org/heritagedata/schemes/225/concepts/138507">
    <skos:narrower rdf:resource="http://purl.org/heritagedata/schemes/225/concepts/137225"/>
    <dcterms:issued rdf:datatype="http://www.w3.org/2001/XMLSchema#dateTime">2019-03-26T16:45:43</dcterms:issued>
    <cc:attributionURL rdf:resource="http://www.historicengland.org.uk"/>
    <rdf:type rdf:resource="http://www.w3.org/2004/02/skos/core#Concept"/>
    <dcterms:identifier>http://purl.org/heritagedata/schemes/225/concepts/138507</dcterms:identifier>
    <skos:narrower rdf:resource="http://purl.org/heritagedata/schemes/225/concepts/125533"/>
    <cc:license rdf:resource="http://creativecommons.org/licenses/by/3.0"/>
    <cc:attributionName xml:lang="en">Historic England</cc:attributionName>
    <skos:broader rdf:resource="http://purl.org/heritagedata/schemes/225/concepts/111358"/>
    <skos:scopeNote xml:lang="en">The Consolidated Vultee Aircraft Corporation. Formed in 1943 with the merging of The Consolidated Aircraft Corporation and Vultee Aircraft, Inc..</skos:scopeNote>
    <skos:inScheme rdf:resource="http://purl.org/heritagedata/schemes/225"/>
    <skos:narrower rdf:resource="http://purl.org/heritagedata/schemes/225/concepts/111417"/>
    <dcterms:publisher rdf:resource="http://www.historicengland.org.uk"/>
    <skos:prefLabel xml:lang="en">Consolidated Vultee</skos:prefLabel>
  </rdf:Description>
  <rdf:Description rdf:about="http://purl.org/heritagedata/schemes/225/concepts/111334">
    <dcterms:identifier>http://purl.org/heritagedata/schemes/225/concepts/111334</dcterms:identifier>
    <skos:scopeNote xml:lang="en">Single-engine, single-seat interceptor fighter developed from the race-winning Schneider Trophy seaplanes. One of the most famous of all combat aircraft, entered RAF service in 1938 and was still in use in the 1950s.</skos:scopeNote>
    <skos:inScheme rdf:resource="http://purl.org/heritagedata/schemes/225"/>
    <skos:broader rdf:resource="http://purl.org/heritagedata/schemes/225/concepts/111353"/>
    <dcterms:publisher rdf:resource="http://www.historicengland.org.uk"/>
    <cc:attributionName xml:lang="en">Historic England</cc:attributionName>
    <skos:prefLabel xml:lang="en">Spitfire</skos:prefLabel>
    <ns1:related rdf:resource="http://purl.org/heritagedata/schemes/225/concepts/137209"/>
    <dcterms:issued rdf:datatype="http://www.w3.org/2001/XMLSchema#dateTime">2019-03-26T16:45:43</dcterms:issued>
    <skos:broader rdf:resource="http://purl.org/heritagedata/schemes/225/concepts/111402"/>
    <cc:attributionURL rdf:resource="http://www.historicengland.org.uk"/>
    <rdf:type rdf:resource="http://www.w3.org/2004/02/skos/core#Concept"/>
    <skos:broader rdf:resource="http://purl.org/heritagedata/schemes/225/concepts/111397"/>
    <cc:license rdf:resource="http://creativecommons.org/licenses/by/3.0"/>
  </rdf:Description>
  <rdf:Description rdf:about="http://purl.org/heritagedata/schemes/225/concepts/140455">
    <skos:prefLabel xml:lang="en">Arado</skos:prefLabel>
    <dcterms:issued rdf:datatype="http://www.w3.org/2001/XMLSchema#dateTime">2019-03-26T16:45:43</dcterms:issued>
    <cc:license rdf:resource="http://creativecommons.org/licenses/by/3.0"/>
    <cc:attributionURL rdf:resource="http://www.historicengland.org.uk"/>
    <dcterms:identifier>http://purl.org/heritagedata/schemes/225/concepts/140455</dcterms:identifier>
    <skos:scopeNote xml:lang="en">Arado Flugzeugwerke. Formed in 1931 in Germany when the aircraft manufacturer Albatros Flugzeugwerke was declared bankrupt and part of it merged with Arado Handells-Gessellschaft.</skos:scopeNote>
    <skos:narrower rdf:resource="http://purl.org/heritagedata/schemes/225/concepts/140447"/>
    <skos:broader rdf:resource="http://purl.org/heritagedata/schemes/225/concepts/111358"/>
    <rdf:type rdf:resource="http://www.w3.org/2004/02/skos/core#Concept"/>
    <skos:inScheme rdf:resource="http://purl.org/heritagedata/schemes/225"/>
    <cc:attributionName xml:lang="en">Historic England</cc:attributionName>
    <dcterms:publisher rdf:resource="http://www.historicengland.org.uk"/>
  </rdf:Description>
  <rdf:Description rdf:about="http://purl.org/heritagedata/schemes/225/concepts/137212">
    <cc:attributionName xml:lang="en">Historic England</cc:attributionName>
    <cc:license rdf:resource="http://creativecommons.org/licenses/by/3.0"/>
    <skos:inScheme rdf:resource="http://purl.org/heritagedata/schemes/225"/>
    <cc:attributionURL rdf:resource="http://www.historicengland.org.uk"/>
    <dcterms:issued rdf:datatype="http://www.w3.org/2001/XMLSchema#dateTime">2019-03-26T16:45:43</dcterms:issued>
    <skos:prefLabel xml:lang="en">P39 Airacobra</skos:prefLabel>
    <dcterms:identifier>http://purl.org/heritagedata/schemes/225/concepts/137212</dcterms:identifier>
    <skos:broader rdf:resource="http://purl.org/heritagedata/schemes/225/concepts/137211"/>
    <skos:broader rdf:resource="http://purl.org/heritagedata/schemes/225/concepts/111402"/>
    <skos:broader rdf:resource="http://purl.org/heritagedata/schemes/225/concepts/111399"/>
    <skos:scopeNote xml:lang="en">Single-seat fighter-bomber with a single, midships engine and tricycle landing gear. After proving a failure as an air-combat fighter, was used mainly in the ground attack role.</skos:scopeNote>
    <dcterms:publisher rdf:resource="http://www.historicengland.org.uk"/>
    <rdf:type rdf:resource="http://www.w3.org/2004/02/skos/core#Concept"/>
  </rdf:Description>
  <rdf:Description rdf:about="http://purl.org/heritagedata/schemes/225/concepts/133205">
    <dcterms:publisher rdf:resource="http://www.historicengland.org.uk"/>
    <skos:broader rdf:resource="http://purl.org/heritagedata/schemes/225/concepts/111358"/>
    <skos:narrower rdf:resource="http://purl.org/heritagedata/schemes/225/concepts/137153"/>
    <skos:narrower rdf:resource="http://purl.org/heritagedata/schemes/225/concepts/133206"/>
    <skos:scopeNote xml:lang="en">Miles Aircraft, Ltd., originally known as Phillips &amp; Powis Aircraft Ltd.. Formed in 1935 as a public company to take over aircraft manufacture from Phillips &amp; Powis Aircraft (Reading) Ltd.</skos:scopeNote>
    <rdf:type rdf:resource="http://www.w3.org/2004/02/skos/core#Concept"/>
    <dcterms:issued rdf:datatype="http://www.w3.org/2001/XMLSchema#dateTime">2019-03-26T16:45:43</dcterms:issued>
    <skos:inScheme rdf:resource="http://purl.org/heritagedata/schemes/225"/>
    <cc:attributionURL rdf:resource="http://www.historicengland.org.uk"/>
    <dcterms:identifier>http://purl.org/heritagedata/schemes/225/concepts/133205</dcterms:identifier>
    <cc:attributionName xml:lang="en">Historic England</cc:attributionName>
    <cc:license rdf:resource="http://creativecommons.org/licenses/by/3.0"/>
    <skos:narrower rdf:resource="http://purl.org/heritagedata/schemes/225/concepts/136592"/>
    <skos:prefLabel xml:lang="en">Miles</skos:prefLabel>
  </rdf:Description>
  <rdf:Description rdf:about="http://purl.org/heritagedata/schemes/225/concepts/133201">
    <dcterms:issued rdf:datatype="http://www.w3.org/2001/XMLSchema#dateTime">2019-03-26T16:45:43</dcterms:issued>
    <skos:scopeNote xml:lang="en">Twin-engined monoplane that served the RAF as an advanced trainer and flying ambulance. Mk. I featured a gun turret and served for gunnery and bombing-crew training. Subsequent versions used for pilot, radio and navigation training.</skos:scopeNote>
    <skos:broader rdf:resource="http://purl.org/heritagedata/schemes/225/concepts/111402"/>
    <skos:inScheme rdf:resource="http://purl.org/heritagedata/schemes/225"/>
    <rdf:type rdf:resource="http://www.w3.org/2004/02/skos/core#Concept"/>
    <skos:broader rdf:resource="http://purl.org/heritagedata/schemes/225/concepts/133200"/>
    <skos:prefLabel xml:lang="en">Oxford</skos:prefLabel>
    <dcterms:identifier>http://purl.org/heritagedata/schemes/225/concepts/133201</dcterms:identifier>
    <dcterms:publisher rdf:resource="http://www.historicengland.org.uk"/>
    <skos:broader rdf:resource="http://purl.org/heritagedata/schemes/225/concepts/111401"/>
    <cc:license rdf:resource="http://creativecommons.org/licenses/by/3.0"/>
    <cc:attributionURL rdf:resource="http://www.historicengland.org.uk"/>
    <cc:attributionName xml:lang="en">Historic England</cc:attributionName>
  </rdf:Description>
  <rdf:Description rdf:about="http://purl.org/heritagedata/schemes/225/concepts/133208">
    <cc:license rdf:resource="http://creativecommons.org/licenses/by/3.0"/>
    <dcterms:publisher rdf:resource="http://www.historicengland.org.uk"/>
    <skos:inScheme rdf:resource="http://purl.org/heritagedata/schemes/225"/>
    <skos:scopeNote xml:lang="en">An aircraft designed for the testing of engines or other aircraft components.</skos:scopeNote>
    <skos:prefLabel xml:lang="en">Test Aircraft</skos:prefLabel>
    <cc:attributionName xml:lang="en">Historic England</cc:attributionName>
    <skos:broader rdf:resource="http://purl.org/heritagedata/schemes/225/concepts/111394"/>
    <dcterms:issued rdf:datatype="http://www.w3.org/2001/XMLSchema#dateTime">2019-03-26T16:45:43</dcterms:issued>
    <cc:attributionURL rdf:resource="http://www.historicengland.org.uk"/>
    <dcterms:identifier>http://purl.org/heritagedata/schemes/225/concepts/133208</dcterms:identifier>
    <rdf:type rdf:resource="http://www.w3.org/2004/02/skos/core#Concept"/>
  </rdf:Description>
  <rdf:Description rdf:about="http://purl.org/heritagedata/schemes/225/concepts/111427">
    <cc:license rdf:resource="http://creativecommons.org/licenses/by/3.0"/>
    <cc:attributionName xml:lang="en">Historic England</cc:attributionName>
    <cc:attributionURL rdf:resource="http://www.historicengland.org.uk"/>
    <skos:inScheme rdf:resource="http://purl.org/heritagedata/schemes/225"/>
    <skos:broader rdf:resource="http://purl.org/heritagedata/schemes/225/concepts/111398"/>
    <dcterms:issued rdf:datatype="http://www.w3.org/2001/XMLSchema#dateTime">2019-03-26T16:45:43</dcterms:issued>
    <skos:broader rdf:resource="http://purl.org/heritagedata/schemes/225/concepts/111402"/>
    <skos:scopeNote xml:lang="en">A progressive development of the DO17, the twin-engined DO217 entered service in 1941. The DO217 saw service as a bomber over the UK and took part in the 'Baedecker' raids of 1942.</skos:scopeNote>
    <rdf:type rdf:resource="http://www.w3.org/2004/02/skos/core#Concept"/>
    <dcterms:publisher rdf:resource="http://www.historicengland.org.uk"/>
    <skos:broader rdf:resource="http://purl.org/heritagedata/schemes/225/concepts/111361"/>
    <skos:prefLabel xml:lang="en">Do217</skos:prefLabel>
    <dcterms:identifier>http://purl.org/heritagedata/schemes/225/concepts/111427</dcterms:identifier>
  </rdf:Description>
  <rdf:Description rdf:about="http://purl.org/heritagedata/schemes/225/concepts/151396">
    <dcterms:issued rdf:datatype="http://www.w3.org/2001/XMLSchema#dateTime">2019-03-26T16:45:43</dcterms:issued>
    <dcterms:publisher rdf:resource="http://www.historicengland.org.uk"/>
    <dcterms:identifier>http://purl.org/heritagedata/schemes/225/concepts/151396</dcterms:identifier>
    <skos:narrower rdf:resource="http://purl.org/heritagedata/schemes/225/concepts/151397"/>
    <skos:broader rdf:resource="http://purl.org/heritagedata/schemes/225/concepts/111358"/>
    <cc:license rdf:resource="http://creativecommons.org/licenses/by/3.0"/>
    <cc:attributionName xml:lang="en">Historic England</cc:attributionName>
    <cc:attributionURL rdf:resource="http://www.historicengland.org.uk"/>
    <skos:inScheme rdf:resource="http://purl.org/heritagedata/schemes/225"/>
    <skos:scopeNote xml:lang="en">A German aircraft manufacturer of the 1930s and 1940s, pre-war the company were noted for making sailplanes and sports planes; during the Second World War they made military aircraft including flying bombs.</skos:scopeNote>
    <skos:prefLabel xml:lang="en">Fieseler</skos:prefLabel>
    <rdf:type rdf:resource="http://www.w3.org/2004/02/skos/core#Concept"/>
  </rdf:Description>
  <rdf:Description rdf:about="http://purl.org/heritagedata/schemes/225/concepts/111424">
    <skos:narrower rdf:resource="http://purl.org/heritagedata/schemes/225/concepts/167015"/>
    <skos:prefLabel xml:lang="en">Transporter</skos:prefLabel>
    <cc:license rdf:resource="http://creativecommons.org/licenses/by/3.0"/>
    <cc:attributionURL rdf:resource="http://www.historicengland.org.uk"/>
    <skos:inScheme rdf:resource="http://purl.org/heritagedata/schemes/225"/>
    <skos:narrower rdf:resource="http://purl.org/heritagedata/schemes/225/concepts/137201"/>
    <skos:narrower rdf:resource="http://purl.org/heritagedata/schemes/225/concepts/138542"/>
    <rdf:type rdf:resource="http://www.w3.org/2004/02/skos/core#Concept"/>
    <skos:narrower rdf:resource="http://purl.org/heritagedata/schemes/225/concepts/137235"/>
    <dcterms:identifier>http://purl.org/heritagedata/schemes/225/concepts/111424</dcterms:identifier>
    <skos:narrower rdf:resource="http://purl.org/heritagedata/schemes/225/concepts/136030"/>
    <skos:narrower rdf:resource="http://purl.org/heritagedata/schemes/225/concepts/137228"/>
    <skos:narrower rdf:resource="http://purl.org/heritagedata/schemes/225/concepts/137232"/>
    <skos:narrower rdf:resource="http://purl.org/heritagedata/schemes/225/concepts/169972"/>
    <skos:narrower rdf:resource="http://purl.org/heritagedata/schemes/225/concepts/137236"/>
    <skos:narrower rdf:resource="http://purl.org/heritagedata/schemes/225/concepts/137111"/>
    <skos:narrower rdf:resource="http://purl.org/heritagedata/schemes/225/concepts/137193"/>
    <skos:narrower rdf:resource="http://purl.org/heritagedata/schemes/225/concepts/167003"/>
    <skos:scopeNote xml:lang="en">An aircraft used for the transportation of troops, supplies, vehicles or passengers.</skos:scopeNote>
    <cc:attributionName xml:lang="en">Historic England</cc:attributionName>
    <skos:narrower rdf:resource="http://purl.org/heritagedata/schemes/225/concepts/167011"/>
    <dcterms:issued rdf:datatype="http://www.w3.org/2001/XMLSchema#dateTime">2019-03-26T16:45:43</dcterms:issued>
    <skos:narrower rdf:resource="http://purl.org/heritagedata/schemes/225/concepts/167002"/>
    <skos:broader rdf:resource="http://purl.org/heritagedata/schemes/225/concepts/111394"/>
    <dcterms:publisher rdf:resource="http://www.historicengland.org.uk"/>
    <skos:narrower rdf:resource="http://purl.org/heritagedata/schemes/225/concepts/167008"/>
    <skos:narrower rdf:resource="http://purl.org/heritagedata/schemes/225/concepts/167014"/>
    <skos:narrower rdf:resource="http://purl.org/heritagedata/schemes/225/concepts/135606"/>
    <skos:narrower rdf:resource="http://purl.org/heritagedata/schemes/225/concepts/137151"/>
  </rdf:Description>
  <rdf:Description rdf:about="http://purl.org/heritagedata/schemes/225/concepts/123733">
    <dcterms:publisher rdf:resource="http://www.historicengland.org.uk"/>
    <cc:license rdf:resource="http://creativecommons.org/licenses/by/3.0"/>
    <rdf:type rdf:resource="http://www.w3.org/2004/02/skos/core#Concept"/>
    <skos:narrower rdf:resource="http://purl.org/heritagedata/schemes/225/concepts/111358"/>
    <dcterms:issued rdf:datatype="http://www.w3.org/2001/XMLSchema#dateTime">2019-03-26T16:45:43</dcterms:issued>
    <skos:prefLabel xml:lang="en">Aircraft Type</skos:prefLabel>
    <cc:attributionName xml:lang="en">Historic England</cc:attributionName>
    <skos:narrower rdf:resource="http://purl.org/heritagedata/schemes/225/concepts/111394"/>
    <skos:inScheme rdf:resource="http://purl.org/heritagedata/schemes/225"/>
    <skos:narrower rdf:resource="http://purl.org/heritagedata/schemes/225/concepts/141131"/>
    <skos:narrower rdf:resource="http://purl.org/heritagedata/schemes/225/concepts/111393"/>
    <dcterms:identifier>http://purl.org/heritagedata/schemes/225/concepts/123733</dcterms:identifier>
    <skos:scopeNote xml:lang="en">Types of aircraft to aid the recording of aircraft remains and crash sites, listing aircraft by form, function and manufacturer.</skos:scopeNote>
    <skos:topConceptOf rdf:resource="http://purl.org/heritagedata/schemes/225"/>
    <cc:attributionURL rdf:resource="http://www.historicengland.org.uk"/>
  </rdf:Description>
  <rdf:Description rdf:about="http://purl.org/heritagedata/schemes/225/concepts/111333">
    <rdf:type rdf:resource="http://www.w3.org/2004/02/skos/core#Concept"/>
    <skos:broader rdf:resource="http://purl.org/heritagedata/schemes/225/concepts/111397"/>
    <dcterms:publisher rdf:resource="http://www.historicengland.org.uk"/>
    <skos:scopeNote xml:lang="en">Single-engine, single-seat fighter manufactured by Messerschmitt. First used as part of Germany's Condor legion during the Spanish Civil War, the 'one-o-nine' was the Luftwaffe's most widely used fighter seeing service throughout World War II.</skos:scopeNote>
    <dcterms:issued rdf:datatype="http://www.w3.org/2001/XMLSchema#dateTime">2019-03-26T16:45:43</dcterms:issued>
    <skos:broader rdf:resource="http://purl.org/heritagedata/schemes/225/concepts/111402"/>
    <skos:prefLabel xml:lang="en">Me109</skos:prefLabel>
    <skos:broader rdf:resource="http://purl.org/heritagedata/schemes/225/concepts/118653"/>
    <cc:attributionName xml:lang="en">Historic England</cc:attributionName>
    <cc:license rdf:resource="http://creativecommons.org/licenses/by/3.0"/>
    <skos:inScheme rdf:resource="http://purl.org/heritagedata/schemes/225"/>
    <cc:attributionURL rdf:resource="http://www.historicengland.org.uk"/>
    <dcterms:identifier>http://purl.org/heritagedata/schemes/225/concepts/111333</dcterms:identifier>
  </rdf:Description>
  <rdf:Description rdf:about="http://purl.org/heritagedata/schemes/225/concepts/111357">
    <cc:attributionName xml:lang="en">Historic England</cc:attributionName>
    <dcterms:identifier>http://purl.org/heritagedata/schemes/225/concepts/111357</dcterms:identifier>
    <dcterms:issued rdf:datatype="http://www.w3.org/2001/XMLSchema#dateTime">2019-03-26T16:45:43</dcterms:issued>
    <skos:narrower rdf:resource="http://purl.org/heritagedata/schemes/225/concepts/136532"/>
    <skos:prefLabel xml:lang="en">Bristol</skos:prefLabel>
    <skos:narrower rdf:resource="http://purl.org/heritagedata/schemes/225/concepts/111429"/>
    <skos:narrower rdf:resource="http://purl.org/heritagedata/schemes/225/concepts/138541"/>
    <dcterms:publisher rdf:resource="http://www.historicengland.org.uk"/>
    <skos:narrower rdf:resource="http://purl.org/heritagedata/schemes/225/concepts/133195"/>
    <skos:narrower rdf:resource="http://purl.org/heritagedata/schemes/225/concepts/111428"/>
    <skos:scopeNote xml:lang="en">The Bristol Aeroplane Co., Ltd.. Founded in 1910 by Sir George White, a pioneer of electric tramways. The company had previously been The British and Colonial Aeroplane Co., Ltd..</skos:scopeNote>
    <skos:broader rdf:resource="http://purl.org/heritagedata/schemes/225/concepts/111358"/>
    <cc:license rdf:resource="http://creativecommons.org/licenses/by/3.0"/>
    <rdf:type rdf:resource="http://www.w3.org/2004/02/skos/core#Concept"/>
    <cc:attributionURL rdf:resource="http://www.historicengland.org.uk"/>
    <skos:inScheme rdf:resource="http://purl.org/heritagedata/schemes/225"/>
  </rdf:Description>
  <rdf:Description rdf:about="http://purl.org/heritagedata/schemes/225/concepts/135851">
    <skos:scopeNote xml:lang="en">An aircraft, usually towed or radio-controlled, designed for use as an air-to-air, or ground-to-air, gunnery target.</skos:scopeNote>
    <dcterms:identifier>http://purl.org/heritagedata/schemes/225/concepts/135851</dcterms:identifier>
    <cc:license rdf:resource="http://creativecommons.org/licenses/by/3.0"/>
    <cc:attributionName xml:lang="en">Historic England</cc:attributionName>
    <cc:attributionURL rdf:resource="http://www.historicengland.org.uk"/>
    <skos:inScheme rdf:resource="http://purl.org/heritagedata/schemes/225"/>
    <rdf:type rdf:resource="http://www.w3.org/2004/02/skos/core#Concept"/>
    <dcterms:issued rdf:datatype="http://www.w3.org/2001/XMLSchema#dateTime">2019-03-26T16:45:43</dcterms:issued>
    <dcterms:publisher rdf:resource="http://www.historicengland.org.uk"/>
    <skos:broader rdf:resource="http://purl.org/heritagedata/schemes/225/concepts/111394"/>
    <skos:prefLabel xml:lang="en">Target</skos:prefLabel>
  </rdf:Description>
  <rdf:Description rdf:about="http://purl.org/heritagedata/schemes/225/concepts/167015">
    <dcterms:issued rdf:datatype="http://www.w3.org/2001/XMLSchema#dateTime">2019-03-26T16:45:43</dcterms:issued>
    <dcterms:publisher rdf:resource="http://www.historicengland.org.uk"/>
    <skos:broader rdf:resource="http://purl.org/heritagedata/schemes/225/concepts/111424"/>
    <skos:broader rdf:resource="http://purl.org/heritagedata/schemes/225/concepts/111415"/>
    <dcterms:identifier>http://purl.org/heritagedata/schemes/225/concepts/167015</dcterms:identifier>
    <cc:attributionName xml:lang="en">Historic England</cc:attributionName>
    <cc:attributionURL rdf:resource="http://www.historicengland.org.uk"/>
    <skos:inScheme rdf:resource="http://purl.org/heritagedata/schemes/225"/>
    <cc:license rdf:resource="http://creativecommons.org/licenses/by/3.0"/>
    <skos:prefLabel xml:lang="en">W10</skos:prefLabel>
    <skos:broader rdf:resource="http://purl.org/heritagedata/schemes/225/concepts/111403"/>
    <rdf:type rdf:resource="http://www.w3.org/2004/02/skos/core#Concept"/>
    <skos:scopeNote xml:lang="en">A British medium-range biplane airliner designed and built by Handley Page in 1921. A twin-engined variant of the Handley Page W series (W8, W9), retired in 1931. Built for Imperial Airways (4 units built).</skos:scopeNote>
  </rdf:Description>
  <rdf:Description rdf:about="http://purl.org/heritagedata/schemes/225/concepts/137190">
    <skos:narrower rdf:resource="http://purl.org/heritagedata/schemes/225/concepts/140425"/>
    <skos:narrower rdf:resource="http://purl.org/heritagedata/schemes/225/concepts/111422"/>
    <skos:narrower rdf:resource="http://purl.org/heritagedata/schemes/225/concepts/125553"/>
    <skos:narrower rdf:resource="http://purl.org/heritagedata/schemes/225/concepts/141296"/>
    <rdf:type rdf:resource="http://www.w3.org/2004/02/skos/core#Concept"/>
    <skos:narrower rdf:resource="http://purl.org/heritagedata/schemes/225/concepts/140095"/>
    <dcterms:issued rdf:datatype="http://www.w3.org/2001/XMLSchema#dateTime">2019-03-26T16:45:43</dcterms:issued>
    <skos:inScheme rdf:resource="http://purl.org/heritagedata/schemes/225"/>
    <cc:attributionURL rdf:resource="http://www.historicengland.org.uk"/>
    <skos:narrower rdf:resource="http://purl.org/heritagedata/schemes/225/concepts/125554"/>
    <cc:attributionName xml:lang="en">Historic England</cc:attributionName>
    <skos:narrower rdf:resource="http://purl.org/heritagedata/schemes/225/concepts/137237"/>
    <skos:narrower rdf:resource="http://purl.org/heritagedata/schemes/225/concepts/125533"/>
    <cc:license rdf:resource="http://creativecommons.org/licenses/by/3.0"/>
    <dcterms:publisher rdf:resource="http://www.historicengland.org.uk"/>
    <skos:prefLabel xml:lang="en">Heavy Bomber</skos:prefLabel>
    <skos:narrower rdf:resource="http://purl.org/heritagedata/schemes/225/concepts/125573"/>
    <skos:narrower rdf:resource="http://purl.org/heritagedata/schemes/225/concepts/111416"/>
    <skos:narrower rdf:resource="http://purl.org/heritagedata/schemes/225/concepts/140424"/>
    <skos:broader rdf:resource="http://purl.org/heritagedata/schemes/225/concepts/111398"/>
    <skos:narrower rdf:resource="http://purl.org/heritagedata/schemes/225/concepts/111377"/>
    <skos:narrower rdf:resource="http://purl.org/heritagedata/schemes/225/concepts/111367"/>
    <dcterms:identifier>http://purl.org/heritagedata/schemes/225/concepts/137190</dcterms:identifier>
    <skos:scopeNote xml:lang="en">Long-range, usually four-engined, bomber designed to carry a large bomb payload.</skos:scopeNote>
  </rdf:Description>
  <rdf:Description rdf:about="http://purl.org/heritagedata/schemes/225/concepts/111443">
    <cc:attributionName xml:lang="en">Historic England</cc:attributionName>
    <dcterms:identifier>http://purl.org/heritagedata/schemes/225/concepts/111443</dcterms:identifier>
    <skos:inScheme rdf:resource="http://purl.org/heritagedata/schemes/225"/>
    <rdf:type rdf:resource="http://www.w3.org/2004/02/skos/core#Concept"/>
    <skos:prefLabel xml:lang="en">Battle</skos:prefLabel>
    <dcterms:issued rdf:datatype="http://www.w3.org/2001/XMLSchema#dateTime">2019-03-26T16:45:43</dcterms:issued>
    <cc:attributionURL rdf:resource="http://www.historicengland.org.uk"/>
    <dcterms:publisher rdf:resource="http://www.historicengland.org.uk"/>
    <cc:license rdf:resource="http://creativecommons.org/licenses/by/3.0"/>
    <skos:broader rdf:resource="http://purl.org/heritagedata/schemes/225/concepts/111402"/>
    <skos:broader rdf:resource="http://purl.org/heritagedata/schemes/225/concepts/111441"/>
    <skos:scopeNote xml:lang="en">British three-seat, single-engine light bomber. All metal in construction, this monoplane had a 1000 lb bomb load.</skos:scopeNote>
    <skos:broader rdf:resource="http://purl.org/heritagedata/schemes/225/concepts/137189"/>
  </rdf:Description>
  <rdf:Description rdf:about="http://purl.org/heritagedata/schemes/225/concepts/137229">
    <skos:broader rdf:resource="http://purl.org/heritagedata/schemes/225/concepts/133198"/>
    <cc:license rdf:resource="http://creativecommons.org/licenses/by/3.0"/>
    <cc:attributionName xml:lang="en">Historic England</cc:attributionName>
    <cc:attributionURL rdf:resource="http://www.historicengland.org.uk"/>
    <skos:inScheme rdf:resource="http://purl.org/heritagedata/schemes/225"/>
    <skos:scopeNote xml:lang="en">Three-seat tactical support aircraft. Entering service with the US 9th Air Force in 1944, the Invader had a bomb load of 4,000 lbs and was later used as a conventional medium bomber.</skos:scopeNote>
    <skos:broader rdf:resource="http://purl.org/heritagedata/schemes/225/concepts/111402"/>
    <rdf:type rdf:resource="http://www.w3.org/2004/02/skos/core#Concept"/>
    <dcterms:identifier>http://purl.org/heritagedata/schemes/225/concepts/137229</dcterms:identifier>
    <dcterms:issued rdf:datatype="http://www.w3.org/2001/XMLSchema#dateTime">2019-03-26T16:45:43</dcterms:issued>
    <dcterms:publisher rdf:resource="http://www.historicengland.org.uk"/>
    <skos:broader rdf:resource="http://purl.org/heritagedata/schemes/225/concepts/139626"/>
    <skos:prefLabel xml:lang="en">Invader</skos:prefLabel>
  </rdf:Description>
  <rdf:Description rdf:about="http://purl.org/heritagedata/schemes/225/concepts/136530">
    <dcterms:identifier>http://purl.org/heritagedata/schemes/225/concepts/136530</dcterms:identifier>
    <skos:prefLabel xml:lang="en">Henley</skos:prefLabel>
    <skos:broader rdf:resource="http://purl.org/heritagedata/schemes/225/concepts/111359"/>
    <cc:license rdf:resource="http://creativecommons.org/licenses/by/3.0"/>
    <cc:attributionURL rdf:resource="http://www.historicengland.org.uk"/>
    <skos:broader rdf:resource="http://purl.org/heritagedata/schemes/225/concepts/135751"/>
    <skos:broader rdf:resource="http://purl.org/heritagedata/schemes/225/concepts/111402"/>
    <dcterms:issued rdf:datatype="http://www.w3.org/2001/XMLSchema#dateTime">2019-03-26T16:45:43</dcterms:issued>
    <skos:scopeNote xml:lang="en">Originally designed as a light bomber but diverted for use as a high speed target tug to replace out-dated biplanes.</skos:scopeNote>
    <rdf:type rdf:resource="http://www.w3.org/2004/02/skos/core#Concept"/>
    <skos:inScheme rdf:resource="http://purl.org/heritagedata/schemes/225"/>
    <cc:attributionName xml:lang="en">Historic England</cc:attributionName>
    <dcterms:publisher rdf:resource="http://www.historicengland.org.uk"/>
  </rdf:Description>
  <rdf:Description rdf:about="http://purl.org/heritagedata/schemes/225/concepts/136592">
    <cc:license rdf:resource="http://creativecommons.org/licenses/by/3.0"/>
    <dcterms:publisher rdf:resource="http://www.historicengland.org.uk"/>
    <dcterms:identifier>http://purl.org/heritagedata/schemes/225/concepts/136592</dcterms:identifier>
    <skos:inScheme rdf:resource="http://purl.org/heritagedata/schemes/225"/>
    <skos:prefLabel xml:lang="en">Magister</skos:prefLabel>
    <skos:broader rdf:resource="http://purl.org/heritagedata/schemes/225/concepts/111401"/>
    <cc:attributionName xml:lang="en">Historic England</cc:attributionName>
    <skos:scopeNote xml:lang="en">Miles M.14 Magister. Single-engine, two-crew training and communications aircraft. Spruce and plywood in construction, with open cockpits and a fixed landing gear, served between 1937 and 1945.</skos:scopeNote>
    <skos:broader rdf:resource="http://purl.org/heritagedata/schemes/225/concepts/111402"/>
    <rdf:type rdf:resource="http://www.w3.org/2004/02/skos/core#Concept"/>
    <skos:broader rdf:resource="http://purl.org/heritagedata/schemes/225/concepts/133205"/>
    <dcterms:issued rdf:datatype="http://www.w3.org/2001/XMLSchema#dateTime">2019-03-26T16:45:43</dcterms:issued>
    <cc:attributionURL rdf:resource="http://www.historicengland.org.uk"/>
  </rdf:Description>
  <rdf:Description rdf:about="http://purl.org/heritagedata/schemes/225/concepts/137195">
    <cc:license rdf:resource="http://creativecommons.org/licenses/by/3.0"/>
    <dcterms:issued rdf:datatype="http://www.w3.org/2001/XMLSchema#dateTime">2019-03-26T16:45:43</dcterms:issued>
    <skos:prefLabel xml:lang="en">Albemarle</skos:prefLabel>
    <skos:scopeNote xml:lang="en">Originally designed as a wood and steel bomber-reconnaissance aircraft, subsequent variations served as special transports, glider tugs and paratroop carriers. Featured a tricycle-style undercarriage.</skos:scopeNote>
    <skos:broader rdf:resource="http://purl.org/heritagedata/schemes/225/concepts/111402"/>
    <cc:attributionName xml:lang="en">Historic England</cc:attributionName>
    <skos:inScheme rdf:resource="http://purl.org/heritagedata/schemes/225"/>
    <dcterms:publisher rdf:resource="http://www.historicengland.org.uk"/>
    <dcterms:identifier>http://purl.org/heritagedata/schemes/225/concepts/137195</dcterms:identifier>
    <skos:broader rdf:resource="http://purl.org/heritagedata/schemes/225/concepts/135730"/>
    <skos:broader rdf:resource="http://purl.org/heritagedata/schemes/225/concepts/111398"/>
    <rdf:type rdf:resource="http://www.w3.org/2004/02/skos/core#Concept"/>
    <cc:attributionURL rdf:resource="http://www.historicengland.org.uk"/>
    <skos:broader rdf:resource="http://purl.org/heritagedata/schemes/225/concepts/111376"/>
  </rdf:Description>
  <rdf:Description rdf:about="http://purl.org/heritagedata/schemes/225/concepts/135850">
    <skos:prefLabel xml:lang="en">Queen Bee</skos:prefLabel>
    <ns1:related rdf:resource="http://purl.org/heritagedata/schemes/225/concepts/135586"/>
    <skos:inScheme rdf:resource="http://purl.org/heritagedata/schemes/225"/>
    <dcterms:identifier>http://purl.org/heritagedata/schemes/225/concepts/135850</dcterms:identifier>
    <skos:scopeNote xml:lang="en">A radio-controlled target tug version of the Tiger Moth used for target practice. 380 were built for the RAF.</skos:scopeNote>
    <dcterms:publisher rdf:resource="http://www.historicengland.org.uk"/>
    <cc:attributionName xml:lang="en">Historic England</cc:attributionName>
    <skos:broader rdf:resource="http://purl.org/heritagedata/schemes/225/concepts/111368"/>
    <dcterms:issued rdf:datatype="http://www.w3.org/2001/XMLSchema#dateTime">2019-03-26T16:45:43</dcterms:issued>
    <skos:broader rdf:resource="http://purl.org/heritagedata/schemes/225/concepts/111403"/>
    <cc:attributionURL rdf:resource="http://www.historicengland.org.uk"/>
    <rdf:type rdf:resource="http://www.w3.org/2004/02/skos/core#Concept"/>
    <skos:broader rdf:resource="http://purl.org/heritagedata/schemes/225/concepts/135751"/>
    <cc:license rdf:resource="http://creativecommons.org/licenses/by/3.0"/>
  </rdf:Description>
  <rdf:Description rdf:about="http://purl.org/heritagedata/schemes/225/concepts/111374">
    <dcterms:publisher rdf:resource="http://www.historicengland.org.uk"/>
    <rdf:type rdf:resource="http://www.w3.org/2004/02/skos/core#Concept"/>
    <cc:license rdf:resource="http://creativecommons.org/licenses/by/3.0"/>
    <skos:narrower rdf:resource="http://purl.org/heritagedata/schemes/225/concepts/136510"/>
    <skos:scopeNote xml:lang="en">Blackburn Aircraft, Ltd., founded by Robert Blackburn, who produced his first aircraft in 1910. Specialised in the production of torpedo-carrying aircraft.</skos:scopeNote>
    <skos:prefLabel xml:lang="en">Blackburn</skos:prefLabel>
    <skos:broader rdf:resource="http://purl.org/heritagedata/schemes/225/concepts/111358"/>
    <cc:attributionName xml:lang="en">Historic England</cc:attributionName>
    <skos:narrower rdf:resource="http://purl.org/heritagedata/schemes/225/concepts/136251"/>
    <skos:inScheme rdf:resource="http://purl.org/heritagedata/schemes/225"/>
    <skos:narrower rdf:resource="http://purl.org/heritagedata/schemes/225/concepts/133194"/>
    <dcterms:identifier>http://purl.org/heritagedata/schemes/225/concepts/111374</dcterms:identifier>
    <skos:narrower rdf:resource="http://purl.org/heritagedata/schemes/225/concepts/136531"/>
    <cc:attributionURL rdf:resource="http://www.historicengland.org.uk"/>
    <skos:narrower rdf:resource="http://purl.org/heritagedata/schemes/225/concepts/111375"/>
    <skos:narrower rdf:resource="http://purl.org/heritagedata/schemes/225/concepts/137196"/>
    <dcterms:issued rdf:datatype="http://www.w3.org/2001/XMLSchema#dateTime">2019-03-26T16:45:43</dcterms:issued>
  </rdf:Description>
  <rdf:Description rdf:about="http://purl.org/heritagedata/schemes/225/concepts/137203">
    <skos:broader rdf:resource="http://purl.org/heritagedata/schemes/225/concepts/111402"/>
    <ns1:related rdf:resource="http://purl.org/heritagedata/schemes/225/concepts/133173"/>
    <dcterms:issued rdf:datatype="http://www.w3.org/2001/XMLSchema#dateTime">2019-03-26T16:45:43</dcterms:issued>
    <dcterms:identifier>http://purl.org/heritagedata/schemes/225/concepts/137203</dcterms:identifier>
    <cc:attributionName xml:lang="en">Historic England</cc:attributionName>
    <cc:license rdf:resource="http://creativecommons.org/licenses/by/3.0"/>
    <skos:inScheme rdf:resource="http://purl.org/heritagedata/schemes/225"/>
    <cc:attributionURL rdf:resource="http://www.historicengland.org.uk"/>
    <skos:scopeNote xml:lang="en">Twin-engined, four-seat medium bomber. A re-engined variant of  the Hampden, less than 200 were built but never became operational due to engine unreliability. Some were converted to Hampdens.</skos:scopeNote>
    <skos:prefLabel xml:lang="en">Hereford</skos:prefLabel>
    <skos:broader rdf:resource="http://purl.org/heritagedata/schemes/225/concepts/139626"/>
    <dcterms:publisher rdf:resource="http://www.historicengland.org.uk"/>
    <skos:broader rdf:resource="http://purl.org/heritagedata/schemes/225/concepts/111415"/>
    <rdf:type rdf:resource="http://www.w3.org/2004/02/skos/core#Concept"/>
  </rdf:Description>
  <rdf:Description rdf:about="http://purl.org/heritagedata/schemes/225/concepts/137194">
    <cc:license rdf:resource="http://creativecommons.org/licenses/by/3.0"/>
    <cc:attributionName xml:lang="en">Historic England</cc:attributionName>
    <cc:attributionURL rdf:resource="http://www.historicengland.org.uk"/>
    <skos:inScheme rdf:resource="http://purl.org/heritagedata/schemes/225"/>
    <skos:broader rdf:resource="http://purl.org/heritagedata/schemes/225/concepts/111393"/>
    <skos:prefLabel xml:lang="en">Airship</skos:prefLabel>
    <dcterms:issued rdf:datatype="http://www.w3.org/2001/XMLSchema#dateTime">2019-03-26T16:45:43</dcterms:issued>
    <rdf:type rdf:resource="http://www.w3.org/2004/02/skos/core#Concept"/>
    <dcterms:identifier>http://purl.org/heritagedata/schemes/225/concepts/137194</dcterms:identifier>
    <dcterms:publisher rdf:resource="http://www.historicengland.org.uk"/>
    <skos:scopeNote xml:lang="en">An aircraft lifted by gas bags, containing hydrogen or helium, but propelled by engines. Also known as a dirigible balloon, firm and streamlined in shape and incapable of high speeds. Used extensively during World War One.</skos:scopeNote>
    <skos:narrower rdf:resource="http://purl.org/heritagedata/schemes/225/concepts/144618"/>
  </rdf:Description>
  <rdf:Description rdf:about="http://purl.org/heritagedata/schemes/225/concepts/138542">
    <rdf:type rdf:resource="http://www.w3.org/2004/02/skos/core#Concept"/>
    <dcterms:issued rdf:datatype="http://www.w3.org/2001/XMLSchema#dateTime">2019-03-26T16:45:43</dcterms:issued>
    <skos:prefLabel xml:lang="en">De Havilland DH18B</skos:prefLabel>
    <dcterms:identifier>http://purl.org/heritagedata/schemes/225/concepts/138542</dcterms:identifier>
    <skos:scopeNote xml:lang="en">Large, single-engine, eight passenger airliner biplane.</skos:scopeNote>
    <skos:broader rdf:resource="http://purl.org/heritagedata/schemes/225/concepts/111424"/>
    <skos:broader rdf:resource="http://purl.org/heritagedata/schemes/225/concepts/111368"/>
    <cc:license rdf:resource="http://creativecommons.org/licenses/by/3.0"/>
    <cc:attributionName xml:lang="en">Historic England</cc:attributionName>
    <cc:attributionURL rdf:resource="http://www.historicengland.org.uk"/>
    <skos:inScheme rdf:resource="http://purl.org/heritagedata/schemes/225"/>
    <skos:broader rdf:resource="http://purl.org/heritagedata/schemes/225/concepts/111403"/>
    <dcterms:publisher rdf:resource="http://www.historicengland.org.uk"/>
  </rdf:Description>
  <rdf:Description rdf:about="http://purl.org/heritagedata/schemes/225/concepts/136524">
    <skos:prefLabel xml:lang="en">Aldershot</skos:prefLabel>
    <dcterms:issued rdf:datatype="http://www.w3.org/2001/XMLSchema#dateTime">2019-03-26T16:45:43</dcterms:issued>
    <skos:broader rdf:resource="http://purl.org/heritagedata/schemes/225/concepts/111403"/>
    <rdf:type rdf:resource="http://www.w3.org/2004/02/skos/core#Concept"/>
    <skos:inScheme rdf:resource="http://purl.org/heritagedata/schemes/225"/>
    <cc:attributionName xml:lang="en">Historic England</cc:attributionName>
    <dcterms:publisher rdf:resource="http://www.historicengland.org.uk"/>
    <skos:broader rdf:resource="http://purl.org/heritagedata/schemes/225/concepts/111355"/>
    <dcterms:identifier>http://purl.org/heritagedata/schemes/225/concepts/136524</dcterms:identifier>
    <cc:license rdf:resource="http://creativecommons.org/licenses/by/3.0"/>
    <cc:attributionURL rdf:resource="http://www.historicengland.org.uk"/>
    <skos:broader rdf:resource="http://purl.org/heritagedata/schemes/225/concepts/111398"/>
    <skos:scopeNote xml:lang="en">A single-engine, heavy, long range, three to five-crew day bomber. Served only with 99 Squadron RAF, 1924-5.</skos:scopeNote>
  </rdf:Description>
  <rdf:Description rdf:about="http://purl.org/heritagedata/schemes/225/concepts/135729">
    <skos:broader rdf:resource="http://purl.org/heritagedata/schemes/225/concepts/135730"/>
    <skos:broader rdf:resource="http://purl.org/heritagedata/schemes/225/concepts/111421"/>
    <dcterms:identifier>http://purl.org/heritagedata/schemes/225/concepts/135729</dcterms:identifier>
    <cc:license rdf:resource="http://creativecommons.org/licenses/by/3.0"/>
    <rdf:type rdf:resource="http://www.w3.org/2004/02/skos/core#Concept"/>
    <cc:attributionURL rdf:resource="http://www.historicengland.org.uk"/>
    <skos:inScheme rdf:resource="http://purl.org/heritagedata/schemes/225"/>
    <dcterms:issued rdf:datatype="http://www.w3.org/2001/XMLSchema#dateTime">2019-03-26T16:45:43</dcterms:issued>
    <skos:broader rdf:resource="http://purl.org/heritagedata/schemes/225/concepts/111395"/>
    <skos:prefLabel xml:lang="en">Sunderland</skos:prefLabel>
    <skos:broader rdf:resource="http://purl.org/heritagedata/schemes/225/concepts/111402"/>
    <dcterms:publisher rdf:resource="http://www.historicengland.org.uk"/>
    <skos:scopeNote xml:lang="en">Four-engine, ten-crew, long-range maritime reconnaissance and anti-submarine aircraft. Developed from the Short C-class Empire airliner. All metal in construction, entered RAF Coastal Command service in 1938.</skos:scopeNote>
    <cc:attributionName xml:lang="en">Historic England</cc:attributionName>
  </rdf:Description>
  <rdf:Description rdf:about="http://purl.org/heritagedata/schemes/225/concepts/138537">
    <cc:attributionURL rdf:resource="http://www.historicengland.org.uk"/>
    <skos:scopeNote xml:lang="en">Developed from the DH4, featured the pilot and gunner cockpits in closer proximity, but suffered from engine reliability problems. Also known as the Ninak, saw service from 1918 to 1931.</skos:scopeNote>
    <skos:broader rdf:resource="http://purl.org/heritagedata/schemes/225/concepts/111403"/>
    <rdf:type rdf:resource="http://www.w3.org/2004/02/skos/core#Concept"/>
    <dcterms:publisher rdf:resource="http://www.historicengland.org.uk"/>
    <cc:attributionName xml:lang="en">Historic England</cc:attributionName>
    <dcterms:issued rdf:datatype="http://www.w3.org/2001/XMLSchema#dateTime">2019-03-26T16:45:43</dcterms:issued>
    <skos:broader rdf:resource="http://purl.org/heritagedata/schemes/225/concepts/136512"/>
    <dcterms:identifier>http://purl.org/heritagedata/schemes/225/concepts/138537</dcterms:identifier>
    <cc:license rdf:resource="http://creativecommons.org/licenses/by/3.0"/>
    <skos:prefLabel xml:lang="en">Airco DH9</skos:prefLabel>
    <skos:inScheme rdf:resource="http://purl.org/heritagedata/schemes/225"/>
    <skos:broader rdf:resource="http://purl.org/heritagedata/schemes/225/concepts/111398"/>
  </rdf:Description>
  <rdf:Description rdf:about="http://purl.org/heritagedata/schemes/225/concepts/134996">
    <cc:attributionName xml:lang="en">Historic England</cc:attributionName>
    <skos:broader rdf:resource="http://purl.org/heritagedata/schemes/225/concepts/111402"/>
    <rdf:type rdf:resource="http://www.w3.org/2004/02/skos/core#Concept"/>
    <skos:broader rdf:resource="http://purl.org/heritagedata/schemes/225/concepts/140074"/>
    <dcterms:issued rdf:datatype="http://www.w3.org/2001/XMLSchema#dateTime">2019-03-26T16:45:43</dcterms:issued>
    <cc:attributionURL rdf:resource="http://www.historicengland.org.uk"/>
    <cc:license rdf:resource="http://creativecommons.org/licenses/by/3.0"/>
    <skos:broader rdf:resource="http://purl.org/heritagedata/schemes/225/concepts/135730"/>
    <skos:inScheme rdf:resource="http://purl.org/heritagedata/schemes/225"/>
    <skos:broader rdf:resource="http://purl.org/heritagedata/schemes/225/concepts/136511"/>
    <skos:broader rdf:resource="http://purl.org/heritagedata/schemes/225/concepts/111356"/>
    <skos:broader rdf:resource="http://purl.org/heritagedata/schemes/225/concepts/134997"/>
    <dcterms:identifier>http://purl.org/heritagedata/schemes/225/concepts/134996</dcterms:identifier>
    <skos:prefLabel xml:lang="en">He115</skos:prefLabel>
    <dcterms:publisher rdf:resource="http://www.historicengland.org.uk"/>
    <skos:scopeNote xml:lang="en">Three-seat, twin-engined minelaying, torpedo-bombing and reconnaissance twin-float seaplane. First flown in 1936, in 1938 it set eight world speed records for its class in various range and payload categories.</skos:scopeNote>
  </rdf:Description>
  <rdf:Description rdf:about="http://purl.org/heritagedata/schemes/225/concepts/140095">
    <skos:broader rdf:resource="http://purl.org/heritagedata/schemes/225/concepts/111403"/>
    <rdf:type rdf:resource="http://www.w3.org/2004/02/skos/core#Concept"/>
    <dcterms:identifier>http://purl.org/heritagedata/schemes/225/concepts/140095</dcterms:identifier>
    <dcterms:publisher rdf:resource="http://www.historicengland.org.uk"/>
    <skos:prefLabel xml:lang="en">Gotha GV</skos:prefLabel>
    <skos:broader rdf:resource="http://purl.org/heritagedata/schemes/225/concepts/137190"/>
    <cc:attributionName xml:lang="en">Historic England</cc:attributionName>
    <cc:attributionURL rdf:resource="http://www.historicengland.org.uk"/>
    <skos:inScheme rdf:resource="http://purl.org/heritagedata/schemes/225"/>
    <cc:license rdf:resource="http://creativecommons.org/licenses/by/3.0"/>
    <skos:broader rdf:resource="http://purl.org/heritagedata/schemes/225/concepts/140097"/>
    <skos:scopeNote xml:lang="en">A World War One German three-crew, twin-engined, long range heavy bomber biplane manufactured by Gothaer Waggonfabrik A.G..  Entering service in 1917, this aircraft incorporated a ventral tunnel allowing the gunner to shoot downwards and to the rear.</skos:scopeNote>
    <dcterms:issued rdf:datatype="http://www.w3.org/2001/XMLSchema#dateTime">2019-03-26T16:45:43</dcterms:issued>
  </rdf:Description>
  <rdf:Description rdf:about="http://purl.org/heritagedata/schemes/225/concepts/137206">
    <dcterms:issued rdf:datatype="http://www.w3.org/2001/XMLSchema#dateTime">2019-03-26T16:45:43</dcterms:issued>
    <dcterms:publisher rdf:resource="http://www.historicengland.org.uk"/>
    <skos:broader rdf:resource="http://purl.org/heritagedata/schemes/225/concepts/137205"/>
    <skos:prefLabel xml:lang="en">Proctor</skos:prefLabel>
    <dcterms:identifier>http://purl.org/heritagedata/schemes/225/concepts/137206</dcterms:identifier>
    <cc:attributionName xml:lang="en">Historic England</cc:attributionName>
    <skos:scopeNote xml:lang="en">Single-engine, spruce and plywood, fabric-covered training and communications low-wing monoplane. Served from 1939 to 1950.</skos:scopeNote>
    <cc:license rdf:resource="http://creativecommons.org/licenses/by/3.0"/>
    <skos:broader rdf:resource="http://purl.org/heritagedata/schemes/225/concepts/111401"/>
    <cc:attributionURL rdf:resource="http://www.historicengland.org.uk"/>
    <skos:inScheme rdf:resource="http://purl.org/heritagedata/schemes/225"/>
    <skos:broader rdf:resource="http://purl.org/heritagedata/schemes/225/concepts/111402"/>
    <rdf:type rdf:resource="http://www.w3.org/2004/02/skos/core#Concept"/>
  </rdf:Description>
  <rdf:Description rdf:about="http://purl.org/heritagedata/schemes/225/concepts/136511">
    <skos:narrower rdf:resource="http://purl.org/heritagedata/schemes/225/concepts/136510"/>
    <dcterms:publisher rdf:resource="http://www.historicengland.org.uk"/>
    <rdf:type rdf:resource="http://www.w3.org/2004/02/skos/core#Concept"/>
    <skos:scopeNote xml:lang="en">Aircraft designed for the carrying and dropping of torpedoes.</skos:scopeNote>
    <skos:narrower rdf:resource="http://purl.org/heritagedata/schemes/225/concepts/136532"/>
    <skos:narrower rdf:resource="http://purl.org/heritagedata/schemes/225/concepts/137219"/>
    <cc:attributionName xml:lang="en">Historic England</cc:attributionName>
    <cc:license rdf:resource="http://creativecommons.org/licenses/by/3.0"/>
    <cc:attributionURL rdf:resource="http://www.historicengland.org.uk"/>
    <skos:narrower rdf:resource="http://purl.org/heritagedata/schemes/225/concepts/140140"/>
    <skos:prefLabel xml:lang="en">Torpedo Bomber</skos:prefLabel>
    <skos:narrower rdf:resource="http://purl.org/heritagedata/schemes/225/concepts/137196"/>
    <dcterms:identifier>http://purl.org/heritagedata/schemes/225/concepts/136511</dcterms:identifier>
    <dcterms:issued rdf:datatype="http://www.w3.org/2001/XMLSchema#dateTime">2019-03-26T16:45:43</dcterms:issued>
    <skos:inScheme rdf:resource="http://purl.org/heritagedata/schemes/225"/>
    <skos:broader rdf:resource="http://purl.org/heritagedata/schemes/225/concepts/111398"/>
    <skos:narrower rdf:resource="http://purl.org/heritagedata/schemes/225/concepts/111375"/>
    <skos:narrower rdf:resource="http://purl.org/heritagedata/schemes/225/concepts/134996"/>
    <skos:narrower rdf:resource="http://purl.org/heritagedata/schemes/225/concepts/137197"/>
  </rdf:Description>
  <rdf:Description rdf:about="http://purl.org/heritagedata/schemes/225/concepts/141257">
    <cc:license rdf:resource="http://creativecommons.org/licenses/by/3.0"/>
    <cc:attributionName xml:lang="en">Historic England</cc:attributionName>
    <dcterms:identifier>http://purl.org/heritagedata/schemes/225/concepts/141257</dcterms:identifier>
    <skos:inScheme rdf:resource="http://purl.org/heritagedata/schemes/225"/>
    <skos:prefLabel xml:lang="en">MkVIII</skos:prefLabel>
    <dcterms:publisher rdf:resource="http://www.historicengland.org.uk"/>
    <rdf:type rdf:resource="http://www.w3.org/2004/02/skos/core#Concept"/>
    <dcterms:issued rdf:datatype="http://www.w3.org/2001/XMLSchema#dateTime">2019-03-26T16:45:43</dcterms:issued>
    <skos:broader rdf:resource="http://purl.org/heritagedata/schemes/225/concepts/141131"/>
    <skos:scopeNote xml:lang="en">Mark 7 or the seventh variant of an aircraft with its associated modifications.</skos:scopeNote>
    <cc:attributionURL rdf:resource="http://www.historicengland.org.uk"/>
  </rdf:Description>
  <rdf:Description rdf:about="http://purl.org/heritagedata/schemes/225/concepts/111359">
    <skos:narrower rdf:resource="http://purl.org/heritagedata/schemes/225/concepts/111360"/>
    <skos:narrower rdf:resource="http://purl.org/heritagedata/schemes/225/concepts/134998"/>
    <skos:prefLabel xml:lang="en">Hawker</skos:prefLabel>
    <skos:broader rdf:resource="http://purl.org/heritagedata/schemes/225/concepts/111358"/>
    <skos:narrower rdf:resource="http://purl.org/heritagedata/schemes/225/concepts/136530"/>
    <rdf:type rdf:resource="http://www.w3.org/2004/02/skos/core#Concept"/>
    <cc:attributionURL rdf:resource="http://www.historicengland.org.uk"/>
    <skos:narrower rdf:resource="http://purl.org/heritagedata/schemes/225/concepts/141207"/>
    <skos:scopeNote xml:lang="en">Hawker Aircraft, Ltd., established 1933 to succeed the H. G. Hawker Engineering Co., Ltd., which had been formed in 1920 as the result of the voluntary liquidation of the renowned Sopwith concern.</skos:scopeNote>
    <skos:narrower rdf:resource="http://purl.org/heritagedata/schemes/225/concepts/137204"/>
    <skos:narrower rdf:resource="http://purl.org/heritagedata/schemes/225/concepts/167009"/>
    <dcterms:publisher rdf:resource="http://www.historicengland.org.uk"/>
    <dcterms:identifier>http://purl.org/heritagedata/schemes/225/concepts/111359</dcterms:identifier>
    <cc:license rdf:resource="http://creativecommons.org/licenses/by/3.0"/>
    <cc:attributionName xml:lang="en">Historic England</cc:attributionName>
    <skos:inScheme rdf:resource="http://purl.org/heritagedata/schemes/225"/>
    <dcterms:issued rdf:datatype="http://www.w3.org/2001/XMLSchema#dateTime">2019-03-26T16:45:43</dcterms:issued>
    <skos:narrower rdf:resource="http://purl.org/heritagedata/schemes/225/concepts/169973"/>
  </rdf:Description>
  <rdf:Description rdf:about="http://purl.org/heritagedata/schemes/225/concepts/111401">
    <skos:narrower rdf:resource="http://purl.org/heritagedata/schemes/225/concepts/136526"/>
    <skos:prefLabel xml:lang="en">Trainer</skos:prefLabel>
    <skos:narrower rdf:resource="http://purl.org/heritagedata/schemes/225/concepts/137206"/>
    <skos:narrower rdf:resource="http://purl.org/heritagedata/schemes/225/concepts/133204"/>
    <skos:narrower rdf:resource="http://purl.org/heritagedata/schemes/225/concepts/111375"/>
    <cc:attributionURL rdf:resource="http://www.historicengland.org.uk"/>
    <skos:narrower rdf:resource="http://purl.org/heritagedata/schemes/225/concepts/133193"/>
    <skos:narrower rdf:resource="http://purl.org/heritagedata/schemes/225/concepts/141213"/>
    <rdf:type rdf:resource="http://www.w3.org/2004/02/skos/core#Concept"/>
    <skos:narrower rdf:resource="http://purl.org/heritagedata/schemes/225/concepts/137153"/>
    <skos:scopeNote xml:lang="en">An aircraft used for the training of pilots, sometimes fitted with dual controls for use by the instructor.</skos:scopeNote>
    <skos:narrower rdf:resource="http://purl.org/heritagedata/schemes/225/concepts/135586"/>
    <skos:narrower rdf:resource="http://purl.org/heritagedata/schemes/225/concepts/137224"/>
    <dcterms:issued rdf:datatype="http://www.w3.org/2001/XMLSchema#dateTime">2019-03-26T16:45:43</dcterms:issued>
    <skos:narrower rdf:resource="http://purl.org/heritagedata/schemes/225/concepts/136592"/>
    <skos:inScheme rdf:resource="http://purl.org/heritagedata/schemes/225"/>
    <cc:license rdf:resource="http://creativecommons.org/licenses/by/3.0"/>
    <skos:narrower rdf:resource="http://purl.org/heritagedata/schemes/225/concepts/137202"/>
    <skos:narrower rdf:resource="http://purl.org/heritagedata/schemes/225/concepts/138538"/>
    <skos:narrower rdf:resource="http://purl.org/heritagedata/schemes/225/concepts/141211"/>
    <skos:narrower rdf:resource="http://purl.org/heritagedata/schemes/225/concepts/133201"/>
    <skos:narrower rdf:resource="http://purl.org/heritagedata/schemes/225/concepts/133206"/>
    <dcterms:publisher rdf:resource="http://www.historicengland.org.uk"/>
    <dcterms:identifier>http://purl.org/heritagedata/schemes/225/concepts/111401</dcterms:identifier>
    <skos:broader rdf:resource="http://purl.org/heritagedata/schemes/225/concepts/111394"/>
    <cc:attributionName xml:lang="en">Historic England</cc:attributionName>
  </rdf:Description>
  <rdf:Description rdf:about="http://purl.org/heritagedata/schemes/225/concepts/111428">
    <cc:attributionName xml:lang="en">Historic England</cc:attributionName>
    <skos:broader rdf:resource="http://purl.org/heritagedata/schemes/225/concepts/111357"/>
    <skos:scopeNote xml:lang="en">British twin-engined light/medium bomber developed from the model 142 civil transport. Noted for its speed, this three-crew monoplane had an all-metal, stressed skin structure and a 1000lb bomb load.</skos:scopeNote>
    <rdf:type rdf:resource="http://www.w3.org/2004/02/skos/core#Concept"/>
    <dcterms:issued rdf:datatype="http://www.w3.org/2001/XMLSchema#dateTime">2019-03-26T16:45:43</dcterms:issued>
    <cc:attributionURL rdf:resource="http://www.historicengland.org.uk"/>
    <dcterms:identifier>http://purl.org/heritagedata/schemes/225/concepts/111428</dcterms:identifier>
    <skos:broader rdf:resource="http://purl.org/heritagedata/schemes/225/concepts/139626"/>
    <cc:license rdf:resource="http://creativecommons.org/licenses/by/3.0"/>
    <skos:broader rdf:resource="http://purl.org/heritagedata/schemes/225/concepts/111402"/>
    <skos:prefLabel xml:lang="en">Blenheim</skos:prefLabel>
    <dcterms:publisher rdf:resource="http://www.historicengland.org.uk"/>
    <skos:inScheme rdf:resource="http://purl.org/heritagedata/schemes/225"/>
  </rdf:Description>
  <rdf:Description rdf:about="http://purl.org/heritagedata/schemes/225/concepts/167002">
    <skos:broader rdf:resource="http://purl.org/heritagedata/schemes/225/concepts/111424"/>
    <skos:prefLabel xml:lang="en">Fokker</skos:prefLabel>
    <dcterms:identifier>http://purl.org/heritagedata/schemes/225/concepts/167002</dcterms:identifier>
    <cc:attributionName xml:lang="en">Historic England</cc:attributionName>
    <cc:attributionURL rdf:resource="http://www.historicengland.org.uk"/>
    <skos:inScheme rdf:resource="http://purl.org/heritagedata/schemes/225"/>
    <skos:broader rdf:resource="http://purl.org/heritagedata/schemes/225/concepts/111402"/>
    <dcterms:issued rdf:datatype="http://www.w3.org/2001/XMLSchema#dateTime">2019-03-26T16:45:43</dcterms:issued>
    <rdf:type rdf:resource="http://www.w3.org/2004/02/skos/core#Concept"/>
    <skos:scopeNote xml:lang="en">Dutch aircraft manufacturer named after its founder, Anthony Fokker. Set up in 1912 in Schwerin, Germany, moving to the Netherlands in 1919. The world's largest aircraft manufacturer in the late 1920s.</skos:scopeNote>
    <dcterms:publisher rdf:resource="http://www.historicengland.org.uk"/>
    <skos:broader rdf:resource="http://purl.org/heritagedata/schemes/225/concepts/111358"/>
    <skos:narrower rdf:resource="http://purl.org/heritagedata/schemes/225/concepts/167006"/>
    <cc:license rdf:resource="http://creativecommons.org/licenses/by/3.0"/>
  </rdf:Description>
  <rdf:Description rdf:about="http://purl.org/heritagedata/schemes/225/concepts/137189">
    <dcterms:publisher rdf:resource="http://www.historicengland.org.uk"/>
    <dcterms:identifier>http://purl.org/heritagedata/schemes/225/concepts/137189</dcterms:identifier>
    <cc:license rdf:resource="http://creativecommons.org/licenses/by/3.0"/>
    <skos:broader rdf:resource="http://purl.org/heritagedata/schemes/225/concepts/111398"/>
    <rdf:type rdf:resource="http://www.w3.org/2004/02/skos/core#Concept"/>
    <cc:attributionURL rdf:resource="http://www.historicengland.org.uk"/>
    <skos:narrower rdf:resource="http://purl.org/heritagedata/schemes/225/concepts/137174"/>
    <skos:prefLabel xml:lang="en">Light Bomber</skos:prefLabel>
    <skos:narrower rdf:resource="http://purl.org/heritagedata/schemes/225/concepts/111443"/>
    <dcterms:issued rdf:datatype="http://www.w3.org/2001/XMLSchema#dateTime">2019-03-26T16:45:43</dcterms:issued>
    <skos:narrower rdf:resource="http://purl.org/heritagedata/schemes/225/concepts/139374"/>
    <cc:attributionName xml:lang="en">Historic England</cc:attributionName>
    <skos:inScheme rdf:resource="http://purl.org/heritagedata/schemes/225"/>
    <skos:scopeNote xml:lang="en">High speed, short to medium-range bomber, usually powered by two engines.</skos:scopeNote>
  </rdf:Description>
  <rdf:Description rdf:about="http://purl.org/heritagedata/schemes/225/concepts/137111">
    <dcterms:identifier>http://purl.org/heritagedata/schemes/225/concepts/137111</dcterms:identifier>
    <skos:broader rdf:resource="http://purl.org/heritagedata/schemes/225/concepts/111424"/>
    <cc:license rdf:resource="http://creativecommons.org/licenses/by/3.0"/>
    <cc:attributionURL rdf:resource="http://www.historicengland.org.uk"/>
    <skos:broader rdf:resource="http://purl.org/heritagedata/schemes/225/concepts/137110"/>
    <skos:prefLabel xml:lang="en">Horsa</skos:prefLabel>
    <dcterms:issued rdf:datatype="http://www.w3.org/2001/XMLSchema#dateTime">2019-03-26T16:45:43</dcterms:issued>
    <skos:broader rdf:resource="http://purl.org/heritagedata/schemes/225/concepts/111402"/>
    <skos:scopeNote xml:lang="en">Troop and general transport glider. Almost entirely wooden in construction, many were manufactured by the furniture industry. Mk I featured a a door-ramp on the port side whilst the Mk II was fitted with a hinged nose.</skos:scopeNote>
    <rdf:type rdf:resource="http://www.w3.org/2004/02/skos/core#Concept"/>
    <skos:broader rdf:resource="http://purl.org/heritagedata/schemes/225/concepts/133200"/>
    <skos:inScheme rdf:resource="http://purl.org/heritagedata/schemes/225"/>
    <cc:attributionName xml:lang="en">Historic England</cc:attributionName>
    <dcterms:publisher rdf:resource="http://www.historicengland.org.uk"/>
  </rdf:Description>
  <rdf:Description rdf:about="http://purl.org/heritagedata/schemes/225/concepts/137224">
    <dcterms:publisher rdf:resource="http://www.historicengland.org.uk"/>
    <skos:broader rdf:resource="http://purl.org/heritagedata/schemes/225/concepts/137223"/>
    <dcterms:identifier>http://purl.org/heritagedata/schemes/225/concepts/137224</dcterms:identifier>
    <dcterms:issued rdf:datatype="http://www.w3.org/2001/XMLSchema#dateTime">2019-03-26T16:45:43</dcterms:issued>
    <skos:broader rdf:resource="http://purl.org/heritagedata/schemes/225/concepts/111402"/>
    <cc:attributionURL rdf:resource="http://www.historicengland.org.uk"/>
    <rdf:type rdf:resource="http://www.w3.org/2004/02/skos/core#Concept"/>
    <skos:prefLabel xml:lang="en">Reliant</skos:prefLabel>
    <cc:attributionName xml:lang="en">Historic England</cc:attributionName>
    <cc:license rdf:resource="http://creativecommons.org/licenses/by/3.0"/>
    <skos:scopeNote xml:lang="en">Single-engine navigation trainer and communications aircraft. Constructed of tubular steel and duralumin frame, with a duralumin and canvas covering, 500 were delivered to the FAA, serving from 1944-5.</skos:scopeNote>
    <skos:broader rdf:resource="http://purl.org/heritagedata/schemes/225/concepts/111401"/>
    <skos:inScheme rdf:resource="http://purl.org/heritagedata/schemes/225"/>
  </rdf:Description>
  <rdf:Description rdf:about="http://purl.org/heritagedata/schemes/225/concepts/133199">
    <cc:license rdf:resource="http://creativecommons.org/licenses/by/3.0"/>
    <skos:inScheme rdf:resource="http://purl.org/heritagedata/schemes/225"/>
    <skos:scopeNote xml:lang="en">American A-20 twin-engined, light, day bomber. Some supplied to the RAF and known as the Boston I. Subsequent variations adapted to night flying and re-christened the Havoc.</skos:scopeNote>
    <dcterms:publisher rdf:resource="http://www.historicengland.org.uk"/>
    <skos:broader rdf:resource="http://purl.org/heritagedata/schemes/225/concepts/133198"/>
    <skos:broader rdf:resource="http://purl.org/heritagedata/schemes/225/concepts/111398"/>
    <dcterms:identifier>http://purl.org/heritagedata/schemes/225/concepts/133199</dcterms:identifier>
    <cc:attributionName xml:lang="en">Historic England</cc:attributionName>
    <skos:broader rdf:resource="http://purl.org/heritagedata/schemes/225/concepts/111402"/>
    <rdf:type rdf:resource="http://www.w3.org/2004/02/skos/core#Concept"/>
    <dcterms:issued rdf:datatype="http://www.w3.org/2001/XMLSchema#dateTime">2019-03-26T16:45:43</dcterms:issued>
    <cc:attributionURL rdf:resource="http://www.historicengland.org.uk"/>
    <ns1:related rdf:resource="http://purl.org/heritagedata/schemes/225/concepts/137174"/>
    <skos:prefLabel xml:lang="en">Boston</skos:prefLabel>
  </rdf:Description>
  <rdf:Description rdf:about="http://purl.org/heritagedata/schemes/225/concepts/111393">
    <skos:narrower rdf:resource="http://purl.org/heritagedata/schemes/225/concepts/111396"/>
    <skos:narrower rdf:resource="http://purl.org/heritagedata/schemes/225/concepts/111403"/>
    <cc:attributionURL rdf:resource="http://www.historicengland.org.uk"/>
    <skos:narrower rdf:resource="http://purl.org/heritagedata/schemes/225/concepts/111402"/>
    <skos:scopeNote xml:lang="en">Aircraft grouped according to their physical form.</skos:scopeNote>
    <skos:inScheme rdf:resource="http://purl.org/heritagedata/schemes/225"/>
    <dcterms:issued rdf:datatype="http://www.w3.org/2001/XMLSchema#dateTime">2019-03-26T16:45:43</dcterms:issued>
    <skos:narrower rdf:resource="http://purl.org/heritagedata/schemes/225/concepts/137194"/>
    <skos:narrower rdf:resource="http://purl.org/heritagedata/schemes/225/concepts/137191"/>
    <skos:prefLabel xml:lang="en">Aircraft &lt;By Form&gt;</skos:prefLabel>
    <dcterms:identifier>http://purl.org/heritagedata/schemes/225/concepts/111393</dcterms:identifier>
    <dcterms:publisher rdf:resource="http://www.historicengland.org.uk"/>
    <skos:broader rdf:resource="http://purl.org/heritagedata/schemes/225/concepts/123733"/>
    <rdf:type rdf:resource="http://www.w3.org/2004/02/skos/core#Concept"/>
    <cc:attributionName xml:lang="en">Historic England</cc:attributionName>
    <cc:license rdf:resource="http://creativecommons.org/licenses/by/3.0"/>
    <skos:narrower rdf:resource="http://purl.org/heritagedata/schemes/225/concepts/137110"/>
    <skos:narrower rdf:resource="http://purl.org/heritagedata/schemes/225/concepts/111430"/>
    <skos:narrower rdf:resource="http://purl.org/heritagedata/schemes/225/concepts/124793"/>
  </rdf:Description>
  <rdf:Description rdf:about="http://purl.org/heritagedata/schemes/225/concepts/141453">
    <cc:license rdf:resource="http://creativecommons.org/licenses/by/3.0"/>
    <cc:attributionName xml:lang="en">Historic England</cc:attributionName>
    <cc:attributionURL rdf:resource="http://www.historicengland.org.uk"/>
    <skos:inScheme rdf:resource="http://purl.org/heritagedata/schemes/225"/>
    <dcterms:issued rdf:datatype="http://www.w3.org/2001/XMLSchema#dateTime">2019-03-26T16:45:43</dcterms:issued>
    <skos:prefLabel xml:lang="en">Dive Bomber</skos:prefLabel>
    <rdf:type rdf:resource="http://www.w3.org/2004/02/skos/core#Concept"/>
    <dcterms:identifier>http://purl.org/heritagedata/schemes/225/concepts/141453</dcterms:identifier>
    <dcterms:publisher rdf:resource="http://www.historicengland.org.uk"/>
    <skos:scopeNote xml:lang="en">A fighter-bomber designed to deploy its bombs during the latter stage of a diving manoeuvre, thus increasing the accuracy of its targetting.</skos:scopeNote>
    <skos:broader rdf:resource="http://purl.org/heritagedata/schemes/225/concepts/111399"/>
  </rdf:Description>
  <rdf:Description rdf:about="http://purl.org/heritagedata/schemes/225/concepts/111430">
    <skos:prefLabel xml:lang="en">Light Aircraft</skos:prefLabel>
    <skos:scopeNote xml:lang="en">Generally understood to mean aircraft whose normal loaded weight is less than 2750kg (6060 lb).</skos:scopeNote>
    <dcterms:issued rdf:datatype="http://www.w3.org/2001/XMLSchema#dateTime">2019-03-26T16:45:43</dcterms:issued>
    <dcterms:publisher rdf:resource="http://www.historicengland.org.uk"/>
    <dcterms:identifier>http://purl.org/heritagedata/schemes/225/concepts/111430</dcterms:identifier>
    <skos:narrower rdf:resource="http://purl.org/heritagedata/schemes/225/concepts/167003"/>
    <cc:license rdf:resource="http://creativecommons.org/licenses/by/3.0"/>
    <cc:attributionName xml:lang="en">Historic England</cc:attributionName>
    <cc:attributionURL rdf:resource="http://www.historicengland.org.uk"/>
    <skos:inScheme rdf:resource="http://purl.org/heritagedata/schemes/225"/>
    <rdf:type rdf:resource="http://www.w3.org/2004/02/skos/core#Concept"/>
    <skos:broader rdf:resource="http://purl.org/heritagedata/schemes/225/concepts/111393"/>
  </rdf:Description>
  <rdf:Description rdf:about="http://purl.org/heritagedata/schemes/225/concepts/169972">
    <skos:broader rdf:resource="http://purl.org/heritagedata/schemes/225/concepts/111403"/>
    <rdf:type rdf:resource="http://www.w3.org/2004/02/skos/core#Concept"/>
    <dcterms:issued rdf:datatype="http://www.w3.org/2001/XMLSchema#dateTime">2019-03-26T16:45:43</dcterms:issued>
    <dcterms:publisher rdf:resource="http://www.historicengland.org.uk"/>
    <skos:broader rdf:resource="http://purl.org/heritagedata/schemes/225/concepts/111368"/>
    <cc:attributionName xml:lang="en">Historic England</cc:attributionName>
    <skos:inScheme rdf:resource="http://purl.org/heritagedata/schemes/225"/>
    <dcterms:identifier>http://purl.org/heritagedata/schemes/225/concepts/169972</dcterms:identifier>
    <skos:scopeNote xml:lang="en">A 1930s British short-haul biplane airliner for 6-8 passengers. It proved an economical and durable craft, despite its relatively primitive plywood construction. Primarily used by the RAF.</skos:scopeNote>
    <skos:broader rdf:resource="http://purl.org/heritagedata/schemes/225/concepts/111424"/>
    <skos:prefLabel xml:lang="en">De Havilland Dragon Rapide</skos:prefLabel>
    <cc:license rdf:resource="http://creativecommons.org/licenses/by/3.0"/>
    <cc:attributionURL rdf:resource="http://www.historicengland.org.uk"/>
  </rdf:Description>
  <rdf:Description rdf:about="http://purl.org/heritagedata/schemes/225/concepts/111376">
    <skos:broader rdf:resource="http://purl.org/heritagedata/schemes/225/concepts/111358"/>
    <skos:narrower rdf:resource="http://purl.org/heritagedata/schemes/225/concepts/138538"/>
    <dcterms:identifier>http://purl.org/heritagedata/schemes/225/concepts/111376</dcterms:identifier>
    <skos:narrower rdf:resource="http://purl.org/heritagedata/schemes/225/concepts/137195"/>
    <dcterms:publisher rdf:resource="http://www.historicengland.org.uk"/>
    <skos:narrower rdf:resource="http://purl.org/heritagedata/schemes/225/concepts/136521"/>
    <cc:attributionName xml:lang="en">Historic England</cc:attributionName>
    <skos:narrower rdf:resource="http://purl.org/heritagedata/schemes/225/concepts/138539"/>
    <rdf:type rdf:resource="http://www.w3.org/2004/02/skos/core#Concept"/>
    <skos:scopeNote xml:lang="en">Sir W. G. Armstrong Whitworth Aircraft, Ltd. formed in 1921. Controlled by the Armstrong Siddeley Development Co., Ltd., a subsidiary of the Hawker Siddeley Aircraft Co., Ltd. from 1935. Pioneers in the development of all-metal aircraft.</skos:scopeNote>
    <dcterms:issued rdf:datatype="http://www.w3.org/2001/XMLSchema#dateTime">2019-03-26T16:45:43</dcterms:issued>
    <skos:narrower rdf:resource="http://purl.org/heritagedata/schemes/225/concepts/111377"/>
    <cc:attributionURL rdf:resource="http://www.historicengland.org.uk"/>
    <cc:license rdf:resource="http://creativecommons.org/licenses/by/3.0"/>
    <skos:prefLabel xml:lang="en">Armstrong Whitworth</skos:prefLabel>
    <skos:inScheme rdf:resource="http://purl.org/heritagedata/schemes/225"/>
    <skos:narrower rdf:resource="http://purl.org/heritagedata/schemes/225/concepts/136522"/>
  </rdf:Description>
  <rdf:Description rdf:about="http://purl.org/heritagedata/schemes/225/concepts/111366">
    <dcterms:publisher rdf:resource="http://www.historicengland.org.uk"/>
    <skos:broader rdf:resource="http://purl.org/heritagedata/schemes/225/concepts/111399"/>
    <skos:broader rdf:resource="http://purl.org/heritagedata/schemes/225/concepts/133214"/>
    <skos:scopeNote xml:lang="en">Single-seat, single-engine fighter-bomber and ground-attack aircraft. Entered service with the Luftwaffe in mid-1941. Approximately 20,000 were constructed between 1941 and the end of the war.</skos:scopeNote>
    <skos:prefLabel xml:lang="en">Fw190</skos:prefLabel>
    <skos:broader rdf:resource="http://purl.org/heritagedata/schemes/225/concepts/111402"/>
    <rdf:type rdf:resource="http://www.w3.org/2004/02/skos/core#Concept"/>
    <dcterms:issued rdf:datatype="http://www.w3.org/2001/XMLSchema#dateTime">2019-03-26T16:45:43</dcterms:issued>
    <skos:inScheme rdf:resource="http://purl.org/heritagedata/schemes/225"/>
    <cc:attributionURL rdf:resource="http://www.historicengland.org.uk"/>
    <dcterms:identifier>http://purl.org/heritagedata/schemes/225/concepts/111366</dcterms:identifier>
    <cc:attributionName xml:lang="en">Historic England</cc:attributionName>
    <cc:license rdf:resource="http://creativecommons.org/licenses/by/3.0"/>
  </rdf:Description>
  <rdf:Description rdf:about="http://purl.org/heritagedata/schemes/225/concepts/137211">
    <dcterms:issued rdf:datatype="http://www.w3.org/2001/XMLSchema#dateTime">2019-03-26T16:45:43</dcterms:issued>
    <dcterms:publisher rdf:resource="http://www.historicengland.org.uk"/>
    <dcterms:identifier>http://purl.org/heritagedata/schemes/225/concepts/137211</dcterms:identifier>
    <skos:broader rdf:resource="http://purl.org/heritagedata/schemes/225/concepts/111358"/>
    <skos:prefLabel xml:lang="en">Bell</skos:prefLabel>
    <skos:narrower rdf:resource="http://purl.org/heritagedata/schemes/225/concepts/137212"/>
    <cc:license rdf:resource="http://creativecommons.org/licenses/by/3.0"/>
    <cc:attributionName xml:lang="en">Historic England</cc:attributionName>
    <cc:attributionURL rdf:resource="http://www.historicengland.org.uk"/>
    <skos:inScheme rdf:resource="http://purl.org/heritagedata/schemes/225"/>
    <skos:scopeNote xml:lang="en">Formed in 1935 by Lawrence D. Bell, Ray P. Whitman and Robert J. Woods, who left the Consolidated Aircraft Corporation when it moved its factory from Buffalo to San Diego. Sub-contracted work before its first original design, the XFM-1, in 1937.</skos:scopeNote>
    <rdf:type rdf:resource="http://www.w3.org/2004/02/skos/core#Concept"/>
  </rdf:Description>
  <rdf:Description rdf:about="http://purl.org/heritagedata/schemes/225/concepts/133206">
    <rdf:type rdf:resource="http://www.w3.org/2004/02/skos/core#Concept"/>
    <dcterms:issued rdf:datatype="http://www.w3.org/2001/XMLSchema#dateTime">2019-03-26T16:45:43</dcterms:issued>
    <dcterms:identifier>http://purl.org/heritagedata/schemes/225/concepts/133206</dcterms:identifier>
    <dcterms:publisher rdf:resource="http://www.historicengland.org.uk"/>
    <skos:scopeNote xml:lang="en">Single-engine, advanced-pilot trainer used in secondary flying training schools. Serving from 1939-50, was also used as a target tug for gunnery practice.</skos:scopeNote>
    <skos:broader rdf:resource="http://purl.org/heritagedata/schemes/225/concepts/133205"/>
    <skos:broader rdf:resource="http://purl.org/heritagedata/schemes/225/concepts/111401"/>
    <cc:license rdf:resource="http://creativecommons.org/licenses/by/3.0"/>
    <cc:attributionName xml:lang="en">Historic England</cc:attributionName>
    <cc:attributionURL rdf:resource="http://www.historicengland.org.uk"/>
    <skos:prefLabel xml:lang="en">Master</skos:prefLabel>
    <skos:inScheme rdf:resource="http://purl.org/heritagedata/schemes/225"/>
    <skos:broader rdf:resource="http://purl.org/heritagedata/schemes/225/concepts/111402"/>
  </rdf:Description>
  <rdf:Description rdf:about="http://purl.org/heritagedata/schemes/225/concepts/141405">
    <skos:altLabel xml:lang="en">C53 Skytrooper</skos:altLabel>
  </rdf:Description>
  <rdf:Description rdf:about="http://purl.org/heritagedata/schemes/225/concepts/151472">
    <skos:broader rdf:resource="http://purl.org/heritagedata/schemes/225/concepts/111368"/>
    <cc:attributionURL rdf:resource="http://www.historicengland.org.uk"/>
    <dcterms:issued rdf:datatype="http://www.w3.org/2001/XMLSchema#dateTime">2019-03-26T16:45:43</dcterms:issued>
    <cc:license rdf:resource="http://creativecommons.org/licenses/by/3.0"/>
    <skos:broader rdf:resource="http://purl.org/heritagedata/schemes/225/concepts/111397"/>
    <dcterms:identifier>http://purl.org/heritagedata/schemes/225/concepts/151472</dcterms:identifier>
    <skos:prefLabel xml:lang="en">Vampire</skos:prefLabel>
    <skos:broader rdf:resource="http://purl.org/heritagedata/schemes/225/concepts/111402"/>
    <rdf:type rdf:resource="http://www.w3.org/2004/02/skos/core#Concept"/>
    <dcterms:publisher rdf:resource="http://www.historicengland.org.uk"/>
    <skos:inScheme rdf:resource="http://purl.org/heritagedata/schemes/225"/>
    <cc:attributionName xml:lang="en">Historic England</cc:attributionName>
    <skos:scopeNote xml:lang="en">A single engine, jet propelled twin boom aircraft which came into service in 1945 in a variety of roles including night fighter, trainer, the carrier-borne Sea Vampire, and the MK5 version, a fighter bomber.  Produced by De Havilland.</skos:scopeNote>
  </rdf:Description>
  <rdf:Description rdf:about="http://purl.org/heritagedata/schemes/225/concepts/141226">
    <dcterms:identifier>http://purl.org/heritagedata/schemes/225/concepts/141226</dcterms:identifier>
    <cc:attributionURL rdf:resource="http://www.historicengland.org.uk"/>
    <cc:license rdf:resource="http://creativecommons.org/licenses/by/3.0"/>
    <skos:prefLabel xml:lang="en">MkXI</skos:prefLabel>
    <skos:scopeNote xml:lang="en">Mark 11 or the eleventh variant of an aircraft with its associated modifications.</skos:scopeNote>
    <skos:broader rdf:resource="http://purl.org/heritagedata/schemes/225/concepts/141131"/>
    <dcterms:issued rdf:datatype="http://www.w3.org/2001/XMLSchema#dateTime">2019-03-26T16:45:43</dcterms:issued>
    <rdf:type rdf:resource="http://www.w3.org/2004/02/skos/core#Concept"/>
    <skos:inScheme rdf:resource="http://purl.org/heritagedata/schemes/225"/>
    <cc:attributionName xml:lang="en">Historic England</cc:attributionName>
    <dcterms:publisher rdf:resource="http://www.historicengland.org.uk"/>
  </rdf:Description>
  <rdf:Description rdf:about="http://purl.org/heritagedata/schemes/225/concepts/140447">
    <skos:broader rdf:resource="http://purl.org/heritagedata/schemes/225/concepts/135730"/>
    <cc:license rdf:resource="http://creativecommons.org/licenses/by/3.0"/>
    <rdf:type rdf:resource="http://www.w3.org/2004/02/skos/core#Concept"/>
    <cc:attributionURL rdf:resource="http://www.historicengland.org.uk"/>
    <skos:inScheme rdf:resource="http://purl.org/heritagedata/schemes/225"/>
    <dcterms:issued rdf:datatype="http://www.w3.org/2001/XMLSchema#dateTime">2019-03-26T16:45:43</dcterms:issued>
    <skos:prefLabel xml:lang="en">Ar 196</skos:prefLabel>
    <skos:broader rdf:resource="http://purl.org/heritagedata/schemes/225/concepts/111402"/>
    <skos:scopeNote xml:lang="en">Single engine, two-crew shipboard reconnaissance and patrol seaplane. Entered service in 1939, this was the last combat floatplane built in Europe.</skos:scopeNote>
    <dcterms:identifier>http://purl.org/heritagedata/schemes/225/concepts/140447</dcterms:identifier>
    <cc:attributionName xml:lang="en">Historic England</cc:attributionName>
    <skos:broader rdf:resource="http://purl.org/heritagedata/schemes/225/concepts/140455"/>
    <dcterms:publisher rdf:resource="http://www.historicengland.org.uk"/>
    <skos:broader rdf:resource="http://purl.org/heritagedata/schemes/225/concepts/134997"/>
  </rdf:Description>
  <rdf:Description rdf:about="http://purl.org/heritagedata/schemes/225/concepts/169973">
    <dcterms:issued rdf:datatype="http://www.w3.org/2001/XMLSchema#dateTime">2019-03-26T16:45:43</dcterms:issued>
    <skos:inScheme rdf:resource="http://purl.org/heritagedata/schemes/225"/>
    <cc:attributionURL rdf:resource="http://www.historicengland.org.uk"/>
    <skos:broader rdf:resource="http://purl.org/heritagedata/schemes/225/concepts/111397"/>
    <cc:attributionName xml:lang="en">Historic England</cc:attributionName>
    <cc:license rdf:resource="http://creativecommons.org/licenses/by/3.0"/>
    <skos:broader rdf:resource="http://purl.org/heritagedata/schemes/225/concepts/111359"/>
    <dcterms:publisher rdf:resource="http://www.historicengland.org.uk"/>
    <skos:scopeNote xml:lang="en">A family of jet fighters capable of vertical/short takeoff and landing. A subsonic aircraft, later designs adapted for use from aircraft carriers. Built between 1967-2003. Used by the RAF and the Royal Navy.</skos:scopeNote>
    <dcterms:identifier>http://purl.org/heritagedata/schemes/225/concepts/169973</dcterms:identifier>
    <skos:prefLabel xml:lang="en">Harrier</skos:prefLabel>
    <rdf:type rdf:resource="http://www.w3.org/2004/02/skos/core#Concept"/>
  </rdf:Description>
  <rdf:Description rdf:about="http://purl.org/heritagedata/schemes/225/concepts/138538">
    <dcterms:identifier>http://purl.org/heritagedata/schemes/225/concepts/138538</dcterms:identifier>
    <skos:prefLabel xml:lang="en">Armstrong Whitworth FK3</skos:prefLabel>
    <cc:attributionName xml:lang="en">Historic England</cc:attributionName>
    <skos:broader rdf:resource="http://purl.org/heritagedata/schemes/225/concepts/111403"/>
    <skos:inScheme rdf:resource="http://purl.org/heritagedata/schemes/225"/>
    <dcterms:publisher rdf:resource="http://www.historicengland.org.uk"/>
    <skos:broader rdf:resource="http://purl.org/heritagedata/schemes/225/concepts/111401"/>
    <skos:broader rdf:resource="http://purl.org/heritagedata/schemes/225/concepts/111376"/>
    <rdf:type rdf:resource="http://www.w3.org/2004/02/skos/core#Concept"/>
    <skos:scopeNote xml:lang="en">A two-seat, reconnaissance biplane developed from the FK2 with a more powerful, but heavier, engine. Primarily used for training in the UK.</skos:scopeNote>
    <skos:broader rdf:resource="http://purl.org/heritagedata/schemes/225/concepts/135730"/>
    <cc:license rdf:resource="http://creativecommons.org/licenses/by/3.0"/>
    <cc:attributionURL rdf:resource="http://www.historicengland.org.uk"/>
    <dcterms:issued rdf:datatype="http://www.w3.org/2001/XMLSchema#dateTime">2019-03-26T16:45:43</dcterms:issued>
  </rdf:Description>
  <rdf:Description rdf:about="http://purl.org/heritagedata/schemes/225/concepts/137199">
    <cc:license rdf:resource="http://creativecommons.org/licenses/by/3.0"/>
    <cc:attributionURL rdf:resource="http://www.historicengland.org.uk"/>
    <rdf:type rdf:resource="http://www.w3.org/2004/02/skos/core#Concept"/>
    <dcterms:identifier>http://purl.org/heritagedata/schemes/225/concepts/137199</dcterms:identifier>
    <dcterms:publisher rdf:resource="http://www.historicengland.org.uk"/>
    <cc:attributionName xml:lang="en">Historic England</cc:attributionName>
    <skos:inScheme rdf:resource="http://purl.org/heritagedata/schemes/225"/>
    <dcterms:issued rdf:datatype="http://www.w3.org/2001/XMLSchema#dateTime">2019-03-26T16:45:43</dcterms:issued>
    <skos:scopeNote xml:lang="en">Single-engine, two-crew fighter, also used for convoy escort and reconnaissance. Designed to operate from aircraft carriers. Entered service with the Fleet Air Arm in 1940 and remained in use until 1945.</skos:scopeNote>
    <skos:prefLabel xml:lang="en">Fulmar</skos:prefLabel>
    <skos:broader rdf:resource="http://purl.org/heritagedata/schemes/225/concepts/111402"/>
    <skos:broader rdf:resource="http://purl.org/heritagedata/schemes/225/concepts/111441"/>
    <skos:broader rdf:resource="http://purl.org/heritagedata/schemes/225/concepts/111397"/>
  </rdf:Description>
  <rdf:Description rdf:about="http://purl.org/heritagedata/schemes/225/concepts/141132">
    <skos:broader rdf:resource="http://purl.org/heritagedata/schemes/225/concepts/141131"/>
    <dcterms:identifier>http://purl.org/heritagedata/schemes/225/concepts/141132</dcterms:identifier>
    <cc:attributionName xml:lang="en">Historic England</cc:attributionName>
    <skos:inScheme rdf:resource="http://purl.org/heritagedata/schemes/225"/>
    <dcterms:publisher rdf:resource="http://www.historicengland.org.uk"/>
    <cc:attributionURL rdf:resource="http://www.historicengland.org.uk"/>
    <rdf:type rdf:resource="http://www.w3.org/2004/02/skos/core#Concept"/>
    <cc:license rdf:resource="http://creativecommons.org/licenses/by/3.0"/>
    <skos:prefLabel xml:lang="en">MkI</skos:prefLabel>
    <skos:scopeNote xml:lang="en">Mark 1 or the first production variation of an aircraft.</skos:scopeNote>
    <dcterms:issued rdf:datatype="http://www.w3.org/2001/XMLSchema#dateTime">2019-03-26T16:45:43</dcterms:issued>
  </rdf:Description>
  <rdf:Description rdf:about="http://purl.org/heritagedata/schemes/225/concepts/111369">
    <dcterms:identifier>http://purl.org/heritagedata/schemes/225/concepts/111369</dcterms:identifier>
    <dcterms:issued rdf:datatype="http://www.w3.org/2001/XMLSchema#dateTime">2019-03-26T16:45:43</dcterms:issued>
    <skos:broader rdf:resource="http://purl.org/heritagedata/schemes/225/concepts/111402"/>
    <rdf:type rdf:resource="http://www.w3.org/2004/02/skos/core#Concept"/>
    <skos:inScheme rdf:resource="http://purl.org/heritagedata/schemes/225"/>
    <dcterms:publisher rdf:resource="http://www.historicengland.org.uk"/>
    <skos:broader rdf:resource="http://purl.org/heritagedata/schemes/225/concepts/111368"/>
    <skos:scopeNote xml:lang="en">Two-seat, twin-engined light/medium bomber celebrated for its speed and versatility. Entering service in 1941, was also adapted for duties as a fighter-bomber, Pathfinder, mine-layer, transport, trainer and photo-reconnaissance aircraft.</skos:scopeNote>
    <cc:license rdf:resource="http://creativecommons.org/licenses/by/3.0"/>
    <skos:prefLabel xml:lang="en">Mosquito</skos:prefLabel>
    <cc:attributionURL rdf:resource="http://www.historicengland.org.uk"/>
    <cc:attributionName xml:lang="en">Historic England</cc:attributionName>
    <skos:broader rdf:resource="http://purl.org/heritagedata/schemes/225/concepts/139626"/>
  </rdf:Description>
  <rdf:Description rdf:about="http://purl.org/heritagedata/schemes/225/concepts/111367">
    <skos:inScheme rdf:resource="http://purl.org/heritagedata/schemes/225"/>
    <dcterms:identifier>http://purl.org/heritagedata/schemes/225/concepts/111367</dcterms:identifier>
    <ns1:related rdf:resource="http://purl.org/heritagedata/schemes/225/concepts/125573"/>
    <dcterms:publisher rdf:resource="http://www.historicengland.org.uk"/>
    <ns1:related rdf:resource="http://purl.org/heritagedata/schemes/225/concepts/136220"/>
    <skos:prefLabel xml:lang="en">Lancaster</skos:prefLabel>
    <skos:broader rdf:resource="http://purl.org/heritagedata/schemes/225/concepts/111402"/>
    <rdf:type rdf:resource="http://www.w3.org/2004/02/skos/core#Concept"/>
    <dcterms:issued rdf:datatype="http://www.w3.org/2001/XMLSchema#dateTime">2019-03-26T16:45:43</dcterms:issued>
    <cc:attributionURL rdf:resource="http://www.historicengland.org.uk"/>
    <skos:scopeNote xml:lang="en">Four-engined heavy bomber, developed by Avro from the twin-engined Manchester. Entered service in 1942 as the RAF's principal night bomber and took part in the 1,000 bomber raids as well as the famous Dam Busters raid.</skos:scopeNote>
    <cc:attributionName xml:lang="en">Historic England</cc:attributionName>
    <cc:license rdf:resource="http://creativecommons.org/licenses/by/3.0"/>
    <skos:broader rdf:resource="http://purl.org/heritagedata/schemes/225/concepts/137190"/>
    <ns1:related rdf:resource="http://purl.org/heritagedata/schemes/225/concepts/137193"/>
    <skos:broader rdf:resource="http://purl.org/heritagedata/schemes/225/concepts/111355"/>
  </rdf:Description>
  <rdf:Description rdf:about="http://purl.org/heritagedata/schemes/225/concepts/138539">
    <skos:prefLabel xml:lang="en">Armstrong Whitworth FK8</skos:prefLabel>
    <cc:attributionName xml:lang="en">Historic England</cc:attributionName>
    <dcterms:publisher rdf:resource="http://www.historicengland.org.uk"/>
    <skos:broader rdf:resource="http://purl.org/heritagedata/schemes/225/concepts/111376"/>
    <rdf:type rdf:resource="http://www.w3.org/2004/02/skos/core#Concept"/>
    <skos:broader rdf:resource="http://purl.org/heritagedata/schemes/225/concepts/111398"/>
    <dcterms:identifier>http://purl.org/heritagedata/schemes/225/concepts/138539</dcterms:identifier>
    <skos:broader rdf:resource="http://purl.org/heritagedata/schemes/225/concepts/135730"/>
    <cc:license rdf:resource="http://creativecommons.org/licenses/by/3.0"/>
    <skos:inScheme rdf:resource="http://purl.org/heritagedata/schemes/225"/>
    <cc:attributionURL rdf:resource="http://www.historicengland.org.uk"/>
    <dcterms:issued rdf:datatype="http://www.w3.org/2001/XMLSchema#dateTime">2019-03-26T16:45:43</dcterms:issued>
    <skos:scopeNote xml:lang="en">Single-engine, two-seat tractor bomber and reconnaissance aircraft. Entered service in 1916 and, during 1917 and 1918, equipped nine RFC squadrons in its reconnaissance role.</skos:scopeNote>
    <skos:broader rdf:resource="http://purl.org/heritagedata/schemes/225/concepts/111403"/>
  </rdf:Description>
  <rdf:Description rdf:about="http://purl.org/heritagedata/schemes/225/concepts/141251">
    <skos:altLabel xml:lang="en">Beechcraft</skos:altLabel>
  </rdf:Description>
  <rdf:Description rdf:about="http://purl.org/heritagedata/schemes/225/concepts/138485">
    <rdf:type rdf:resource="http://www.w3.org/2004/02/skos/core#Concept"/>
    <skos:broader rdf:resource="http://purl.org/heritagedata/schemes/225/concepts/138484"/>
    <dcterms:publisher rdf:resource="http://www.historicengland.org.uk"/>
    <skos:scopeNote xml:lang="en">Single-engine, single-seat fighter. Entered service in 1943 as a land-based fighter. Converted to a carrierborne fighter in 1944 for use by US Navy and Fleet Air Arm. Mostly saw action in the Pacific and Far East.</skos:scopeNote>
    <dcterms:issued rdf:datatype="http://www.w3.org/2001/XMLSchema#dateTime">2019-03-26T16:45:43</dcterms:issued>
    <skos:broader rdf:resource="http://purl.org/heritagedata/schemes/225/concepts/111402"/>
    <skos:broader rdf:resource="http://purl.org/heritagedata/schemes/225/concepts/111397"/>
    <cc:attributionName xml:lang="en">Historic England</cc:attributionName>
    <cc:license rdf:resource="http://creativecommons.org/licenses/by/3.0"/>
    <skos:inScheme rdf:resource="http://purl.org/heritagedata/schemes/225"/>
    <cc:attributionURL rdf:resource="http://www.historicengland.org.uk"/>
    <skos:prefLabel xml:lang="en">Corsair</skos:prefLabel>
    <dcterms:identifier>http://purl.org/heritagedata/schemes/225/concepts/138485</dcterms:identifier>
  </rdf:Description>
  <rdf:Description rdf:about="http://purl.org/heritagedata/schemes/225/concepts/138532">
    <skos:broader rdf:resource="http://purl.org/heritagedata/schemes/225/concepts/111403"/>
    <dcterms:identifier>http://purl.org/heritagedata/schemes/225/concepts/138532</dcterms:identifier>
    <skos:broader rdf:resource="http://purl.org/heritagedata/schemes/225/concepts/136512"/>
    <skos:broader rdf:resource="http://purl.org/heritagedata/schemes/225/concepts/111397"/>
    <cc:attributionName xml:lang="en">Historic England</cc:attributionName>
    <cc:license rdf:resource="http://creativecommons.org/licenses/by/3.0"/>
    <skos:inScheme rdf:resource="http://purl.org/heritagedata/schemes/225"/>
    <cc:attributionURL rdf:resource="http://www.historicengland.org.uk"/>
    <skos:prefLabel xml:lang="en">Airco DH1</skos:prefLabel>
    <skos:scopeNote xml:lang="en">A single-seat, pusher prop, escort and patrol-fighter. Used in the UK in a Home Defence role until superseded in 1917.</skos:scopeNote>
    <dcterms:publisher rdf:resource="http://www.historicengland.org.uk"/>
    <dcterms:issued rdf:datatype="http://www.w3.org/2001/XMLSchema#dateTime">2019-03-26T16:45:43</dcterms:issued>
    <rdf:type rdf:resource="http://www.w3.org/2004/02/skos/core#Concept"/>
  </rdf:Description>
  <rdf:Description rdf:about="http://purl.org/heritagedata/schemes/225/concepts/141303">
    <skos:scopeNote xml:lang="en">A Mark 2A aircraft which has undergone slight modifications to enhance performance or armament.</skos:scopeNote>
    <skos:prefLabel xml:lang="en">MkIIB</skos:prefLabel>
    <skos:broader rdf:resource="http://purl.org/heritagedata/schemes/225/concepts/141131"/>
    <dcterms:publisher rdf:resource="http://www.historicengland.org.uk"/>
    <rdf:type rdf:resource="http://www.w3.org/2004/02/skos/core#Concept"/>
    <cc:attributionName xml:lang="en">Historic England</cc:attributionName>
    <cc:license rdf:resource="http://creativecommons.org/licenses/by/3.0"/>
    <skos:inScheme rdf:resource="http://purl.org/heritagedata/schemes/225"/>
    <cc:attributionURL rdf:resource="http://www.historicengland.org.uk"/>
    <dcterms:issued rdf:datatype="http://www.w3.org/2001/XMLSchema#dateTime">2019-03-26T16:45:43</dcterms:issued>
    <dcterms:identifier>http://purl.org/heritagedata/schemes/225/concepts/141303</dcterms:identifier>
  </rdf:Description>
  <rdf:Description rdf:about="http://purl.org/heritagedata/schemes/225/concepts/140425">
    <skos:broader rdf:resource="http://purl.org/heritagedata/schemes/225/concepts/137190"/>
    <dcterms:identifier>http://purl.org/heritagedata/schemes/225/concepts/140425</dcterms:identifier>
    <dcterms:publisher rdf:resource="http://www.historicengland.org.uk"/>
    <skos:broader rdf:resource="http://purl.org/heritagedata/schemes/225/concepts/111415"/>
    <skos:scopeNote xml:lang="en">Four-engined, five to seven crew, heavy bomber biplane. Entered service in 1918.</skos:scopeNote>
    <skos:broader rdf:resource="http://purl.org/heritagedata/schemes/225/concepts/111403"/>
    <cc:attributionURL rdf:resource="http://www.historicengland.org.uk"/>
    <rdf:type rdf:resource="http://www.w3.org/2004/02/skos/core#Concept"/>
    <skos:prefLabel xml:lang="en">V1500</skos:prefLabel>
    <cc:attributionName xml:lang="en">Historic England</cc:attributionName>
    <cc:license rdf:resource="http://creativecommons.org/licenses/by/3.0"/>
    <dcterms:issued rdf:datatype="http://www.w3.org/2001/XMLSchema#dateTime">2019-03-26T16:45:43</dcterms:issued>
    <skos:inScheme rdf:resource="http://purl.org/heritagedata/schemes/225"/>
  </rdf:Description>
  <rdf:Description rdf:about="http://purl.org/heritagedata/schemes/225/concepts/137150">
    <skos:inScheme rdf:resource="http://purl.org/heritagedata/schemes/225"/>
    <skos:broader rdf:resource="http://purl.org/heritagedata/schemes/225/concepts/111417"/>
    <skos:broader rdf:resource="http://purl.org/heritagedata/schemes/225/concepts/135730"/>
    <cc:license rdf:resource="http://creativecommons.org/licenses/by/3.0"/>
    <cc:attributionURL rdf:resource="http://www.historicengland.org.uk"/>
    <skos:broader rdf:resource="http://purl.org/heritagedata/schemes/225/concepts/111402"/>
    <dcterms:identifier>http://purl.org/heritagedata/schemes/225/concepts/137150</dcterms:identifier>
    <rdf:type rdf:resource="http://www.w3.org/2004/02/skos/core#Concept"/>
    <skos:scopeNote xml:lang="en">American-built, twin-engined flying-boat designed for maritime patrol and reconnaissance. Entered US Naval service in 1936 as the PBY-1; christened the Catalina by the RAF, who used it from 1939 on.</skos:scopeNote>
    <dcterms:issued rdf:datatype="http://www.w3.org/2001/XMLSchema#dateTime">2019-03-26T16:45:43</dcterms:issued>
    <dcterms:publisher rdf:resource="http://www.historicengland.org.uk"/>
    <skos:prefLabel xml:lang="en">Catalina</skos:prefLabel>
    <skos:broader rdf:resource="http://purl.org/heritagedata/schemes/225/concepts/111395"/>
    <cc:attributionName xml:lang="en">Historic England</cc:attributionName>
  </rdf:Description>
  <rdf:Description rdf:about="http://purl.org/heritagedata/schemes/225/concepts/136516">
    <skos:altLabel xml:lang="en">Dh5</skos:altLabel>
  </rdf:Description>
  <rdf:Description rdf:about="http://purl.org/heritagedata/schemes/225/concepts/137213">
    <skos:narrower rdf:resource="http://purl.org/heritagedata/schemes/225/concepts/137214"/>
    <dcterms:publisher rdf:resource="http://www.historicengland.org.uk"/>
    <cc:license rdf:resource="http://creativecommons.org/licenses/by/3.0"/>
    <rdf:type rdf:resource="http://www.w3.org/2004/02/skos/core#Concept"/>
    <cc:attributionURL rdf:resource="http://www.historicengland.org.uk"/>
    <dcterms:identifier>http://purl.org/heritagedata/schemes/225/concepts/137213</dcterms:identifier>
    <skos:prefLabel xml:lang="en">Brewster</skos:prefLabel>
    <skos:narrower rdf:resource="http://purl.org/heritagedata/schemes/225/concepts/137215"/>
    <skos:broader rdf:resource="http://purl.org/heritagedata/schemes/225/concepts/111358"/>
    <dcterms:issued rdf:datatype="http://www.w3.org/2001/XMLSchema#dateTime">2019-03-26T16:45:43</dcterms:issued>
    <skos:scopeNote xml:lang="en">The Brewster Aeronautical Corporation was founded in 1932, taking over the plant, equipment, designs and goodwill of Brewster &amp; Co., Inc.'s aircraft division. Initially manufacturing seaplane components, later designed and produced complete aircraft.</skos:scopeNote>
    <cc:attributionName xml:lang="en">Historic England</cc:attributionName>
    <skos:inScheme rdf:resource="http://purl.org/heritagedata/schemes/225"/>
  </rdf:Description>
  <rdf:Description rdf:about="http://purl.org/heritagedata/schemes/225/concepts/137226">
    <skos:broader rdf:resource="http://purl.org/heritagedata/schemes/225/concepts/111402"/>
    <skos:broader rdf:resource="http://purl.org/heritagedata/schemes/225/concepts/135751"/>
    <dcterms:publisher rdf:resource="http://www.historicengland.org.uk"/>
    <skos:broader rdf:resource="http://purl.org/heritagedata/schemes/225/concepts/137225"/>
    <skos:prefLabel xml:lang="en">Vengeance</skos:prefLabel>
    <dcterms:identifier>http://purl.org/heritagedata/schemes/225/concepts/137226</dcterms:identifier>
    <cc:license rdf:resource="http://creativecommons.org/licenses/by/3.0"/>
    <rdf:type rdf:resource="http://www.w3.org/2004/02/skos/core#Concept"/>
    <cc:attributionURL rdf:resource="http://www.historicengland.org.uk"/>
    <skos:inScheme rdf:resource="http://purl.org/heritagedata/schemes/225"/>
    <cc:attributionName xml:lang="en">Historic England</cc:attributionName>
    <dcterms:issued rdf:datatype="http://www.w3.org/2001/XMLSchema#dateTime">2019-03-26T16:45:43</dcterms:issued>
    <skos:scopeNote xml:lang="en">Single-engine aircraft designed as a dive-bomber. Found to be inadequate in this role, a number of those delivered to the RAF were used as target tugs. Entered service in 1941.</skos:scopeNote>
  </rdf:Description>
  <rdf:Description rdf:about="http://purl.org/heritagedata/schemes/225/concepts/138534">
    <skos:inScheme rdf:resource="http://purl.org/heritagedata/schemes/225"/>
    <dcterms:publisher rdf:resource="http://www.historicengland.org.uk"/>
    <cc:license rdf:resource="http://creativecommons.org/licenses/by/3.0"/>
    <dcterms:identifier>http://purl.org/heritagedata/schemes/225/concepts/138534</dcterms:identifier>
    <skos:broader rdf:resource="http://purl.org/heritagedata/schemes/225/concepts/111398"/>
    <rdf:type rdf:resource="http://www.w3.org/2004/02/skos/core#Concept"/>
    <cc:attributionURL rdf:resource="http://www.historicengland.org.uk"/>
    <dcterms:issued rdf:datatype="http://www.w3.org/2001/XMLSchema#dateTime">2019-03-26T16:45:43</dcterms:issued>
    <skos:broader rdf:resource="http://purl.org/heritagedata/schemes/225/concepts/136512"/>
    <skos:prefLabel xml:lang="en">Airco DH4</skos:prefLabel>
    <skos:broader rdf:resource="http://purl.org/heritagedata/schemes/225/concepts/111403"/>
    <cc:attributionName xml:lang="en">Historic England</cc:attributionName>
    <skos:scopeNote xml:lang="en">A two-seat, single-engine bomber. Fast, versatile and well armed, but with a fuel tank poorly placed between pilot and gunner, was considered to be the best day bomber of the First World War. Later entered civil service.</skos:scopeNote>
  </rdf:Description>
  <rdf:Description rdf:about="http://purl.org/heritagedata/schemes/225/concepts/137110">
    <cc:attributionName xml:lang="en">Historic England</cc:attributionName>
    <skos:narrower rdf:resource="http://purl.org/heritagedata/schemes/225/concepts/137202"/>
    <rdf:type rdf:resource="http://www.w3.org/2004/02/skos/core#Concept"/>
    <dcterms:identifier>http://purl.org/heritagedata/schemes/225/concepts/137110</dcterms:identifier>
    <skos:narrower rdf:resource="http://purl.org/heritagedata/schemes/225/concepts/137201"/>
    <cc:attributionURL rdf:resource="http://www.historicengland.org.uk"/>
    <skos:prefLabel xml:lang="en">Glider</skos:prefLabel>
    <skos:narrower rdf:resource="http://purl.org/heritagedata/schemes/225/concepts/137111"/>
    <dcterms:publisher rdf:resource="http://www.historicengland.org.uk"/>
    <cc:license rdf:resource="http://creativecommons.org/licenses/by/3.0"/>
    <skos:scopeNote xml:lang="en">An engineless aeroplane, designed to be towed aloft, that travels suspended by upward air currents.</skos:scopeNote>
    <skos:narrower rdf:resource="http://purl.org/heritagedata/schemes/225/concepts/137228"/>
    <dcterms:issued rdf:datatype="http://www.w3.org/2001/XMLSchema#dateTime">2019-03-26T16:45:43</dcterms:issued>
    <skos:broader rdf:resource="http://purl.org/heritagedata/schemes/225/concepts/111393"/>
    <skos:inScheme rdf:resource="http://purl.org/heritagedata/schemes/225"/>
  </rdf:Description>
  <rdf:Description rdf:about="http://purl.org/heritagedata/schemes/225/concepts/141497">
    <skos:broader rdf:resource="http://purl.org/heritagedata/schemes/225/concepts/111394"/>
    <skos:inScheme rdf:resource="http://purl.org/heritagedata/schemes/225"/>
    <rdf:type rdf:resource="http://www.w3.org/2004/02/skos/core#Concept"/>
    <cc:attributionURL rdf:resource="http://www.historicengland.org.uk"/>
    <cc:license rdf:resource="http://creativecommons.org/licenses/by/3.0"/>
    <skos:prefLabel xml:lang="en">Air Sea Rescue</skos:prefLabel>
    <dcterms:issued rdf:datatype="http://www.w3.org/2001/XMLSchema#dateTime">2019-03-26T16:45:43</dcterms:issued>
    <dcterms:identifier>http://purl.org/heritagedata/schemes/225/concepts/141497</dcterms:identifier>
    <skos:scopeNote xml:lang="en">An aircraft engaged in rescuing persons in danger at sea.</skos:scopeNote>
    <dcterms:publisher rdf:resource="http://www.historicengland.org.uk"/>
    <cc:attributionName xml:lang="en">Historic England</cc:attributionName>
  </rdf:Description>
  <rdf:Description rdf:about="http://purl.org/heritagedata/schemes/225/concepts/140065">
    <dcterms:publisher rdf:resource="http://www.historicengland.org.uk"/>
    <dcterms:identifier>http://purl.org/heritagedata/schemes/225/concepts/140065</dcterms:identifier>
    <skos:broader rdf:resource="http://purl.org/heritagedata/schemes/225/concepts/111441"/>
    <cc:license rdf:resource="http://creativecommons.org/licenses/by/3.0"/>
    <rdf:type rdf:resource="http://www.w3.org/2004/02/skos/core#Concept"/>
    <cc:attributionURL rdf:resource="http://www.historicengland.org.uk"/>
    <skos:broader rdf:resource="http://purl.org/heritagedata/schemes/225/concepts/111397"/>
    <dcterms:issued rdf:datatype="http://www.w3.org/2001/XMLSchema#dateTime">2019-03-26T16:45:43</dcterms:issued>
    <skos:scopeNote xml:lang="en">Single-engine, two or three-crew pre-World War 2 biplane fighter and general purpose aircraft. First flown in 1931, the Seal was a Naval variant on the Fairey Gordon and a forerunner of the Swordfish.</skos:scopeNote>
    <skos:prefLabel xml:lang="en">Seal</skos:prefLabel>
    <skos:broader rdf:resource="http://purl.org/heritagedata/schemes/225/concepts/111403"/>
    <cc:attributionName xml:lang="en">Historic England</cc:attributionName>
    <skos:inScheme rdf:resource="http://purl.org/heritagedata/schemes/225"/>
  </rdf:Description>
  <rdf:Description rdf:about="http://purl.org/heritagedata/schemes/225/concepts/133209">
    <skos:inScheme rdf:resource="http://purl.org/heritagedata/schemes/225"/>
    <dcterms:publisher rdf:resource="http://www.historicengland.org.uk"/>
    <skos:broader rdf:resource="http://purl.org/heritagedata/schemes/225/concepts/111353"/>
    <skos:scopeNote xml:lang="en">Single-seat carrierborne jet fighter. Originally conceived as an RAF land-fighter, entered Fleet Air Arm service in 1951 and was the first jet fighter to be standardised in first-line squadrons.</skos:scopeNote>
    <dcterms:identifier>http://purl.org/heritagedata/schemes/225/concepts/133209</dcterms:identifier>
    <skos:broader rdf:resource="http://purl.org/heritagedata/schemes/225/concepts/111397"/>
    <skos:prefLabel xml:lang="en">Attacker</skos:prefLabel>
    <cc:license rdf:resource="http://creativecommons.org/licenses/by/3.0"/>
    <skos:broader rdf:resource="http://purl.org/heritagedata/schemes/225/concepts/111402"/>
    <rdf:type rdf:resource="http://www.w3.org/2004/02/skos/core#Concept"/>
    <dcterms:issued rdf:datatype="http://www.w3.org/2001/XMLSchema#dateTime">2019-03-26T16:45:43</dcterms:issued>
    <cc:attributionURL rdf:resource="http://www.historicengland.org.uk"/>
    <cc:attributionName xml:lang="en">Historic England</cc:attributionName>
  </rdf:Description>
  <rdf:Description rdf:about="http://purl.org/heritagedata/schemes/225/concepts/167001">
    <dcterms:issued rdf:datatype="http://www.w3.org/2001/XMLSchema#dateTime">2019-03-26T16:45:43</dcterms:issued>
    <skos:inScheme rdf:resource="http://purl.org/heritagedata/schemes/225"/>
    <cc:attributionURL rdf:resource="http://www.historicengland.org.uk"/>
    <cc:attributionName xml:lang="en">Historic England</cc:attributionName>
    <cc:license rdf:resource="http://creativecommons.org/licenses/by/3.0"/>
    <dcterms:identifier>http://purl.org/heritagedata/schemes/225/concepts/167001</dcterms:identifier>
    <dcterms:publisher rdf:resource="http://www.historicengland.org.uk"/>
    <skos:broader rdf:resource="http://purl.org/heritagedata/schemes/225/concepts/111399"/>
    <skos:prefLabel xml:lang="en">F84 Thunderjet</skos:prefLabel>
    <skos:broader rdf:resource="http://purl.org/heritagedata/schemes/225/concepts/125494"/>
    <skos:scopeNote xml:lang="en">An American turbojet fighter-bomber aircraft. The F-84 was the first production fighter aircraft to utilize in-flight refuelling and the first fighter capable of carrying a nuclear weapon. Designed by Alexander Kartveli, 1946.</skos:scopeNote>
    <skos:broader rdf:resource="http://purl.org/heritagedata/schemes/225/concepts/111402"/>
    <rdf:type rdf:resource="http://www.w3.org/2004/02/skos/core#Concept"/>
  </rdf:Description>
  <rdf:Description rdf:about="http://purl.org/heritagedata/schemes/225/concepts/125593">
    <cc:license rdf:resource="http://creativecommons.org/licenses/by/3.0"/>
    <rdf:type rdf:resource="http://www.w3.org/2004/02/skos/core#Concept"/>
    <cc:attributionURL rdf:resource="http://www.historicengland.org.uk"/>
    <skos:inScheme rdf:resource="http://purl.org/heritagedata/schemes/225"/>
    <cc:attributionName xml:lang="en">Historic England</cc:attributionName>
    <dcterms:issued rdf:datatype="http://www.w3.org/2001/XMLSchema#dateTime">2019-03-26T16:45:43</dcterms:issued>
    <skos:scopeNote xml:lang="en">American twin-engined medium bomber. Entered service with the US 22nd Bombardment Group at Langley Field in February 1941. Also served with the 14th and 39th RAF squadrons.</skos:scopeNote>
    <skos:broader rdf:resource="http://purl.org/heritagedata/schemes/225/concepts/111402"/>
    <skos:broader rdf:resource="http://purl.org/heritagedata/schemes/225/concepts/139626"/>
    <skos:prefLabel xml:lang="en">B26 Marauder</skos:prefLabel>
    <dcterms:publisher rdf:resource="http://www.historicengland.org.uk"/>
    <dcterms:identifier>http://purl.org/heritagedata/schemes/225/concepts/125593</dcterms:identifier>
    <skos:broader rdf:resource="http://purl.org/heritagedata/schemes/225/concepts/125613"/>
  </rdf:Description>
  <rdf:Description rdf:about="http://purl.org/heritagedata/schemes/225/concepts/124793">
    <skos:scopeNote xml:lang="en">A pilotless aircraft armed with explosives and fuelled to stall over its intended target.</skos:scopeNote>
    <rdf:type rdf:resource="http://www.w3.org/2004/02/skos/core#Concept"/>
    <cc:license rdf:resource="http://creativecommons.org/licenses/by/3.0"/>
    <cc:attributionName xml:lang="en">Historic England</cc:attributionName>
    <cc:attributionURL rdf:resource="http://www.historicengland.org.uk"/>
    <skos:inScheme rdf:resource="http://purl.org/heritagedata/schemes/225"/>
    <dcterms:identifier>http://purl.org/heritagedata/schemes/225/concepts/124793</dcterms:identifier>
    <skos:prefLabel xml:lang="en">Flying Bomb</skos:prefLabel>
    <dcterms:issued rdf:datatype="http://www.w3.org/2001/XMLSchema#dateTime">2019-03-26T16:45:43</dcterms:issued>
    <skos:broader rdf:resource="http://purl.org/heritagedata/schemes/225/concepts/111393"/>
    <dcterms:publisher rdf:resource="http://www.historicengland.org.uk"/>
    <skos:narrower rdf:resource="http://purl.org/heritagedata/schemes/225/concepts/124794"/>
  </rdf:Description>
  <rdf:Description rdf:about="http://purl.org/heritagedata/schemes/225/concepts/133207">
    <cc:license rdf:resource="http://creativecommons.org/licenses/by/3.0"/>
    <cc:attributionName xml:lang="en">Historic England</cc:attributionName>
    <cc:attributionURL rdf:resource="http://www.historicengland.org.uk"/>
    <skos:inScheme rdf:resource="http://purl.org/heritagedata/schemes/225"/>
    <dcterms:issued rdf:datatype="http://www.w3.org/2001/XMLSchema#dateTime">2019-03-26T16:45:43</dcterms:issued>
    <skos:prefLabel xml:lang="en">Folland</skos:prefLabel>
    <rdf:type rdf:resource="http://www.w3.org/2004/02/skos/core#Concept"/>
    <dcterms:identifier>http://purl.org/heritagedata/schemes/225/concepts/133207</dcterms:identifier>
    <dcterms:publisher rdf:resource="http://www.historicengland.org.uk"/>
    <skos:narrower rdf:resource="http://purl.org/heritagedata/schemes/225/concepts/138543"/>
    <skos:scopeNote xml:lang="en">Formed in 1936 as British Marine Aircraft Ltd. to construct civil flying-boats. In 1937, with the arrival of H P Folland, formerly Chief designer for Gloster Aircraft Co., became Folland Aircraft, Ltd..</skos:scopeNote>
    <skos:broader rdf:resource="http://purl.org/heritagedata/schemes/225/concepts/111358"/>
  </rdf:Description>
  <rdf:Description rdf:about="http://purl.org/heritagedata/schemes/225/concepts/140411">
    <skos:inScheme rdf:resource="http://purl.org/heritagedata/schemes/225"/>
    <skos:broader rdf:resource="http://purl.org/heritagedata/schemes/225/concepts/111441"/>
    <dcterms:identifier>http://purl.org/heritagedata/schemes/225/concepts/140411</dcterms:identifier>
    <skos:scopeNote xml:lang="en">A single-engine, two-crew biplane day bomber and general purpose aircraft, developed from the IIIF (some of which were converted into Gordons) and first flown in 1931.</skos:scopeNote>
    <cc:license rdf:resource="http://creativecommons.org/licenses/by/3.0"/>
    <cc:attributionURL rdf:resource="http://www.historicengland.org.uk"/>
    <skos:prefLabel xml:lang="en">Gordon</skos:prefLabel>
    <skos:broader rdf:resource="http://purl.org/heritagedata/schemes/225/concepts/111398"/>
    <rdf:type rdf:resource="http://www.w3.org/2004/02/skos/core#Concept"/>
    <dcterms:issued rdf:datatype="http://www.w3.org/2001/XMLSchema#dateTime">2019-03-26T16:45:43</dcterms:issued>
    <dcterms:publisher rdf:resource="http://www.historicengland.org.uk"/>
    <cc:attributionName xml:lang="en">Historic England</cc:attributionName>
  </rdf:Description>
  <rdf:Description rdf:about="http://purl.org/heritagedata/schemes/225/concepts/137221">
    <skos:broader rdf:resource="http://purl.org/heritagedata/schemes/225/concepts/111402"/>
    <skos:prefLabel xml:lang="en">F4F Wildcat</skos:prefLabel>
    <dcterms:identifier>http://purl.org/heritagedata/schemes/225/concepts/137221</dcterms:identifier>
    <dcterms:publisher rdf:resource="http://www.historicengland.org.uk"/>
    <rdf:type rdf:resource="http://www.w3.org/2004/02/skos/core#Concept"/>
    <skos:broader rdf:resource="http://purl.org/heritagedata/schemes/225/concepts/111397"/>
    <cc:attributionName xml:lang="en">Historic England</cc:attributionName>
    <cc:license rdf:resource="http://creativecommons.org/licenses/by/3.0"/>
    <skos:inScheme rdf:resource="http://purl.org/heritagedata/schemes/225"/>
    <cc:attributionURL rdf:resource="http://www.historicengland.org.uk"/>
    <dcterms:issued rdf:datatype="http://www.w3.org/2001/XMLSchema#dateTime">2019-03-26T16:45:43</dcterms:issued>
    <skos:broader rdf:resource="http://purl.org/heritagedata/schemes/225/concepts/137218"/>
    <skos:scopeNote xml:lang="en">American, single-engine fighter designed for operation from US Naval aircraft carriers. Produced between 1940 and 1945, Wildcats provided to the British Fleet Air Arm were renamed Martlets.</skos:scopeNote>
    <ns1:related rdf:resource="http://purl.org/heritagedata/schemes/225/concepts/137220"/>
  </rdf:Description>
  <rdf:Description rdf:about="http://purl.org/heritagedata/schemes/225/concepts/111363">
    <skos:prefLabel xml:lang="en">Ju87</skos:prefLabel>
    <dcterms:identifier>http://purl.org/heritagedata/schemes/225/concepts/111363</dcterms:identifier>
    <dcterms:issued rdf:datatype="http://www.w3.org/2001/XMLSchema#dateTime">2019-03-26T16:45:43</dcterms:issued>
    <skos:broader rdf:resource="http://purl.org/heritagedata/schemes/225/concepts/111402"/>
    <rdf:type rdf:resource="http://www.w3.org/2004/02/skos/core#Concept"/>
    <skos:inScheme rdf:resource="http://purl.org/heritagedata/schemes/225"/>
    <dcterms:publisher rdf:resource="http://www.historicengland.org.uk"/>
    <cc:attributionName xml:lang="en">Historic England</cc:attributionName>
    <skos:scopeNote xml:lang="en">A single-engine dive-bomber, the JU87 was very successful during the invasions of Poland and France but suffered heavy losses during the Battle of Britain. Withdrawn from NW Europe in 1941 for use in the Mediterranean and on the Eastern Front.</skos:scopeNote>
    <cc:license rdf:resource="http://creativecommons.org/licenses/by/3.0"/>
    <skos:broader rdf:resource="http://purl.org/heritagedata/schemes/225/concepts/111362"/>
    <cc:attributionURL rdf:resource="http://www.historicengland.org.uk"/>
    <skos:broader rdf:resource="http://purl.org/heritagedata/schemes/225/concepts/111398"/>
  </rdf:Description>
  <rdf:Description rdf:about="http://purl.org/heritagedata/schemes/225/concepts/137130">
    <cc:attributionName xml:lang="en">Historic England</cc:attributionName>
    <skos:inScheme rdf:resource="http://purl.org/heritagedata/schemes/225"/>
    <skos:broader rdf:resource="http://purl.org/heritagedata/schemes/225/concepts/111420"/>
    <skos:broader rdf:resource="http://purl.org/heritagedata/schemes/225/concepts/135730"/>
    <skos:broader rdf:resource="http://purl.org/heritagedata/schemes/225/concepts/111402"/>
    <cc:license rdf:resource="http://creativecommons.org/licenses/by/3.0"/>
    <dcterms:identifier>http://purl.org/heritagedata/schemes/225/concepts/137130</dcterms:identifier>
    <cc:attributionURL rdf:resource="http://www.historicengland.org.uk"/>
    <ns1:related rdf:resource="http://purl.org/heritagedata/schemes/225/concepts/111419"/>
    <rdf:type rdf:resource="http://www.w3.org/2004/02/skos/core#Concept"/>
    <skos:scopeNote xml:lang="en">Twin-engined air/sea rescue and anti-submarine patrol aircraft. Originally developed from the Wellington and intended as a bomber, entered RAF Coastal Command service in 1943. Fitted with a Leigh Light and ASV radar.</skos:scopeNote>
    <skos:prefLabel xml:lang="en">Warwick</skos:prefLabel>
    <dcterms:issued rdf:datatype="http://www.w3.org/2001/XMLSchema#dateTime">2019-03-26T16:45:43</dcterms:issued>
    <dcterms:publisher rdf:resource="http://www.historicengland.org.uk"/>
  </rdf:Description>
  <rdf:Description rdf:about="http://purl.org/heritagedata/schemes/225/concepts/136593">
    <rdf:type rdf:resource="http://www.w3.org/2004/02/skos/core#Concept"/>
    <dcterms:issued rdf:datatype="http://www.w3.org/2001/XMLSchema#dateTime">2019-03-26T16:45:43</dcterms:issued>
    <dcterms:publisher rdf:resource="http://www.historicengland.org.uk"/>
    <skos:prefLabel xml:lang="en">Gladiator</skos:prefLabel>
    <dcterms:identifier>http://purl.org/heritagedata/schemes/225/concepts/136593</dcterms:identifier>
    <skos:broader rdf:resource="http://purl.org/heritagedata/schemes/225/concepts/111403"/>
    <cc:license rdf:resource="http://creativecommons.org/licenses/by/3.0"/>
    <cc:attributionName xml:lang="en">Historic England</cc:attributionName>
    <cc:attributionURL rdf:resource="http://www.historicengland.org.uk"/>
    <skos:inScheme rdf:resource="http://purl.org/heritagedata/schemes/225"/>
    <skos:broader rdf:resource="http://purl.org/heritagedata/schemes/225/concepts/111397"/>
    <skos:broader rdf:resource="http://purl.org/heritagedata/schemes/225/concepts/111413"/>
    <skos:scopeNote xml:lang="en">Single-seat, single-engine biplane fighter. In operational service from 1939 to 1941, this was the last, and believed to be the best, biplane to be flown in the RAF. All-metal in construction with fabric and aluminium covering.</skos:scopeNote>
  </rdf:Description>
  <rdf:Description rdf:about="http://purl.org/heritagedata/schemes/225/concepts/151397">
    <dcterms:issued rdf:datatype="http://www.w3.org/2001/XMLSchema#dateTime">2019-03-26T16:45:43</dcterms:issued>
    <skos:prefLabel xml:lang="en">Fi 103</skos:prefLabel>
    <cc:attributionName xml:lang="en">Historic England</cc:attributionName>
    <skos:inScheme rdf:resource="http://purl.org/heritagedata/schemes/225"/>
    <dcterms:publisher rdf:resource="http://www.historicengland.org.uk"/>
    <skos:broader rdf:resource="http://purl.org/heritagedata/schemes/225/concepts/124794"/>
    <dcterms:identifier>http://purl.org/heritagedata/schemes/225/concepts/151397</dcterms:identifier>
    <skos:broader rdf:resource="http://purl.org/heritagedata/schemes/225/concepts/151396"/>
    <skos:scopeNote xml:lang="en">The Fi 103 is the more technical nomenclature for the Second World War German V1 flying bomb, produced by Fieseler. Multiple index together with Fieseler and flying bomb for maximum chance of retrieval for users.</skos:scopeNote>
    <cc:license rdf:resource="http://creativecommons.org/licenses/by/3.0"/>
    <rdf:type rdf:resource="http://www.w3.org/2004/02/skos/core#Concept"/>
    <cc:attributionURL rdf:resource="http://www.historicengland.org.uk"/>
  </rdf:Description>
  <rdf:Description rdf:about="http://purl.org/heritagedata/schemes/225/concepts/111361">
    <skos:narrower rdf:resource="http://purl.org/heritagedata/schemes/225/concepts/137234"/>
    <dcterms:issued rdf:datatype="http://www.w3.org/2001/XMLSchema#dateTime">2019-03-26T16:45:43</dcterms:issued>
    <skos:narrower rdf:resource="http://purl.org/heritagedata/schemes/225/concepts/137235"/>
    <dcterms:identifier>http://purl.org/heritagedata/schemes/225/concepts/111361</dcterms:identifier>
    <cc:attributionName xml:lang="en">Historic England</cc:attributionName>
    <skos:inScheme rdf:resource="http://purl.org/heritagedata/schemes/225"/>
    <skos:prefLabel xml:lang="en">Dornier</skos:prefLabel>
    <skos:narrower rdf:resource="http://purl.org/heritagedata/schemes/225/concepts/111426"/>
    <dcterms:publisher rdf:resource="http://www.historicengland.org.uk"/>
    <skos:narrower rdf:resource="http://purl.org/heritagedata/schemes/225/concepts/111427"/>
    <skos:scopeNote xml:lang="en">Originally the Zeppelin Werk Lindau G.m.b.H., developed metal aircraft from World War One under the guidance of Dr. Ing. Claude Dornier, changing its name to Dornier-Werke G.m.b.H. in 1922.</skos:scopeNote>
    <skos:broader rdf:resource="http://purl.org/heritagedata/schemes/225/concepts/111358"/>
    <cc:license rdf:resource="http://creativecommons.org/licenses/by/3.0"/>
    <rdf:type rdf:resource="http://www.w3.org/2004/02/skos/core#Concept"/>
    <cc:attributionURL rdf:resource="http://www.historicengland.org.uk"/>
  </rdf:Description>
  <rdf:Description rdf:about="http://purl.org/heritagedata/schemes/225/concepts/111429">
    <skos:broader rdf:resource="http://purl.org/heritagedata/schemes/225/concepts/111402"/>
    <dcterms:issued rdf:datatype="http://www.w3.org/2001/XMLSchema#dateTime">2019-03-26T16:45:43</dcterms:issued>
    <dcterms:identifier>http://purl.org/heritagedata/schemes/225/concepts/111429</dcterms:identifier>
    <cc:attributionName xml:lang="en">Historic England</cc:attributionName>
    <cc:license rdf:resource="http://creativecommons.org/licenses/by/3.0"/>
    <skos:inScheme rdf:resource="http://purl.org/heritagedata/schemes/225"/>
    <cc:attributionURL rdf:resource="http://www.historicengland.org.uk"/>
    <skos:broader rdf:resource="http://purl.org/heritagedata/schemes/225/concepts/111423"/>
    <skos:scopeNote xml:lang="en">British two-seat, twin-engined night fighter. Also used for roles such as long-range escort fighter, ground-attack and anti-shipping strike aircraft, bomber, torpedo-carrier and rocket fighter.</skos:scopeNote>
    <dcterms:publisher rdf:resource="http://www.historicengland.org.uk"/>
    <skos:prefLabel xml:lang="en">Beaufighter</skos:prefLabel>
    <rdf:type rdf:resource="http://www.w3.org/2004/02/skos/core#Concept"/>
    <skos:broader rdf:resource="http://purl.org/heritagedata/schemes/225/concepts/111357"/>
  </rdf:Description>
  <rdf:Description rdf:about="http://purl.org/heritagedata/schemes/225/concepts/141225">
    <skos:inScheme rdf:resource="http://purl.org/heritagedata/schemes/225"/>
    <dcterms:identifier>http://purl.org/heritagedata/schemes/225/concepts/141225</dcterms:identifier>
    <cc:license rdf:resource="http://creativecommons.org/licenses/by/3.0"/>
    <cc:attributionURL rdf:resource="http://www.historicengland.org.uk"/>
    <rdf:type rdf:resource="http://www.w3.org/2004/02/skos/core#Concept"/>
    <skos:prefLabel xml:lang="en">MkX</skos:prefLabel>
    <skos:scopeNote xml:lang="en">Mark 10 or the tenth variant of an aircraft with its associated modifications.</skos:scopeNote>
    <skos:broader rdf:resource="http://purl.org/heritagedata/schemes/225/concepts/141131"/>
    <dcterms:issued rdf:datatype="http://www.w3.org/2001/XMLSchema#dateTime">2019-03-26T16:45:43</dcterms:issued>
    <dcterms:publisher rdf:resource="http://www.historicengland.org.uk"/>
    <cc:attributionName xml:lang="en">Historic England</cc:attributionName>
  </rdf:Description>
  <rdf:Description rdf:about="http://purl.org/heritagedata/schemes/225/concepts/136030">
    <dcterms:publisher rdf:resource="http://www.historicengland.org.uk"/>
    <skos:broader rdf:resource="http://purl.org/heritagedata/schemes/225/concepts/111402"/>
    <dcterms:issued rdf:datatype="http://www.w3.org/2001/XMLSchema#dateTime">2019-03-26T16:45:43</dcterms:issued>
    <skos:inScheme rdf:resource="http://purl.org/heritagedata/schemes/225"/>
    <cc:attributionURL rdf:resource="http://www.historicengland.org.uk"/>
    <rdf:type rdf:resource="http://www.w3.org/2004/02/skos/core#Concept"/>
    <skos:scopeNote xml:lang="en">Impressed civil, twin-engined airliner converted to a military transport. Thirty were ordered for military use, though only eleven were actually built. Entered service in 1940, with the last being scrapped in 1950.</skos:scopeNote>
    <skos:prefLabel xml:lang="en">Flamingo</skos:prefLabel>
    <cc:attributionName xml:lang="en">Historic England</cc:attributionName>
    <cc:license rdf:resource="http://creativecommons.org/licenses/by/3.0"/>
    <skos:broader rdf:resource="http://purl.org/heritagedata/schemes/225/concepts/111368"/>
    <dcterms:identifier>http://purl.org/heritagedata/schemes/225/concepts/136030</dcterms:identifier>
    <skos:broader rdf:resource="http://purl.org/heritagedata/schemes/225/concepts/111424"/>
  </rdf:Description>
  <rdf:Description rdf:about="http://purl.org/heritagedata/schemes/225/concepts/141215">
    <cc:license rdf:resource="http://creativecommons.org/licenses/by/3.0"/>
    <cc:attributionURL rdf:resource="http://www.historicengland.org.uk"/>
    <dcterms:issued rdf:datatype="http://www.w3.org/2001/XMLSchema#dateTime">2019-03-26T16:45:43</dcterms:issued>
    <dcterms:publisher rdf:resource="http://www.historicengland.org.uk"/>
    <cc:attributionName xml:lang="en">Historic England</cc:attributionName>
    <skos:inScheme rdf:resource="http://purl.org/heritagedata/schemes/225"/>
    <rdf:type rdf:resource="http://www.w3.org/2004/02/skos/core#Concept"/>
    <skos:broader rdf:resource="http://purl.org/heritagedata/schemes/225/concepts/141131"/>
    <skos:prefLabel xml:lang="en">MkIII</skos:prefLabel>
    <dcterms:identifier>http://purl.org/heritagedata/schemes/225/concepts/141215</dcterms:identifier>
    <skos:scopeNote xml:lang="en">Mark 3 or the third variant of an aircraft with its associated modifications.</skos:scopeNote>
  </rdf:Description>
  <rdf:Description rdf:about="http://purl.org/heritagedata/schemes/225/concepts/124794">
    <skos:prefLabel xml:lang="en">V1</skos:prefLabel>
    <dcterms:identifier>http://purl.org/heritagedata/schemes/225/concepts/124794</dcterms:identifier>
    <cc:license rdf:resource="http://creativecommons.org/licenses/by/3.0"/>
    <cc:attributionURL rdf:resource="http://www.historicengland.org.uk"/>
    <skos:narrower rdf:resource="http://purl.org/heritagedata/schemes/225/concepts/151397"/>
    <dcterms:issued rdf:datatype="http://www.w3.org/2001/XMLSchema#dateTime">2019-03-26T16:45:43</dcterms:issued>
    <skos:scopeNote xml:lang="en">Jet-propelled, pilotless aircraft carrying a one-ton explosive warhead. Also known as the Fieseler FI-103, the V1 was nicknamed the doodlebug, or buzz bomb.</skos:scopeNote>
    <skos:broader rdf:resource="http://purl.org/heritagedata/schemes/225/concepts/124793"/>
    <rdf:type rdf:resource="http://www.w3.org/2004/02/skos/core#Concept"/>
    <skos:inScheme rdf:resource="http://purl.org/heritagedata/schemes/225"/>
    <cc:attributionName xml:lang="en">Historic England</cc:attributionName>
    <dcterms:publisher rdf:resource="http://www.historicengland.org.uk"/>
  </rdf:Description>
  <rdf:Description rdf:about="http://purl.org/heritagedata/schemes/225/concepts/111413">
    <skos:narrower rdf:resource="http://purl.org/heritagedata/schemes/225/concepts/167858"/>
    <cc:license rdf:resource="http://creativecommons.org/licenses/by/3.0"/>
    <cc:attributionName xml:lang="en">Historic England</cc:attributionName>
    <skos:inScheme rdf:resource="http://purl.org/heritagedata/schemes/225"/>
    <skos:prefLabel xml:lang="en">Gloster</skos:prefLabel>
    <skos:narrower rdf:resource="http://purl.org/heritagedata/schemes/225/concepts/136593"/>
    <skos:broader rdf:resource="http://purl.org/heritagedata/schemes/225/concepts/111358"/>
    <skos:narrower rdf:resource="http://purl.org/heritagedata/schemes/225/concepts/111414"/>
    <skos:scopeNote xml:lang="en">Gloster Aircraft Co., Ltd. formed in 1917, later became part of the Hawker Siddeley Group. First British or American company to design, build and fly a jet-propelled aircraft.</skos:scopeNote>
    <skos:narrower rdf:resource="http://purl.org/heritagedata/schemes/225/concepts/167000"/>
    <cc:attributionURL rdf:resource="http://www.historicengland.org.uk"/>
    <rdf:type rdf:resource="http://www.w3.org/2004/02/skos/core#Concept"/>
    <dcterms:issued rdf:datatype="http://www.w3.org/2001/XMLSchema#dateTime">2019-03-26T16:45:43</dcterms:issued>
    <skos:narrower rdf:resource="http://purl.org/heritagedata/schemes/225/concepts/136231"/>
    <dcterms:identifier>http://purl.org/heritagedata/schemes/225/concepts/111413</dcterms:identifier>
    <dcterms:publisher rdf:resource="http://www.historicengland.org.uk"/>
  </rdf:Description>
  <rdf:Description rdf:about="http://purl.org/heritagedata/schemes/225/concepts/137214">
    <skos:broader rdf:resource="http://purl.org/heritagedata/schemes/225/concepts/135751"/>
    <cc:attributionURL rdf:resource="http://www.historicengland.org.uk"/>
    <skos:scopeNote xml:lang="en">Originally ordered as land based dive-bombers, with 950 being delivered to the RAF, none are known to have flown operationally, instead apparently serving as target tugs. Bermuda was the name given to the Brewster SB2A Buccaneer in RAF service.</skos:scopeNote>
    <skos:broader rdf:resource="http://purl.org/heritagedata/schemes/225/concepts/111402"/>
    <rdf:type rdf:resource="http://www.w3.org/2004/02/skos/core#Concept"/>
    <dcterms:publisher rdf:resource="http://www.historicengland.org.uk"/>
    <skos:broader rdf:resource="http://purl.org/heritagedata/schemes/225/concepts/137213"/>
    <cc:attributionName xml:lang="en">Historic England</cc:attributionName>
    <dcterms:issued rdf:datatype="http://www.w3.org/2001/XMLSchema#dateTime">2019-03-26T16:45:43</dcterms:issued>
    <skos:inScheme rdf:resource="http://purl.org/heritagedata/schemes/225"/>
    <skos:prefLabel xml:lang="en">Bermuda</skos:prefLabel>
    <cc:license rdf:resource="http://creativecommons.org/licenses/by/3.0"/>
    <dcterms:identifier>http://purl.org/heritagedata/schemes/225/concepts/137214</dcterms:identifier>
  </rdf:Description>
  <rdf:Description rdf:about="http://purl.org/heritagedata/schemes/225/concepts/138536">
    <dcterms:identifier>http://purl.org/heritagedata/schemes/225/concepts/138536</dcterms:identifier>
    <cc:license rdf:resource="http://creativecommons.org/licenses/by/3.0"/>
    <cc:attributionName xml:lang="en">Historic England</cc:attributionName>
    <cc:attributionURL rdf:resource="http://www.historicengland.org.uk"/>
    <skos:inScheme rdf:resource="http://purl.org/heritagedata/schemes/225"/>
    <skos:scopeNote xml:lang="en">Originally designed as a trainer but relegated to use by the RNAS in a Maritime Reconnaissance and anti-submarine role when the Avro 504 became the standard trainer.</skos:scopeNote>
    <skos:broader rdf:resource="http://purl.org/heritagedata/schemes/225/concepts/135730"/>
    <dcterms:issued rdf:datatype="http://www.w3.org/2001/XMLSchema#dateTime">2019-03-26T16:45:43</dcterms:issued>
    <skos:prefLabel xml:lang="en">Airco DH6</skos:prefLabel>
    <skos:broader rdf:resource="http://purl.org/heritagedata/schemes/225/concepts/111403"/>
    <rdf:type rdf:resource="http://www.w3.org/2004/02/skos/core#Concept"/>
    <dcterms:publisher rdf:resource="http://www.historicengland.org.uk"/>
    <skos:broader rdf:resource="http://purl.org/heritagedata/schemes/225/concepts/136512"/>
  </rdf:Description>
  <rdf:Description rdf:about="http://purl.org/heritagedata/schemes/225/concepts/137208">
    <skos:broader rdf:resource="http://purl.org/heritagedata/schemes/225/concepts/111353"/>
    <skos:scopeNote xml:lang="en">Twin-engined, seven-crew, coastal reconnaissance, biplane flying-boat. Designed to the same specification as the Saro London, entered service in 1937. Also serving in an anti-submarine role, was replaced by the Consolidated Canso (Catalina) in 1943.</skos:scopeNote>
    <skos:broader rdf:resource="http://purl.org/heritagedata/schemes/225/concepts/111395"/>
    <dcterms:publisher rdf:resource="http://www.historicengland.org.uk"/>
    <cc:attributionName xml:lang="en">Historic England</cc:attributionName>
    <rdf:type rdf:resource="http://www.w3.org/2004/02/skos/core#Concept"/>
    <skos:broader rdf:resource="http://purl.org/heritagedata/schemes/225/concepts/135730"/>
    <cc:license rdf:resource="http://creativecommons.org/licenses/by/3.0"/>
    <skos:inScheme rdf:resource="http://purl.org/heritagedata/schemes/225"/>
    <cc:attributionURL rdf:resource="http://www.historicengland.org.uk"/>
    <dcterms:issued rdf:datatype="http://www.w3.org/2001/XMLSchema#dateTime">2019-03-26T16:45:43</dcterms:issued>
    <dcterms:identifier>http://purl.org/heritagedata/schemes/225/concepts/137208</dcterms:identifier>
    <skos:prefLabel xml:lang="en">Stranraer</skos:prefLabel>
    <skos:broader rdf:resource="http://purl.org/heritagedata/schemes/225/concepts/111403"/>
  </rdf:Description>
  <rdf:Description rdf:about="http://purl.org/heritagedata/schemes/225/concepts/138546">
    <cc:license rdf:resource="http://creativecommons.org/licenses/by/3.0"/>
    <skos:broader rdf:resource="http://purl.org/heritagedata/schemes/225/concepts/135730"/>
    <dcterms:publisher rdf:resource="http://www.historicengland.org.uk"/>
    <skos:inScheme rdf:resource="http://purl.org/heritagedata/schemes/225"/>
    <skos:prefLabel xml:lang="en">Felixstowe F5</skos:prefLabel>
    <cc:attributionName xml:lang="en">Historic England</cc:attributionName>
    <skos:broader rdf:resource="http://purl.org/heritagedata/schemes/225/concepts/136252"/>
    <skos:broader rdf:resource="http://purl.org/heritagedata/schemes/225/concepts/111403"/>
    <rdf:type rdf:resource="http://www.w3.org/2004/02/skos/core#Concept"/>
    <dcterms:identifier>http://purl.org/heritagedata/schemes/225/concepts/138546</dcterms:identifier>
    <dcterms:issued rdf:datatype="http://www.w3.org/2001/XMLSchema#dateTime">2019-03-26T16:45:43</dcterms:issued>
    <skos:scopeNote xml:lang="en">Four-crew, twin-engined, general reconnaissance flying-boat. Entered service after World War One, becoming the RAF's standard flying-boat until replaced by the Supermarine Southampton in 1925.</skos:scopeNote>
    <cc:attributionURL rdf:resource="http://www.historicengland.org.uk"/>
    <skos:broader rdf:resource="http://purl.org/heritagedata/schemes/225/concepts/111395"/>
  </rdf:Description>
  <rdf:Description rdf:about="http://purl.org/heritagedata/schemes/225/concepts/141359">
    <cc:attributionURL rdf:resource="http://www.historicengland.org.uk"/>
    <skos:narrower rdf:resource="http://purl.org/heritagedata/schemes/225/concepts/141353"/>
    <rdf:type rdf:resource="http://www.w3.org/2004/02/skos/core#Concept"/>
    <skos:broader rdf:resource="http://purl.org/heritagedata/schemes/225/concepts/111394"/>
    <dcterms:publisher rdf:resource="http://www.historicengland.org.uk"/>
    <cc:attributionName xml:lang="en">Historic England</cc:attributionName>
    <dcterms:identifier>http://purl.org/heritagedata/schemes/225/concepts/141359</dcterms:identifier>
    <skos:inScheme rdf:resource="http://purl.org/heritagedata/schemes/225"/>
    <dcterms:issued rdf:datatype="http://www.w3.org/2001/XMLSchema#dateTime">2019-03-26T16:45:43</dcterms:issued>
    <skos:prefLabel xml:lang="en">Communications</skos:prefLabel>
    <skos:scopeNote xml:lang="en">An aircraft used to facilitate communications, for example in a military context.</skos:scopeNote>
    <skos:narrower rdf:resource="http://purl.org/heritagedata/schemes/225/concepts/141399"/>
    <cc:license rdf:resource="http://creativecommons.org/licenses/by/3.0"/>
  </rdf:Description>
  <rdf:Description rdf:about="http://purl.org/heritagedata/schemes/225/concepts/111377">
    <dcterms:issued rdf:datatype="http://www.w3.org/2001/XMLSchema#dateTime">2019-03-26T16:45:43</dcterms:issued>
    <dcterms:publisher rdf:resource="http://www.historicengland.org.uk"/>
    <dcterms:identifier>http://purl.org/heritagedata/schemes/225/concepts/111377</dcterms:identifier>
    <skos:scopeNote xml:lang="en">Twin-engined bomber. The Whitley was the first 'heavy' bomber to be built in quantity for the RAF and made the first bombing attack on Germany in May 1940. It was later used for convoy protection and reconnaissance.</skos:scopeNote>
    <skos:prefLabel xml:lang="en">Whitley</skos:prefLabel>
    <skos:broader rdf:resource="http://purl.org/heritagedata/schemes/225/concepts/137190"/>
    <cc:license rdf:resource="http://creativecommons.org/licenses/by/3.0"/>
    <cc:attributionName xml:lang="en">Historic England</cc:attributionName>
    <cc:attributionURL rdf:resource="http://www.historicengland.org.uk"/>
    <skos:inScheme rdf:resource="http://purl.org/heritagedata/schemes/225"/>
    <skos:broader rdf:resource="http://purl.org/heritagedata/schemes/225/concepts/111402"/>
    <rdf:type rdf:resource="http://www.w3.org/2004/02/skos/core#Concept"/>
    <skos:broader rdf:resource="http://purl.org/heritagedata/schemes/225/concepts/111376"/>
  </rdf:Description>
  <rdf:Description rdf:about="http://purl.org/heritagedata/schemes/225/concepts/125493">
    <skos:broader rdf:resource="http://purl.org/heritagedata/schemes/225/concepts/111399"/>
    <dcterms:issued rdf:datatype="http://www.w3.org/2001/XMLSchema#dateTime">2019-03-26T16:45:43</dcterms:issued>
    <cc:attributionName xml:lang="en">Historic England</cc:attributionName>
    <skos:broader rdf:resource="http://purl.org/heritagedata/schemes/225/concepts/111402"/>
    <skos:broader rdf:resource="http://purl.org/heritagedata/schemes/225/concepts/125494"/>
    <skos:inScheme rdf:resource="http://purl.org/heritagedata/schemes/225"/>
    <skos:prefLabel xml:lang="en">P47 Thunderbolt</skos:prefLabel>
    <dcterms:publisher rdf:resource="http://www.historicengland.org.uk"/>
    <cc:attributionURL rdf:resource="http://www.historicengland.org.uk"/>
    <dcterms:identifier>http://purl.org/heritagedata/schemes/225/concepts/125493</dcterms:identifier>
    <cc:license rdf:resource="http://creativecommons.org/licenses/by/3.0"/>
    <rdf:type rdf:resource="http://www.w3.org/2004/02/skos/core#Concept"/>
    <skos:scopeNote xml:lang="en">Single-seat, single-engine fighter-bomber. Fitted with eight fixed forward-firing machine guns in the wings, plus two 1000lb bombs or six rocket projectiles.</skos:scopeNote>
  </rdf:Description>
  <rdf:Description rdf:about="http://purl.org/heritagedata/schemes/225/concepts/136521">
    <dcterms:publisher rdf:resource="http://www.historicengland.org.uk"/>
    <skos:inScheme rdf:resource="http://purl.org/heritagedata/schemes/225"/>
    <skos:prefLabel xml:lang="en">Atlas</skos:prefLabel>
    <rdf:type rdf:resource="http://www.w3.org/2004/02/skos/core#Concept"/>
    <cc:license rdf:resource="http://creativecommons.org/licenses/by/3.0"/>
    <dcterms:identifier>http://purl.org/heritagedata/schemes/225/concepts/136521</dcterms:identifier>
    <cc:attributionURL rdf:resource="http://www.historicengland.org.uk"/>
    <dcterms:issued rdf:datatype="http://www.w3.org/2001/XMLSchema#dateTime">2019-03-26T16:45:43</dcterms:issued>
    <skos:broader rdf:resource="http://purl.org/heritagedata/schemes/225/concepts/111376"/>
    <cc:attributionName xml:lang="en">Historic England</cc:attributionName>
    <skos:scopeNote xml:lang="en">A two-seat, general purpose biplane. The first to be designed specifically for an Army Co-operation role, it entered service in late 1927. Ended its service as a communications and advanced trainer aircraft.</skos:scopeNote>
    <skos:broader rdf:resource="http://purl.org/heritagedata/schemes/225/concepts/111403"/>
  </rdf:Description>
  <rdf:Description rdf:about="http://purl.org/heritagedata/schemes/225/concepts/136526">
    <cc:attributionURL rdf:resource="http://www.historicengland.org.uk"/>
    <rdf:type rdf:resource="http://www.w3.org/2004/02/skos/core#Concept"/>
    <skos:prefLabel xml:lang="en">Tutor</skos:prefLabel>
    <cc:attributionName xml:lang="en">Historic England</cc:attributionName>
    <cc:license rdf:resource="http://creativecommons.org/licenses/by/3.0"/>
    <dcterms:identifier>http://purl.org/heritagedata/schemes/225/concepts/136526</dcterms:identifier>
    <skos:broader rdf:resource="http://purl.org/heritagedata/schemes/225/concepts/111401"/>
    <skos:scopeNote xml:lang="en">A two-seat trainer chosen to replace the Avro 504. 380 entered RAF service with many finding their way onto the civilian market at the end of their careers.</skos:scopeNote>
    <dcterms:publisher rdf:resource="http://www.historicengland.org.uk"/>
    <skos:broader rdf:resource="http://purl.org/heritagedata/schemes/225/concepts/111355"/>
    <skos:inScheme rdf:resource="http://purl.org/heritagedata/schemes/225"/>
    <dcterms:issued rdf:datatype="http://www.w3.org/2001/XMLSchema#dateTime">2019-03-26T16:45:43</dcterms:issued>
    <skos:broader rdf:resource="http://purl.org/heritagedata/schemes/225/concepts/111403"/>
  </rdf:Description>
  <rdf:Description rdf:about="http://purl.org/heritagedata/schemes/225/concepts/137218">
    <skos:narrower rdf:resource="http://purl.org/heritagedata/schemes/225/concepts/137220"/>
    <skos:scopeNote xml:lang="en">The Grumman Aircraft Engineering Corporation founded by Leroy R Grumman and incorporated in 1929.</skos:scopeNote>
    <dcterms:identifier>http://purl.org/heritagedata/schemes/225/concepts/137218</dcterms:identifier>
    <skos:narrower rdf:resource="http://purl.org/heritagedata/schemes/225/concepts/137219"/>
    <cc:license rdf:resource="http://creativecommons.org/licenses/by/3.0"/>
    <cc:attributionName xml:lang="en">Historic England</cc:attributionName>
    <cc:attributionURL rdf:resource="http://www.historicengland.org.uk"/>
    <skos:inScheme rdf:resource="http://purl.org/heritagedata/schemes/225"/>
    <skos:narrower rdf:resource="http://purl.org/heritagedata/schemes/225/concepts/137221"/>
    <dcterms:issued rdf:datatype="http://www.w3.org/2001/XMLSchema#dateTime">2019-03-26T16:45:43</dcterms:issued>
    <skos:prefLabel xml:lang="en">Grumman</skos:prefLabel>
    <rdf:type rdf:resource="http://www.w3.org/2004/02/skos/core#Concept"/>
    <dcterms:publisher rdf:resource="http://www.historicengland.org.uk"/>
    <skos:broader rdf:resource="http://purl.org/heritagedata/schemes/225/concepts/111358"/>
  </rdf:Description>
  <rdf:Description rdf:about="http://purl.org/heritagedata/schemes/225/concepts/136220">
    <dcterms:identifier>http://purl.org/heritagedata/schemes/225/concepts/136220</dcterms:identifier>
    <cc:attributionName xml:lang="en">Historic England</cc:attributionName>
    <cc:attributionURL rdf:resource="http://www.historicengland.org.uk"/>
    <skos:inScheme rdf:resource="http://purl.org/heritagedata/schemes/225"/>
    <skos:scopeNote xml:lang="en">Twin-engined, medium bomber with a 1200 mile range and a bomb load in excess of 10,000 lb. Entered service in 1940, but engine faults resulted in retirement in 1942 with its design later modified into the acclaimed four-engine Lancaster bomber.</skos:scopeNote>
    <cc:license rdf:resource="http://creativecommons.org/licenses/by/3.0"/>
    <skos:prefLabel xml:lang="en">Manchester</skos:prefLabel>
    <dcterms:issued rdf:datatype="http://www.w3.org/2001/XMLSchema#dateTime">2019-03-26T16:45:43</dcterms:issued>
    <skos:broader rdf:resource="http://purl.org/heritagedata/schemes/225/concepts/111402"/>
    <rdf:type rdf:resource="http://www.w3.org/2004/02/skos/core#Concept"/>
    <ns1:related rdf:resource="http://purl.org/heritagedata/schemes/225/concepts/111367"/>
    <skos:broader rdf:resource="http://purl.org/heritagedata/schemes/225/concepts/139626"/>
    <dcterms:publisher rdf:resource="http://www.historicengland.org.uk"/>
    <skos:broader rdf:resource="http://purl.org/heritagedata/schemes/225/concepts/111355"/>
  </rdf:Description>
  <rdf:Description rdf:about="http://purl.org/heritagedata/schemes/225/concepts/111422">
    <skos:inScheme rdf:resource="http://purl.org/heritagedata/schemes/225"/>
    <rdf:type rdf:resource="http://www.w3.org/2004/02/skos/core#Concept"/>
    <skos:prefLabel xml:lang="en">Stirling</skos:prefLabel>
    <skos:broader rdf:resource="http://purl.org/heritagedata/schemes/225/concepts/137190"/>
    <skos:broader rdf:resource="http://purl.org/heritagedata/schemes/225/concepts/111402"/>
    <skos:broader rdf:resource="http://purl.org/heritagedata/schemes/225/concepts/111421"/>
    <skos:scopeNote xml:lang="en">Seven/eight-crew, heavy night-bomber. The first four-engine bomber to join the RAF, with a bomb load of 14000 lb, entered service in 1940. Superseded as a bomber by the Lancaster and Halifax, later versions served as transports and tugs.</skos:scopeNote>
    <cc:license rdf:resource="http://creativecommons.org/licenses/by/3.0"/>
    <cc:attributionURL rdf:resource="http://www.historicengland.org.uk"/>
    <dcterms:issued rdf:datatype="http://www.w3.org/2001/XMLSchema#dateTime">2019-03-26T16:45:43</dcterms:issued>
    <dcterms:identifier>http://purl.org/heritagedata/schemes/225/concepts/111422</dcterms:identifier>
    <dcterms:publisher rdf:resource="http://www.historicengland.org.uk"/>
    <cc:attributionName xml:lang="en">Historic England</cc:attributionName>
  </rdf:Description>
  <rdf:Description rdf:about="http://purl.org/heritagedata/schemes/225/concepts/137220">
    <skos:scopeNote xml:lang="en">American, single-engine fighter designed for operation from US Naval aircraft carriers. The Hellcat was a more powerful version of the Wildcat, a total of 1000 being provided to the Fleet Air Arm under Lend-Lease.</skos:scopeNote>
    <skos:broader rdf:resource="http://purl.org/heritagedata/schemes/225/concepts/111402"/>
    <rdf:type rdf:resource="http://www.w3.org/2004/02/skos/core#Concept"/>
    <dcterms:publisher rdf:resource="http://www.historicengland.org.uk"/>
    <skos:broader rdf:resource="http://purl.org/heritagedata/schemes/225/concepts/137218"/>
    <cc:license rdf:resource="http://creativecommons.org/licenses/by/3.0"/>
    <cc:attributionName xml:lang="en">Historic England</cc:attributionName>
    <cc:attributionURL rdf:resource="http://www.historicengland.org.uk"/>
    <skos:inScheme rdf:resource="http://purl.org/heritagedata/schemes/225"/>
    <dcterms:identifier>http://purl.org/heritagedata/schemes/225/concepts/137220</dcterms:identifier>
    <skos:prefLabel xml:lang="en">F6F Hellcat</skos:prefLabel>
    <dcterms:issued rdf:datatype="http://www.w3.org/2001/XMLSchema#dateTime">2019-03-26T16:45:43</dcterms:issued>
    <ns1:related rdf:resource="http://purl.org/heritagedata/schemes/225/concepts/137221"/>
    <skos:broader rdf:resource="http://purl.org/heritagedata/schemes/225/concepts/111397"/>
  </rdf:Description>
  <rdf:Description rdf:about="http://purl.org/heritagedata/schemes/225/concepts/167006">
    <cc:attributionName xml:lang="en">Historic England</cc:attributionName>
    <cc:license rdf:resource="http://creativecommons.org/licenses/by/3.0"/>
    <skos:inScheme rdf:resource="http://purl.org/heritagedata/schemes/225"/>
    <cc:attributionURL rdf:resource="http://www.historicengland.org.uk"/>
    <dcterms:issued rdf:datatype="http://www.w3.org/2001/XMLSchema#dateTime">2019-03-26T16:45:43</dcterms:issued>
    <skos:prefLabel xml:lang="en">Fokker FVIII</skos:prefLabel>
    <skos:scopeNote xml:lang="en">A large twin-engined airliner produced by the Dutch aircraft manufacturer Fokker in the 1920s. First flight March 1927. Designed by Reinhold Platz. Mixed construction, fuselage/ tail in steel covered with plywood, canvas and duralumin (11 units built).</skos:scopeNote>
    <dcterms:identifier>http://purl.org/heritagedata/schemes/225/concepts/167006</dcterms:identifier>
    <skos:broader rdf:resource="http://purl.org/heritagedata/schemes/225/concepts/167002"/>
    <dcterms:publisher rdf:resource="http://www.historicengland.org.uk"/>
    <rdf:type rdf:resource="http://www.w3.org/2004/02/skos/core#Concept"/>
  </rdf:Description>
  <rdf:Description rdf:about="http://purl.org/heritagedata/schemes/225/concepts/167009">
    <cc:attributionName xml:lang="en">Historic England</cc:attributionName>
    <skos:inScheme rdf:resource="http://purl.org/heritagedata/schemes/225"/>
    <skos:broader rdf:resource="http://purl.org/heritagedata/schemes/225/concepts/136031"/>
    <skos:broader rdf:resource="http://purl.org/heritagedata/schemes/225/concepts/111359"/>
    <dcterms:identifier>http://purl.org/heritagedata/schemes/225/concepts/167009</dcterms:identifier>
    <skos:scopeNote xml:lang="en">A British two-seater army co-operation aircraft manufactured by Hawker Aircraft for the Royal Air Force. A Hart variant biplane that first flew in 1931, becoming a prominent British aircraft in the inter-war period with over 700 units built.</skos:scopeNote>
    <skos:prefLabel xml:lang="en">Audax</skos:prefLabel>
    <cc:license rdf:resource="http://creativecommons.org/licenses/by/3.0"/>
    <cc:attributionURL rdf:resource="http://www.historicengland.org.uk"/>
    <rdf:type rdf:resource="http://www.w3.org/2004/02/skos/core#Concept"/>
    <skos:broader rdf:resource="http://purl.org/heritagedata/schemes/225/concepts/111403"/>
    <dcterms:issued rdf:datatype="http://www.w3.org/2001/XMLSchema#dateTime">2019-03-26T16:45:43</dcterms:issued>
    <dcterms:publisher rdf:resource="http://www.historicengland.org.uk"/>
  </rdf:Description>
  <rdf:Description rdf:about="http://purl.org/heritagedata/schemes/225/concepts/111373">
    <dcterms:identifier>http://purl.org/heritagedata/schemes/225/concepts/111373</dcterms:identifier>
    <dcterms:issued rdf:datatype="http://www.w3.org/2001/XMLSchema#dateTime">2019-03-26T16:45:43</dcterms:issued>
    <skos:broader rdf:resource="http://purl.org/heritagedata/schemes/225/concepts/111423"/>
    <cc:attributionName xml:lang="en">Historic England</cc:attributionName>
    <skos:scopeNote xml:lang="en">Developed as a long range, heavy day-fighter, the ME110 found its niche as a night fighter. It saw service over Southern and Eastern England during the Battle of Britain but lost out in the daytime to the faster British fighters.</skos:scopeNote>
    <skos:broader rdf:resource="http://purl.org/heritagedata/schemes/225/concepts/111402"/>
    <skos:inScheme rdf:resource="http://purl.org/heritagedata/schemes/225"/>
    <skos:prefLabel xml:lang="en">Me110</skos:prefLabel>
    <dcterms:publisher rdf:resource="http://www.historicengland.org.uk"/>
    <cc:attributionURL rdf:resource="http://www.historicengland.org.uk"/>
    <cc:license rdf:resource="http://creativecommons.org/licenses/by/3.0"/>
    <rdf:type rdf:resource="http://www.w3.org/2004/02/skos/core#Concept"/>
    <skos:broader rdf:resource="http://purl.org/heritagedata/schemes/225/concepts/118653"/>
  </rdf:Description>
  <rdf:Description rdf:about="http://purl.org/heritagedata/schemes/225/concepts/125554">
    <cc:license rdf:resource="http://creativecommons.org/licenses/by/3.0"/>
    <cc:attributionURL rdf:resource="http://www.historicengland.org.uk"/>
    <dcterms:issued rdf:datatype="http://www.w3.org/2001/XMLSchema#dateTime">2019-03-26T16:45:43</dcterms:issued>
    <skos:broader rdf:resource="http://purl.org/heritagedata/schemes/225/concepts/111433"/>
    <ns1:related rdf:resource="http://purl.org/heritagedata/schemes/225/concepts/141268"/>
    <dcterms:publisher rdf:resource="http://www.historicengland.org.uk"/>
    <cc:attributionName xml:lang="en">Historic England</cc:attributionName>
    <skos:inScheme rdf:resource="http://purl.org/heritagedata/schemes/225"/>
    <rdf:type rdf:resource="http://www.w3.org/2004/02/skos/core#Concept"/>
    <dcterms:identifier>http://purl.org/heritagedata/schemes/225/concepts/125554</dcterms:identifier>
    <skos:broader rdf:resource="http://purl.org/heritagedata/schemes/225/concepts/111402"/>
    <skos:broader rdf:resource="http://purl.org/heritagedata/schemes/225/concepts/137190"/>
    <skos:prefLabel xml:lang="en">B29 Superfortress</skos:prefLabel>
    <skos:scopeNote xml:lang="en">American, four-engine, long range, heavy strategic bomber. Entered service in 1943 and used exclusively against Japanese forces. The B29s Enola Gay and Bock's Car were used to drop atomic bombs on Hiroshima and Nagasaki in 1945.</skos:scopeNote>
  </rdf:Description>
  <rdf:Description rdf:about="http://purl.org/heritagedata/schemes/225/concepts/152401">
    <dcterms:issued rdf:datatype="http://www.w3.org/2001/XMLSchema#dateTime">2019-03-26T16:45:43</dcterms:issued>
    <dcterms:identifier>http://purl.org/heritagedata/schemes/225/concepts/152401</dcterms:identifier>
    <skos:prefLabel xml:lang="en">F4 Phantom</skos:prefLabel>
    <cc:attributionURL rdf:resource="http://www.historicengland.org.uk"/>
    <skos:scopeNote xml:lang="en">A tandem two-seat, twin-engined, all-weather, long-range supersonic jet interceptor fighter/fighter-bomber originally developed for the United States Navy by McDonnell Aircraft.It first entered service in 1960 with the U.S. Navy.</skos:scopeNote>
    <skos:inScheme rdf:resource="http://purl.org/heritagedata/schemes/225"/>
    <dcterms:publisher rdf:resource="http://www.historicengland.org.uk"/>
    <cc:license rdf:resource="http://creativecommons.org/licenses/by/3.0"/>
    <cc:attributionName xml:lang="en">Historic England</cc:attributionName>
    <skos:broader rdf:resource="http://purl.org/heritagedata/schemes/225/concepts/111397"/>
    <skos:broader rdf:resource="http://purl.org/heritagedata/schemes/225/concepts/152400"/>
    <skos:broader rdf:resource="http://purl.org/heritagedata/schemes/225/concepts/111402"/>
    <rdf:type rdf:resource="http://www.w3.org/2004/02/skos/core#Concept"/>
  </rdf:Description>
  <rdf:Description rdf:about="http://purl.org/heritagedata/schemes/225/concepts/111438">
    <skos:altLabel xml:lang="en">Superfortress</skos:altLabel>
  </rdf:Description>
  <rdf:Description rdf:about="http://purl.org/heritagedata/schemes/225/concepts/111370">
    <skos:broader rdf:resource="http://purl.org/heritagedata/schemes/225/concepts/139626"/>
    <cc:license rdf:resource="http://creativecommons.org/licenses/by/3.0"/>
    <dcterms:publisher rdf:resource="http://www.historicengland.org.uk"/>
    <cc:attributionURL rdf:resource="http://www.historicengland.org.uk"/>
    <skos:inScheme rdf:resource="http://purl.org/heritagedata/schemes/225"/>
    <skos:broader rdf:resource="http://purl.org/heritagedata/schemes/225/concepts/111356"/>
    <cc:attributionName xml:lang="en">Historic England</cc:attributionName>
    <skos:broader rdf:resource="http://purl.org/heritagedata/schemes/225/concepts/111402"/>
    <rdf:type rdf:resource="http://www.w3.org/2004/02/skos/core#Concept"/>
    <skos:scopeNote xml:lang="en">The main German, medium bomber of the war, the HE111 first saw action during the Spanish Civil War. HE111s took part in the Battle of Britain and from 1944 onwards were used to launch airborne flying bombs against London.</skos:scopeNote>
    <dcterms:issued rdf:datatype="http://www.w3.org/2001/XMLSchema#dateTime">2019-03-26T16:45:43</dcterms:issued>
    <skos:prefLabel xml:lang="en">He111</skos:prefLabel>
    <dcterms:identifier>http://purl.org/heritagedata/schemes/225/concepts/111370</dcterms:identifier>
  </rdf:Description>
  <rdf:Description rdf:about="http://purl.org/heritagedata/schemes/225/concepts/111360">
    <skos:broader rdf:resource="http://purl.org/heritagedata/schemes/225/concepts/111359"/>
    <skos:inScheme rdf:resource="http://purl.org/heritagedata/schemes/225"/>
    <dcterms:issued rdf:datatype="http://www.w3.org/2001/XMLSchema#dateTime">2019-03-26T16:45:43</dcterms:issued>
    <dcterms:publisher rdf:resource="http://www.historicengland.org.uk"/>
    <rdf:type rdf:resource="http://www.w3.org/2004/02/skos/core#Concept"/>
    <skos:broader rdf:resource="http://purl.org/heritagedata/schemes/225/concepts/111402"/>
    <skos:scopeNote xml:lang="en">Single-engine, single-seat fighter, also adapted as a night-fighter, fighter-bomber, rocket-projectile fighter and tank-buster. The first monoplane to enter RAF service with 14,000 being produced between 1937 and 1944.</skos:scopeNote>
    <skos:prefLabel xml:lang="en">Hurricane</skos:prefLabel>
    <skos:broader rdf:resource="http://purl.org/heritagedata/schemes/225/concepts/111397"/>
    <cc:attributionName xml:lang="en">Historic England</cc:attributionName>
    <cc:license rdf:resource="http://creativecommons.org/licenses/by/3.0"/>
    <dcterms:identifier>http://purl.org/heritagedata/schemes/225/concepts/111360</dcterms:identifier>
    <cc:attributionURL rdf:resource="http://www.historicengland.org.uk"/>
  </rdf:Description>
  <rdf:Description rdf:about="http://purl.org/heritagedata/schemes/225/concepts/133173">
    <cc:license rdf:resource="http://creativecommons.org/licenses/by/3.0"/>
    <rdf:type rdf:resource="http://www.w3.org/2004/02/skos/core#Concept"/>
    <cc:attributionURL rdf:resource="http://www.historicengland.org.uk"/>
    <skos:inScheme rdf:resource="http://purl.org/heritagedata/schemes/225"/>
    <cc:attributionName xml:lang="en">Historic England</cc:attributionName>
    <dcterms:identifier>http://purl.org/heritagedata/schemes/225/concepts/133173</dcterms:identifier>
    <dcterms:issued rdf:datatype="http://www.w3.org/2001/XMLSchema#dateTime">2019-03-26T16:45:43</dcterms:issued>
    <skos:prefLabel xml:lang="en">Hampden</skos:prefLabel>
    <skos:broader rdf:resource="http://purl.org/heritagedata/schemes/225/concepts/111402"/>
    <skos:broader rdf:resource="http://purl.org/heritagedata/schemes/225/concepts/139626"/>
    <skos:scopeNote xml:lang="en">Four-seat, twin-engined medium bomber. Entered service in 1938. After serving Bomber Command from 1939-42, was converted to a torpedo-bomber and mine-layer with RAF Coastal Command.</skos:scopeNote>
    <dcterms:publisher rdf:resource="http://www.historicengland.org.uk"/>
    <ns1:related rdf:resource="http://purl.org/heritagedata/schemes/225/concepts/137203"/>
    <skos:broader rdf:resource="http://purl.org/heritagedata/schemes/225/concepts/111415"/>
  </rdf:Description>
  <rdf:Description rdf:about="http://purl.org/heritagedata/schemes/225/concepts/136610">
    <rdf:type rdf:resource="http://www.w3.org/2004/02/skos/core#Concept"/>
    <dcterms:issued rdf:datatype="http://www.w3.org/2001/XMLSchema#dateTime">2019-03-26T16:45:43</dcterms:issued>
    <dcterms:publisher rdf:resource="http://www.historicengland.org.uk"/>
    <skos:broader rdf:resource="http://purl.org/heritagedata/schemes/225/concepts/111395"/>
    <skos:broader rdf:resource="http://purl.org/heritagedata/schemes/225/concepts/135730"/>
    <skos:scopeNote xml:lang="en">Three/four-crew, single-engine, shipboard observation and air/sea rescue amphibian seaplane. Entered RAF service in 1936. Also employed for gunnery spotting, anti-submarine and convoy protection duties.</skos:scopeNote>
    <cc:attributionName xml:lang="en">Historic England</cc:attributionName>
    <dcterms:identifier>http://purl.org/heritagedata/schemes/225/concepts/136610</dcterms:identifier>
    <cc:attributionURL rdf:resource="http://www.historicengland.org.uk"/>
    <cc:license rdf:resource="http://creativecommons.org/licenses/by/3.0"/>
    <skos:prefLabel xml:lang="en">Walrus</skos:prefLabel>
    <skos:broader rdf:resource="http://purl.org/heritagedata/schemes/225/concepts/135930"/>
    <skos:inScheme rdf:resource="http://purl.org/heritagedata/schemes/225"/>
    <skos:broader rdf:resource="http://purl.org/heritagedata/schemes/225/concepts/111403"/>
  </rdf:Description>
  <rdf:Description rdf:about="http://purl.org/heritagedata/schemes/225/concepts/138484">
    <skos:broader rdf:resource="http://purl.org/heritagedata/schemes/225/concepts/111358"/>
    <dcterms:identifier>http://purl.org/heritagedata/schemes/225/concepts/138484</dcterms:identifier>
    <rdf:type rdf:resource="http://www.w3.org/2004/02/skos/core#Concept"/>
    <skos:narrower rdf:resource="http://purl.org/heritagedata/schemes/225/concepts/138485"/>
    <skos:scopeNote xml:lang="en">Chance Vought Division of the United Aircraft Corporation. Was reconstituted as a separate division in 1943, after being part of the Vought-Sikorsky division, to concentrate on the production of combat aircraft.</skos:scopeNote>
    <dcterms:issued rdf:datatype="http://www.w3.org/2001/XMLSchema#dateTime">2019-03-26T16:45:43</dcterms:issued>
    <skos:inScheme rdf:resource="http://purl.org/heritagedata/schemes/225"/>
    <cc:attributionURL rdf:resource="http://www.historicengland.org.uk"/>
    <skos:prefLabel xml:lang="en">Chance Vought</skos:prefLabel>
    <cc:attributionName xml:lang="en">Historic England</cc:attributionName>
    <cc:license rdf:resource="http://creativecommons.org/licenses/by/3.0"/>
    <dcterms:publisher rdf:resource="http://www.historicengland.org.uk"/>
  </rdf:Description>
  <rdf:Description rdf:about="http://purl.org/heritagedata/schemes/225/concepts/141212">
    <skos:prefLabel xml:lang="en">Beech</skos:prefLabel>
    <cc:attributionName xml:lang="en">Historic England</cc:attributionName>
    <skos:inScheme rdf:resource="http://purl.org/heritagedata/schemes/225"/>
    <dcterms:identifier>http://purl.org/heritagedata/schemes/225/concepts/141212</dcterms:identifier>
    <dcterms:publisher rdf:resource="http://www.historicengland.org.uk"/>
    <cc:attributionURL rdf:resource="http://www.historicengland.org.uk"/>
    <rdf:type rdf:resource="http://www.w3.org/2004/02/skos/core#Concept"/>
    <skos:narrower rdf:resource="http://purl.org/heritagedata/schemes/225/concepts/141213"/>
    <skos:scopeNote xml:lang="en">Beech Aircraft Corporation, also known as Beechcraft, established 1932</skos:scopeNote>
    <cc:license rdf:resource="http://creativecommons.org/licenses/by/3.0"/>
    <skos:broader rdf:resource="http://purl.org/heritagedata/schemes/225/concepts/111358"/>
    <dcterms:issued rdf:datatype="http://www.w3.org/2001/XMLSchema#dateTime">2019-03-26T16:45:43</dcterms:issued>
  </rdf:Description>
  <rdf:Description rdf:about="http://purl.org/heritagedata/schemes/225/concepts/137209">
    <skos:prefLabel xml:lang="en">Seafire</skos:prefLabel>
    <dcterms:issued rdf:datatype="http://www.w3.org/2001/XMLSchema#dateTime">2019-03-26T16:45:43</dcterms:issued>
    <dcterms:publisher rdf:resource="http://www.historicengland.org.uk"/>
    <skos:scopeNote xml:lang="en">Single-engine, single-seat carrierborne fighter: a Spitfire VB fitted with an arrester hook. Modifications on later versions included folding wings, rocket-assisted take-off gear and conversion for photo-reconnaissance duties.</skos:scopeNote>
    <skos:broader rdf:resource="http://purl.org/heritagedata/schemes/225/concepts/111402"/>
    <skos:broader rdf:resource="http://purl.org/heritagedata/schemes/225/concepts/111353"/>
    <cc:license rdf:resource="http://creativecommons.org/licenses/by/3.0"/>
    <rdf:type rdf:resource="http://www.w3.org/2004/02/skos/core#Concept"/>
    <cc:attributionURL rdf:resource="http://www.historicengland.org.uk"/>
    <skos:inScheme rdf:resource="http://purl.org/heritagedata/schemes/225"/>
    <cc:attributionName xml:lang="en">Historic England</cc:attributionName>
    <dcterms:identifier>http://purl.org/heritagedata/schemes/225/concepts/137209</dcterms:identifier>
    <ns1:related rdf:resource="http://purl.org/heritagedata/schemes/225/concepts/111334"/>
    <skos:broader rdf:resource="http://purl.org/heritagedata/schemes/225/concepts/111397"/>
  </rdf:Description>
  <rdf:Description rdf:about="http://purl.org/heritagedata/schemes/225/concepts/136528">
    <skos:altLabel xml:lang="en">F2b</skos:altLabel>
  </rdf:Description>
  <rdf:Description rdf:about="http://purl.org/heritagedata/schemes/225/concepts/134997">
    <skos:broader rdf:resource="http://purl.org/heritagedata/schemes/225/concepts/111396"/>
    <dcterms:identifier>http://purl.org/heritagedata/schemes/225/concepts/134997</dcterms:identifier>
    <skos:narrower rdf:resource="http://purl.org/heritagedata/schemes/225/concepts/140140"/>
    <cc:attributionName xml:lang="en">Historic England</cc:attributionName>
    <skos:inScheme rdf:resource="http://purl.org/heritagedata/schemes/225"/>
    <skos:scopeNote xml:lang="en">A type of seaplane, with one or more slender pontoons (known as "floats") mounted under the fuselage to provide buoyancy.</skos:scopeNote>
    <skos:narrower rdf:resource="http://purl.org/heritagedata/schemes/225/concepts/136231"/>
    <skos:narrower rdf:resource="http://purl.org/heritagedata/schemes/225/concepts/140447"/>
    <cc:attributionURL rdf:resource="http://www.historicengland.org.uk"/>
    <skos:prefLabel xml:lang="en">Floatplane</skos:prefLabel>
    <dcterms:publisher rdf:resource="http://www.historicengland.org.uk"/>
    <rdf:type rdf:resource="http://www.w3.org/2004/02/skos/core#Concept"/>
    <cc:license rdf:resource="http://creativecommons.org/licenses/by/3.0"/>
    <skos:narrower rdf:resource="http://purl.org/heritagedata/schemes/225/concepts/134996"/>
    <dcterms:issued rdf:datatype="http://www.w3.org/2001/XMLSchema#dateTime">2019-03-26T16:45:43</dcterms:issued>
  </rdf:Description>
  <rdf:Description rdf:about="http://purl.org/heritagedata/schemes/225/concepts/138540">
    <cc:license rdf:resource="http://creativecommons.org/licenses/by/3.0"/>
    <rdf:type rdf:resource="http://www.w3.org/2004/02/skos/core#Concept"/>
    <cc:attributionURL rdf:resource="http://www.historicengland.org.uk"/>
    <skos:inScheme rdf:resource="http://purl.org/heritagedata/schemes/225"/>
    <dcterms:issued rdf:datatype="http://www.w3.org/2001/XMLSchema#dateTime">2019-03-26T16:45:43</dcterms:issued>
    <skos:broader rdf:resource="http://purl.org/heritagedata/schemes/225/concepts/111403"/>
    <dcterms:identifier>http://purl.org/heritagedata/schemes/225/concepts/138540</dcterms:identifier>
    <skos:broader rdf:resource="http://purl.org/heritagedata/schemes/225/concepts/111355"/>
    <dcterms:publisher rdf:resource="http://www.historicengland.org.uk"/>
    <cc:attributionName xml:lang="en">Historic England</cc:attributionName>
    <skos:scopeNote xml:lang="en">An important two-seat, tractor biplane, initially used by the RFC in a reconnaissance role and by the RNAS as a bomber. Later converted to a single-seat Home Defence fighter and ultimately used as a trainer.</skos:scopeNote>
    <skos:prefLabel xml:lang="en">Avro 504</skos:prefLabel>
  </rdf:Description>
  <rdf:Description rdf:about="http://purl.org/heritagedata/schemes/225/concepts/137234">
    <skos:scopeNote xml:lang="en">German single-engine, four-seat maritime patrol and reconnaissance flying-boat. In production between 1934 and 1940, the DO18 was replaced by the three engined DO24.</skos:scopeNote>
    <skos:inScheme rdf:resource="http://purl.org/heritagedata/schemes/225"/>
    <rdf:type rdf:resource="http://www.w3.org/2004/02/skos/core#Concept"/>
    <skos:broader rdf:resource="http://purl.org/heritagedata/schemes/225/concepts/111402"/>
    <dcterms:identifier>http://purl.org/heritagedata/schemes/225/concepts/137234</dcterms:identifier>
    <cc:license rdf:resource="http://creativecommons.org/licenses/by/3.0"/>
    <skos:broader rdf:resource="http://purl.org/heritagedata/schemes/225/concepts/111361"/>
    <cc:attributionURL rdf:resource="http://www.historicengland.org.uk"/>
    <skos:broader rdf:resource="http://purl.org/heritagedata/schemes/225/concepts/111395"/>
    <dcterms:issued rdf:datatype="http://www.w3.org/2001/XMLSchema#dateTime">2019-03-26T16:45:43</dcterms:issued>
    <skos:broader rdf:resource="http://purl.org/heritagedata/schemes/225/concepts/135730"/>
    <skos:prefLabel xml:lang="en">Do18</skos:prefLabel>
    <dcterms:publisher rdf:resource="http://www.historicengland.org.uk"/>
    <cc:attributionName xml:lang="en">Historic England</cc:attributionName>
  </rdf:Description>
  <rdf:Description rdf:about="http://purl.org/heritagedata/schemes/225/concepts/139054">
    <skos:altLabel xml:lang="en">Liberator</skos:altLabel>
  </rdf:Description>
  <rdf:Description rdf:about="http://purl.org/heritagedata/schemes/225/concepts/140424">
    <skos:broader rdf:resource="http://purl.org/heritagedata/schemes/225/concepts/111403"/>
    <skos:broader rdf:resource="http://purl.org/heritagedata/schemes/225/concepts/111420"/>
    <rdf:type rdf:resource="http://www.w3.org/2004/02/skos/core#Concept"/>
    <dcterms:identifier>http://purl.org/heritagedata/schemes/225/concepts/140424</dcterms:identifier>
    <dcterms:publisher rdf:resource="http://www.historicengland.org.uk"/>
    <cc:license rdf:resource="http://creativecommons.org/licenses/by/3.0"/>
    <skos:scopeNote xml:lang="en">Twin-engine, three-crew, long-range heavy bomber biplane. Entered service in 1917. Of wooden construction with a fabric covering, the Vimy was fitted with a skid under the nose of its fuselage to prevent tipping forward upon landing.</skos:scopeNote>
    <skos:broader rdf:resource="http://purl.org/heritagedata/schemes/225/concepts/137190"/>
    <cc:attributionName xml:lang="en">Historic England</cc:attributionName>
    <cc:attributionURL rdf:resource="http://www.historicengland.org.uk"/>
    <skos:inScheme rdf:resource="http://purl.org/heritagedata/schemes/225"/>
    <skos:prefLabel xml:lang="en">Vimy</skos:prefLabel>
    <dcterms:issued rdf:datatype="http://www.w3.org/2001/XMLSchema#dateTime">2019-03-26T16:45:43</dcterms:issued>
  </rdf:Description>
  <rdf:Description rdf:about="http://purl.org/heritagedata/schemes/225/concepts/111396">
    <skos:scopeNote xml:lang="en">An aircraft designed to land on water. They can be divided into 2 types: Flying boats (designed with a hull allowing the aircraft to land directly on water) and Floatplanes (where the undercarriage was replaced by fixed floats).</skos:scopeNote>
    <skos:narrower rdf:resource="http://purl.org/heritagedata/schemes/225/concepts/111395"/>
    <cc:attributionName xml:lang="en">Historic England</cc:attributionName>
    <cc:license rdf:resource="http://creativecommons.org/licenses/by/3.0"/>
    <skos:inScheme rdf:resource="http://purl.org/heritagedata/schemes/225"/>
    <cc:attributionURL rdf:resource="http://www.historicengland.org.uk"/>
    <dcterms:issued rdf:datatype="http://www.w3.org/2001/XMLSchema#dateTime">2019-03-26T16:45:43</dcterms:issued>
    <skos:narrower rdf:resource="http://purl.org/heritagedata/schemes/225/concepts/134997"/>
    <dcterms:identifier>http://purl.org/heritagedata/schemes/225/concepts/111396</dcterms:identifier>
    <skos:prefLabel xml:lang="en">Seaplane</skos:prefLabel>
    <dcterms:publisher rdf:resource="http://www.historicengland.org.uk"/>
    <skos:broader rdf:resource="http://purl.org/heritagedata/schemes/225/concepts/111393"/>
    <rdf:type rdf:resource="http://www.w3.org/2004/02/skos/core#Concept"/>
  </rdf:Description>
  <rdf:Description rdf:about="http://purl.org/heritagedata/schemes/225/concepts/135751">
    <skos:broader rdf:resource="http://purl.org/heritagedata/schemes/225/concepts/139053"/>
    <rdf:type rdf:resource="http://www.w3.org/2004/02/skos/core#Concept"/>
    <skos:narrower rdf:resource="http://purl.org/heritagedata/schemes/225/concepts/137226"/>
    <skos:narrower rdf:resource="http://purl.org/heritagedata/schemes/225/concepts/135850"/>
    <skos:narrower rdf:resource="http://purl.org/heritagedata/schemes/225/concepts/136531"/>
    <dcterms:publisher rdf:resource="http://www.historicengland.org.uk"/>
    <dcterms:identifier>http://purl.org/heritagedata/schemes/225/concepts/135751</dcterms:identifier>
    <skos:narrower rdf:resource="http://purl.org/heritagedata/schemes/225/concepts/136530"/>
    <cc:license rdf:resource="http://creativecommons.org/licenses/by/3.0"/>
    <cc:attributionName xml:lang="en">Historic England</cc:attributionName>
    <cc:attributionURL rdf:resource="http://www.historicengland.org.uk"/>
    <skos:inScheme rdf:resource="http://purl.org/heritagedata/schemes/225"/>
    <skos:scopeNote xml:lang="en">An aircraft used for the towing of targets.</skos:scopeNote>
    <skos:narrower rdf:resource="http://purl.org/heritagedata/schemes/225/concepts/137214"/>
    <skos:prefLabel xml:lang="en">Target Tug</skos:prefLabel>
    <dcterms:issued rdf:datatype="http://www.w3.org/2001/XMLSchema#dateTime">2019-03-26T16:45:43</dcterms:issued>
  </rdf:Description>
  <rdf:Description rdf:about="http://purl.org/heritagedata/schemes/225/concepts/111440">
    <skos:altLabel xml:lang="en">Bf110</skos:altLabel>
  </rdf:Description>
  <rdf:Description rdf:about="http://purl.org/heritagedata/schemes/225/concepts/133204">
    <cc:attributionURL rdf:resource="http://www.historicengland.org.uk"/>
    <rdf:type rdf:resource="http://www.w3.org/2004/02/skos/core#Concept"/>
    <skos:scopeNote xml:lang="en">Two-seat, single-engine, advanced-pilot trainer. Square-winged and fitted with dual controls, this popular trainer was used by British Commonwealth, as well as American and Canadian, air forces.</skos:scopeNote>
    <cc:attributionName xml:lang="en">Historic England</cc:attributionName>
    <cc:license rdf:resource="http://creativecommons.org/licenses/by/3.0"/>
    <skos:broader rdf:resource="http://purl.org/heritagedata/schemes/225/concepts/111401"/>
    <skos:broader rdf:resource="http://purl.org/heritagedata/schemes/225/concepts/125513"/>
    <skos:prefLabel xml:lang="en">Harvard</skos:prefLabel>
    <dcterms:publisher rdf:resource="http://www.historicengland.org.uk"/>
    <dcterms:identifier>http://purl.org/heritagedata/schemes/225/concepts/133204</dcterms:identifier>
    <skos:inScheme rdf:resource="http://purl.org/heritagedata/schemes/225"/>
    <dcterms:issued rdf:datatype="http://www.w3.org/2001/XMLSchema#dateTime">2019-03-26T16:45:43</dcterms:issued>
    <skos:broader rdf:resource="http://purl.org/heritagedata/schemes/225/concepts/111402"/>
  </rdf:Description>
  <rdf:Description rdf:about="http://purl.org/heritagedata/schemes/225/concepts/137201">
    <rdf:type rdf:resource="http://www.w3.org/2004/02/skos/core#Concept"/>
    <cc:license rdf:resource="http://creativecommons.org/licenses/by/3.0"/>
    <dcterms:publisher rdf:resource="http://www.historicengland.org.uk"/>
    <dcterms:issued rdf:datatype="http://www.w3.org/2001/XMLSchema#dateTime">2019-03-26T16:45:43</dcterms:issued>
    <skos:scopeNote xml:lang="en">Wood and fabric transport glider, twenty of which were produced with twin Bristol Mercury engines. Fitted with a hinged nose for loading and unloading, this was the largest glider used by the RAF and could accomodate a 7-ton tank.</skos:scopeNote>
    <skos:prefLabel xml:lang="en">Hamilcar</skos:prefLabel>
    <skos:broader rdf:resource="http://purl.org/heritagedata/schemes/225/concepts/111402"/>
    <skos:inScheme rdf:resource="http://purl.org/heritagedata/schemes/225"/>
    <cc:attributionName xml:lang="en">Historic England</cc:attributionName>
    <skos:broader rdf:resource="http://purl.org/heritagedata/schemes/225/concepts/137110"/>
    <skos:broader rdf:resource="http://purl.org/heritagedata/schemes/225/concepts/137200"/>
    <cc:attributionURL rdf:resource="http://www.historicengland.org.uk"/>
    <skos:broader rdf:resource="http://purl.org/heritagedata/schemes/225/concepts/111424"/>
    <dcterms:identifier>http://purl.org/heritagedata/schemes/225/concepts/137201</dcterms:identifier>
  </rdf:Description>
  <rdf:Description rdf:about="http://purl.org/heritagedata/schemes/225/concepts/111395">
    <skos:narrower rdf:resource="http://purl.org/heritagedata/schemes/225/concepts/136591"/>
    <skos:scopeNote xml:lang="en">An aeroplane with the capability to land at sea, the underside of its fuselage shaped like the hull of a sea-going vessel and designed to make contact with the water.</skos:scopeNote>
    <skos:broader rdf:resource="http://purl.org/heritagedata/schemes/225/concepts/111396"/>
    <skos:narrower rdf:resource="http://purl.org/heritagedata/schemes/225/concepts/137235"/>
    <skos:narrower rdf:resource="http://purl.org/heritagedata/schemes/225/concepts/137234"/>
    <skos:narrower rdf:resource="http://purl.org/heritagedata/schemes/225/concepts/135729"/>
    <skos:inScheme rdf:resource="http://purl.org/heritagedata/schemes/225"/>
    <cc:attributionName xml:lang="en">Historic England</cc:attributionName>
    <skos:narrower rdf:resource="http://purl.org/heritagedata/schemes/225/concepts/138546"/>
    <skos:narrower rdf:resource="http://purl.org/heritagedata/schemes/225/concepts/137150"/>
    <cc:license rdf:resource="http://creativecommons.org/licenses/by/3.0"/>
    <dcterms:identifier>http://purl.org/heritagedata/schemes/225/concepts/111395</dcterms:identifier>
    <cc:attributionURL rdf:resource="http://www.historicengland.org.uk"/>
    <dcterms:issued rdf:datatype="http://www.w3.org/2001/XMLSchema#dateTime">2019-03-26T16:45:43</dcterms:issued>
    <rdf:type rdf:resource="http://www.w3.org/2004/02/skos/core#Concept"/>
    <dcterms:publisher rdf:resource="http://www.historicengland.org.uk"/>
    <skos:narrower rdf:resource="http://purl.org/heritagedata/schemes/225/concepts/136250"/>
    <skos:prefLabel xml:lang="en">Flying Boat</skos:prefLabel>
    <skos:narrower rdf:resource="http://purl.org/heritagedata/schemes/225/concepts/137208"/>
    <skos:narrower rdf:resource="http://purl.org/heritagedata/schemes/225/concepts/136610"/>
    <skos:narrower rdf:resource="http://purl.org/heritagedata/schemes/225/concepts/136251"/>
  </rdf:Description>
  <rdf:Description rdf:about="http://purl.org/heritagedata/schemes/225/concepts/137223">
    <skos:broader rdf:resource="http://purl.org/heritagedata/schemes/225/concepts/111358"/>
    <rdf:type rdf:resource="http://www.w3.org/2004/02/skos/core#Concept"/>
    <dcterms:publisher rdf:resource="http://www.historicengland.org.uk"/>
    <skos:narrower rdf:resource="http://purl.org/heritagedata/schemes/225/concepts/137224"/>
    <skos:scopeNote xml:lang="en">The Stinson Division of The Consolidated Vultee Aircraft Corporation. Originally the Stinson Aircraft Division of the Aviation Manufacturing Corpn., who were taken over by Vultee Aircraft Inc., who merged with the Consolidated Aircraft Corpn. in 1943.</skos:scopeNote>
    <dcterms:issued rdf:datatype="http://www.w3.org/2001/XMLSchema#dateTime">2019-03-26T16:45:43</dcterms:issued>
    <skos:prefLabel xml:lang="en">Stinson</skos:prefLabel>
    <cc:attributionName xml:lang="en">Historic England</cc:attributionName>
    <cc:license rdf:resource="http://creativecommons.org/licenses/by/3.0"/>
    <skos:inScheme rdf:resource="http://purl.org/heritagedata/schemes/225"/>
    <cc:attributionURL rdf:resource="http://www.historicengland.org.uk"/>
    <dcterms:identifier>http://purl.org/heritagedata/schemes/225/concepts/137223</dcterms:identifier>
  </rdf:Description>
  <rdf:Description rdf:about="http://purl.org/heritagedata/schemes/225/concepts/137196">
    <dcterms:publisher rdf:resource="http://www.historicengland.org.uk"/>
    <skos:broader rdf:resource="http://purl.org/heritagedata/schemes/225/concepts/136511"/>
    <skos:broader rdf:resource="http://purl.org/heritagedata/schemes/225/concepts/111402"/>
    <rdf:type rdf:resource="http://www.w3.org/2004/02/skos/core#Concept"/>
    <cc:attributionURL rdf:resource="http://www.historicengland.org.uk"/>
    <skos:scopeNote xml:lang="en">Fleet Air Arm fighter and torpedo-bomber, designed for operation from aircraft carriers. All-metal in construction, it entered service in 1944 and was rendered obsolete after the war by the advent of the jet aircraft.</skos:scopeNote>
    <dcterms:issued rdf:datatype="http://www.w3.org/2001/XMLSchema#dateTime">2019-03-26T16:45:43</dcterms:issued>
    <skos:inScheme rdf:resource="http://purl.org/heritagedata/schemes/225"/>
    <skos:broader rdf:resource="http://purl.org/heritagedata/schemes/225/concepts/111374"/>
    <dcterms:identifier>http://purl.org/heritagedata/schemes/225/concepts/137196</dcterms:identifier>
    <skos:broader rdf:resource="http://purl.org/heritagedata/schemes/225/concepts/111397"/>
    <cc:attributionName xml:lang="en">Historic England</cc:attributionName>
    <cc:license rdf:resource="http://creativecommons.org/licenses/by/3.0"/>
    <skos:prefLabel xml:lang="en">Firebrand</skos:prefLabel>
  </rdf:Description>
  <rdf:Description rdf:about="http://purl.org/heritagedata/schemes/225/concepts/141209">
    <cc:license rdf:resource="http://creativecommons.org/licenses/by/3.0"/>
    <cc:attributionURL rdf:resource="http://www.historicengland.org.uk"/>
    <dcterms:publisher rdf:resource="http://www.historicengland.org.uk"/>
    <cc:attributionName xml:lang="en">Historic England</cc:attributionName>
    <dcterms:identifier>http://purl.org/heritagedata/schemes/225/concepts/141209</dcterms:identifier>
    <skos:inScheme rdf:resource="http://purl.org/heritagedata/schemes/225"/>
    <rdf:type rdf:resource="http://www.w3.org/2004/02/skos/core#Concept"/>
    <skos:broader rdf:resource="http://purl.org/heritagedata/schemes/225/concepts/141131"/>
    <skos:scopeNote xml:lang="en">A Mark 2B aircraft with which has undergone further modifications to enhance performance or armament.</skos:scopeNote>
    <dcterms:issued rdf:datatype="http://www.w3.org/2001/XMLSchema#dateTime">2019-03-26T16:45:43</dcterms:issued>
    <skos:prefLabel xml:lang="en">MkIIC</skos:prefLabel>
  </rdf:Description>
  <rdf:Description rdf:about="http://purl.org/heritagedata/schemes/225/concepts/138508">
    <dcterms:issued rdf:datatype="http://www.w3.org/2001/XMLSchema#dateTime">2019-03-26T16:45:43</dcterms:issued>
    <skos:broader rdf:resource="http://purl.org/heritagedata/schemes/225/concepts/111358"/>
    <rdf:type rdf:resource="http://www.w3.org/2004/02/skos/core#Concept"/>
    <skos:inScheme rdf:resource="http://purl.org/heritagedata/schemes/225"/>
    <dcterms:publisher rdf:resource="http://www.historicengland.org.uk"/>
    <dcterms:identifier>http://purl.org/heritagedata/schemes/225/concepts/138508</dcterms:identifier>
    <skos:narrower rdf:resource="http://purl.org/heritagedata/schemes/225/concepts/111420"/>
    <skos:narrower rdf:resource="http://purl.org/heritagedata/schemes/225/concepts/111353"/>
    <cc:license rdf:resource="http://creativecommons.org/licenses/by/3.0"/>
    <skos:scopeNote xml:lang="en">Vickers-Armstrongs Ltd.. In 1938 took over Vickers (Aviation) Ltd., which itself had taken control of Supermarine Aviation Works Ltd. in 1928.</skos:scopeNote>
    <cc:attributionURL rdf:resource="http://www.historicengland.org.uk"/>
    <cc:attributionName xml:lang="en">Historic England</cc:attributionName>
    <skos:prefLabel xml:lang="en">Vickers Armstrongs</skos:prefLabel>
  </rdf:Description>
  <rdf:Description rdf:about="http://purl.org/heritagedata/schemes/225/concepts/136250">
    <skos:broader rdf:resource="http://purl.org/heritagedata/schemes/225/concepts/111353"/>
    <cc:license rdf:resource="http://creativecommons.org/licenses/by/3.0"/>
    <cc:attributionName xml:lang="en">Historic England</cc:attributionName>
    <cc:attributionURL rdf:resource="http://www.historicengland.org.uk"/>
    <skos:inScheme rdf:resource="http://purl.org/heritagedata/schemes/225"/>
    <dcterms:identifier>http://purl.org/heritagedata/schemes/225/concepts/136250</dcterms:identifier>
    <rdf:type rdf:resource="http://www.w3.org/2004/02/skos/core#Concept"/>
    <dcterms:issued rdf:datatype="http://www.w3.org/2001/XMLSchema#dateTime">2019-03-26T16:45:43</dcterms:issued>
    <skos:scopeNote xml:lang="en">Interbellum, twin-engined, five-crew, biplane flying-boat with a characteristic triple tail-fin. Entered service in 1925 and used for general reconnaissance duties. The Mk.I had a wooden fuselage, whilst the Mk.II's was metal in construction.</skos:scopeNote>
    <skos:prefLabel xml:lang="en">Southampton</skos:prefLabel>
    <skos:broader rdf:resource="http://purl.org/heritagedata/schemes/225/concepts/135730"/>
    <skos:broader rdf:resource="http://purl.org/heritagedata/schemes/225/concepts/111395"/>
    <dcterms:publisher rdf:resource="http://www.historicengland.org.uk"/>
    <skos:broader rdf:resource="http://purl.org/heritagedata/schemes/225/concepts/111403"/>
  </rdf:Description>
  <rdf:Description rdf:about="http://purl.org/heritagedata/schemes/225/concepts/137191">
    <skos:inScheme rdf:resource="http://purl.org/heritagedata/schemes/225"/>
    <rdf:type rdf:resource="http://www.w3.org/2004/02/skos/core#Concept"/>
    <skos:prefLabel xml:lang="en">Triplane</skos:prefLabel>
    <skos:scopeNote xml:lang="en">An aeroplane featuring three wings, or planes, placed one above the other either side of its fuselage.</skos:scopeNote>
    <cc:license rdf:resource="http://creativecommons.org/licenses/by/3.0"/>
    <cc:attributionURL rdf:resource="http://www.historicengland.org.uk"/>
    <dcterms:issued rdf:datatype="http://www.w3.org/2001/XMLSchema#dateTime">2019-03-26T16:45:43</dcterms:issued>
    <skos:broader rdf:resource="http://purl.org/heritagedata/schemes/225/concepts/111393"/>
    <dcterms:identifier>http://purl.org/heritagedata/schemes/225/concepts/137191</dcterms:identifier>
    <dcterms:publisher rdf:resource="http://www.historicengland.org.uk"/>
    <cc:attributionName xml:lang="en">Historic England</cc:attributionName>
  </rdf:Description>
  <rdf:Description rdf:about="http://purl.org/heritagedata/schemes/225/concepts/111375">
    <skos:broader rdf:resource="http://purl.org/heritagedata/schemes/225/concepts/136511"/>
    <cc:attributionName xml:lang="en">Historic England</cc:attributionName>
    <skos:inScheme rdf:resource="http://purl.org/heritagedata/schemes/225"/>
    <skos:prefLabel xml:lang="en">Botha</skos:prefLabel>
    <skos:broader rdf:resource="http://purl.org/heritagedata/schemes/225/concepts/111402"/>
    <skos:scopeNote xml:lang="en">Four-crew, twin-engined monoplane designed as a torpedo-bomber and reconnaissance aircraft for RAF Coastal Command. Withdrawn from operations in November 1940 and downgraded to a trainer.</skos:scopeNote>
    <dcterms:publisher rdf:resource="http://www.historicengland.org.uk"/>
    <skos:broader rdf:resource="http://purl.org/heritagedata/schemes/225/concepts/111401"/>
    <skos:broader rdf:resource="http://purl.org/heritagedata/schemes/225/concepts/111374"/>
    <rdf:type rdf:resource="http://www.w3.org/2004/02/skos/core#Concept"/>
    <dcterms:identifier>http://purl.org/heritagedata/schemes/225/concepts/111375</dcterms:identifier>
    <skos:broader rdf:resource="http://purl.org/heritagedata/schemes/225/concepts/135730"/>
    <cc:license rdf:resource="http://creativecommons.org/licenses/by/3.0"/>
    <cc:attributionURL rdf:resource="http://www.historicengland.org.uk"/>
    <dcterms:issued rdf:datatype="http://www.w3.org/2001/XMLSchema#dateTime">2019-03-26T16:45:43</dcterms:issued>
  </rdf:Description>
  <rdf:Description rdf:about="http://purl.org/heritagedata/schemes/225/concepts/137222">
    <skos:altLabel xml:lang="en">Martlet</skos:altLabel>
  </rdf:Description>
  <rdf:Description rdf:about="http://purl.org/heritagedata/schemes/225/concepts/135930">
    <cc:license rdf:resource="http://creativecommons.org/licenses/by/3.0"/>
    <skos:narrower rdf:resource="http://purl.org/heritagedata/schemes/225/concepts/135931"/>
    <skos:scopeNote xml:lang="en">Westland Aircraft Ltd., formed in 1935 to take over the aircraft branch of Petters Ltd., previously known as the Westland Aircraft Works.</skos:scopeNote>
    <cc:attributionName xml:lang="en">Historic England</cc:attributionName>
    <skos:inScheme rdf:resource="http://purl.org/heritagedata/schemes/225"/>
    <dcterms:publisher rdf:resource="http://www.historicengland.org.uk"/>
    <cc:attributionURL rdf:resource="http://www.historicengland.org.uk"/>
    <skos:narrower rdf:resource="http://purl.org/heritagedata/schemes/225/concepts/135932"/>
    <skos:narrower rdf:resource="http://purl.org/heritagedata/schemes/225/concepts/136610"/>
    <rdf:type rdf:resource="http://www.w3.org/2004/02/skos/core#Concept"/>
    <dcterms:issued rdf:datatype="http://www.w3.org/2001/XMLSchema#dateTime">2019-03-26T16:45:43</dcterms:issued>
    <dcterms:identifier>http://purl.org/heritagedata/schemes/225/concepts/135930</dcterms:identifier>
    <skos:broader rdf:resource="http://purl.org/heritagedata/schemes/225/concepts/111358"/>
    <skos:prefLabel xml:lang="en">Westland</skos:prefLabel>
  </rdf:Description>
  <rdf:Description rdf:about="http://purl.org/heritagedata/schemes/225/concepts/136532">
    <skos:scopeNote xml:lang="en">Twin-engined, four-seat torpedo-bomber designed to replace the Vildebeest. Entered service with RAF Coastal Command in 1939. Later versions incorporated a remote-controlled machine gun with periscope sight.</skos:scopeNote>
    <cc:license rdf:resource="http://creativecommons.org/licenses/by/3.0"/>
    <cc:attributionName xml:lang="en">Historic England</cc:attributionName>
    <cc:attributionURL rdf:resource="http://www.historicengland.org.uk"/>
    <skos:inScheme rdf:resource="http://purl.org/heritagedata/schemes/225"/>
    <skos:broader rdf:resource="http://purl.org/heritagedata/schemes/225/concepts/111357"/>
    <dcterms:identifier>http://purl.org/heritagedata/schemes/225/concepts/136532</dcterms:identifier>
    <skos:broader rdf:resource="http://purl.org/heritagedata/schemes/225/concepts/111402"/>
    <skos:prefLabel xml:lang="en">Beaufort</skos:prefLabel>
    <rdf:type rdf:resource="http://www.w3.org/2004/02/skos/core#Concept"/>
    <dcterms:issued rdf:datatype="http://www.w3.org/2001/XMLSchema#dateTime">2019-03-26T16:45:43</dcterms:issued>
    <dcterms:publisher rdf:resource="http://www.historicengland.org.uk"/>
    <skos:broader rdf:resource="http://purl.org/heritagedata/schemes/225/concepts/136511"/>
  </rdf:Description>
  <rdf:Description rdf:about="http://purl.org/heritagedata/schemes/225/concepts/167010">
    <cc:attributionName xml:lang="en">Historic England</cc:attributionName>
    <skos:inScheme rdf:resource="http://purl.org/heritagedata/schemes/225"/>
    <skos:broader rdf:resource="http://purl.org/heritagedata/schemes/225/concepts/111358"/>
    <rdf:type rdf:resource="http://www.w3.org/2004/02/skos/core#Concept"/>
    <skos:prefLabel xml:lang="en">Farman</skos:prefLabel>
    <dcterms:issued rdf:datatype="http://www.w3.org/2001/XMLSchema#dateTime">2019-03-26T16:45:43</dcterms:issued>
    <skos:scopeNote xml:lang="en">Farman Aviation Works was an aircraft company founded and run by the brothers Richard, Henri, and Maurice Farman in 1908. The firm made pusher biplane aircraft for military and training purposes, it was eventually dissolved in 1956.</skos:scopeNote>
    <cc:attributionURL rdf:resource="http://www.historicengland.org.uk"/>
    <cc:license rdf:resource="http://creativecommons.org/licenses/by/3.0"/>
    <dcterms:publisher rdf:resource="http://www.historicengland.org.uk"/>
    <skos:narrower rdf:resource="http://purl.org/heritagedata/schemes/225/concepts/167011"/>
    <dcterms:identifier>http://purl.org/heritagedata/schemes/225/concepts/167010</dcterms:identifier>
  </rdf:Description>
  <rdf:Description rdf:about="http://purl.org/heritagedata/schemes/225/concepts/141296">
    <cc:attributionName xml:lang="en">Historic England</cc:attributionName>
    <skos:broader rdf:resource="http://purl.org/heritagedata/schemes/225/concepts/111402"/>
    <rdf:type rdf:resource="http://www.w3.org/2004/02/skos/core#Concept"/>
    <skos:broader rdf:resource="http://purl.org/heritagedata/schemes/225/concepts/137190"/>
    <dcterms:issued rdf:datatype="http://www.w3.org/2001/XMLSchema#dateTime">2019-03-26T16:45:43</dcterms:issued>
    <skos:prefLabel xml:lang="en">Pb4Y Liberator</skos:prefLabel>
    <dcterms:identifier>http://purl.org/heritagedata/schemes/225/concepts/141296</dcterms:identifier>
    <cc:attributionURL rdf:resource="http://www.historicengland.org.uk"/>
    <ns1:related rdf:resource="http://purl.org/heritagedata/schemes/225/concepts/125533"/>
    <cc:license rdf:resource="http://creativecommons.org/licenses/by/3.0"/>
    <skos:broader rdf:resource="http://purl.org/heritagedata/schemes/225/concepts/135730"/>
    <skos:scopeNote xml:lang="en">US Navy version of the four-engined, six-crew B24 heavy bomber. Modified for long-range reconnaissance duty and used as a patrol-bomber against shipping and submarines.</skos:scopeNote>
    <dcterms:publisher rdf:resource="http://www.historicengland.org.uk"/>
    <skos:inScheme rdf:resource="http://purl.org/heritagedata/schemes/225"/>
    <skos:broader rdf:resource="http://purl.org/heritagedata/schemes/225/concepts/111417"/>
  </rdf:Description>
  <rdf:Description rdf:about="http://purl.org/heritagedata/schemes/225/concepts/141253">
    <skos:broader rdf:resource="http://purl.org/heritagedata/schemes/225/concepts/141131"/>
    <dcterms:publisher rdf:resource="http://www.historicengland.org.uk"/>
    <rdf:type rdf:resource="http://www.w3.org/2004/02/skos/core#Concept"/>
    <skos:prefLabel xml:lang="en">MkIF</skos:prefLabel>
    <cc:attributionName xml:lang="en">Historic England</cc:attributionName>
    <cc:license rdf:resource="http://creativecommons.org/licenses/by/3.0"/>
    <skos:inScheme rdf:resource="http://purl.org/heritagedata/schemes/225"/>
    <cc:attributionURL rdf:resource="http://www.historicengland.org.uk"/>
    <dcterms:issued rdf:datatype="http://www.w3.org/2001/XMLSchema#dateTime">2019-03-26T16:45:43</dcterms:issued>
    <skos:scopeNote xml:lang="en">A Mark 1E aircraft which has undergone further modifications to enhance performance or armament.</skos:scopeNote>
    <dcterms:identifier>http://purl.org/heritagedata/schemes/225/concepts/141253</dcterms:identifier>
  </rdf:Description>
  <rdf:Description rdf:about="http://purl.org/heritagedata/schemes/225/concepts/136525">
    <cc:attributionURL rdf:resource="http://www.historicengland.org.uk"/>
    <rdf:type rdf:resource="http://www.w3.org/2004/02/skos/core#Concept"/>
    <dcterms:issued rdf:datatype="http://www.w3.org/2001/XMLSchema#dateTime">2019-03-26T16:45:43</dcterms:issued>
    <cc:attributionName xml:lang="en">Historic England</cc:attributionName>
    <cc:license rdf:resource="http://creativecommons.org/licenses/by/3.0"/>
    <dcterms:identifier>http://purl.org/heritagedata/schemes/225/concepts/136525</dcterms:identifier>
    <skos:scopeNote xml:lang="en">A biplane, reconnaissance aircraft with a crew of 3 or 4 which equipped 3 and 22 squadrons RAF before passing to the Fleet Air Arm. Produced in two variants.</skos:scopeNote>
    <skos:broader rdf:resource="http://purl.org/heritagedata/schemes/225/concepts/135730"/>
    <dcterms:publisher rdf:resource="http://www.historicengland.org.uk"/>
    <skos:broader rdf:resource="http://purl.org/heritagedata/schemes/225/concepts/111355"/>
    <skos:inScheme rdf:resource="http://purl.org/heritagedata/schemes/225"/>
    <skos:prefLabel xml:lang="en">Bison</skos:prefLabel>
    <skos:broader rdf:resource="http://purl.org/heritagedata/schemes/225/concepts/111403"/>
  </rdf:Description>
  <rdf:Description rdf:about="http://purl.org/heritagedata/schemes/225/concepts/111425">
    <skos:altLabel xml:lang="en">Stuka</skos:altLabel>
  </rdf:Description>
  <rdf:Description rdf:about="http://purl.org/heritagedata/schemes/225/concepts/152400">
    <cc:attributionURL rdf:resource="http://www.historicengland.org.uk"/>
    <skos:broader rdf:resource="http://purl.org/heritagedata/schemes/225/concepts/111358"/>
    <rdf:type rdf:resource="http://www.w3.org/2004/02/skos/core#Concept"/>
    <dcterms:publisher rdf:resource="http://www.historicengland.org.uk"/>
    <skos:scopeNote xml:lang="en">McDonnell Douglas was a major American aerospace manufacturer and defense contractor, producing a number of famous commercial and military aircraft.</skos:scopeNote>
    <cc:attributionName xml:lang="en">Historic England</cc:attributionName>
    <dcterms:issued rdf:datatype="http://www.w3.org/2001/XMLSchema#dateTime">2019-03-26T16:45:43</dcterms:issued>
    <skos:inScheme rdf:resource="http://purl.org/heritagedata/schemes/225"/>
    <skos:prefLabel xml:lang="en">Mcdonnell Douglas</skos:prefLabel>
    <skos:narrower rdf:resource="http://purl.org/heritagedata/schemes/225/concepts/152401"/>
    <dcterms:identifier>http://purl.org/heritagedata/schemes/225/concepts/152400</dcterms:identifier>
    <cc:license rdf:resource="http://creativecommons.org/licenses/by/3.0"/>
  </rdf:Description>
  <rdf:Description rdf:about="http://purl.org/heritagedata/schemes/225/concepts/137207">
    <skos:scopeNote xml:lang="en">A British aero- and marine-engineering company based on the Isle of Wight specializing in the construction of flying boats.</skos:scopeNote>
    <skos:narrower rdf:resource="http://purl.org/heritagedata/schemes/225/concepts/136591"/>
    <cc:attributionName xml:lang="en">Historic England</cc:attributionName>
    <skos:inScheme rdf:resource="http://purl.org/heritagedata/schemes/225"/>
    <skos:prefLabel xml:lang="en">Saunders Roe</skos:prefLabel>
    <dcterms:publisher rdf:resource="http://www.historicengland.org.uk"/>
    <dcterms:identifier>http://purl.org/heritagedata/schemes/225/concepts/137207</dcterms:identifier>
    <rdf:type rdf:resource="http://www.w3.org/2004/02/skos/core#Concept"/>
    <cc:attributionURL rdf:resource="http://www.historicengland.org.uk"/>
    <cc:license rdf:resource="http://creativecommons.org/licenses/by/3.0"/>
    <skos:broader rdf:resource="http://purl.org/heritagedata/schemes/225/concepts/111358"/>
    <dcterms:issued rdf:datatype="http://www.w3.org/2001/XMLSchema#dateTime">2019-03-26T16:45:43</dcterms:issued>
  </rdf:Description>
  <rdf:Description rdf:about="http://purl.org/heritagedata/schemes/225/concepts/137205">
    <cc:license rdf:resource="http://creativecommons.org/licenses/by/3.0"/>
    <dcterms:identifier>http://purl.org/heritagedata/schemes/225/concepts/137205</dcterms:identifier>
    <skos:prefLabel xml:lang="en">Percival</skos:prefLabel>
    <dcterms:publisher rdf:resource="http://www.historicengland.org.uk"/>
    <skos:inScheme rdf:resource="http://purl.org/heritagedata/schemes/225"/>
    <cc:attributionName xml:lang="en">Historic England</cc:attributionName>
    <skos:scopeNote xml:lang="en">The Percival Aircraft Company was formed in 1932 and re-organized as Percival Aircraft Ltd. in 1937, when the works moved from Gravesend to Luton.</skos:scopeNote>
    <skos:broader rdf:resource="http://purl.org/heritagedata/schemes/225/concepts/111358"/>
    <rdf:type rdf:resource="http://www.w3.org/2004/02/skos/core#Concept"/>
    <dcterms:issued rdf:datatype="http://www.w3.org/2001/XMLSchema#dateTime">2019-03-26T16:45:43</dcterms:issued>
    <skos:narrower rdf:resource="http://purl.org/heritagedata/schemes/225/concepts/137206"/>
    <cc:attributionURL rdf:resource="http://www.historicengland.org.uk"/>
  </rdf:Description>
  <rdf:Description rdf:about="http://purl.org/heritagedata/schemes/225/concepts/137233">
    <skos:altLabel xml:lang="en">Do215</skos:altLabel>
  </rdf:Description>
  <rdf:Description rdf:about="http://purl.org/heritagedata/schemes/225/concepts/137204">
    <skos:scopeNote xml:lang="en">Single-engine, single-seat fighter-bomber developed from the Typhoon and the abandoned Tornado. Entered service in 1944 with its greatest success being in destroying V.1. flying bombs. One of the fastest World War 2 aircraft, with a top speed of 436 mph.</skos:scopeNote>
    <skos:broader rdf:resource="http://purl.org/heritagedata/schemes/225/concepts/111402"/>
    <rdf:type rdf:resource="http://www.w3.org/2004/02/skos/core#Concept"/>
    <skos:broader rdf:resource="http://purl.org/heritagedata/schemes/225/concepts/111399"/>
    <dcterms:issued rdf:datatype="http://www.w3.org/2001/XMLSchema#dateTime">2019-03-26T16:45:43</dcterms:issued>
    <dcterms:publisher rdf:resource="http://www.historicengland.org.uk"/>
    <ns1:related rdf:resource="http://purl.org/heritagedata/schemes/225/concepts/134998"/>
    <dcterms:identifier>http://purl.org/heritagedata/schemes/225/concepts/137204</dcterms:identifier>
    <cc:attributionName xml:lang="en">Historic England</cc:attributionName>
    <skos:prefLabel xml:lang="en">Tempest</skos:prefLabel>
    <skos:inScheme rdf:resource="http://purl.org/heritagedata/schemes/225"/>
    <skos:broader rdf:resource="http://purl.org/heritagedata/schemes/225/concepts/111359"/>
    <cc:license rdf:resource="http://creativecommons.org/licenses/by/3.0"/>
    <cc:attributionURL rdf:resource="http://www.historicengland.org.uk"/>
  </rdf:Description>
  <rdf:Description rdf:about="http://purl.org/heritagedata/schemes/225/concepts/167011">
    <skos:broader rdf:resource="http://purl.org/heritagedata/schemes/225/concepts/111424"/>
    <skos:scopeNote xml:lang="en">A civil passenger transport biplane produced by the Farman Aviation Works from 1919. Instrumental in the creation of early airlines and commercial routes in Europe after World War I. Initially designed in 1918 as a heavy bomber. Some 60 units built.</skos:scopeNote>
    <dcterms:publisher rdf:resource="http://www.historicengland.org.uk"/>
    <cc:license rdf:resource="http://creativecommons.org/licenses/by/3.0"/>
    <cc:attributionName xml:lang="en">Historic England</cc:attributionName>
    <cc:attributionURL rdf:resource="http://www.historicengland.org.uk"/>
    <skos:inScheme rdf:resource="http://purl.org/heritagedata/schemes/225"/>
    <dcterms:identifier>http://purl.org/heritagedata/schemes/225/concepts/167011</dcterms:identifier>
    <skos:broader rdf:resource="http://purl.org/heritagedata/schemes/225/concepts/111403"/>
    <rdf:type rdf:resource="http://www.w3.org/2004/02/skos/core#Concept"/>
    <dcterms:issued rdf:datatype="http://www.w3.org/2001/XMLSchema#dateTime">2019-03-26T16:45:43</dcterms:issued>
    <skos:prefLabel xml:lang="en">F60 Goliath</skos:prefLabel>
    <skos:broader rdf:resource="http://purl.org/heritagedata/schemes/225/concepts/167010"/>
  </rdf:Description>
  <rdf:Description rdf:about="http://purl.org/heritagedata/schemes/225/concepts/141211">
    <dcterms:publisher rdf:resource="http://www.historicengland.org.uk"/>
    <skos:broader rdf:resource="http://purl.org/heritagedata/schemes/225/concepts/111401"/>
    <skos:scopeNote xml:lang="en">A twin engined advanced trainer aircraft developed for the military by the US firm of Cessna</skos:scopeNote>
    <rdf:type rdf:resource="http://www.w3.org/2004/02/skos/core#Concept"/>
    <skos:broader rdf:resource="http://purl.org/heritagedata/schemes/225/concepts/141210"/>
    <cc:license rdf:resource="http://creativecommons.org/licenses/by/3.0"/>
    <cc:attributionURL rdf:resource="http://www.historicengland.org.uk"/>
    <dcterms:issued rdf:datatype="http://www.w3.org/2001/XMLSchema#dateTime">2019-03-26T16:45:43</dcterms:issued>
    <skos:prefLabel xml:lang="en">AT8</skos:prefLabel>
    <skos:inScheme rdf:resource="http://purl.org/heritagedata/schemes/225"/>
    <dcterms:identifier>http://purl.org/heritagedata/schemes/225/concepts/141211</dcterms:identifier>
    <cc:attributionName xml:lang="en">Historic England</cc:attributionName>
    <skos:broader rdf:resource="http://purl.org/heritagedata/schemes/225/concepts/111402"/>
  </rdf:Description>
  <rdf:Description rdf:about="http://purl.org/heritagedata/schemes/225/concepts/141213">
    <skos:broader rdf:resource="http://purl.org/heritagedata/schemes/225/concepts/141212"/>
    <cc:attributionName xml:lang="en">Historic England</cc:attributionName>
    <cc:license rdf:resource="http://creativecommons.org/licenses/by/3.0"/>
    <skos:inScheme rdf:resource="http://purl.org/heritagedata/schemes/225"/>
    <cc:attributionURL rdf:resource="http://www.historicengland.org.uk"/>
    <dcterms:issued rdf:datatype="http://www.w3.org/2001/XMLSchema#dateTime">2019-03-26T16:45:43</dcterms:issued>
    <skos:scopeNote xml:lang="en">A twin engine advanced trainer developed by Beech/ Beechcraft , a US firm, used in WWII</skos:scopeNote>
    <skos:broader rdf:resource="http://purl.org/heritagedata/schemes/225/concepts/111401"/>
    <dcterms:identifier>http://purl.org/heritagedata/schemes/225/concepts/141213</dcterms:identifier>
    <skos:prefLabel xml:lang="en">AT7</skos:prefLabel>
    <skos:broader rdf:resource="http://purl.org/heritagedata/schemes/225/concepts/111402"/>
    <dcterms:publisher rdf:resource="http://www.historicengland.org.uk"/>
    <rdf:type rdf:resource="http://www.w3.org/2004/02/skos/core#Concept"/>
  </rdf:Description>
  <rdf:Description rdf:about="http://purl.org/heritagedata/schemes/225/concepts/133193">
    <skos:broader rdf:resource="http://purl.org/heritagedata/schemes/225/concepts/111401"/>
    <skos:broader rdf:resource="http://purl.org/heritagedata/schemes/225/concepts/111355"/>
    <skos:prefLabel xml:lang="en">Anson</skos:prefLabel>
    <dcterms:issued rdf:datatype="http://www.w3.org/2001/XMLSchema#dateTime">2019-03-26T16:45:43</dcterms:issued>
    <skos:scopeNote xml:lang="en">Twin-engined monoplane originally designed as a reconnaissance aircraft, but also widely used as a trainer. Entered RAF service in 1936.</skos:scopeNote>
    <skos:broader rdf:resource="http://purl.org/heritagedata/schemes/225/concepts/111402"/>
    <cc:attributionURL rdf:resource="http://www.historicengland.org.uk"/>
    <rdf:type rdf:resource="http://www.w3.org/2004/02/skos/core#Concept"/>
    <cc:license rdf:resource="http://creativecommons.org/licenses/by/3.0"/>
    <dcterms:identifier>http://purl.org/heritagedata/schemes/225/concepts/133193</dcterms:identifier>
    <skos:inScheme rdf:resource="http://purl.org/heritagedata/schemes/225"/>
    <skos:broader rdf:resource="http://purl.org/heritagedata/schemes/225/concepts/135730"/>
    <dcterms:publisher rdf:resource="http://www.historicengland.org.uk"/>
    <cc:attributionName xml:lang="en">Historic England</cc:attributionName>
  </rdf:Description>
  <rdf:Description rdf:about="http://purl.org/heritagedata/schemes/225/concepts/167007">
    <dcterms:publisher rdf:resource="http://www.historicengland.org.uk"/>
    <rdf:type rdf:resource="http://www.w3.org/2004/02/skos/core#Concept"/>
    <skos:prefLabel xml:lang="en">Nieuport</skos:prefLabel>
    <cc:license rdf:resource="http://creativecommons.org/licenses/by/3.0"/>
    <cc:attributionURL rdf:resource="http://www.historicengland.org.uk"/>
    <dcterms:issued rdf:datatype="http://www.w3.org/2001/XMLSchema#dateTime">2019-03-26T16:45:43</dcterms:issued>
    <dcterms:identifier>http://purl.org/heritagedata/schemes/225/concepts/167007</dcterms:identifier>
    <skos:narrower rdf:resource="http://purl.org/heritagedata/schemes/225/concepts/167008"/>
    <skos:broader rdf:resource="http://purl.org/heritagedata/schemes/225/concepts/111358"/>
    <cc:attributionName xml:lang="en">Historic England</cc:attributionName>
    <skos:scopeNote xml:lang="en">A French aeroplane company that primarily built racing aircraft before World War I and fighter aircraft during World War I and between the wars. First set up in 1902 as manufacturer of engine components, then aircraft in 1911 as Nieuport et Deplante.</skos:scopeNote>
    <skos:inScheme rdf:resource="http://purl.org/heritagedata/schemes/225"/>
  </rdf:Description>
  <rdf:Description rdf:about="http://purl.org/heritagedata/schemes/225/concepts/136513">
    <skos:altLabel xml:lang="en">Dh1</skos:altLabel>
  </rdf:Description>
  <rdf:Description rdf:about="http://purl.org/heritagedata/schemes/225/concepts/136517">
    <skos:altLabel xml:lang="en">Dh6</skos:altLabel>
  </rdf:Description>
  <rdf:Description rdf:about="http://purl.org/heritagedata/schemes/225/concepts/136590">
    <skos:altLabel xml:lang="en">Saro</skos:altLabel>
  </rdf:Description>
  <rdf:Description rdf:about="http://purl.org/heritagedata/schemes/225/concepts/141258">
    <cc:attributionURL rdf:resource="http://www.historicengland.org.uk"/>
    <rdf:type rdf:resource="http://www.w3.org/2004/02/skos/core#Concept"/>
    <dcterms:identifier>http://purl.org/heritagedata/schemes/225/concepts/141258</dcterms:identifier>
    <cc:attributionName xml:lang="en">Historic England</cc:attributionName>
    <cc:license rdf:resource="http://creativecommons.org/licenses/by/3.0"/>
    <skos:broader rdf:resource="http://purl.org/heritagedata/schemes/225/concepts/141131"/>
    <skos:prefLabel xml:lang="en">MkIV</skos:prefLabel>
    <dcterms:publisher rdf:resource="http://www.historicengland.org.uk"/>
    <skos:scopeNote xml:lang="en">Mark 4 or the fourth variant of an aircraft with its associated modifications.</skos:scopeNote>
    <dcterms:issued rdf:datatype="http://www.w3.org/2001/XMLSchema#dateTime">2019-03-26T16:45:43</dcterms:issued>
    <skos:inScheme rdf:resource="http://purl.org/heritagedata/schemes/225"/>
  </rdf:Description>
  <rdf:Description rdf:about="http://purl.org/heritagedata/schemes/225/concepts/125517">
    <skos:broader rdf:resource="http://purl.org/heritagedata/schemes/225/concepts/111402"/>
    <skos:broader rdf:resource="http://purl.org/heritagedata/schemes/225/concepts/111399"/>
    <dcterms:publisher rdf:resource="http://www.historicengland.org.uk"/>
    <skos:scopeNote xml:lang="en">Twin-engined, single-seat fighter-bomber. Flown by USAAF fighter groups from 1942, excelled as a ground-support fighter. Could carry two 1600 lb bombs or rocket projectiles.</skos:scopeNote>
    <rdf:type rdf:resource="http://www.w3.org/2004/02/skos/core#Concept"/>
    <cc:attributionName xml:lang="en">Historic England</cc:attributionName>
    <cc:license rdf:resource="http://creativecommons.org/licenses/by/3.0"/>
    <skos:inScheme rdf:resource="http://purl.org/heritagedata/schemes/225"/>
    <cc:attributionURL rdf:resource="http://www.historicengland.org.uk"/>
    <dcterms:issued rdf:datatype="http://www.w3.org/2001/XMLSchema#dateTime">2019-03-26T16:45:43</dcterms:issued>
    <skos:prefLabel xml:lang="en">P38 Lightning</skos:prefLabel>
    <skos:broader rdf:resource="http://purl.org/heritagedata/schemes/225/concepts/125516"/>
    <dcterms:identifier>http://purl.org/heritagedata/schemes/225/concepts/125517</dcterms:identifier>
  </rdf:Description>
  <rdf:Description rdf:about="http://purl.org/heritagedata/schemes/225/concepts/141268">
    <dcterms:identifier>http://purl.org/heritagedata/schemes/225/concepts/141268</dcterms:identifier>
    <ns1:related rdf:resource="http://purl.org/heritagedata/schemes/225/concepts/125554"/>
    <skos:inScheme rdf:resource="http://purl.org/heritagedata/schemes/225"/>
    <rdf:type rdf:resource="http://www.w3.org/2004/02/skos/core#Concept"/>
    <skos:prefLabel xml:lang="en">F13 Superfortress</skos:prefLabel>
    <skos:broader rdf:resource="http://purl.org/heritagedata/schemes/225/concepts/111433"/>
    <cc:license rdf:resource="http://creativecommons.org/licenses/by/3.0"/>
    <dcterms:publisher rdf:resource="http://www.historicengland.org.uk"/>
    <cc:attributionURL rdf:resource="http://www.historicengland.org.uk"/>
    <dcterms:issued rdf:datatype="http://www.w3.org/2001/XMLSchema#dateTime">2019-03-26T16:45:43</dcterms:issued>
    <skos:broader rdf:resource="http://purl.org/heritagedata/schemes/225/concepts/111400"/>
    <skos:scopeNote xml:lang="en">A photo- reconnaissance variant of the Boeing Superfortress, used from 1944, initally deployed in the Pacific war, later for Cold war duties over Europe.</skos:scopeNote>
    <cc:attributionName xml:lang="en">Historic England</cc:attributionName>
    <skos:broader rdf:resource="http://purl.org/heritagedata/schemes/225/concepts/111402"/>
  </rdf:Description>
  <rdf:Description rdf:about="http://purl.org/heritagedata/schemes/225/concepts/137228">
    <dcterms:identifier>http://purl.org/heritagedata/schemes/225/concepts/137228</dcterms:identifier>
    <dcterms:issued rdf:datatype="http://www.w3.org/2001/XMLSchema#dateTime">2019-03-26T16:45:43</dcterms:issued>
    <dcterms:publisher rdf:resource="http://www.historicengland.org.uk"/>
    <rdf:type rdf:resource="http://www.w3.org/2004/02/skos/core#Concept"/>
    <skos:prefLabel xml:lang="en">CG4A Hadrian</skos:prefLabel>
    <skos:broader rdf:resource="http://purl.org/heritagedata/schemes/225/concepts/137227"/>
    <cc:license rdf:resource="http://creativecommons.org/licenses/by/3.0"/>
    <skos:broader rdf:resource="http://purl.org/heritagedata/schemes/225/concepts/111402"/>
    <cc:attributionName xml:lang="en">Historic England</cc:attributionName>
    <skos:broader rdf:resource="http://purl.org/heritagedata/schemes/225/concepts/137110"/>
    <skos:inScheme rdf:resource="http://purl.org/heritagedata/schemes/225"/>
    <cc:attributionURL rdf:resource="http://www.historicengland.org.uk"/>
    <skos:scopeNote xml:lang="en">American troop and supply-glider constructed from steel tube and fabric-covered wood, with a hinged nose to allow loading and unloading of troops or light vehicles. Also known as the Haig, this was the only US glider to see combat service.</skos:scopeNote>
    <skos:broader rdf:resource="http://purl.org/heritagedata/schemes/225/concepts/111424"/>
  </rdf:Description>
  <rdf:Description rdf:about="http://purl.org/heritagedata/schemes/225/concepts/133195">
    <skos:prefLabel xml:lang="en">Bulldog</skos:prefLabel>
    <skos:broader rdf:resource="http://purl.org/heritagedata/schemes/225/concepts/111403"/>
    <rdf:type rdf:resource="http://www.w3.org/2004/02/skos/core#Concept"/>
    <skos:broader rdf:resource="http://purl.org/heritagedata/schemes/225/concepts/111357"/>
    <dcterms:publisher rdf:resource="http://www.historicengland.org.uk"/>
    <cc:license rdf:resource="http://creativecommons.org/licenses/by/3.0"/>
    <cc:attributionName xml:lang="en">Historic England</cc:attributionName>
    <cc:attributionURL rdf:resource="http://www.historicengland.org.uk"/>
    <skos:inScheme rdf:resource="http://purl.org/heritagedata/schemes/225"/>
    <skos:scopeNote xml:lang="en">A single-seat, biplane fighter. One of the last open cockpit types to see widespread service with the RAF, equipping 10 squadrons and, at one point, 70% of the Home Defence fighter force.</skos:scopeNote>
    <skos:broader rdf:resource="http://purl.org/heritagedata/schemes/225/concepts/111397"/>
    <dcterms:identifier>http://purl.org/heritagedata/schemes/225/concepts/133195</dcterms:identifier>
    <dcterms:issued rdf:datatype="http://www.w3.org/2001/XMLSchema#dateTime">2019-03-26T16:45:43</dcterms:issued>
  </rdf:Description>
  <rdf:Description rdf:about="http://purl.org/heritagedata/schemes/225/concepts/141214">
    <skos:inScheme rdf:resource="http://purl.org/heritagedata/schemes/225"/>
    <cc:license rdf:resource="http://creativecommons.org/licenses/by/3.0"/>
    <cc:attributionURL rdf:resource="http://www.historicengland.org.uk"/>
    <skos:scopeNote xml:lang="en">A Mark 5A aircraft which has undergone further modifications to enhance performance or armament.</skos:scopeNote>
    <rdf:type rdf:resource="http://www.w3.org/2004/02/skos/core#Concept"/>
    <skos:broader rdf:resource="http://purl.org/heritagedata/schemes/225/concepts/141131"/>
    <dcterms:issued rdf:datatype="http://www.w3.org/2001/XMLSchema#dateTime">2019-03-26T16:45:43</dcterms:issued>
    <dcterms:publisher rdf:resource="http://www.historicengland.org.uk"/>
    <skos:prefLabel xml:lang="en">MkVB</skos:prefLabel>
    <cc:attributionName xml:lang="en">Historic England</cc:attributionName>
    <dcterms:identifier>http://purl.org/heritagedata/schemes/225/concepts/141214</dcterms:identifier>
  </rdf:Description>
  <rdf:Description rdf:about="http://purl.org/heritagedata/schemes/225/concepts/140416">
    <dcterms:identifier>http://purl.org/heritagedata/schemes/225/concepts/140416</dcterms:identifier>
    <dcterms:publisher rdf:resource="http://www.historicengland.org.uk"/>
    <cc:attributionName xml:lang="en">Historic England</cc:attributionName>
    <rdf:type rdf:resource="http://www.w3.org/2004/02/skos/core#Concept"/>
    <skos:broader rdf:resource="http://purl.org/heritagedata/schemes/225/concepts/111397"/>
    <cc:license rdf:resource="http://creativecommons.org/licenses/by/3.0"/>
    <skos:inScheme rdf:resource="http://purl.org/heritagedata/schemes/225"/>
    <cc:attributionURL rdf:resource="http://www.historicengland.org.uk"/>
    <dcterms:issued rdf:datatype="http://www.w3.org/2001/XMLSchema#dateTime">2019-03-26T16:45:43</dcterms:issued>
    <skos:scopeNote xml:lang="en">Single-seat, single-engine fighter biplane renowned for its high performance and manoeuvrability. Entered service in 1917.</skos:scopeNote>
    <skos:broader rdf:resource="http://purl.org/heritagedata/schemes/225/concepts/136232"/>
    <ns1:related rdf:resource="http://purl.org/heritagedata/schemes/225/concepts/136233"/>
    <skos:broader rdf:resource="http://purl.org/heritagedata/schemes/225/concepts/111403"/>
    <skos:prefLabel xml:lang="en">Camel</skos:prefLabel>
  </rdf:Description>
  <rdf:Description rdf:about="http://purl.org/heritagedata/schemes/225/concepts/133198">
    <rdf:type rdf:resource="http://www.w3.org/2004/02/skos/core#Concept"/>
    <dcterms:identifier>http://purl.org/heritagedata/schemes/225/concepts/133198</dcterms:identifier>
    <cc:license rdf:resource="http://creativecommons.org/licenses/by/3.0"/>
    <cc:attributionName xml:lang="en">Historic England</cc:attributionName>
    <cc:attributionURL rdf:resource="http://www.historicengland.org.uk"/>
    <skos:inScheme rdf:resource="http://purl.org/heritagedata/schemes/225"/>
    <skos:prefLabel xml:lang="en">Douglas</skos:prefLabel>
    <skos:narrower rdf:resource="http://purl.org/heritagedata/schemes/225/concepts/137151"/>
    <dcterms:issued rdf:datatype="http://www.w3.org/2001/XMLSchema#dateTime">2019-03-26T16:45:43</dcterms:issued>
    <skos:narrower rdf:resource="http://purl.org/heritagedata/schemes/225/concepts/137229"/>
    <dcterms:publisher rdf:resource="http://www.historicengland.org.uk"/>
    <skos:narrower rdf:resource="http://purl.org/heritagedata/schemes/225/concepts/133199"/>
    <skos:narrower rdf:resource="http://purl.org/heritagedata/schemes/225/concepts/137174"/>
    <skos:broader rdf:resource="http://purl.org/heritagedata/schemes/225/concepts/111358"/>
    <skos:scopeNote xml:lang="en">The Douglas Aircraft Company, Inc., established in 1920, reorganized in 1928. Produced such notable aircraft as the Dakota.</skos:scopeNote>
  </rdf:Description>
  <rdf:Description rdf:about="http://purl.org/heritagedata/schemes/225/concepts/140423">
    <skos:altLabel xml:lang="en">Sb2a Buccaneer</skos:altLabel>
  </rdf:Description>
  <rdf:Description rdf:about="http://purl.org/heritagedata/schemes/225/concepts/141196">
    <dcterms:publisher rdf:resource="http://www.historicengland.org.uk"/>
    <rdf:type rdf:resource="http://www.w3.org/2004/02/skos/core#Concept"/>
    <skos:broader rdf:resource="http://purl.org/heritagedata/schemes/225/concepts/141131"/>
    <dcterms:issued rdf:datatype="http://www.w3.org/2001/XMLSchema#dateTime">2019-03-26T16:45:43</dcterms:issued>
    <skos:prefLabel xml:lang="en">MkII</skos:prefLabel>
    <cc:attributionName xml:lang="en">Historic England</cc:attributionName>
    <skos:inScheme rdf:resource="http://purl.org/heritagedata/schemes/225"/>
    <dcterms:identifier>http://purl.org/heritagedata/schemes/225/concepts/141196</dcterms:identifier>
    <skos:scopeNote xml:lang="en">Mark 2 or the second variant of an aircraft with its associated modifications.</skos:scopeNote>
    <cc:license rdf:resource="http://creativecommons.org/licenses/by/3.0"/>
    <cc:attributionURL rdf:resource="http://www.historicengland.org.uk"/>
  </rdf:Description>
  <rdf:Description rdf:about="http://purl.org/heritagedata/schemes/225/concepts/125614">
    <cc:license rdf:resource="http://creativecommons.org/licenses/by/3.0"/>
    <cc:attributionURL rdf:resource="http://www.historicengland.org.uk"/>
    <rdf:type rdf:resource="http://www.w3.org/2004/02/skos/core#Concept"/>
    <dcterms:identifier>http://purl.org/heritagedata/schemes/225/concepts/125614</dcterms:identifier>
    <dcterms:publisher rdf:resource="http://www.historicengland.org.uk"/>
    <cc:attributionName xml:lang="en">Historic England</cc:attributionName>
    <skos:inScheme rdf:resource="http://purl.org/heritagedata/schemes/225"/>
    <dcterms:issued rdf:datatype="http://www.w3.org/2001/XMLSchema#dateTime">2019-03-26T16:45:43</dcterms:issued>
    <skos:scopeNote xml:lang="en">The English Electric Company Limited. Formed in 1918, but didn't move into aircraft production until 1938, at the Government's request. Continued to develop aircraft after the war and in 1948 produced the `Canberra', Britain's first jet-propelled bomber.</skos:scopeNote>
    <skos:prefLabel xml:lang="en">English Electric</skos:prefLabel>
    <skos:narrower rdf:resource="http://purl.org/heritagedata/schemes/225/concepts/125518"/>
    <skos:broader rdf:resource="http://purl.org/heritagedata/schemes/225/concepts/111358"/>
  </rdf:Description>
  <rdf:Description rdf:about="http://purl.org/heritagedata/schemes/225/concepts/141204">
    <dcterms:issued rdf:datatype="http://www.w3.org/2001/XMLSchema#dateTime">2019-03-26T16:45:43</dcterms:issued>
    <skos:inScheme rdf:resource="http://purl.org/heritagedata/schemes/225"/>
    <cc:attributionURL rdf:resource="http://www.historicengland.org.uk"/>
    <cc:attributionName xml:lang="en">Historic England</cc:attributionName>
    <cc:license rdf:resource="http://creativecommons.org/licenses/by/3.0"/>
    <dcterms:identifier>http://purl.org/heritagedata/schemes/225/concepts/141204</dcterms:identifier>
    <skos:prefLabel xml:lang="en">MkIC</skos:prefLabel>
    <dcterms:publisher rdf:resource="http://www.historicengland.org.uk"/>
    <skos:broader rdf:resource="http://purl.org/heritagedata/schemes/225/concepts/141131"/>
    <skos:scopeNote xml:lang="en">A Mark 1B aircraft which has undergone further modification to enhance performance or armament.</skos:scopeNote>
    <rdf:type rdf:resource="http://www.w3.org/2004/02/skos/core#Concept"/>
  </rdf:Description>
  <rdf:Description rdf:about="http://purl.org/heritagedata/schemes/225/concepts/138545">
    <skos:altLabel xml:lang="en">Dh18b</skos:altLabel>
  </rdf:Description>
  <rdf:Description rdf:about="http://purl.org/heritagedata/schemes/225/concepts/133197">
    <skos:altLabel xml:lang="en">Tomahawk</skos:altLabel>
  </rdf:Description>
  <rdf:Description rdf:about="http://purl.org/heritagedata/schemes/225/concepts/136523">
    <skos:altLabel xml:lang="en">504</skos:altLabel>
  </rdf:Description>
  <rdf:Description rdf:about="http://purl.org/heritagedata/schemes/225/concepts/140422">
    <skos:altLabel xml:lang="en">Doodlebug</skos:altLabel>
  </rdf:Description>
  <rdf:Description rdf:about="http://purl.org/heritagedata/schemes/225/concepts/111437">
    <skos:altLabel xml:lang="en">Flying Fortress</skos:altLabel>
  </rdf:Description>
  <rdf:Description rdf:about="http://purl.org/heritagedata/schemes/225/concepts/137240">
    <skos:altLabel xml:lang="en">Condor</skos:altLabel>
  </rdf:Description>
  <rdf:Description rdf:about="http://purl.org/heritagedata/schemes/225/concepts/139053">
    <skos:prefLabel xml:lang="en">Tug</skos:prefLabel>
    <cc:license rdf:resource="http://creativecommons.org/licenses/by/3.0"/>
    <rdf:type rdf:resource="http://www.w3.org/2004/02/skos/core#Concept"/>
    <cc:attributionURL rdf:resource="http://www.historicengland.org.uk"/>
    <skos:inScheme rdf:resource="http://purl.org/heritagedata/schemes/225"/>
    <dcterms:issued rdf:datatype="http://www.w3.org/2001/XMLSchema#dateTime">2019-03-26T16:45:43</dcterms:issued>
    <cc:attributionName xml:lang="en">Historic England</cc:attributionName>
    <skos:narrower rdf:resource="http://purl.org/heritagedata/schemes/225/concepts/139049"/>
    <skos:broader rdf:resource="http://purl.org/heritagedata/schemes/225/concepts/111394"/>
    <dcterms:identifier>http://purl.org/heritagedata/schemes/225/concepts/139053</dcterms:identifier>
    <dcterms:publisher rdf:resource="http://www.historicengland.org.uk"/>
    <skos:narrower rdf:resource="http://purl.org/heritagedata/schemes/225/concepts/135751"/>
    <skos:scopeNote xml:lang="en">An aircraft used for towing another aircraft or object, such as a glider or target.</skos:scopeNote>
  </rdf:Description>
  <rdf:Description rdf:about="http://purl.org/heritagedata/schemes/225/concepts/138483">
    <skos:altLabel xml:lang="en">U6a Beaver</skos:altLabel>
  </rdf:Description>
  <rdf:Description rdf:about="http://purl.org/heritagedata/schemes/225/concepts/140421">
    <skos:altLabel xml:lang="en">Fieseler Fi103</skos:altLabel>
  </rdf:Description>
  <rdf:Description rdf:about="http://purl.org/heritagedata/schemes/225/concepts/111439">
    <skos:altLabel xml:lang="en">Bf109</skos:altLabel>
  </rdf:Description>
  <rdf:Description rdf:about="http://purl.org/heritagedata/schemes/225/concepts/167013">
    <skos:altLabel xml:lang="en">Bleriot Aeronautique</skos:altLabel>
  </rdf:Description>
  <rdf:Description rdf:about="http://purl.org/heritagedata/schemes/225/concepts/133233">
    <skos:altLabel xml:lang="en">Fo108</skos:altLabel>
  </rdf:Description>
  <rdf:Description rdf:about="http://purl.org/heritagedata/schemes/225/concepts/111431">
    <skos:altLabel xml:lang="en">Pencil Bomber</skos:altLabel>
  </rdf:Description>
  <rdf:Description rdf:about="http://purl.org/heritagedata/schemes/225/concepts/136253">
    <skos:altLabel xml:lang="en">F5</skos:altLabel>
  </rdf:Description>
  <rdf:Description rdf:about="http://purl.org/heritagedata/schemes/225/concepts/167005">
    <skos:altLabel xml:lang="en">Sabrejet</skos:altLabel>
  </rdf:Description>
  <rdf:Description rdf:about="http://purl.org/heritagedata/schemes/225/concepts/138463">
    <skos:altLabel xml:lang="en">Haig</skos:altLabel>
  </rdf:Description>
  <rdf:Description rdf:about="http://purl.org/heritagedata/schemes/225/concepts/136518">
    <skos:altLabel xml:lang="en">Dh9</skos:altLabel>
  </rdf:Description>
  <rdf:Description rdf:about="http://purl.org/heritagedata/schemes/225/concepts/137230">
    <skos:altLabel xml:lang="en">C47 Skytrain</skos:altLabel>
  </rdf:Description>
  <rdf:Description rdf:about="http://purl.org/heritagedata/schemes/225/concepts/136520">
    <skos:altLabel xml:lang="en">Fk8</skos:altLabel>
  </rdf:Description>
  <rdf:Description rdf:about="http://purl.org/heritagedata/schemes/225/concepts/138462">
    <skos:altLabel xml:lang="en">Warhawk</skos:altLabel>
  </rdf:Description>
  <rdf:Description rdf:about="http://purl.org/heritagedata/schemes/225/concepts/136519">
    <skos:altLabel xml:lang="en">Fk3</skos:altLabel>
  </rdf:Description>
  <rdf:Description rdf:about="http://purl.org/heritagedata/schemes/225/concepts/136514">
    <skos:altLabel xml:lang="en">Dh2</skos:altLabel>
  </rdf:Description>
  <rdf:Description rdf:about="http://purl.org/heritagedata/schemes/225/concepts/136527">
    <skos:altLabel xml:lang="en">Prefect</skos:altLabel>
  </rdf:Description>
  <rdf:Description rdf:about="http://purl.org/heritagedata/schemes/225/concepts/137210">
    <skos:altLabel xml:lang="en">Sea Otter</skos:altLabel>
  </rdf:Description>
</rdf:RDF>